<?xml version="1.0" encoding="UTF-8"?>

<!-- Discussion document: version 2012-05-10, 2012-08-03.
  Dag Endresen, Global Biodiversity Information Facility (GBIF)
  Edward Baker, Natural History Museum, London (NHM)

 This RDF Vocabulary is based on the Darwin Core extension developed at the 
  GBIF Vocabulary Server at http://vocabularies.gbif.org/vocabularies/geo_chronostrat
  by Edward Baker (NHM London).
-->

<!DOCTYPE rdf:RDF [
  <!ENTITY geotime          "http://rs.gbif.org/terms/geotime/geotimeConcept#">
  <!ENTITY contact          "http://rs.gbif.org/terms/geotime/geotimeContact#">
  <!ENTITY history          "http://rs.gbif.org/terms/geotime/archive/">
]>


<rdf:RDF
  xmlns:rdf="http://www.w3.org/1999/02/22-rdf-syntax-ns#"
  xmlns:rdfs="http://www.w3.org/2000/01/rdf-schema#"
  xmlns:xsd="http://www.w3.org/2001/XMLSchema#"
  xmlns:owl="http://www.w3.org/2002/07/owl#"
  xmlns:skos="http://www.w3.org/2004/02/skos/core#"
  xmlns:foaf="http://xmlns.com/foaf/0.1/"
  xmlns:vs="http://www.w3.org/2003/06/sw-vocab-status/ns#"
  xmlns:vann="http://purl.org/vocab/vann/"
  xmlns:dc="http://purl.org/dc/elements/1.1/"
  xmlns:dcterms="http://purl.org/dc/terms/"
  xmlns:dcmitype="http://purl.org/dc/dcmitype/"
  xmlns:geo="http://www.w3.org/2003/01/geo/wgs84_pos#"
  xmlns:dwc="http://rs.tdwg.org/dwc/terms/"
  xmlns:geotime="&geotime;"
  xml:base="&geotime;"
>


<!-- ### Vocabulary of Terms (skos:ConceptScheme) ### -->

  <skos:ConceptScheme rdf:about="&geotime;">
    <rdfs:label xml:lang="en">Geological time periods and events</rdfs:label>
    <rdfs:comment xml:lang="en">Standard nomenclature for paleontological intervals of time and events based on GTS2004.</rdfs:comment>
    <dcterms:created>2012-05-10</dcterms:created>
    <dcterms:modified>2012-08-03</dcterms:modified>
    <owl:versionInfo xml:lang="en">Draft version, 3 August 2012, not yet published</owl:versionInfo>
    <dcterms:creator rdf:resource="&contact;NHM_UK"/>
    <dcterms:contributor rdf:resource="&contact;EdwardBaker"/>
    <dcterms:contributor rdf:resource="&contact;DagEndresen"/>
    <dcterms:publisher rdf:resource="&contact;GBIF"/> <!-- who is the publisher ?? -->
    <dcterms:license rdf:resource="http://creativecommons.org/publicdomain/zero/1.0/"/> <!-- NB! Licence rights...? -->
    <dcterms:rights xml:lang="en">Creative Commons Public Domain license; see http://creativecommons.org/publicdomain/zero/1.0/. You are free to copy, distribute and transmit the work; to remix/adapt the work (e.g. to import the ontology and create specializations of its elements), all without asking permissions. If you wish to provide attribution you may include the statement: "This work is based on the Darwin Core extension for genebanks".</dcterms:rights>
    <dcterms:accessRights>public</dcterms:accessRights>
    <vann:preferredNamespaceUri>&geotime;</vann:preferredNamespaceUri>
    <vann:preferredNamespacePrefix>geotime</vann:preferredNamespacePrefix>
    <foaf:homepage rdf:resource="http://kos.gbif.org/wiki/geotime"/> <!-- Could a home page be established here...?? -->
    <dcterms:bibliographicCitation>Baker E, Johnson KG, Young JR (2011). The future of the past in the present: biodiversity informatics and geological time. ZooKeys 150:397-405. doi: 10.3897/zookeys.150.2350</dcterms:bibliographicCitation>
    <dcterms:bibliographicCitation>Gradstein FM, Ogg JG, and Smith AG (2004). A geological time scale 2004. Cambridge University Press. doi:10.4095/215638. ISBN: 9780521786737.</dcterms:bibliographicCitation>
    <skos:editorialNote xml:lang="en">Notice that the base URI for the GeoTime vocabulary (draft version) is "http://rs.gbif.org/terms/geotime#". Please make sure that you are only using element identifiers in this namespace, e.g. "http://rs.gbif.org/terms/geotime#TERM". There may be copies of the vocabulary file on the Web which can be retrieved from other locations, but those locations should not be used as the basis of identifiers.</skos:editorialNote>
    <skos:scopeNote>The GeoTime vocabulary provides the nomenclature for geological time periods based on the Geologic Time Scale 2004 (GTS2004). These terms are used by a number of controlled value vocabularies designed to be used together with the TDWG Darwin Core standard...[what the vocabulary does and does not cover]</skos:scopeNote>
    <rdfs:seeAlso rdf:resource="http://en.wikipedia.org/wiki/Geologic_time_scale"/>
  </skos:ConceptScheme>


<!-- ### Collection of Terms (skos:Collection) ###
 Labelled collections can be used to group the terms under this sub-heading.
 -->

  <skos:Collection rdf:about="&geotime;TimePeriod">
    <rdfs:label xml:lang="en">Geological time period</rdfs:label>
    <rdfs:comment xml:lang="en">Geological time period.</rdfs:comment>
    <skos:broader rdf:resource="geotime:Chronostratigraphic"/>
    <skos:broader rdf:resource="geotime:Magnetostratigraphic"/>
    <skos:narrowMatch rdf:resource="dwc:Event"/>
    <skos:narrowMatch rdf:resource="dcmitype:Event"/>
  </skos:Collection>

  <skos:Collection rdf:about="&geotime;Chronostratigraphic">
    <rdfs:label xml:lang="en">Chronostratigraphic scale</rdfs:label>
    <rdfs:comment xml:lang="en">Standard stratigraphic nomenclature based on palaeontological intervals of time defined by recognised fossil assemblages.</rdfs:comment>
    <skos:narrower rdf:resource="geotime:TimePeriod"/>
    <skos:narrowMatch rdf:resource="dwc:Event"/>
    <skos:narrowMatch rdf:resource="dcmitype:Event"/>
  </skos:Collection>

  <skos:Collection rdf:about="&geotime;Magnetostratigraphic">
    <rdfs:label xml:lang="en">Magnetostratigraphic scale</rdfs:label>
    <rdfs:comment xml:lang="en">Magnetostratigraphy provides he correlation of biostratigraphic datums to marine magnetic anomalies.</rdfs:comment>
    <skos:narrower rdf:resource="geotime:TimePeriod"/>
    <skos:narrowMatch rdf:resource="dwc:Event"/>
    <skos:narrowMatch rdf:resource="dcmitype:Event"/>
  </skos:Collection>

<!-- External concepts as skos:Collection for the categories of the geological time periods
     Can we perhaps use the Wikipedia URLs as URIs here...? - in other words perhaps using 
     rdf:about="http://en.wikipedia.org/wiki/Eon_(geology)" instead of "rdf:about=geotime:Eon" etc...???
     rdf:about="http://dbpedia.org/data/Eon" is another alternative.
 -->

  <skos:Collection rdf:about="&geotime;Eon">
    <skos:prefLabel xml:lang="en">Eon</skos:prefLabel>
    <skos:definition xml:lang="en">Category for geological time periods spanning more than half a billion years.</skos:definition>
    <rdfs:seeAlso rdf:resource="http://en.wikipedia.org/wiki/Eon_(geology)"/>
    <dcterms:created>2012-05-10</dcterms:created>
    <dcterms:modified>2012-08-03</dcterms:modified>
    <dcterms:hasVersion rdf:resource="&geotimeHistory;Eon"/>
    <rdfs:isDefinedBy rdf:resource="&geotime;"/>
    <skos:inScheme rdf:resource="&geotime;"/>
    <vs:term_status>unstable</vs:term_status>
    <skos:narrower rdf:resource="geotime:TimePeriod"/>
    <skos:narrower rdf:resource="geotime:Chronostratigraphic"/>
  </skos:Collection>

  <skos:Collection rdf:about="&geotime;Era">
    <skos:prefLabel xml:lang="en">Era</skos:prefLabel>
    <skos:definition xml:lang="en">Category for geological time periods spanning several hundred million years.</skos:definition>
    <rdfs:seeAlso rdf:resource="http://en.wikipedia.org/wiki/Era_(geology)"/>
    <dcterms:created>2012-05-10</dcterms:created>
    <dcterms:modified>2012-08-03</dcterms:modified>
    <dcterms:hasVersion rdf:resource="&geotimeHistory;Era"/>
    <rdfs:isDefinedBy rdf:resource="&geotime;"/>
    <skos:inScheme rdf:resource="&geotime;"/>
    <vs:term_status>unstable</vs:term_status>
    <skos:narrower rdf:resource="geotime:TimePeriod"/>
    <skos:narrower rdf:resource="geotime:Chronostratigraphic"/>
  </skos:Collection>

  <skos:Collection rdf:about="&geotime;SubEra">
    <skos:prefLabel xml:lang="en">Sub-Era</skos:prefLabel>
    <skos:definition xml:lang="en">Sub-category for geological time periods spanning several hundred million years.</skos:definition>
    <rdfs:seeAlso rdf:resource="http://en.wikipedia.org/wiki/Era_(geology)"/>
    <dcterms:created>2012-05-10</dcterms:created>
    <dcterms:modified>2012-08-03</dcterms:modified>
    <dcterms:hasVersion rdf:resource="&geotimeHistory;SubEra"/>
    <rdfs:isDefinedBy rdf:resource="&geotime;"/>
    <skos:inScheme rdf:resource="&geotime;"/>
    <vs:term_status>unstable</vs:term_status>
    <skos:narrower rdf:resource="geotime:TimePeriod"/>
    <skos:narrower rdf:resource="geotime:Chronostratigraphic"/>
  </skos:Collection>

  <skos:Collection rdf:about="&geotime;Period">
    <skos:prefLabel xml:lang="en">Period</skos:prefLabel>
    <skos:definition xml:lang="en">Category for geological time periods with a time spanning las than an Era and more than an Epoch.</skos:definition>
    <rdfs:seeAlso rdf:resource="http://en.wikipedia.org/wiki/Period_(geology)"/>
    <dcterms:created>2012-05-10</dcterms:created>
    <dcterms:modified>2012-08-03</dcterms:modified>
    <dcterms:hasVersion rdf:resource="&geotimeHistory;Period"/>
    <rdfs:isDefinedBy rdf:resource="&geotime;"/>
    <skos:inScheme rdf:resource="&geotime;"/>
    <vs:term_status>unstable</vs:term_status>
    <skos:narrower rdf:resource="geotime:TimePeriod"/>
    <skos:narrower rdf:resource="geotime:Chronostratigraphic"/>
  </skos:Collection>

  <skos:Collection rdf:about="&geotime;SubPeriod">
    <skos:prefLabel xml:lang="en">Sub-Period</skos:prefLabel>
    <skos:definition xml:lang="en">Sub-category for geological time periods with a time spanning las than an Era and more than an Epoch.</skos:definition>
    <rdfs:seeAlso rdf:resource="http://en.wikipedia.org/wiki/Period_(geology)"/>
    <dcterms:created>2012-05-10</dcterms:created>
    <dcterms:modified>2012-08-03</dcterms:modified>
    <dcterms:hasVersion rdf:resource="&geotimeHistory;SubPeriod"/>
    <rdfs:isDefinedBy rdf:resource="&geotime;"/>
    <skos:inScheme rdf:resource="&geotime;"/>
    <vs:term_status>unstable</vs:term_status>
    <skos:narrower rdf:resource="geotime:TimePeriod"/>
    <skos:narrower rdf:resource="geotime:Chronostratigraphic"/>
  </skos:Collection>

  <skos:Collection rdf:about="&geotime;Epoch">
    <skos:prefLabel xml:lang="en">Epoch</skos:prefLabel>
    <skos:definition xml:lang="en">Category for geological time periods spanning tens of million years.</skos:definition>
    <rdfs:seeAlso rdf:resource="http://en.wikipedia.org/wiki/Epoch_(geology)"/>
    <dcterms:created>2012-05-10</dcterms:created>
    <dcterms:modified>2012-08-03</dcterms:modified>
    <dcterms:hasVersion rdf:resource="&geotimeHistory;Epoch"/>
    <rdfs:isDefinedBy rdf:resource="&geotime;"/>
    <skos:inScheme rdf:resource="&geotime;"/>
    <vs:term_status>unstable</vs:term_status>
    <skos:narrower rdf:resource="geotime:TimePeriod"/>
    <skos:narrower rdf:resource="geotime:Chronostratigraphic"/>
  </skos:Collection>

  <skos:Collection rdf:about="&geotime;Stage">
    <skos:prefLabel xml:lang="en">Stage</skos:prefLabel>
    <skos:definition xml:lang="en">Category for geological time periods spanning millions of years.</skos:definition>
    <rdfs:seeAlso rdf:resource="http://en.wikipedia.org/wiki/Stage_(stratigraphy)"/>
    <dcterms:created>2012-05-10</dcterms:created>
    <dcterms:modified>2012-08-03</dcterms:modified>
    <dcterms:hasVersion rdf:resource="&geotimeHistory;Stage"/>
    <rdfs:isDefinedBy rdf:resource="&geotime;"/>
    <skos:inScheme rdf:resource="&geotime;"/>
    <vs:term_status>unstable</vs:term_status>
    <skos:narrower rdf:resource="geotime:TimePeriod"/>
    <skos:narrower rdf:resource="geotime:Chronostratigraphic"/>
  </skos:Collection>



<!-- ### Datatype declaration, Internal annotation properties ### -->

<!-- Dag Endresen, 2012-05-10: 
     Is "base" and "top" the appropriate label to use for the onset and end of the time periods...?
     Perhaps we could label the start of the time period (base) simply as "geotime:start", 
     and the end of the time periods (top) simply as "geotime:end"...?
     It also seems to me as if Gradstein et al (2004) discuss "base" as both of the 
     boundaries of the time period, and not only the start or lower boundary...?
 -->

  <rdf:Property rdf:about="&geotime;start">
    <rdfs:label xml:lang="en-US">Start of time period</rdfs:label>
    <rdfs:comment xml:lang="en-US">The start of the geological time period is indicated as million years ago.</rdfs:comment>
    <rdfs:isDefinedBy rdf:resource="&geotime;"/>
    <dcterms:created>2012-05-10</dcterms:created>
    <dcterms:modified>2012-08-03</dcterms:modified>
    <dcterms:hasVersion rdf:resource="&history;20120803/geotime#start"/>
    <rdfs:range rdf:resource="http://www.w3.org/2000/01/rdf-schema#Literal"/>
    <rdf:type rdf:resource="http://www.w3.org/1999/02/22-rdf-syntax-ns#Property"/>
    <rdfs:Datatype rdf:resource="xsd:decimal"/>
  </rdf:Property>

  <rdf:Property rdf:about="&geotime;end">
    <rdfs:label xml:lang="en-US">End of time period</rdfs:label>
    <rdfs:comment xml:lang="en-US">The end of the geological time period is indicated as million years ago.</rdfs:comment>
    <rdfs:isDefinedBy rdf:resource="&geotime;"/>
    <dcterms:created>2012-05-10</dcterms:created>
    <dcterms:modified>2012-08-03</dcterms:modified>
    <dcterms:hasVersion rdf:resource="&history;20120803/geotime#end"/>
    <rdfs:range rdf:resource="http://www.w3.org/2000/01/rdf-schema#Literal"/>
    <rdf:type rdf:resource="http://www.w3.org/1999/02/22-rdf-syntax-ns#Property"/>
    <rdfs:Datatype rdf:resource="xsd:decimal"/>
  </rdf:Property>

  <rdf:Property rdf:about="&geotime;rangeType">
    <rdfs:label xml:lang="en-US">Range type</rdfs:label>
    <rdfs:comment xml:lang="en-US">The range type of the geological time period is one of Eon, Era, Sub-Era, Period, Sub-Period, Epoch, Stage or Substage.</rdfs:comment>
    <skos:example>Eon, Era, Sub-Era, Period, Sub-Period, Epoch, Stage or Substage</skos:example>
    <rdfs:isDefinedBy rdf:resource="&geotime;"/>
    <dcterms:created>2012-05-10</dcterms:created>
    <dcterms:modified>2012-08-03</dcterms:modified>
    <dcterms:hasVersion rdf:resource="&history;20120803/geotime#rangeType"/>
    <rdfs:range rdf:resource="http://www.w3.org/2000/01/rdf-schema#Literal"/>
    <rdf:type rdf:resource="http://www.w3.org/1999/02/22-rdf-syntax-ns#Property"/>
  </rdf:Property>

  <rdf:Property rdf:about="&geotime;rangeTypeURI">
    <rdfs:label xml:lang="en-US">Range type URI</rdfs:label>
    <rdfs:comment xml:lang="en-US">The range type of the geological time period is one of Eon, Era, Sub-Era, Period, Sub-Period, Epoch, Stage or Substage.</rdfs:comment>
    <skos:example>geotime:Eon, geotime:Era, geotime:SubEra, geotime:Period, geotime:SubPeriod, geotime:Epoch, geotime:Stage or geotime:Substage</skos:example>
    <rdfs:isDefinedBy rdf:resource="&geotime;"/>
    <dcterms:created>2012-05-10</dcterms:created>
    <dcterms:modified>2012-08-03</dcterms:modified>
    <dcterms:hasVersion rdf:resource="&history;20120803/geotime#rangeType"/>
    <rdf:type rdf:resource="http://www.w3.org/1999/02/22-rdf-syntax-ns#Property"/>
  </rdf:Property>

  <rdf:Property rdf:about="&geotime;polarity">
    <rdfs:label xml:lang="en-US">Polarity</rdfs:label>
    <rdfs:comment xml:lang="en-US">The polarity describes ... (N, R)</rdfs:comment>
    <skos:example>N, R</skos:example>
    <rdfs:isDefinedBy rdf:resource="&geotime;"/>
    <dcterms:created>2012-05-10</dcterms:created>
    <dcterms:modified>2012-08-03</dcterms:modified>
    <dcterms:hasVersion rdf:resource="&history;20120803/geotime#polarity"/>
    <rdfs:range rdf:resource="http://www.w3.org/2000/01/rdf-schema#Literal"/>
    <rdf:type rdf:resource="http://www.w3.org/1999/02/22-rdf-syntax-ns#Property"/>
  </rdf:Property>

  <rdf:Property rdf:about="&geotime;regionName">
    <rdfs:label xml:lang="en-US">Region name</rdfs:label>
    <rdfs:comment xml:lang="en-US">The region name describes ...</rdfs:comment>
    <skos:example>Brunhes, Jaramillo</skos:example>
    <rdfs:isDefinedBy rdf:resource="&geotime;"/>
    <dcterms:created>2012-05-10</dcterms:created>
    <dcterms:modified>2012-08-03</dcterms:modified>
    <dcterms:hasVersion rdf:resource="&history;20120803/geotime#regionName"/>
    <rdfs:range rdf:resource="http://www.w3.org/2000/01/rdf-schema#Literal"/>
    <rdf:type rdf:resource="http://www.w3.org/1999/02/22-rdf-syntax-ns#Property"/>
  </rdf:Property>

  <rdfs:Datatype rdf:about="&geotime;bioColID">
    <skos:prefLabel xml:lang="en">Biodiversity Collections Index ID</skos:prefLabel>
    <skos:definition xml:lang="en">An index of biodiversity collections, providing persistent identifiers based on LSID URIs.</skos:definition>
    <skos:example xml:lang="en">http://biocol.org/urn:lsid:biocol.org:col:34665</skos:example>
    <skos:note xml:lang="en">The Biodiversity Collections Index is available at http://biocol.org/</skos:note>
    <dcterms:created>2012-05-10</dcterms:created>
    <dcterms:modified>2012-08-03</dcterms:modified>
    <dcterms:hasVersion rdf:resource="&history;20120803/geotime#bioColID"/>
    <vann:termGroup rdf:resource="&geotime;DatatypeProperty"/>
    <rdfs:isDefinedBy rdf:resource="&geotime;"/>
    <skos:inScheme rdf:resource="&geotime;"/>
    <vs:term_status>unstable</vs:term_status>
    <skos:closeMatch rdf:resource="dcterms:identifier"/>
    <skos:relatedMatch rdf:resource="http://biocol.org/"/>
    <rdf:type rdf:resource="http://www.w3.org/2000/01/rdf-schema#Datatype"/>
    <rdf:type rdf:resource="http://www.w3.org/2002/07/owl#DatatypeProperty"/>
  </rdfs:Datatype>





<!-- ### INDIVIDUAL CONCEPTS (skos:Concept) ### -->

<!--
 Terms (skos:Concept) are described by the following properties:
  @rdf:about 			(provides the identifier for the term)
  skos:prefLabel 		(human readable name or label for the term)
  skos:definition 		(brief and unambigous definition)
  rdfs:seeAlso  		(link to Wiki discussion page, link to term documentation resources)
  skos:note 			(notes on how to use for each term)
  skos:scopeNote 		(what the term does and does not cover)
  dcterms:created 		(when the RDF description was created, for each term)
  dcterms:modified 		(when the RDF description was updated, for each term)
  dcterms:issued 		(when the RDF description was issued/published, for each term)
  skos:inScheme			(terms belong to an identifiable vocabulary managed by an expert group)    
  rdfs:isDefinedBy 		(terms are defined by an identifiable vocabulary or resource [namespace])
  vs:term_status 		(all terms here are considered "unstable", and scheduled to be deprecated)
  skos:altLabel 		(for synonym labels such as the MultiCrop Passport Descriptors)
  dcterms:source 		(link to source description for each term)

  // Cross-walk between terms and concepts in other concept schemes:
  skos:relatedMatch		(when the term has a related match to another concept [in another conceptScheme])
  skos:exactMatch		(when the term has an exact match to another concept [in another conceptScheme])
  skos:closeMatch		(when the term has a close match to another concept [in another conceptScheme])
  skos:narrowMatch		(when the term has a narower hierarchal match to another concept [in another conceptScheme])
  skos:broadMatch		(when the term has a broader hierarchal match to another concept [in another conceptScheme])
  skos:related			(when the term has a related match to another concept)
  skos:narrower			(when the term has a narrower hierarchal match to another concept)
  skos:broader			(when the term has a broader hierarchal match to another concept)

  // Potentially useful annotation properties:
  dcterms:isReplacedBy 	(if a term is deprecated and replaced by another term)
  dcterms:replaces 		(can be used if the TERM replaces a previous TERM)
  vann:termGroup		(used for organizing terms into groups, collection or category of terms)
  dcterms:hasVersion 	(the terms of the RDF vocabularies have a version declared in a history resource)
  dcterms:identifier 	(we could also provide other identifiers than the URI here)
  rdf:type 				(type is here implicit when using skos:Concept for the "RDF molecules")

  // proposed NOT to be used here... (??)
  rdfs:label 			(human readable name for the term, same as skos:prefLabel)
  rdfs:domain			(defines the resources used as subjects when a concept is used as an annotation property)
  rdfs:range			(defines the resources used as objects when a concept is used as an annotation property)
  rdfs:subPropertyOf 	(when the term can be seen as instance of a broader vocabulary term [Property])
  rdfs:subClassOf 		(when the term can be seen as instance of a broader vocabulary term [Class])
-->


<!-- Example of the XML syntax generated by the GBIF Vocabulary Server, 
     http://vocabularies.gbif.org/vocabularies/geo_chronostrat
     - and the same term described by this RDF Vocabulary.

 <concept 
  dc:URI="node/160489" 
  dc:description="http://vocabularies.gbif.org/geo_chronostrat/Phanerozoic" 
  dc:identifier="Phanerozoic" 
  dc:created="2011-01-11T11:50:40+00:00" 
  dc:modified="2011-01-11T11:50:41+00:00" 
  dc:title="Phanerozoic" notes="" reference="" 
  rangeType="Eon" base="" top="">
  <preferred>
   <term 
    dc:created="2011-01-11T11:50:43+00:00" 
    dc:modified="2011-01-11T11:50:43+00:00" 
    dc:title="Phanerozoic" reference="en"
    standardConcept="Phanerozoic" xml:lang="en"/>
  </preferred>
  <alternative/>
 </concept>

  <skos:Concept rdf:about="&geotime;Phanerozoic">
    <skos:prefLabel xml:lang="en">Phanerozoic</skos:prefLabel>
    <skos:definition xml:lang="en">The Phanerozoic time period started 542  million years (Ma) before present (BP) and ended 0 Ma BP.</skos:definition>
    <rdfs:seeAlso rdf:resource="http://kos.gbif.org/wiki/geotime:Phanerozoic"/>
    <geotime:rangeType>Eon</geotime:rangeType>
    <geotime:rangeTypeURI rdf:resource="&geotime;Eon"/>
    <geotime:start>542</geotime:base>
    <geotime:end>0</geotime:top>
    <dcterms:created>2011-01-11</dcterms:issued>
    <dcterms:modified>2012-08-03</dcterms:modified>
    <dcterms:hasVersion rdf:resource="&history;20120803/geotime#Phanerozoic"/>
    <rdfs:isDefinedBy rdf:resource="&geotime;"/>
    <skos:inScheme rdf:resource="&geotime;"/>
    <vann:termGroup rdf:resource="&geotime;Eon"/>
    <vs:term_status>unstable</vs:term_status>
  </skos:Concept>
-->


<!-- Chronostratigraphic scale -->

<skos:Concept rdf:about="&geotime;Phanerozoic">	<skos:prefLabel xml:lang="en">Phanerozoic</skos:prefLabel>	<skos:definition>The Phanerozoic time period started 542  million years (Ma) before present (BP) and ended 0 Ma BP.</skos:definition>	<rdfs:seeAlso rdf:resource="http://kos.gbif.org/wiki/geotime:Phanerozoic"/>	<geotime:rangeType>Eon</geotime:rangeType>	<geotime:rangeTypeURI rdf:resource="&geotime;Eon"/>	<geotime:start>542</geotime:start>	<geotime:end>0</geotime:end>		<dcterms:created>2011-01-11</dcterms:created>	<dcterms:modified>2012-08-03</dcterms:modified>	<dcterms:hasVersion rdf:resource="&history;20120803/geotime#Phanerozoic"/>	<rdfs:isDefinedBy rdf:resource="&geotime;"/>	<skos:inScheme rdf:resource="&geotime;"/>	<vann:termGroup rdf:resource="&geotime;Eon"/>	<vann:termGroup rdf:resource="&geotime;Chronostratigraphic"/>	<vs:term_status>unstable</vs:term_status>	</skos:Concept>
<skos:Concept rdf:about="&geotime;Proterozoic">	<skos:prefLabel xml:lang="en">Proterozoic</skos:prefLabel>	<skos:definition>The Proterozoic time period started 2500  million years (Ma) before present (BP) and ended 542 Ma BP.</skos:definition>	<rdfs:seeAlso rdf:resource="http://kos.gbif.org/wiki/geotime:Proterozoic"/>	<geotime:rangeType>Eon</geotime:rangeType>	<geotime:rangeTypeURI rdf:resource="&geotime;Eon"/>	<geotime:start>2500</geotime:start>	<geotime:end>542</geotime:end>		<dcterms:created>2011-01-11</dcterms:created>	<dcterms:modified>2012-08-03</dcterms:modified>	<dcterms:hasVersion rdf:resource="&history;20120803/geotime#Proterozoic"/>	<rdfs:isDefinedBy rdf:resource="&geotime;"/>	<skos:inScheme rdf:resource="&geotime;"/>	<vann:termGroup rdf:resource="&geotime;Eon"/>	<vann:termGroup rdf:resource="&geotime;Chronostratigraphic"/>	<vs:term_status>unstable</vs:term_status>	</skos:Concept>
<skos:Concept rdf:about="&geotime;Archean">	<skos:prefLabel xml:lang="en">Archean</skos:prefLabel>	<skos:definition>The Archean time period started 4500  million years (Ma) before present (BP) and ended 2500 Ma BP.</skos:definition>	<rdfs:seeAlso rdf:resource="http://kos.gbif.org/wiki/geotime:Archean"/>	<geotime:rangeType>Eon</geotime:rangeType>	<geotime:rangeTypeURI rdf:resource="&geotime;Eon"/>	<geotime:start>4500</geotime:start>	<geotime:end>2500</geotime:end>		<dcterms:created>2011-01-11</dcterms:created>	<dcterms:modified>2012-08-03</dcterms:modified>	<dcterms:hasVersion rdf:resource="&history;20120803/geotime#Archean"/>	<rdfs:isDefinedBy rdf:resource="&geotime;"/>	<skos:inScheme rdf:resource="&geotime;"/>	<vann:termGroup rdf:resource="&geotime;Eon"/>	<vann:termGroup rdf:resource="&geotime;Chronostratigraphic"/>	<vs:term_status>unstable</vs:term_status>	</skos:Concept>
<skos:Concept rdf:about="&geotime;Holocene">	<skos:prefLabel xml:lang="en">Holocene</skos:prefLabel>	<skos:definition>The Holocene time period started 0.0115  million years (Ma) before present (BP) and ended 0 Ma BP.</skos:definition>	<rdfs:seeAlso rdf:resource="http://kos.gbif.org/wiki/geotime:Holocene"/>	<geotime:rangeType>Epoch</geotime:rangeType>	<geotime:rangeTypeURI rdf:resource="&geotime;Epoch"/>	<geotime:start>0.0115</geotime:start>	<geotime:end>0</geotime:end>	<skos:narrower>Neogene</skos:narrower>	<dcterms:created>2011-01-11</dcterms:created>	<dcterms:modified>2012-08-03</dcterms:modified>	<dcterms:hasVersion rdf:resource="&history;20120803/geotime#Holocene"/>	<rdfs:isDefinedBy rdf:resource="&geotime;"/>	<skos:inScheme rdf:resource="&geotime;"/>	<vann:termGroup rdf:resource="&geotime;Epoch"/>	<vann:termGroup rdf:resource="&geotime;Chronostratigraphic"/>	<vs:term_status>unstable</vs:term_status>	</skos:Concept>
<skos:Concept rdf:about="&geotime;Pleistocene">	<skos:prefLabel xml:lang="en">Pleistocene</skos:prefLabel>	<skos:definition>The Pleistocene time period started 1.806  million years (Ma) before present (BP) and ended 0.0115 Ma BP.</skos:definition>	<rdfs:seeAlso rdf:resource="http://kos.gbif.org/wiki/geotime:Pleistocene"/>	<geotime:rangeType>Epoch</geotime:rangeType>	<geotime:rangeTypeURI rdf:resource="&geotime;Epoch"/>	<geotime:start>1.806</geotime:start>	<geotime:end>0.0115</geotime:end>	<skos:narrower>Neogene</skos:narrower>	<dcterms:created>2011-01-11</dcterms:created>	<dcterms:modified>2012-08-03</dcterms:modified>	<dcterms:hasVersion rdf:resource="&history;20120803/geotime#Pleistocene"/>	<rdfs:isDefinedBy rdf:resource="&geotime;"/>	<skos:inScheme rdf:resource="&geotime;"/>	<vann:termGroup rdf:resource="&geotime;Epoch"/>	<vann:termGroup rdf:resource="&geotime;Chronostratigraphic"/>	<vs:term_status>unstable</vs:term_status>	</skos:Concept>
<skos:Concept rdf:about="&geotime;Pliocene">	<skos:prefLabel xml:lang="en">Pliocene</skos:prefLabel>	<skos:definition>The Pliocene time period started 5.333  million years (Ma) before present (BP) and ended 1.806 Ma BP.</skos:definition>	<rdfs:seeAlso rdf:resource="http://kos.gbif.org/wiki/geotime:Pliocene"/>	<geotime:rangeType>Epoch</geotime:rangeType>	<geotime:rangeTypeURI rdf:resource="&geotime;Epoch"/>	<geotime:start>5.333</geotime:start>	<geotime:end>1.806</geotime:end>	<skos:narrower>Neogene</skos:narrower>	<dcterms:created>2011-01-11</dcterms:created>	<dcterms:modified>2012-08-03</dcterms:modified>	<dcterms:hasVersion rdf:resource="&history;20120803/geotime#Pliocene"/>	<rdfs:isDefinedBy rdf:resource="&geotime;"/>	<skos:inScheme rdf:resource="&geotime;"/>	<vann:termGroup rdf:resource="&geotime;Epoch"/>	<vann:termGroup rdf:resource="&geotime;Chronostratigraphic"/>	<vs:term_status>unstable</vs:term_status>	</skos:Concept>
<skos:Concept rdf:about="&geotime;Miocene">	<skos:prefLabel xml:lang="en">Miocene</skos:prefLabel>	<skos:definition>The Miocene time period started 23.03  million years (Ma) before present (BP) and ended 5.333 Ma BP.</skos:definition>	<rdfs:seeAlso rdf:resource="http://kos.gbif.org/wiki/geotime:Miocene"/>	<geotime:rangeType>Epoch</geotime:rangeType>	<geotime:rangeTypeURI rdf:resource="&geotime;Epoch"/>	<geotime:start>23.03</geotime:start>	<geotime:end>5.333</geotime:end>	<skos:narrower>Neogene</skos:narrower>	<dcterms:created>2011-01-11</dcterms:created>	<dcterms:modified>2012-08-03</dcterms:modified>	<dcterms:hasVersion rdf:resource="&history;20120803/geotime#Miocene"/>	<rdfs:isDefinedBy rdf:resource="&geotime;"/>	<skos:inScheme rdf:resource="&geotime;"/>	<vann:termGroup rdf:resource="&geotime;Epoch"/>	<vann:termGroup rdf:resource="&geotime;Chronostratigraphic"/>	<vs:term_status>unstable</vs:term_status>	</skos:Concept>
<skos:Concept rdf:about="&geotime;Oligocene">	<skos:prefLabel xml:lang="en">Oligocene</skos:prefLabel>	<skos:definition>The Oligocene time period started 33.9  million years (Ma) before present (BP) and ended 23.03 Ma BP.</skos:definition>	<rdfs:seeAlso rdf:resource="http://kos.gbif.org/wiki/geotime:Oligocene"/>	<geotime:rangeType>Epoch</geotime:rangeType>	<geotime:rangeTypeURI rdf:resource="&geotime;Epoch"/>	<geotime:start>33.9</geotime:start>	<geotime:end>23.03</geotime:end>	<skos:narrower>Paleogene</skos:narrower>	<dcterms:created>2011-01-11</dcterms:created>	<dcterms:modified>2012-08-03</dcterms:modified>	<dcterms:hasVersion rdf:resource="&history;20120803/geotime#Oligocene"/>	<rdfs:isDefinedBy rdf:resource="&geotime;"/>	<skos:inScheme rdf:resource="&geotime;"/>	<vann:termGroup rdf:resource="&geotime;Epoch"/>	<vann:termGroup rdf:resource="&geotime;Chronostratigraphic"/>	<vs:term_status>unstable</vs:term_status>	</skos:Concept>
<skos:Concept rdf:about="&geotime;Eocene">	<skos:prefLabel xml:lang="en">Eocene</skos:prefLabel>	<skos:definition>The Eocene time period started 55.8  million years (Ma) before present (BP) and ended 33.9 Ma BP.</skos:definition>	<rdfs:seeAlso rdf:resource="http://kos.gbif.org/wiki/geotime:Eocene"/>	<geotime:rangeType>Epoch</geotime:rangeType>	<geotime:rangeTypeURI rdf:resource="&geotime;Epoch"/>	<geotime:start>55.8</geotime:start>	<geotime:end>33.9</geotime:end>	<skos:narrower>Paleogene</skos:narrower>	<dcterms:created>2011-01-11</dcterms:created>	<dcterms:modified>2012-08-03</dcterms:modified>	<dcterms:hasVersion rdf:resource="&history;20120803/geotime#Eocene"/>	<rdfs:isDefinedBy rdf:resource="&geotime;"/>	<skos:inScheme rdf:resource="&geotime;"/>	<vann:termGroup rdf:resource="&geotime;Epoch"/>	<vann:termGroup rdf:resource="&geotime;Chronostratigraphic"/>	<vs:term_status>unstable</vs:term_status>	</skos:Concept>
<skos:Concept rdf:about="&geotime;Paleocene">	<skos:prefLabel xml:lang="en">Paleocene</skos:prefLabel>	<skos:definition>The Paleocene time period started 65.5  million years (Ma) before present (BP) and ended 55.8 Ma BP.</skos:definition>	<rdfs:seeAlso rdf:resource="http://kos.gbif.org/wiki/geotime:Paleocene"/>	<geotime:rangeType>Epoch</geotime:rangeType>	<geotime:rangeTypeURI rdf:resource="&geotime;Epoch"/>	<geotime:start>65.5</geotime:start>	<geotime:end>55.8</geotime:end>	<skos:narrower>Paleogene</skos:narrower>	<dcterms:created>2011-01-11</dcterms:created>	<dcterms:modified>2012-08-03</dcterms:modified>	<dcterms:hasVersion rdf:resource="&history;20120803/geotime#Paleocene"/>	<rdfs:isDefinedBy rdf:resource="&geotime;"/>	<skos:inScheme rdf:resource="&geotime;"/>	<vann:termGroup rdf:resource="&geotime;Epoch"/>	<vann:termGroup rdf:resource="&geotime;Chronostratigraphic"/>	<vs:term_status>unstable</vs:term_status>	</skos:Concept>
<skos:Concept rdf:about="&geotime;LateCretaceous">	<skos:prefLabel xml:lang="en">Late Cretaceous</skos:prefLabel>	<skos:definition>The Late Cretaceous time period started 99.6  million years (Ma) before present (BP) and ended 65.5 Ma BP.</skos:definition>	<rdfs:seeAlso rdf:resource="http://kos.gbif.org/wiki/geotime:LateCretaceous"/>	<geotime:rangeType>Epoch</geotime:rangeType>	<geotime:rangeTypeURI rdf:resource="&geotime;Epoch"/>	<geotime:start>99.6</geotime:start>	<geotime:end>65.5</geotime:end>	<skos:narrower>Cretaceous</skos:narrower>	<dcterms:created>2011-01-11</dcterms:created>	<dcterms:modified>2012-08-03</dcterms:modified>	<dcterms:hasVersion rdf:resource="&history;20120803/geotime#LateCretaceous"/>	<rdfs:isDefinedBy rdf:resource="&geotime;"/>	<skos:inScheme rdf:resource="&geotime;"/>	<vann:termGroup rdf:resource="&geotime;Epoch"/>	<vann:termGroup rdf:resource="&geotime;Chronostratigraphic"/>	<vs:term_status>unstable</vs:term_status>	</skos:Concept>
<skos:Concept rdf:about="&geotime;EarlyCretaceous">	<skos:prefLabel xml:lang="en">Early Cretaceous</skos:prefLabel>	<skos:definition>The Early Cretaceous time period started 145.46  million years (Ma) before present (BP) and ended 99.6 Ma BP.</skos:definition>	<rdfs:seeAlso rdf:resource="http://kos.gbif.org/wiki/geotime:EarlyCretaceous"/>	<geotime:rangeType>Epoch</geotime:rangeType>	<geotime:rangeTypeURI rdf:resource="&geotime;Epoch"/>	<geotime:start>145.46</geotime:start>	<geotime:end>99.6</geotime:end>	<skos:narrower>Cretaceous</skos:narrower>	<dcterms:created>2011-01-11</dcterms:created>	<dcterms:modified>2012-08-03</dcterms:modified>	<dcterms:hasVersion rdf:resource="&history;20120803/geotime#EarlyCretaceous"/>	<rdfs:isDefinedBy rdf:resource="&geotime;"/>	<skos:inScheme rdf:resource="&geotime;"/>	<vann:termGroup rdf:resource="&geotime;Epoch"/>	<vann:termGroup rdf:resource="&geotime;Chronostratigraphic"/>	<vs:term_status>unstable</vs:term_status>	</skos:Concept>
<skos:Concept rdf:about="&geotime;LateJurassic">	<skos:prefLabel xml:lang="en">Late Jurassic</skos:prefLabel>	<skos:definition>The Late Jurassic time period started 161.21  million years (Ma) before present (BP) and ended 145.46 Ma BP.</skos:definition>	<rdfs:seeAlso rdf:resource="http://kos.gbif.org/wiki/geotime:LateJurassic"/>	<geotime:rangeType>Epoch</geotime:rangeType>	<geotime:rangeTypeURI rdf:resource="&geotime;Epoch"/>	<geotime:start>161.21</geotime:start>	<geotime:end>145.46</geotime:end>	<skos:narrower>Jurassic</skos:narrower>	<dcterms:created>2011-01-11</dcterms:created>	<dcterms:modified>2012-08-03</dcterms:modified>	<dcterms:hasVersion rdf:resource="&history;20120803/geotime#LateJurassic"/>	<rdfs:isDefinedBy rdf:resource="&geotime;"/>	<skos:inScheme rdf:resource="&geotime;"/>	<vann:termGroup rdf:resource="&geotime;Epoch"/>	<vann:termGroup rdf:resource="&geotime;Chronostratigraphic"/>	<vs:term_status>unstable</vs:term_status>	</skos:Concept>
<skos:Concept rdf:about="&geotime;MiddleJurassic">	<skos:prefLabel xml:lang="en">Middle Jurassic</skos:prefLabel>	<skos:definition>The Middle Jurassic time period started 175.6  million years (Ma) before present (BP) and ended 161.21 Ma BP.</skos:definition>	<rdfs:seeAlso rdf:resource="http://kos.gbif.org/wiki/geotime:MiddleJurassic"/>	<geotime:rangeType>Epoch</geotime:rangeType>	<geotime:rangeTypeURI rdf:resource="&geotime;Epoch"/>	<geotime:start>175.6</geotime:start>	<geotime:end>161.21</geotime:end>	<skos:narrower>Jurassic</skos:narrower>	<dcterms:created>2011-01-11</dcterms:created>	<dcterms:modified>2012-08-03</dcterms:modified>	<dcterms:hasVersion rdf:resource="&history;20120803/geotime#MiddleJurassic"/>	<rdfs:isDefinedBy rdf:resource="&geotime;"/>	<skos:inScheme rdf:resource="&geotime;"/>	<vann:termGroup rdf:resource="&geotime;Epoch"/>	<vann:termGroup rdf:resource="&geotime;Chronostratigraphic"/>	<vs:term_status>unstable</vs:term_status>	</skos:Concept>
<skos:Concept rdf:about="&geotime;EarlyJurassic">	<skos:prefLabel xml:lang="en">Early Jurassic</skos:prefLabel>	<skos:definition>The Early Jurassic time period started 199.6  million years (Ma) before present (BP) and ended 175.6 Ma BP.</skos:definition>	<rdfs:seeAlso rdf:resource="http://kos.gbif.org/wiki/geotime:EarlyJurassic"/>	<geotime:rangeType>Epoch</geotime:rangeType>	<geotime:rangeTypeURI rdf:resource="&geotime;Epoch"/>	<geotime:start>199.6</geotime:start>	<geotime:end>175.6</geotime:end>	<skos:narrower>Jurassic</skos:narrower>	<dcterms:created>2011-01-11</dcterms:created>	<dcterms:modified>2012-08-03</dcterms:modified>	<dcterms:hasVersion rdf:resource="&history;20120803/geotime#EarlyJurassic"/>	<rdfs:isDefinedBy rdf:resource="&geotime;"/>	<skos:inScheme rdf:resource="&geotime;"/>	<vann:termGroup rdf:resource="&geotime;Epoch"/>	<vann:termGroup rdf:resource="&geotime;Chronostratigraphic"/>	<vs:term_status>unstable</vs:term_status>	</skos:Concept>
<skos:Concept rdf:about="&geotime;LateTriassic">	<skos:prefLabel xml:lang="en">Late Triassic</skos:prefLabel>	<skos:definition>The Late Triassic time period started 228.01  million years (Ma) before present (BP) and ended 199.6 Ma BP.</skos:definition>	<rdfs:seeAlso rdf:resource="http://kos.gbif.org/wiki/geotime:LateTriassic"/>	<geotime:rangeType>Epoch</geotime:rangeType>	<geotime:rangeTypeURI rdf:resource="&geotime;Epoch"/>	<geotime:start>228.01</geotime:start>	<geotime:end>199.6</geotime:end>		<dcterms:created>2011-01-11</dcterms:created>	<dcterms:modified>2012-08-03</dcterms:modified>	<dcterms:hasVersion rdf:resource="&history;20120803/geotime#LateTriassic"/>	<rdfs:isDefinedBy rdf:resource="&geotime;"/>	<skos:inScheme rdf:resource="&geotime;"/>	<vann:termGroup rdf:resource="&geotime;Epoch"/>	<vann:termGroup rdf:resource="&geotime;Chronostratigraphic"/>	<vs:term_status>unstable</vs:term_status>	</skos:Concept>
<skos:Concept rdf:about="&geotime;MiddleTriassic">	<skos:prefLabel xml:lang="en">Middle Triassic</skos:prefLabel>	<skos:definition>The Middle Triassic time period started 245.17  million years (Ma) before present (BP) and ended 228.01 Ma BP.</skos:definition>	<rdfs:seeAlso rdf:resource="http://kos.gbif.org/wiki/geotime:MiddleTriassic"/>	<geotime:rangeType>Epoch</geotime:rangeType>	<geotime:rangeTypeURI rdf:resource="&geotime;Epoch"/>	<geotime:start>245.17</geotime:start>	<geotime:end>228.01</geotime:end>		<dcterms:created>2011-01-11</dcterms:created>	<dcterms:modified>2012-08-03</dcterms:modified>	<dcterms:hasVersion rdf:resource="&history;20120803/geotime#MiddleTriassic"/>	<rdfs:isDefinedBy rdf:resource="&geotime;"/>	<skos:inScheme rdf:resource="&geotime;"/>	<vann:termGroup rdf:resource="&geotime;Epoch"/>	<vann:termGroup rdf:resource="&geotime;Chronostratigraphic"/>	<vs:term_status>unstable</vs:term_status>	</skos:Concept>
<skos:Concept rdf:about="&geotime;EarlyTriassic">	<skos:prefLabel xml:lang="en">Early Triassic</skos:prefLabel>	<skos:definition>The Early Triassic time period started 251  million years (Ma) before present (BP) and ended 245.17 Ma BP.</skos:definition>	<rdfs:seeAlso rdf:resource="http://kos.gbif.org/wiki/geotime:EarlyTriassic"/>	<geotime:rangeType>Epoch</geotime:rangeType>	<geotime:rangeTypeURI rdf:resource="&geotime;Epoch"/>	<geotime:start>251</geotime:start>	<geotime:end>245.17</geotime:end>		<dcterms:created>2011-01-11</dcterms:created>	<dcterms:modified>2012-08-03</dcterms:modified>	<dcterms:hasVersion rdf:resource="&history;20120803/geotime#EarlyTriassic"/>	<rdfs:isDefinedBy rdf:resource="&geotime;"/>	<skos:inScheme rdf:resource="&geotime;"/>	<vann:termGroup rdf:resource="&geotime;Epoch"/>	<vann:termGroup rdf:resource="&geotime;Chronostratigraphic"/>	<vs:term_status>unstable</vs:term_status>	</skos:Concept>
<skos:Concept rdf:about="&geotime;LatePermian">	<skos:prefLabel xml:lang="en">Late Permian</skos:prefLabel>	<skos:definition>The Late Permian time period started 260.4  million years (Ma) before present (BP) and ended 251 Ma BP.</skos:definition>	<rdfs:seeAlso rdf:resource="http://kos.gbif.org/wiki/geotime:LatePermian"/>	<geotime:rangeType>Epoch</geotime:rangeType>	<geotime:rangeTypeURI rdf:resource="&geotime;Epoch"/>	<geotime:start>260.4</geotime:start>	<geotime:end>251</geotime:end>		<dcterms:created>2011-01-11</dcterms:created>	<dcterms:modified>2012-08-03</dcterms:modified>	<dcterms:hasVersion rdf:resource="&history;20120803/geotime#LatePermian"/>	<rdfs:isDefinedBy rdf:resource="&geotime;"/>	<skos:inScheme rdf:resource="&geotime;"/>	<vann:termGroup rdf:resource="&geotime;Epoch"/>	<vann:termGroup rdf:resource="&geotime;Chronostratigraphic"/>	<vs:term_status>unstable</vs:term_status>	</skos:Concept>
<skos:Concept rdf:about="&geotime;MiddlePermian">	<skos:prefLabel xml:lang="en">Middle Permian</skos:prefLabel>	<skos:definition>The Middle Permian time period started 270.6  million years (Ma) before present (BP) and ended 260.4 Ma BP.</skos:definition>	<rdfs:seeAlso rdf:resource="http://kos.gbif.org/wiki/geotime:MiddlePermian"/>	<geotime:rangeType>Epoch</geotime:rangeType>	<geotime:rangeTypeURI rdf:resource="&geotime;Epoch"/>	<geotime:start>270.6</geotime:start>	<geotime:end>260.4</geotime:end>		<dcterms:created>2011-01-11</dcterms:created>	<dcterms:modified>2012-08-03</dcterms:modified>	<dcterms:hasVersion rdf:resource="&history;20120803/geotime#MiddlePermian"/>	<rdfs:isDefinedBy rdf:resource="&geotime;"/>	<skos:inScheme rdf:resource="&geotime;"/>	<vann:termGroup rdf:resource="&geotime;Epoch"/>	<vann:termGroup rdf:resource="&geotime;Chronostratigraphic"/>	<vs:term_status>unstable</vs:term_status>	</skos:Concept>
<skos:Concept rdf:about="&geotime;EarlyPermian">	<skos:prefLabel xml:lang="en">Early Permian</skos:prefLabel>	<skos:definition>The Early Permian time period started 299  million years (Ma) before present (BP) and ended 270.6 Ma BP.</skos:definition>	<rdfs:seeAlso rdf:resource="http://kos.gbif.org/wiki/geotime:EarlyPermian"/>	<geotime:rangeType>Epoch</geotime:rangeType>	<geotime:rangeTypeURI rdf:resource="&geotime;Epoch"/>	<geotime:start>299</geotime:start>	<geotime:end>270.6</geotime:end>		<dcterms:created>2011-01-11</dcterms:created>	<dcterms:modified>2012-08-03</dcterms:modified>	<dcterms:hasVersion rdf:resource="&history;20120803/geotime#EarlyPermian"/>	<rdfs:isDefinedBy rdf:resource="&geotime;"/>	<skos:inScheme rdf:resource="&geotime;"/>	<vann:termGroup rdf:resource="&geotime;Epoch"/>	<vann:termGroup rdf:resource="&geotime;Chronostratigraphic"/>	<vs:term_status>unstable</vs:term_status>	</skos:Concept>
<skos:Concept rdf:about="&geotime;LatePennsylvanian">	<skos:prefLabel xml:lang="en">Late Pennsylvanian</skos:prefLabel>	<skos:definition>The Late Pennsylvanian time period started 306.5  million years (Ma) before present (BP) and ended 299 Ma BP.</skos:definition>	<rdfs:seeAlso rdf:resource="http://kos.gbif.org/wiki/geotime:LatePennsylvanian"/>	<geotime:rangeType>Epoch</geotime:rangeType>	<geotime:rangeTypeURI rdf:resource="&geotime;Epoch"/>	<geotime:start>306.5</geotime:start>	<geotime:end>299</geotime:end>		<dcterms:created>2011-01-11</dcterms:created>	<dcterms:modified>2012-08-03</dcterms:modified>	<dcterms:hasVersion rdf:resource="&history;20120803/geotime#LatePennsylvanian"/>	<rdfs:isDefinedBy rdf:resource="&geotime;"/>	<skos:inScheme rdf:resource="&geotime;"/>	<vann:termGroup rdf:resource="&geotime;Epoch"/>	<vann:termGroup rdf:resource="&geotime;Chronostratigraphic"/>	<vs:term_status>unstable</vs:term_status>	</skos:Concept>
<skos:Concept rdf:about="&geotime;MiddlePennsylvanian">	<skos:prefLabel xml:lang="en">Middle Pennsylvanian</skos:prefLabel>	<skos:definition>The Middle Pennsylvanian time period started 311.7  million years (Ma) before present (BP) and ended 306.5 Ma BP.</skos:definition>	<rdfs:seeAlso rdf:resource="http://kos.gbif.org/wiki/geotime:MiddlePennsylvanian"/>	<geotime:rangeType>Epoch</geotime:rangeType>	<geotime:rangeTypeURI rdf:resource="&geotime;Epoch"/>	<geotime:start>311.7</geotime:start>	<geotime:end>306.5</geotime:end>		<dcterms:created>2011-01-11</dcterms:created>	<dcterms:modified>2012-08-03</dcterms:modified>	<dcterms:hasVersion rdf:resource="&history;20120803/geotime#MiddlePennsylvanian"/>	<rdfs:isDefinedBy rdf:resource="&geotime;"/>	<skos:inScheme rdf:resource="&geotime;"/>	<vann:termGroup rdf:resource="&geotime;Epoch"/>	<vann:termGroup rdf:resource="&geotime;Chronostratigraphic"/>	<vs:term_status>unstable</vs:term_status>	</skos:Concept>
<skos:Concept rdf:about="&geotime;EarlyPennsylvanian">	<skos:prefLabel xml:lang="en">Early Pennsylvanian</skos:prefLabel>	<skos:definition>The Early Pennsylvanian time period started 318.1  million years (Ma) before present (BP) and ended 311.7 Ma BP.</skos:definition>	<rdfs:seeAlso rdf:resource="http://kos.gbif.org/wiki/geotime:EarlyPennsylvanian"/>	<geotime:rangeType>Epoch</geotime:rangeType>	<geotime:rangeTypeURI rdf:resource="&geotime;Epoch"/>	<geotime:start>318.1</geotime:start>	<geotime:end>311.7</geotime:end>		<dcterms:created>2011-01-11</dcterms:created>	<dcterms:modified>2012-08-03</dcterms:modified>	<dcterms:hasVersion rdf:resource="&history;20120803/geotime#EarlyPennsylvanian"/>	<rdfs:isDefinedBy rdf:resource="&geotime;"/>	<skos:inScheme rdf:resource="&geotime;"/>	<vann:termGroup rdf:resource="&geotime;Epoch"/>	<vann:termGroup rdf:resource="&geotime;Chronostratigraphic"/>	<vs:term_status>unstable</vs:term_status>	</skos:Concept>
<skos:Concept rdf:about="&geotime;LateMississippian">	<skos:prefLabel xml:lang="en">Late Mississippian</skos:prefLabel>	<skos:definition>The Late Mississippian time period started 326.4  million years (Ma) before present (BP) and ended 318.1 Ma BP.</skos:definition>	<rdfs:seeAlso rdf:resource="http://kos.gbif.org/wiki/geotime:LateMississippian"/>	<geotime:rangeType>Epoch</geotime:rangeType>	<geotime:rangeTypeURI rdf:resource="&geotime;Epoch"/>	<geotime:start>326.4</geotime:start>	<geotime:end>318.1</geotime:end>		<dcterms:created>2011-01-11</dcterms:created>	<dcterms:modified>2012-08-03</dcterms:modified>	<dcterms:hasVersion rdf:resource="&history;20120803/geotime#LateMississippian"/>	<rdfs:isDefinedBy rdf:resource="&geotime;"/>	<skos:inScheme rdf:resource="&geotime;"/>	<vann:termGroup rdf:resource="&geotime;Epoch"/>	<vann:termGroup rdf:resource="&geotime;Chronostratigraphic"/>	<vs:term_status>unstable</vs:term_status>	</skos:Concept>
<skos:Concept rdf:about="&geotime;MiddleMississippian">	<skos:prefLabel xml:lang="en">Middle Mississippian</skos:prefLabel>	<skos:definition>The Middle Mississippian time period started 345.3  million years (Ma) before present (BP) and ended 326.4 Ma BP.</skos:definition>	<rdfs:seeAlso rdf:resource="http://kos.gbif.org/wiki/geotime:MiddleMississippian"/>	<geotime:rangeType>Epoch</geotime:rangeType>	<geotime:rangeTypeURI rdf:resource="&geotime;Epoch"/>	<geotime:start>345.3</geotime:start>	<geotime:end>326.4</geotime:end>		<dcterms:created>2011-01-11</dcterms:created>	<dcterms:modified>2012-08-03</dcterms:modified>	<dcterms:hasVersion rdf:resource="&history;20120803/geotime#MiddleMississippian"/>	<rdfs:isDefinedBy rdf:resource="&geotime;"/>	<skos:inScheme rdf:resource="&geotime;"/>	<vann:termGroup rdf:resource="&geotime;Epoch"/>	<vann:termGroup rdf:resource="&geotime;Chronostratigraphic"/>	<vs:term_status>unstable</vs:term_status>	</skos:Concept>
<skos:Concept rdf:about="&geotime;EarlyMississippian">	<skos:prefLabel xml:lang="en">Early Mississippian</skos:prefLabel>	<skos:definition>The Early Mississippian time period started 359.2  million years (Ma) before present (BP) and ended 345.3 Ma BP.</skos:definition>	<rdfs:seeAlso rdf:resource="http://kos.gbif.org/wiki/geotime:EarlyMississippian"/>	<geotime:rangeType>Epoch</geotime:rangeType>	<geotime:rangeTypeURI rdf:resource="&geotime;Epoch"/>	<geotime:start>359.2</geotime:start>	<geotime:end>345.3</geotime:end>		<dcterms:created>2011-01-11</dcterms:created>	<dcterms:modified>2012-08-03</dcterms:modified>	<dcterms:hasVersion rdf:resource="&history;20120803/geotime#EarlyMississippian"/>	<rdfs:isDefinedBy rdf:resource="&geotime;"/>	<skos:inScheme rdf:resource="&geotime;"/>	<vann:termGroup rdf:resource="&geotime;Epoch"/>	<vann:termGroup rdf:resource="&geotime;Chronostratigraphic"/>	<vs:term_status>unstable</vs:term_status>	</skos:Concept>
<skos:Concept rdf:about="&geotime;LateDevonian">	<skos:prefLabel xml:lang="en">Late Devonian</skos:prefLabel>	<skos:definition>The Late Devonian time period started 385.3  million years (Ma) before present (BP) and ended 359.2 Ma BP.</skos:definition>	<rdfs:seeAlso rdf:resource="http://kos.gbif.org/wiki/geotime:LateDevonian"/>	<geotime:rangeType>Epoch</geotime:rangeType>	<geotime:rangeTypeURI rdf:resource="&geotime;Epoch"/>	<geotime:start>385.3</geotime:start>	<geotime:end>359.2</geotime:end>		<dcterms:created>2011-01-11</dcterms:created>	<dcterms:modified>2012-08-03</dcterms:modified>	<dcterms:hasVersion rdf:resource="&history;20120803/geotime#LateDevonian"/>	<rdfs:isDefinedBy rdf:resource="&geotime;"/>	<skos:inScheme rdf:resource="&geotime;"/>	<vann:termGroup rdf:resource="&geotime;Epoch"/>	<vann:termGroup rdf:resource="&geotime;Chronostratigraphic"/>	<vs:term_status>unstable</vs:term_status>	</skos:Concept>
<skos:Concept rdf:about="&geotime;MiddleDevonian">	<skos:prefLabel xml:lang="en">Middle Devonian</skos:prefLabel>	<skos:definition>The Middle Devonian time period started 397.5  million years (Ma) before present (BP) and ended 385.3 Ma BP.</skos:definition>	<rdfs:seeAlso rdf:resource="http://kos.gbif.org/wiki/geotime:MiddleDevonian"/>	<geotime:rangeType>Epoch</geotime:rangeType>	<geotime:rangeTypeURI rdf:resource="&geotime;Epoch"/>	<geotime:start>397.5</geotime:start>	<geotime:end>385.3</geotime:end>		<dcterms:created>2011-01-11</dcterms:created>	<dcterms:modified>2012-08-03</dcterms:modified>	<dcterms:hasVersion rdf:resource="&history;20120803/geotime#MiddleDevonian"/>	<rdfs:isDefinedBy rdf:resource="&geotime;"/>	<skos:inScheme rdf:resource="&geotime;"/>	<vann:termGroup rdf:resource="&geotime;Epoch"/>	<vann:termGroup rdf:resource="&geotime;Chronostratigraphic"/>	<vs:term_status>unstable</vs:term_status>	</skos:Concept>
<skos:Concept rdf:about="&geotime;EarlyDevonian">	<skos:prefLabel xml:lang="en">Early Devonian</skos:prefLabel>	<skos:definition>The Early Devonian time period started 416  million years (Ma) before present (BP) and ended 397.5 Ma BP.</skos:definition>	<rdfs:seeAlso rdf:resource="http://kos.gbif.org/wiki/geotime:EarlyDevonian"/>	<geotime:rangeType>Epoch</geotime:rangeType>	<geotime:rangeTypeURI rdf:resource="&geotime;Epoch"/>	<geotime:start>416</geotime:start>	<geotime:end>397.5</geotime:end>		<dcterms:created>2011-01-11</dcterms:created>	<dcterms:modified>2012-08-03</dcterms:modified>	<dcterms:hasVersion rdf:resource="&history;20120803/geotime#EarlyDevonian"/>	<rdfs:isDefinedBy rdf:resource="&geotime;"/>	<skos:inScheme rdf:resource="&geotime;"/>	<vann:termGroup rdf:resource="&geotime;Epoch"/>	<vann:termGroup rdf:resource="&geotime;Chronostratigraphic"/>	<vs:term_status>unstable</vs:term_status>	</skos:Concept>
<skos:Concept rdf:about="&geotime;latestSilurian">	<skos:prefLabel xml:lang="en">latest Silurian</skos:prefLabel>	<skos:definition>The latest Silurian time period started 418.7  million years (Ma) before present (BP) and ended 416 Ma BP.</skos:definition>	<rdfs:seeAlso rdf:resource="http://kos.gbif.org/wiki/geotime:latestSilurian"/>	<geotime:rangeType>Epoch</geotime:rangeType>	<geotime:rangeTypeURI rdf:resource="&geotime;Epoch"/>	<geotime:start>418.7</geotime:start>	<geotime:end>416</geotime:end>		<dcterms:created>2011-01-11</dcterms:created>	<dcterms:modified>2012-08-03</dcterms:modified>	<dcterms:hasVersion rdf:resource="&history;20120803/geotime#latestSilurian"/>	<rdfs:isDefinedBy rdf:resource="&geotime;"/>	<skos:inScheme rdf:resource="&geotime;"/>	<vann:termGroup rdf:resource="&geotime;Epoch"/>	<vann:termGroup rdf:resource="&geotime;Chronostratigraphic"/>	<vs:term_status>unstable</vs:term_status>	</skos:Concept>
<skos:Concept rdf:about="&geotime;LateSilurian">	<skos:prefLabel xml:lang="en">Late Silurian</skos:prefLabel>	<skos:definition>The Late Silurian time period started 422.9  million years (Ma) before present (BP) and ended 418.7 Ma BP.</skos:definition>	<rdfs:seeAlso rdf:resource="http://kos.gbif.org/wiki/geotime:LateSilurian"/>	<geotime:rangeType>Epoch</geotime:rangeType>	<geotime:rangeTypeURI rdf:resource="&geotime;Epoch"/>	<geotime:start>422.9</geotime:start>	<geotime:end>418.7</geotime:end>		<dcterms:created>2011-01-11</dcterms:created>	<dcterms:modified>2012-08-03</dcterms:modified>	<dcterms:hasVersion rdf:resource="&history;20120803/geotime#LateSilurian"/>	<rdfs:isDefinedBy rdf:resource="&geotime;"/>	<skos:inScheme rdf:resource="&geotime;"/>	<vann:termGroup rdf:resource="&geotime;Epoch"/>	<vann:termGroup rdf:resource="&geotime;Chronostratigraphic"/>	<vs:term_status>unstable</vs:term_status>	</skos:Concept>
<skos:Concept rdf:about="&geotime;MiddleSilurian">	<skos:prefLabel xml:lang="en">Middle Silurian</skos:prefLabel>	<skos:definition>The Middle Silurian time period started 428.2  million years (Ma) before present (BP) and ended 422.9 Ma BP.</skos:definition>	<rdfs:seeAlso rdf:resource="http://kos.gbif.org/wiki/geotime:MiddleSilurian"/>	<geotime:rangeType>Epoch</geotime:rangeType>	<geotime:rangeTypeURI rdf:resource="&geotime;Epoch"/>	<geotime:start>428.2</geotime:start>	<geotime:end>422.9</geotime:end>		<dcterms:created>2011-01-11</dcterms:created>	<dcterms:modified>2012-08-03</dcterms:modified>	<dcterms:hasVersion rdf:resource="&history;20120803/geotime#MiddleSilurian"/>	<rdfs:isDefinedBy rdf:resource="&geotime;"/>	<skos:inScheme rdf:resource="&geotime;"/>	<vann:termGroup rdf:resource="&geotime;Epoch"/>	<vann:termGroup rdf:resource="&geotime;Chronostratigraphic"/>	<vs:term_status>unstable</vs:term_status>	</skos:Concept>
<skos:Concept rdf:about="&geotime;EarlySilurian">	<skos:prefLabel xml:lang="en">Early Silurian</skos:prefLabel>	<skos:definition>The Early Silurian time period started 443.7  million years (Ma) before present (BP) and ended 428.2 Ma BP.</skos:definition>	<rdfs:seeAlso rdf:resource="http://kos.gbif.org/wiki/geotime:EarlySilurian"/>	<geotime:rangeType>Epoch</geotime:rangeType>	<geotime:rangeTypeURI rdf:resource="&geotime;Epoch"/>	<geotime:start>443.7</geotime:start>	<geotime:end>428.2</geotime:end>		<dcterms:created>2011-01-11</dcterms:created>	<dcterms:modified>2012-08-03</dcterms:modified>	<dcterms:hasVersion rdf:resource="&history;20120803/geotime#EarlySilurian"/>	<rdfs:isDefinedBy rdf:resource="&geotime;"/>	<skos:inScheme rdf:resource="&geotime;"/>	<vann:termGroup rdf:resource="&geotime;Epoch"/>	<vann:termGroup rdf:resource="&geotime;Chronostratigraphic"/>	<vs:term_status>unstable</vs:term_status>	</skos:Concept>
<skos:Concept rdf:about="&geotime;LateOrdovician">	<skos:prefLabel xml:lang="en">Late Ordovician</skos:prefLabel>	<skos:definition>The Late Ordovician time period started 460.9  million years (Ma) before present (BP) and ended 443.7 Ma BP.</skos:definition>	<rdfs:seeAlso rdf:resource="http://kos.gbif.org/wiki/geotime:LateOrdovician"/>	<geotime:rangeType>Epoch</geotime:rangeType>	<geotime:rangeTypeURI rdf:resource="&geotime;Epoch"/>	<geotime:start>460.9</geotime:start>	<geotime:end>443.7</geotime:end>		<dcterms:created>2011-01-11</dcterms:created>	<dcterms:modified>2012-08-03</dcterms:modified>	<dcterms:hasVersion rdf:resource="&history;20120803/geotime#LateOrdovician"/>	<rdfs:isDefinedBy rdf:resource="&geotime;"/>	<skos:inScheme rdf:resource="&geotime;"/>	<vann:termGroup rdf:resource="&geotime;Epoch"/>	<vann:termGroup rdf:resource="&geotime;Chronostratigraphic"/>	<vs:term_status>unstable</vs:term_status>	</skos:Concept>
<skos:Concept rdf:about="&geotime;MiddleOrdovician">	<skos:prefLabel xml:lang="en">Middle Ordovician</skos:prefLabel>	<skos:definition>The Middle Ordovician time period started 471.8  million years (Ma) before present (BP) and ended 460.9 Ma BP.</skos:definition>	<rdfs:seeAlso rdf:resource="http://kos.gbif.org/wiki/geotime:MiddleOrdovician"/>	<geotime:rangeType>Epoch</geotime:rangeType>	<geotime:rangeTypeURI rdf:resource="&geotime;Epoch"/>	<geotime:start>471.8</geotime:start>	<geotime:end>460.9</geotime:end>		<dcterms:created>2011-01-11</dcterms:created>	<dcterms:modified>2012-08-03</dcterms:modified>	<dcterms:hasVersion rdf:resource="&history;20120803/geotime#MiddleOrdovician"/>	<rdfs:isDefinedBy rdf:resource="&geotime;"/>	<skos:inScheme rdf:resource="&geotime;"/>	<vann:termGroup rdf:resource="&geotime;Epoch"/>	<vann:termGroup rdf:resource="&geotime;Chronostratigraphic"/>	<vs:term_status>unstable</vs:term_status>	</skos:Concept>
<skos:Concept rdf:about="&geotime;EarlyOrdovician">	<skos:prefLabel xml:lang="en">Early Ordovician</skos:prefLabel>	<skos:definition>The Early Ordovician time period started 488.3  million years (Ma) before present (BP) and ended 471.8 Ma BP.</skos:definition>	<rdfs:seeAlso rdf:resource="http://kos.gbif.org/wiki/geotime:EarlyOrdovician"/>	<geotime:rangeType>Epoch</geotime:rangeType>	<geotime:rangeTypeURI rdf:resource="&geotime;Epoch"/>	<geotime:start>488.3</geotime:start>	<geotime:end>471.8</geotime:end>		<dcterms:created>2011-01-11</dcterms:created>	<dcterms:modified>2012-08-03</dcterms:modified>	<dcterms:hasVersion rdf:resource="&history;20120803/geotime#EarlyOrdovician"/>	<rdfs:isDefinedBy rdf:resource="&geotime;"/>	<skos:inScheme rdf:resource="&geotime;"/>	<vann:termGroup rdf:resource="&geotime;Epoch"/>	<vann:termGroup rdf:resource="&geotime;Chronostratigraphic"/>	<vs:term_status>unstable</vs:term_status>	</skos:Concept>
<skos:Concept rdf:about="&geotime;LateCambrian">	<skos:prefLabel xml:lang="en">Late Cambrian</skos:prefLabel>	<skos:definition>The Late Cambrian time period started 501  million years (Ma) before present (BP) and ended 488.3 Ma BP.</skos:definition>	<rdfs:seeAlso rdf:resource="http://kos.gbif.org/wiki/geotime:LateCambrian"/>	<geotime:rangeType>Epoch</geotime:rangeType>	<geotime:rangeTypeURI rdf:resource="&geotime;Epoch"/>	<geotime:start>501</geotime:start>	<geotime:end>488.3</geotime:end>		<dcterms:created>2011-01-11</dcterms:created>	<dcterms:modified>2012-08-03</dcterms:modified>	<dcterms:hasVersion rdf:resource="&history;20120803/geotime#LateCambrian"/>	<rdfs:isDefinedBy rdf:resource="&geotime;"/>	<skos:inScheme rdf:resource="&geotime;"/>	<vann:termGroup rdf:resource="&geotime;Epoch"/>	<vann:termGroup rdf:resource="&geotime;Chronostratigraphic"/>	<vs:term_status>unstable</vs:term_status>	</skos:Concept>
<skos:Concept rdf:about="&geotime;MiddleCambrian">	<skos:prefLabel xml:lang="en">Middle Cambrian</skos:prefLabel>	<skos:definition>The Middle Cambrian time period started 513  million years (Ma) before present (BP) and ended 501 Ma BP.</skos:definition>	<rdfs:seeAlso rdf:resource="http://kos.gbif.org/wiki/geotime:MiddleCambrian"/>	<geotime:rangeType>Epoch</geotime:rangeType>	<geotime:rangeTypeURI rdf:resource="&geotime;Epoch"/>	<geotime:start>513</geotime:start>	<geotime:end>501</geotime:end>		<dcterms:created>2011-01-11</dcterms:created>	<dcterms:modified>2012-08-03</dcterms:modified>	<dcterms:hasVersion rdf:resource="&history;20120803/geotime#MiddleCambrian"/>	<rdfs:isDefinedBy rdf:resource="&geotime;"/>	<skos:inScheme rdf:resource="&geotime;"/>	<vann:termGroup rdf:resource="&geotime;Epoch"/>	<vann:termGroup rdf:resource="&geotime;Chronostratigraphic"/>	<vs:term_status>unstable</vs:term_status>	</skos:Concept>
<skos:Concept rdf:about="&geotime;EarlyCambrian">	<skos:prefLabel xml:lang="en">Early Cambrian</skos:prefLabel>	<skos:definition>The Early Cambrian time period started 542  million years (Ma) before present (BP) and ended 513 Ma BP.</skos:definition>	<rdfs:seeAlso rdf:resource="http://kos.gbif.org/wiki/geotime:EarlyCambrian"/>	<geotime:rangeType>Epoch</geotime:rangeType>	<geotime:rangeTypeURI rdf:resource="&geotime;Epoch"/>	<geotime:start>542</geotime:start>	<geotime:end>513</geotime:end>		<dcterms:created>2011-01-11</dcterms:created>	<dcterms:modified>2012-08-03</dcterms:modified>	<dcterms:hasVersion rdf:resource="&history;20120803/geotime#EarlyCambrian"/>	<rdfs:isDefinedBy rdf:resource="&geotime;"/>	<skos:inScheme rdf:resource="&geotime;"/>	<vann:termGroup rdf:resource="&geotime;Epoch"/>	<vann:termGroup rdf:resource="&geotime;Chronostratigraphic"/>	<vs:term_status>unstable</vs:term_status>	</skos:Concept>
<skos:Concept rdf:about="&geotime;Cenozoic">	<skos:prefLabel xml:lang="en">Cenozoic</skos:prefLabel>	<skos:definition>The Cenozoic time period started 65.5  million years (Ma) before present (BP) and ended 0 Ma BP.</skos:definition>	<rdfs:seeAlso rdf:resource="http://kos.gbif.org/wiki/geotime:Cenozoic"/>	<geotime:rangeType>Era</geotime:rangeType>	<geotime:rangeTypeURI rdf:resource="&geotime;Era"/>	<geotime:start>65.5</geotime:start>	<geotime:end>0</geotime:end>	<skos:narrower>Phanerozoic</skos:narrower>	<dcterms:created>2011-01-11</dcterms:created>	<dcterms:modified>2012-08-03</dcterms:modified>	<dcterms:hasVersion rdf:resource="&history;20120803/geotime#Cenozoic"/>	<rdfs:isDefinedBy rdf:resource="&geotime;"/>	<skos:inScheme rdf:resource="&geotime;"/>	<vann:termGroup rdf:resource="&geotime;Era"/>	<vann:termGroup rdf:resource="&geotime;Chronostratigraphic"/>	<vs:term_status>unstable</vs:term_status>	</skos:Concept>
<skos:Concept rdf:about="&geotime;Mesozoic">	<skos:prefLabel xml:lang="en">Mesozoic</skos:prefLabel>	<skos:definition>The Mesozoic time period started 251  million years (Ma) before present (BP) and ended 65.5 Ma BP.</skos:definition>	<rdfs:seeAlso rdf:resource="http://kos.gbif.org/wiki/geotime:Mesozoic"/>	<geotime:rangeType>Era</geotime:rangeType>	<geotime:rangeTypeURI rdf:resource="&geotime;Era"/>	<geotime:start>251</geotime:start>	<geotime:end>65.5</geotime:end>	<skos:narrower>Phanerozoic</skos:narrower>	<dcterms:created>2011-01-11</dcterms:created>	<dcterms:modified>2012-08-03</dcterms:modified>	<dcterms:hasVersion rdf:resource="&history;20120803/geotime#Mesozoic"/>	<rdfs:isDefinedBy rdf:resource="&geotime;"/>	<skos:inScheme rdf:resource="&geotime;"/>	<vann:termGroup rdf:resource="&geotime;Era"/>	<vann:termGroup rdf:resource="&geotime;Chronostratigraphic"/>	<vs:term_status>unstable</vs:term_status>	</skos:Concept>
<skos:Concept rdf:about="&geotime;Paleozoic">	<skos:prefLabel xml:lang="en">Paleozoic</skos:prefLabel>	<skos:definition>The Paleozoic time period started 542  million years (Ma) before present (BP) and ended 251 Ma BP.</skos:definition>	<rdfs:seeAlso rdf:resource="http://kos.gbif.org/wiki/geotime:Paleozoic"/>	<geotime:rangeType>Era</geotime:rangeType>	<geotime:rangeTypeURI rdf:resource="&geotime;Era"/>	<geotime:start>542</geotime:start>	<geotime:end>251</geotime:end>	<skos:narrower>Phanerozoic</skos:narrower>	<dcterms:created>2011-01-11</dcterms:created>	<dcterms:modified>2012-08-03</dcterms:modified>	<dcterms:hasVersion rdf:resource="&history;20120803/geotime#Paleozoic"/>	<rdfs:isDefinedBy rdf:resource="&geotime;"/>	<skos:inScheme rdf:resource="&geotime;"/>	<vann:termGroup rdf:resource="&geotime;Era"/>	<vann:termGroup rdf:resource="&geotime;Chronostratigraphic"/>	<vs:term_status>unstable</vs:term_status>	</skos:Concept>
<skos:Concept rdf:about="&geotime;Neoproterozoic">	<skos:prefLabel xml:lang="en">Neoproterozoic</skos:prefLabel>	<skos:definition>The Neoproterozoic time period started 1000  million years (Ma) before present (BP) and ended 542 Ma BP.</skos:definition>	<rdfs:seeAlso rdf:resource="http://kos.gbif.org/wiki/geotime:Neoproterozoic"/>	<geotime:rangeType>Era</geotime:rangeType>	<geotime:rangeTypeURI rdf:resource="&geotime;Era"/>	<geotime:start>1000</geotime:start>	<geotime:end>542</geotime:end>	<skos:narrower>Proterozoic</skos:narrower>	<dcterms:created>2011-01-11</dcterms:created>	<dcterms:modified>2012-08-03</dcterms:modified>	<dcterms:hasVersion rdf:resource="&history;20120803/geotime#Neoproterozoic"/>	<rdfs:isDefinedBy rdf:resource="&geotime;"/>	<skos:inScheme rdf:resource="&geotime;"/>	<vann:termGroup rdf:resource="&geotime;Era"/>	<vann:termGroup rdf:resource="&geotime;Chronostratigraphic"/>	<vs:term_status>unstable</vs:term_status>	</skos:Concept>
<skos:Concept rdf:about="&geotime;Mesoproterozoic">	<skos:prefLabel xml:lang="en">Mesoproterozoic</skos:prefLabel>	<skos:definition>The Mesoproterozoic time period started 1600  million years (Ma) before present (BP) and ended 1000 Ma BP.</skos:definition>	<rdfs:seeAlso rdf:resource="http://kos.gbif.org/wiki/geotime:Mesoproterozoic"/>	<geotime:rangeType>Era</geotime:rangeType>	<geotime:rangeTypeURI rdf:resource="&geotime;Era"/>	<geotime:start>1600</geotime:start>	<geotime:end>1000</geotime:end>	<skos:narrower>Proterozoic</skos:narrower>	<dcterms:created>2011-01-11</dcterms:created>	<dcterms:modified>2012-08-03</dcterms:modified>	<dcterms:hasVersion rdf:resource="&history;20120803/geotime#Mesoproterozoic"/>	<rdfs:isDefinedBy rdf:resource="&geotime;"/>	<skos:inScheme rdf:resource="&geotime;"/>	<vann:termGroup rdf:resource="&geotime;Era"/>	<vann:termGroup rdf:resource="&geotime;Chronostratigraphic"/>	<vs:term_status>unstable</vs:term_status>	</skos:Concept>
<skos:Concept rdf:about="&geotime;Paleoproterozoic">	<skos:prefLabel xml:lang="en">Paleoproterozoic</skos:prefLabel>	<skos:definition>The Paleoproterozoic time period started 2500  million years (Ma) before present (BP) and ended 1600 Ma BP.</skos:definition>	<rdfs:seeAlso rdf:resource="http://kos.gbif.org/wiki/geotime:Paleoproterozoic"/>	<geotime:rangeType>Era</geotime:rangeType>	<geotime:rangeTypeURI rdf:resource="&geotime;Era"/>	<geotime:start>2500</geotime:start>	<geotime:end>1600</geotime:end>	<skos:narrower>Proterozoic</skos:narrower>	<dcterms:created>2011-01-11</dcterms:created>	<dcterms:modified>2012-08-03</dcterms:modified>	<dcterms:hasVersion rdf:resource="&history;20120803/geotime#Paleoproterozoic"/>	<rdfs:isDefinedBy rdf:resource="&geotime;"/>	<skos:inScheme rdf:resource="&geotime;"/>	<vann:termGroup rdf:resource="&geotime;Era"/>	<vann:termGroup rdf:resource="&geotime;Chronostratigraphic"/>	<vs:term_status>unstable</vs:term_status>	</skos:Concept>
<skos:Concept rdf:about="&geotime;Neoarchean">	<skos:prefLabel xml:lang="en">Neoarchean</skos:prefLabel>	<skos:definition>The Neoarchean time period started 2800  million years (Ma) before present (BP) and ended 2500 Ma BP.</skos:definition>	<rdfs:seeAlso rdf:resource="http://kos.gbif.org/wiki/geotime:Neoarchean"/>	<geotime:rangeType>Era</geotime:rangeType>	<geotime:rangeTypeURI rdf:resource="&geotime;Era"/>	<geotime:start>2800</geotime:start>	<geotime:end>2500</geotime:end>	<skos:narrower>Archean</skos:narrower>	<dcterms:created>2011-01-11</dcterms:created>	<dcterms:modified>2012-08-03</dcterms:modified>	<dcterms:hasVersion rdf:resource="&history;20120803/geotime#Neoarchean"/>	<rdfs:isDefinedBy rdf:resource="&geotime;"/>	<skos:inScheme rdf:resource="&geotime;"/>	<vann:termGroup rdf:resource="&geotime;Era"/>	<vann:termGroup rdf:resource="&geotime;Chronostratigraphic"/>	<vs:term_status>unstable</vs:term_status>	</skos:Concept>
<skos:Concept rdf:about="&geotime;Mesoarchean">	<skos:prefLabel xml:lang="en">Mesoarchean</skos:prefLabel>	<skos:definition>The Mesoarchean time period started 3200  million years (Ma) before present (BP) and ended 2800 Ma BP.</skos:definition>	<rdfs:seeAlso rdf:resource="http://kos.gbif.org/wiki/geotime:Mesoarchean"/>	<geotime:rangeType>Era</geotime:rangeType>	<geotime:rangeTypeURI rdf:resource="&geotime;Era"/>	<geotime:start>3200</geotime:start>	<geotime:end>2800</geotime:end>	<skos:narrower>Archean</skos:narrower>	<dcterms:created>2011-01-11</dcterms:created>	<dcterms:modified>2012-08-03</dcterms:modified>	<dcterms:hasVersion rdf:resource="&history;20120803/geotime#Mesoarchean"/>	<rdfs:isDefinedBy rdf:resource="&geotime;"/>	<skos:inScheme rdf:resource="&geotime;"/>	<vann:termGroup rdf:resource="&geotime;Era"/>	<vann:termGroup rdf:resource="&geotime;Chronostratigraphic"/>	<vs:term_status>unstable</vs:term_status>	</skos:Concept>
<skos:Concept rdf:about="&geotime;Paleoarchean">	<skos:prefLabel xml:lang="en">Paleoarchean</skos:prefLabel>	<skos:definition>The Paleoarchean time period started 3600  million years (Ma) before present (BP) and ended 3200 Ma BP.</skos:definition>	<rdfs:seeAlso rdf:resource="http://kos.gbif.org/wiki/geotime:Paleoarchean"/>	<geotime:rangeType>Era</geotime:rangeType>	<geotime:rangeTypeURI rdf:resource="&geotime;Era"/>	<geotime:start>3600</geotime:start>	<geotime:end>3200</geotime:end>	<skos:narrower>Archean</skos:narrower>	<dcterms:created>2011-01-11</dcterms:created>	<dcterms:modified>2012-08-03</dcterms:modified>	<dcterms:hasVersion rdf:resource="&history;20120803/geotime#Paleoarchean"/>	<rdfs:isDefinedBy rdf:resource="&geotime;"/>	<skos:inScheme rdf:resource="&geotime;"/>	<vann:termGroup rdf:resource="&geotime;Era"/>	<vann:termGroup rdf:resource="&geotime;Chronostratigraphic"/>	<vs:term_status>unstable</vs:term_status>	</skos:Concept>
<skos:Concept rdf:about="&geotime;EoarcheanHadean">	<skos:prefLabel xml:lang="en">Eoarchean Hadean</skos:prefLabel>	<skos:definition>The Eoarchean Hadean time period started 4500  million years (Ma) before present (BP) and ended 3600 Ma BP.</skos:definition>	<rdfs:seeAlso rdf:resource="http://kos.gbif.org/wiki/geotime:EoarcheanHadean"/>	<geotime:rangeType>Era</geotime:rangeType>	<geotime:rangeTypeURI rdf:resource="&geotime;Era"/>	<geotime:start>4500</geotime:start>	<geotime:end>3600</geotime:end>	<skos:narrower>Archean</skos:narrower>	<dcterms:created>2011-01-11</dcterms:created>	<dcterms:modified>2012-08-03</dcterms:modified>	<dcterms:hasVersion rdf:resource="&history;20120803/geotime#EoarcheanHadean"/>	<rdfs:isDefinedBy rdf:resource="&geotime;"/>	<skos:inScheme rdf:resource="&geotime;"/>	<vann:termGroup rdf:resource="&geotime;Era"/>	<vann:termGroup rdf:resource="&geotime;Chronostratigraphic"/>	<vs:term_status>unstable</vs:term_status>	</skos:Concept>
<skos:Concept rdf:about="&geotime;Neogene">	<skos:prefLabel xml:lang="en">Neogene</skos:prefLabel>	<skos:definition>The Neogene time period started 23.03  million years (Ma) before present (BP) and ended 0 Ma BP.</skos:definition>	<rdfs:seeAlso rdf:resource="http://kos.gbif.org/wiki/geotime:Neogene"/>	<geotime:rangeType>Period</geotime:rangeType>	<geotime:rangeTypeURI rdf:resource="&geotime;Period"/>	<geotime:start>23.03</geotime:start>	<geotime:end>0</geotime:end>	<skos:narrower>Phanerozoic</skos:narrower>	<dcterms:created>2011-01-11</dcterms:created>	<dcterms:modified>2012-08-03</dcterms:modified>	<dcterms:hasVersion rdf:resource="&history;20120803/geotime#Neogene"/>	<rdfs:isDefinedBy rdf:resource="&geotime;"/>	<skos:inScheme rdf:resource="&geotime;"/>	<vann:termGroup rdf:resource="&geotime;Period"/>	<vann:termGroup rdf:resource="&geotime;Chronostratigraphic"/>	<vs:term_status>unstable</vs:term_status>	</skos:Concept>
<skos:Concept rdf:about="&geotime;Paleogene">	<skos:prefLabel xml:lang="en">Paleogene</skos:prefLabel>	<skos:definition>The Paleogene time period started 65.5  million years (Ma) before present (BP) and ended 23.03 Ma BP.</skos:definition>	<rdfs:seeAlso rdf:resource="http://kos.gbif.org/wiki/geotime:Paleogene"/>	<geotime:rangeType>Period</geotime:rangeType>	<geotime:rangeTypeURI rdf:resource="&geotime;Period"/>	<geotime:start>65.5</geotime:start>	<geotime:end>23.03</geotime:end>	<skos:narrower>Cenozoic</skos:narrower>	<dcterms:created>2011-01-11</dcterms:created>	<dcterms:modified>2012-08-03</dcterms:modified>	<dcterms:hasVersion rdf:resource="&history;20120803/geotime#Paleogene"/>	<rdfs:isDefinedBy rdf:resource="&geotime;"/>	<skos:inScheme rdf:resource="&geotime;"/>	<vann:termGroup rdf:resource="&geotime;Period"/>	<vann:termGroup rdf:resource="&geotime;Chronostratigraphic"/>	<vs:term_status>unstable</vs:term_status>	</skos:Concept>
<skos:Concept rdf:about="&geotime;Cretaceous">	<skos:prefLabel xml:lang="en">Cretaceous</skos:prefLabel>	<skos:definition>The Cretaceous time period started 145.46  million years (Ma) before present (BP) and ended 65.5 Ma BP.</skos:definition>	<rdfs:seeAlso rdf:resource="http://kos.gbif.org/wiki/geotime:Cretaceous"/>	<geotime:rangeType>Period</geotime:rangeType>	<geotime:rangeTypeURI rdf:resource="&geotime;Period"/>	<geotime:start>145.46</geotime:start>	<geotime:end>65.5</geotime:end>	<skos:narrower>Mesozoic</skos:narrower>	<dcterms:created>2011-01-11</dcterms:created>	<dcterms:modified>2012-08-03</dcterms:modified>	<dcterms:hasVersion rdf:resource="&history;20120803/geotime#Cretaceous"/>	<rdfs:isDefinedBy rdf:resource="&geotime;"/>	<skos:inScheme rdf:resource="&geotime;"/>	<vann:termGroup rdf:resource="&geotime;Period"/>	<vann:termGroup rdf:resource="&geotime;Chronostratigraphic"/>	<vs:term_status>unstable</vs:term_status>	</skos:Concept>
<skos:Concept rdf:about="&geotime;Jurassic">	<skos:prefLabel xml:lang="en">Jurassic</skos:prefLabel>	<skos:definition>The Jurassic time period started 199.6  million years (Ma) before present (BP) and ended 145.46 Ma BP.</skos:definition>	<rdfs:seeAlso rdf:resource="http://kos.gbif.org/wiki/geotime:Jurassic"/>	<geotime:rangeType>Period</geotime:rangeType>	<geotime:rangeTypeURI rdf:resource="&geotime;Period"/>	<geotime:start>199.6</geotime:start>	<geotime:end>145.46</geotime:end>	<skos:narrower>Mesozoic</skos:narrower>	<dcterms:created>2011-01-11</dcterms:created>	<dcterms:modified>2012-08-03</dcterms:modified>	<dcterms:hasVersion rdf:resource="&history;20120803/geotime#Jurassic"/>	<rdfs:isDefinedBy rdf:resource="&geotime;"/>	<skos:inScheme rdf:resource="&geotime;"/>	<vann:termGroup rdf:resource="&geotime;Period"/>	<vann:termGroup rdf:resource="&geotime;Chronostratigraphic"/>	<vs:term_status>unstable</vs:term_status>	</skos:Concept>
<skos:Concept rdf:about="&geotime;Triassic">	<skos:prefLabel xml:lang="en">Triassic</skos:prefLabel>	<skos:definition>The Triassic time period started 251  million years (Ma) before present (BP) and ended 199.6 Ma BP.</skos:definition>	<rdfs:seeAlso rdf:resource="http://kos.gbif.org/wiki/geotime:Triassic"/>	<geotime:rangeType>Period</geotime:rangeType>	<geotime:rangeTypeURI rdf:resource="&geotime;Period"/>	<geotime:start>251</geotime:start>	<geotime:end>199.6</geotime:end>	<skos:narrower>Mesozoic</skos:narrower>	<dcterms:created>2011-01-11</dcterms:created>	<dcterms:modified>2012-08-03</dcterms:modified>	<dcterms:hasVersion rdf:resource="&history;20120803/geotime#Triassic"/>	<rdfs:isDefinedBy rdf:resource="&geotime;"/>	<skos:inScheme rdf:resource="&geotime;"/>	<vann:termGroup rdf:resource="&geotime;Period"/>	<vann:termGroup rdf:resource="&geotime;Chronostratigraphic"/>	<vs:term_status>unstable</vs:term_status>	</skos:Concept>
<skos:Concept rdf:about="&geotime;Permian">	<skos:prefLabel xml:lang="en">Permian</skos:prefLabel>	<skos:definition>The Permian time period started 299  million years (Ma) before present (BP) and ended 251 Ma BP.</skos:definition>	<rdfs:seeAlso rdf:resource="http://kos.gbif.org/wiki/geotime:Permian"/>	<geotime:rangeType>Period</geotime:rangeType>	<geotime:rangeTypeURI rdf:resource="&geotime;Period"/>	<geotime:start>299</geotime:start>	<geotime:end>251</geotime:end>	<skos:narrower>Paleozoic</skos:narrower>	<dcterms:created>2011-01-11</dcterms:created>	<dcterms:modified>2012-08-03</dcterms:modified>	<dcterms:hasVersion rdf:resource="&history;20120803/geotime#Permian"/>	<rdfs:isDefinedBy rdf:resource="&geotime;"/>	<skos:inScheme rdf:resource="&geotime;"/>	<vann:termGroup rdf:resource="&geotime;Period"/>	<vann:termGroup rdf:resource="&geotime;Chronostratigraphic"/>	<vs:term_status>unstable</vs:term_status>	</skos:Concept>
<skos:Concept rdf:about="&geotime;Carboniferous">	<skos:prefLabel xml:lang="en">Carboniferous</skos:prefLabel>	<skos:definition>The Carboniferous time period started 359.2  million years (Ma) before present (BP) and ended 299 Ma BP.</skos:definition>	<rdfs:seeAlso rdf:resource="http://kos.gbif.org/wiki/geotime:Carboniferous"/>	<geotime:rangeType>Period</geotime:rangeType>	<geotime:rangeTypeURI rdf:resource="&geotime;Period"/>	<geotime:start>359.2</geotime:start>	<geotime:end>299</geotime:end>	<skos:narrower>Paleozoic</skos:narrower>	<dcterms:created>2011-01-11</dcterms:created>	<dcterms:modified>2012-08-03</dcterms:modified>	<dcterms:hasVersion rdf:resource="&history;20120803/geotime#Carboniferous"/>	<rdfs:isDefinedBy rdf:resource="&geotime;"/>	<skos:inScheme rdf:resource="&geotime;"/>	<vann:termGroup rdf:resource="&geotime;Period"/>	<vann:termGroup rdf:resource="&geotime;Chronostratigraphic"/>	<vs:term_status>unstable</vs:term_status>	</skos:Concept>
<skos:Concept rdf:about="&geotime;Devonian">	<skos:prefLabel xml:lang="en">Devonian</skos:prefLabel>	<skos:definition>The Devonian time period started 416  million years (Ma) before present (BP) and ended 359.2 Ma BP.</skos:definition>	<rdfs:seeAlso rdf:resource="http://kos.gbif.org/wiki/geotime:Devonian"/>	<geotime:rangeType>Period</geotime:rangeType>	<geotime:rangeTypeURI rdf:resource="&geotime;Period"/>	<geotime:start>416</geotime:start>	<geotime:end>359.2</geotime:end>	<skos:narrower>Paleozoic</skos:narrower>	<dcterms:created>2011-01-11</dcterms:created>	<dcterms:modified>2012-08-03</dcterms:modified>	<dcterms:hasVersion rdf:resource="&history;20120803/geotime#Devonian"/>	<rdfs:isDefinedBy rdf:resource="&geotime;"/>	<skos:inScheme rdf:resource="&geotime;"/>	<vann:termGroup rdf:resource="&geotime;Period"/>	<vann:termGroup rdf:resource="&geotime;Chronostratigraphic"/>	<vs:term_status>unstable</vs:term_status>	</skos:Concept>
<skos:Concept rdf:about="&geotime;Silurian">	<skos:prefLabel xml:lang="en">Silurian</skos:prefLabel>	<skos:definition>The Silurian time period started 443.7  million years (Ma) before present (BP) and ended 416 Ma BP.</skos:definition>	<rdfs:seeAlso rdf:resource="http://kos.gbif.org/wiki/geotime:Silurian"/>	<geotime:rangeType>Period</geotime:rangeType>	<geotime:rangeTypeURI rdf:resource="&geotime;Period"/>	<geotime:start>443.7</geotime:start>	<geotime:end>416</geotime:end>	<skos:narrower>Paleozoic</skos:narrower>	<dcterms:created>2011-01-11</dcterms:created>	<dcterms:modified>2012-08-03</dcterms:modified>	<dcterms:hasVersion rdf:resource="&history;20120803/geotime#Silurian"/>	<rdfs:isDefinedBy rdf:resource="&geotime;"/>	<skos:inScheme rdf:resource="&geotime;"/>	<vann:termGroup rdf:resource="&geotime;Period"/>	<vann:termGroup rdf:resource="&geotime;Chronostratigraphic"/>	<vs:term_status>unstable</vs:term_status>	</skos:Concept>
<skos:Concept rdf:about="&geotime;Ordovician">	<skos:prefLabel xml:lang="en">Ordovician</skos:prefLabel>	<skos:definition>The Ordovician time period started 488.3  million years (Ma) before present (BP) and ended 443.7 Ma BP.</skos:definition>	<rdfs:seeAlso rdf:resource="http://kos.gbif.org/wiki/geotime:Ordovician"/>	<geotime:rangeType>Period</geotime:rangeType>	<geotime:rangeTypeURI rdf:resource="&geotime;Period"/>	<geotime:start>488.3</geotime:start>	<geotime:end>443.7</geotime:end>	<skos:narrower>Paleozoic</skos:narrower>	<dcterms:created>2011-01-11</dcterms:created>	<dcterms:modified>2012-08-03</dcterms:modified>	<dcterms:hasVersion rdf:resource="&history;20120803/geotime#Ordovician"/>	<rdfs:isDefinedBy rdf:resource="&geotime;"/>	<skos:inScheme rdf:resource="&geotime;"/>	<vann:termGroup rdf:resource="&geotime;Period"/>	<vann:termGroup rdf:resource="&geotime;Chronostratigraphic"/>	<vs:term_status>unstable</vs:term_status>	</skos:Concept>
<skos:Concept rdf:about="&geotime;Cambrian">	<skos:prefLabel xml:lang="en">Cambrian</skos:prefLabel>	<skos:definition>The Cambrian time period started 542  million years (Ma) before present (BP) and ended 488.3 Ma BP.</skos:definition>	<rdfs:seeAlso rdf:resource="http://kos.gbif.org/wiki/geotime:Cambrian"/>	<geotime:rangeType>Period</geotime:rangeType>	<geotime:rangeTypeURI rdf:resource="&geotime;Period"/>	<geotime:start>542</geotime:start>	<geotime:end>488.3</geotime:end>	<skos:narrower>Paleozoic</skos:narrower>	<dcterms:created>2011-01-11</dcterms:created>	<dcterms:modified>2012-08-03</dcterms:modified>	<dcterms:hasVersion rdf:resource="&history;20120803/geotime#Cambrian"/>	<rdfs:isDefinedBy rdf:resource="&geotime;"/>	<skos:inScheme rdf:resource="&geotime;"/>	<vann:termGroup rdf:resource="&geotime;Period"/>	<vann:termGroup rdf:resource="&geotime;Chronostratigraphic"/>	<vs:term_status>unstable</vs:term_status>	</skos:Concept>
<skos:Concept rdf:about="&geotime;Ediacaran">	<skos:prefLabel xml:lang="en">Ediacaran</skos:prefLabel>	<skos:definition>The Ediacaran time period started 650  million years (Ma) before present (BP) and ended 542 Ma BP.</skos:definition>	<rdfs:seeAlso rdf:resource="http://kos.gbif.org/wiki/geotime:Ediacaran"/>	<geotime:rangeType>Period</geotime:rangeType>	<geotime:rangeTypeURI rdf:resource="&geotime;Period"/>	<geotime:start>650</geotime:start>	<geotime:end>542</geotime:end>	<skos:narrower>Neoproterozoic</skos:narrower>	<dcterms:created>2011-01-11</dcterms:created>	<dcterms:modified>2012-08-03</dcterms:modified>	<dcterms:hasVersion rdf:resource="&history;20120803/geotime#Ediacaran"/>	<rdfs:isDefinedBy rdf:resource="&geotime;"/>	<skos:inScheme rdf:resource="&geotime;"/>	<vann:termGroup rdf:resource="&geotime;Period"/>	<vann:termGroup rdf:resource="&geotime;Chronostratigraphic"/>	<vs:term_status>unstable</vs:term_status>	</skos:Concept>
<skos:Concept rdf:about="&geotime;Cryogenian">	<skos:prefLabel xml:lang="en">Cryogenian</skos:prefLabel>	<skos:definition>The Cryogenian time period started 850  million years (Ma) before present (BP) and ended 650 Ma BP.</skos:definition>	<rdfs:seeAlso rdf:resource="http://kos.gbif.org/wiki/geotime:Cryogenian"/>	<geotime:rangeType>Period</geotime:rangeType>	<geotime:rangeTypeURI rdf:resource="&geotime;Period"/>	<geotime:start>850</geotime:start>	<geotime:end>650</geotime:end>	<skos:narrower>Neoproterozoic</skos:narrower>	<dcterms:created>2011-01-11</dcterms:created>	<dcterms:modified>2012-08-03</dcterms:modified>	<dcterms:hasVersion rdf:resource="&history;20120803/geotime#Cryogenian"/>	<rdfs:isDefinedBy rdf:resource="&geotime;"/>	<skos:inScheme rdf:resource="&geotime;"/>	<vann:termGroup rdf:resource="&geotime;Period"/>	<vann:termGroup rdf:resource="&geotime;Chronostratigraphic"/>	<vs:term_status>unstable</vs:term_status>	</skos:Concept>
<skos:Concept rdf:about="&geotime;Tonian">	<skos:prefLabel xml:lang="en">Tonian</skos:prefLabel>	<skos:definition>The Tonian time period started 1000  million years (Ma) before present (BP) and ended 850 Ma BP.</skos:definition>	<rdfs:seeAlso rdf:resource="http://kos.gbif.org/wiki/geotime:Tonian"/>	<geotime:rangeType>Period</geotime:rangeType>	<geotime:rangeTypeURI rdf:resource="&geotime;Period"/>	<geotime:start>1000</geotime:start>	<geotime:end>850</geotime:end>	<skos:narrower>Neoproterozoic</skos:narrower>	<dcterms:created>2011-01-11</dcterms:created>	<dcterms:modified>2012-08-03</dcterms:modified>	<dcterms:hasVersion rdf:resource="&history;20120803/geotime#Tonian"/>	<rdfs:isDefinedBy rdf:resource="&geotime;"/>	<skos:inScheme rdf:resource="&geotime;"/>	<vann:termGroup rdf:resource="&geotime;Period"/>	<vann:termGroup rdf:resource="&geotime;Chronostratigraphic"/>	<vs:term_status>unstable</vs:term_status>	</skos:Concept>
<skos:Concept rdf:about="&geotime;Stenian">	<skos:prefLabel xml:lang="en">Stenian</skos:prefLabel>	<skos:definition>The Stenian time period started 1200  million years (Ma) before present (BP) and ended 1000 Ma BP.</skos:definition>	<rdfs:seeAlso rdf:resource="http://kos.gbif.org/wiki/geotime:Stenian"/>	<geotime:rangeType>Period</geotime:rangeType>	<geotime:rangeTypeURI rdf:resource="&geotime;Period"/>	<geotime:start>1200</geotime:start>	<geotime:end>1000</geotime:end>	<skos:narrower>Neoproterozoic</skos:narrower>	<dcterms:created>2011-01-11</dcterms:created>	<dcterms:modified>2012-08-03</dcterms:modified>	<dcterms:hasVersion rdf:resource="&history;20120803/geotime#Stenian"/>	<rdfs:isDefinedBy rdf:resource="&geotime;"/>	<skos:inScheme rdf:resource="&geotime;"/>	<vann:termGroup rdf:resource="&geotime;Period"/>	<vann:termGroup rdf:resource="&geotime;Chronostratigraphic"/>	<vs:term_status>unstable</vs:term_status>	</skos:Concept>
<skos:Concept rdf:about="&geotime;Ectasian">	<skos:prefLabel xml:lang="en">Ectasian</skos:prefLabel>	<skos:definition>The Ectasian time period started 1400  million years (Ma) before present (BP) and ended 1200 Ma BP.</skos:definition>	<rdfs:seeAlso rdf:resource="http://kos.gbif.org/wiki/geotime:Ectasian"/>	<geotime:rangeType>Period</geotime:rangeType>	<geotime:rangeTypeURI rdf:resource="&geotime;Period"/>	<geotime:start>1400</geotime:start>	<geotime:end>1200</geotime:end>	<skos:narrower>Mesoproterozoic</skos:narrower>	<dcterms:created>2011-01-11</dcterms:created>	<dcterms:modified>2012-08-03</dcterms:modified>	<dcterms:hasVersion rdf:resource="&history;20120803/geotime#Ectasian"/>	<rdfs:isDefinedBy rdf:resource="&geotime;"/>	<skos:inScheme rdf:resource="&geotime;"/>	<vann:termGroup rdf:resource="&geotime;Period"/>	<vann:termGroup rdf:resource="&geotime;Chronostratigraphic"/>	<vs:term_status>unstable</vs:term_status>	</skos:Concept>
<skos:Concept rdf:about="&geotime;Calymmian">	<skos:prefLabel xml:lang="en">Calymmian</skos:prefLabel>	<skos:definition>The Calymmian time period started 1600  million years (Ma) before present (BP) and ended 1400 Ma BP.</skos:definition>	<rdfs:seeAlso rdf:resource="http://kos.gbif.org/wiki/geotime:Calymmian"/>	<geotime:rangeType>Period</geotime:rangeType>	<geotime:rangeTypeURI rdf:resource="&geotime;Period"/>	<geotime:start>1600</geotime:start>	<geotime:end>1400</geotime:end>	<skos:narrower>Mesoproterozoic</skos:narrower>	<dcterms:created>2011-01-11</dcterms:created>	<dcterms:modified>2012-08-03</dcterms:modified>	<dcterms:hasVersion rdf:resource="&history;20120803/geotime#Calymmian"/>	<rdfs:isDefinedBy rdf:resource="&geotime;"/>	<skos:inScheme rdf:resource="&geotime;"/>	<vann:termGroup rdf:resource="&geotime;Period"/>	<vann:termGroup rdf:resource="&geotime;Chronostratigraphic"/>	<vs:term_status>unstable</vs:term_status>	</skos:Concept>
<skos:Concept rdf:about="&geotime;Statherian">	<skos:prefLabel xml:lang="en">Statherian</skos:prefLabel>	<skos:definition>The Statherian time period started 1800  million years (Ma) before present (BP) and ended 1600 Ma BP.</skos:definition>	<rdfs:seeAlso rdf:resource="http://kos.gbif.org/wiki/geotime:Statherian"/>	<geotime:rangeType>Period</geotime:rangeType>	<geotime:rangeTypeURI rdf:resource="&geotime;Period"/>	<geotime:start>1800</geotime:start>	<geotime:end>1600</geotime:end>	<skos:narrower>Paleoproterozoic</skos:narrower>	<dcterms:created>2011-01-11</dcterms:created>	<dcterms:modified>2012-08-03</dcterms:modified>	<dcterms:hasVersion rdf:resource="&history;20120803/geotime#Statherian"/>	<rdfs:isDefinedBy rdf:resource="&geotime;"/>	<skos:inScheme rdf:resource="&geotime;"/>	<vann:termGroup rdf:resource="&geotime;Period"/>	<vann:termGroup rdf:resource="&geotime;Chronostratigraphic"/>	<vs:term_status>unstable</vs:term_status>	</skos:Concept>
<skos:Concept rdf:about="&geotime;Orosirian">	<skos:prefLabel xml:lang="en">Orosirian</skos:prefLabel>	<skos:definition>The Orosirian time period started 2050  million years (Ma) before present (BP) and ended 1800 Ma BP.</skos:definition>	<rdfs:seeAlso rdf:resource="http://kos.gbif.org/wiki/geotime:Orosirian"/>	<geotime:rangeType>Period</geotime:rangeType>	<geotime:rangeTypeURI rdf:resource="&geotime;Period"/>	<geotime:start>2050</geotime:start>	<geotime:end>1800</geotime:end>	<skos:narrower>Paleoproterozoic</skos:narrower>	<dcterms:created>2011-01-11</dcterms:created>	<dcterms:modified>2012-08-03</dcterms:modified>	<dcterms:hasVersion rdf:resource="&history;20120803/geotime#Orosirian"/>	<rdfs:isDefinedBy rdf:resource="&geotime;"/>	<skos:inScheme rdf:resource="&geotime;"/>	<vann:termGroup rdf:resource="&geotime;Period"/>	<vann:termGroup rdf:resource="&geotime;Chronostratigraphic"/>	<vs:term_status>unstable</vs:term_status>	</skos:Concept>
<skos:Concept rdf:about="&geotime;Rhyacian">	<skos:prefLabel xml:lang="en">Rhyacian</skos:prefLabel>	<skos:definition>The Rhyacian time period started 2300  million years (Ma) before present (BP) and ended 2050 Ma BP.</skos:definition>	<rdfs:seeAlso rdf:resource="http://kos.gbif.org/wiki/geotime:Rhyacian"/>	<geotime:rangeType>Period</geotime:rangeType>	<geotime:rangeTypeURI rdf:resource="&geotime;Period"/>	<geotime:start>2300</geotime:start>	<geotime:end>2050</geotime:end>	<skos:narrower>Paleoproterozoic</skos:narrower>	<dcterms:created>2011-01-11</dcterms:created>	<dcterms:modified>2012-08-03</dcterms:modified>	<dcterms:hasVersion rdf:resource="&history;20120803/geotime#Rhyacian"/>	<rdfs:isDefinedBy rdf:resource="&geotime;"/>	<skos:inScheme rdf:resource="&geotime;"/>	<vann:termGroup rdf:resource="&geotime;Period"/>	<vann:termGroup rdf:resource="&geotime;Chronostratigraphic"/>	<vs:term_status>unstable</vs:term_status>	</skos:Concept>
<skos:Concept rdf:about="&geotime;Siderian">	<skos:prefLabel xml:lang="en">Siderian</skos:prefLabel>	<skos:definition>The Siderian time period started 2500  million years (Ma) before present (BP) and ended 2300 Ma BP.</skos:definition>	<rdfs:seeAlso rdf:resource="http://kos.gbif.org/wiki/geotime:Siderian"/>	<geotime:rangeType>Period</geotime:rangeType>	<geotime:rangeTypeURI rdf:resource="&geotime;Period"/>	<geotime:start>2500</geotime:start>	<geotime:end>2300</geotime:end>	<skos:narrower>Paleoproterozoic</skos:narrower>	<dcterms:created>2011-01-11</dcterms:created>	<dcterms:modified>2012-08-03</dcterms:modified>	<dcterms:hasVersion rdf:resource="&history;20120803/geotime#Siderian"/>	<rdfs:isDefinedBy rdf:resource="&geotime;"/>	<skos:inScheme rdf:resource="&geotime;"/>	<vann:termGroup rdf:resource="&geotime;Period"/>	<vann:termGroup rdf:resource="&geotime;Chronostratigraphic"/>	<vs:term_status>unstable</vs:term_status>	</skos:Concept>
<skos:Concept rdf:about="&geotime;LatePleistocene">	<skos:prefLabel xml:lang="en">Late Pleistocene</skos:prefLabel>	<skos:definition>The Late Pleistocene time period started 0.126  million years (Ma) before present (BP) and ended 0 Ma BP.</skos:definition>	<rdfs:seeAlso rdf:resource="http://kos.gbif.org/wiki/geotime:LatePleistocene"/>	<geotime:rangeType>Stage</geotime:rangeType>	<geotime:rangeTypeURI rdf:resource="&geotime;Stage"/>	<geotime:start>0.126</geotime:start>	<geotime:end>0</geotime:end>		<dcterms:created>2011-01-11</dcterms:created>	<dcterms:modified>2012-08-03</dcterms:modified>	<dcterms:hasVersion rdf:resource="&history;20120803/geotime#LatePleistocene"/>	<rdfs:isDefinedBy rdf:resource="&geotime;"/>	<skos:inScheme rdf:resource="&geotime;"/>	<vann:termGroup rdf:resource="&geotime;Stage"/>	<vann:termGroup rdf:resource="&geotime;Chronostratigraphic"/>	<vs:term_status>unstable</vs:term_status>	</skos:Concept>
<skos:Concept rdf:about="&geotime;MiddlePleistocene">	<skos:prefLabel xml:lang="en">Middle Pleistocene</skos:prefLabel>	<skos:definition>The Middle Pleistocene time period started 0.781  million years (Ma) before present (BP) and ended 0.126 Ma BP.</skos:definition>	<rdfs:seeAlso rdf:resource="http://kos.gbif.org/wiki/geotime:MiddlePleistocene"/>	<geotime:rangeType>Stage</geotime:rangeType>	<geotime:rangeTypeURI rdf:resource="&geotime;Stage"/>	<geotime:start>0.781</geotime:start>	<geotime:end>0.126</geotime:end>		<dcterms:created>2011-01-11</dcterms:created>	<dcterms:modified>2012-08-03</dcterms:modified>	<dcterms:hasVersion rdf:resource="&history;20120803/geotime#MiddlePleistocene"/>	<rdfs:isDefinedBy rdf:resource="&geotime;"/>	<skos:inScheme rdf:resource="&geotime;"/>	<vann:termGroup rdf:resource="&geotime;Stage"/>	<vann:termGroup rdf:resource="&geotime;Chronostratigraphic"/>	<vs:term_status>unstable</vs:term_status>	</skos:Concept>
<skos:Concept rdf:about="&geotime;EarlyPleistocene">	<skos:prefLabel xml:lang="en">Early Pleistocene</skos:prefLabel>	<skos:definition>The Early Pleistocene time period started 1.806  million years (Ma) before present (BP) and ended 0.781 Ma BP.</skos:definition>	<rdfs:seeAlso rdf:resource="http://kos.gbif.org/wiki/geotime:EarlyPleistocene"/>	<geotime:rangeType>Stage</geotime:rangeType>	<geotime:rangeTypeURI rdf:resource="&geotime;Stage"/>	<geotime:start>1.806</geotime:start>	<geotime:end>0.781</geotime:end>		<dcterms:created>2011-01-11</dcterms:created>	<dcterms:modified>2012-08-03</dcterms:modified>	<dcterms:hasVersion rdf:resource="&history;20120803/geotime#EarlyPleistocene"/>	<rdfs:isDefinedBy rdf:resource="&geotime;"/>	<skos:inScheme rdf:resource="&geotime;"/>	<vann:termGroup rdf:resource="&geotime;Stage"/>	<vann:termGroup rdf:resource="&geotime;Chronostratigraphic"/>	<vs:term_status>unstable</vs:term_status>	</skos:Concept>
<skos:Concept rdf:about="&geotime;Gelasian">	<skos:prefLabel xml:lang="en">Gelasian</skos:prefLabel>	<skos:definition>The Gelasian time period started 2.588  million years (Ma) before present (BP) and ended 1.806 Ma BP.</skos:definition>	<rdfs:seeAlso rdf:resource="http://kos.gbif.org/wiki/geotime:Gelasian"/>	<geotime:rangeType>Stage</geotime:rangeType>	<geotime:rangeTypeURI rdf:resource="&geotime;Stage"/>	<geotime:start>2.588</geotime:start>	<geotime:end>1.806</geotime:end>		<dcterms:created>2011-01-11</dcterms:created>	<dcterms:modified>2012-08-03</dcterms:modified>	<dcterms:hasVersion rdf:resource="&history;20120803/geotime#Gelasian"/>	<rdfs:isDefinedBy rdf:resource="&geotime;"/>	<skos:inScheme rdf:resource="&geotime;"/>	<vann:termGroup rdf:resource="&geotime;Stage"/>	<vann:termGroup rdf:resource="&geotime;Chronostratigraphic"/>	<vs:term_status>unstable</vs:term_status>	</skos:Concept>
<skos:Concept rdf:about="&geotime;Piacenzian">	<skos:prefLabel xml:lang="en">Piacenzian</skos:prefLabel>	<skos:definition>The Piacenzian time period started 3.6  million years (Ma) before present (BP) and ended 2.588 Ma BP.</skos:definition>	<rdfs:seeAlso rdf:resource="http://kos.gbif.org/wiki/geotime:Piacenzian"/>	<geotime:rangeType>Stage</geotime:rangeType>	<geotime:rangeTypeURI rdf:resource="&geotime;Stage"/>	<geotime:start>3.6</geotime:start>	<geotime:end>2.588</geotime:end>		<dcterms:created>2011-01-11</dcterms:created>	<dcterms:modified>2012-08-03</dcterms:modified>	<dcterms:hasVersion rdf:resource="&history;20120803/geotime#Piacenzian"/>	<rdfs:isDefinedBy rdf:resource="&geotime;"/>	<skos:inScheme rdf:resource="&geotime;"/>	<vann:termGroup rdf:resource="&geotime;Stage"/>	<vann:termGroup rdf:resource="&geotime;Chronostratigraphic"/>	<vs:term_status>unstable</vs:term_status>	</skos:Concept>
<skos:Concept rdf:about="&geotime;Zanclean">	<skos:prefLabel xml:lang="en">Zanclean</skos:prefLabel>	<skos:definition>The Zanclean time period started 5.333  million years (Ma) before present (BP) and ended 3.6 Ma BP.</skos:definition>	<rdfs:seeAlso rdf:resource="http://kos.gbif.org/wiki/geotime:Zanclean"/>	<geotime:rangeType>Stage</geotime:rangeType>	<geotime:rangeTypeURI rdf:resource="&geotime;Stage"/>	<geotime:start>5.333</geotime:start>	<geotime:end>3.6</geotime:end>		<dcterms:created>2011-01-11</dcterms:created>	<dcterms:modified>2012-08-03</dcterms:modified>	<dcterms:hasVersion rdf:resource="&history;20120803/geotime#Zanclean"/>	<rdfs:isDefinedBy rdf:resource="&geotime;"/>	<skos:inScheme rdf:resource="&geotime;"/>	<vann:termGroup rdf:resource="&geotime;Stage"/>	<vann:termGroup rdf:resource="&geotime;Chronostratigraphic"/>	<vs:term_status>unstable</vs:term_status>	</skos:Concept>
<skos:Concept rdf:about="&geotime;Messinian">	<skos:prefLabel xml:lang="en">Messinian</skos:prefLabel>	<skos:definition>The Messinian time period started 7.248  million years (Ma) before present (BP) and ended 5.333 Ma BP.</skos:definition>	<rdfs:seeAlso rdf:resource="http://kos.gbif.org/wiki/geotime:Messinian"/>	<geotime:rangeType>Stage</geotime:rangeType>	<geotime:rangeTypeURI rdf:resource="&geotime;Stage"/>	<geotime:start>7.248</geotime:start>	<geotime:end>5.333</geotime:end>		<dcterms:created>2011-01-11</dcterms:created>	<dcterms:modified>2012-08-03</dcterms:modified>	<dcterms:hasVersion rdf:resource="&history;20120803/geotime#Messinian"/>	<rdfs:isDefinedBy rdf:resource="&geotime;"/>	<skos:inScheme rdf:resource="&geotime;"/>	<vann:termGroup rdf:resource="&geotime;Stage"/>	<vann:termGroup rdf:resource="&geotime;Chronostratigraphic"/>	<vs:term_status>unstable</vs:term_status>	</skos:Concept>
<skos:Concept rdf:about="&geotime;Tortonian">	<skos:prefLabel xml:lang="en">Tortonian</skos:prefLabel>	<skos:definition>The Tortonian time period started 11.608  million years (Ma) before present (BP) and ended 7.248 Ma BP.</skos:definition>	<rdfs:seeAlso rdf:resource="http://kos.gbif.org/wiki/geotime:Tortonian"/>	<geotime:rangeType>Stage</geotime:rangeType>	<geotime:rangeTypeURI rdf:resource="&geotime;Stage"/>	<geotime:start>11.608</geotime:start>	<geotime:end>7.248</geotime:end>		<dcterms:created>2011-01-11</dcterms:created>	<dcterms:modified>2012-08-03</dcterms:modified>	<dcterms:hasVersion rdf:resource="&history;20120803/geotime#Tortonian"/>	<rdfs:isDefinedBy rdf:resource="&geotime;"/>	<skos:inScheme rdf:resource="&geotime;"/>	<vann:termGroup rdf:resource="&geotime;Stage"/>	<vann:termGroup rdf:resource="&geotime;Chronostratigraphic"/>	<vs:term_status>unstable</vs:term_status>	</skos:Concept>
<skos:Concept rdf:about="&geotime;Serravillian">	<skos:prefLabel xml:lang="en">Serravillian</skos:prefLabel>	<skos:definition>The Serravillian time period started 13.64  million years (Ma) before present (BP) and ended 11.608 Ma BP.</skos:definition>	<rdfs:seeAlso rdf:resource="http://kos.gbif.org/wiki/geotime:Serravillian"/>	<geotime:rangeType>Stage</geotime:rangeType>	<geotime:rangeTypeURI rdf:resource="&geotime;Stage"/>	<geotime:start>13.64</geotime:start>	<geotime:end>11.608</geotime:end>		<dcterms:created>2011-01-11</dcterms:created>	<dcterms:modified>2012-08-03</dcterms:modified>	<dcterms:hasVersion rdf:resource="&history;20120803/geotime#Serravillian"/>	<rdfs:isDefinedBy rdf:resource="&geotime;"/>	<skos:inScheme rdf:resource="&geotime;"/>	<vann:termGroup rdf:resource="&geotime;Stage"/>	<vann:termGroup rdf:resource="&geotime;Chronostratigraphic"/>	<vs:term_status>unstable</vs:term_status>	</skos:Concept>
<skos:Concept rdf:about="&geotime;Langhian">	<skos:prefLabel xml:lang="en">Langhian</skos:prefLabel>	<skos:definition>The Langhian time period started 15.97  million years (Ma) before present (BP) and ended 13.64 Ma BP.</skos:definition>	<rdfs:seeAlso rdf:resource="http://kos.gbif.org/wiki/geotime:Langhian"/>	<geotime:rangeType>Stage</geotime:rangeType>	<geotime:rangeTypeURI rdf:resource="&geotime;Stage"/>	<geotime:start>15.97</geotime:start>	<geotime:end>13.64</geotime:end>		<dcterms:created>2011-01-11</dcterms:created>	<dcterms:modified>2012-08-03</dcterms:modified>	<dcterms:hasVersion rdf:resource="&history;20120803/geotime#Langhian"/>	<rdfs:isDefinedBy rdf:resource="&geotime;"/>	<skos:inScheme rdf:resource="&geotime;"/>	<vann:termGroup rdf:resource="&geotime;Stage"/>	<vann:termGroup rdf:resource="&geotime;Chronostratigraphic"/>	<vs:term_status>unstable</vs:term_status>	</skos:Concept>
<skos:Concept rdf:about="&geotime;Burdigalian">	<skos:prefLabel xml:lang="en">Burdigalian</skos:prefLabel>	<skos:definition>The Burdigalian time period started 20.43  million years (Ma) before present (BP) and ended 15.97 Ma BP.</skos:definition>	<rdfs:seeAlso rdf:resource="http://kos.gbif.org/wiki/geotime:Burdigalian"/>	<geotime:rangeType>Stage</geotime:rangeType>	<geotime:rangeTypeURI rdf:resource="&geotime;Stage"/>	<geotime:start>20.43</geotime:start>	<geotime:end>15.97</geotime:end>		<dcterms:created>2011-01-11</dcterms:created>	<dcterms:modified>2012-08-03</dcterms:modified>	<dcterms:hasVersion rdf:resource="&history;20120803/geotime#Burdigalian"/>	<rdfs:isDefinedBy rdf:resource="&geotime;"/>	<skos:inScheme rdf:resource="&geotime;"/>	<vann:termGroup rdf:resource="&geotime;Stage"/>	<vann:termGroup rdf:resource="&geotime;Chronostratigraphic"/>	<vs:term_status>unstable</vs:term_status>	</skos:Concept>
<skos:Concept rdf:about="&geotime;Aquitanian">	<skos:prefLabel xml:lang="en">Aquitanian</skos:prefLabel>	<skos:definition>The Aquitanian time period started 23.03  million years (Ma) before present (BP) and ended 20.43 Ma BP.</skos:definition>	<rdfs:seeAlso rdf:resource="http://kos.gbif.org/wiki/geotime:Aquitanian"/>	<geotime:rangeType>Stage</geotime:rangeType>	<geotime:rangeTypeURI rdf:resource="&geotime;Stage"/>	<geotime:start>23.03</geotime:start>	<geotime:end>20.43</geotime:end>		<dcterms:created>2011-01-11</dcterms:created>	<dcterms:modified>2012-08-03</dcterms:modified>	<dcterms:hasVersion rdf:resource="&history;20120803/geotime#Aquitanian"/>	<rdfs:isDefinedBy rdf:resource="&geotime;"/>	<skos:inScheme rdf:resource="&geotime;"/>	<vann:termGroup rdf:resource="&geotime;Stage"/>	<vann:termGroup rdf:resource="&geotime;Chronostratigraphic"/>	<vs:term_status>unstable</vs:term_status>	</skos:Concept>
<skos:Concept rdf:about="&geotime;Chattian">	<skos:prefLabel xml:lang="en">Chattian</skos:prefLabel>	<skos:definition>The Chattian time period started 28.4  million years (Ma) before present (BP) and ended 23.03 Ma BP.</skos:definition>	<rdfs:seeAlso rdf:resource="http://kos.gbif.org/wiki/geotime:Chattian"/>	<geotime:rangeType>Stage</geotime:rangeType>	<geotime:rangeTypeURI rdf:resource="&geotime;Stage"/>	<geotime:start>28.4</geotime:start>	<geotime:end>23.03</geotime:end>		<dcterms:created>2011-01-11</dcterms:created>	<dcterms:modified>2012-08-03</dcterms:modified>	<dcterms:hasVersion rdf:resource="&history;20120803/geotime#Chattian"/>	<rdfs:isDefinedBy rdf:resource="&geotime;"/>	<skos:inScheme rdf:resource="&geotime;"/>	<vann:termGroup rdf:resource="&geotime;Stage"/>	<vann:termGroup rdf:resource="&geotime;Chronostratigraphic"/>	<vs:term_status>unstable</vs:term_status>	</skos:Concept>
<skos:Concept rdf:about="&geotime;Rupelian">	<skos:prefLabel xml:lang="en">Rupelian</skos:prefLabel>	<skos:definition>The Rupelian time period started 33.9  million years (Ma) before present (BP) and ended 28.4 Ma BP.</skos:definition>	<rdfs:seeAlso rdf:resource="http://kos.gbif.org/wiki/geotime:Rupelian"/>	<geotime:rangeType>Stage</geotime:rangeType>	<geotime:rangeTypeURI rdf:resource="&geotime;Stage"/>	<geotime:start>33.9</geotime:start>	<geotime:end>28.4</geotime:end>		<dcterms:created>2011-01-11</dcterms:created>	<dcterms:modified>2012-08-03</dcterms:modified>	<dcterms:hasVersion rdf:resource="&history;20120803/geotime#Rupelian"/>	<rdfs:isDefinedBy rdf:resource="&geotime;"/>	<skos:inScheme rdf:resource="&geotime;"/>	<vann:termGroup rdf:resource="&geotime;Stage"/>	<vann:termGroup rdf:resource="&geotime;Chronostratigraphic"/>	<vs:term_status>unstable</vs:term_status>	</skos:Concept>
<skos:Concept rdf:about="&geotime;Priabonian">	<skos:prefLabel xml:lang="en">Priabonian</skos:prefLabel>	<skos:definition>The Priabonian time period started 37.2  million years (Ma) before present (BP) and ended 33.9 Ma BP.</skos:definition>	<rdfs:seeAlso rdf:resource="http://kos.gbif.org/wiki/geotime:Priabonian"/>	<geotime:rangeType>Stage</geotime:rangeType>	<geotime:rangeTypeURI rdf:resource="&geotime;Stage"/>	<geotime:start>37.2</geotime:start>	<geotime:end>33.9</geotime:end>		<dcterms:created>2011-01-11</dcterms:created>	<dcterms:modified>2012-08-03</dcterms:modified>	<dcterms:hasVersion rdf:resource="&history;20120803/geotime#Priabonian"/>	<rdfs:isDefinedBy rdf:resource="&geotime;"/>	<skos:inScheme rdf:resource="&geotime;"/>	<vann:termGroup rdf:resource="&geotime;Stage"/>	<vann:termGroup rdf:resource="&geotime;Chronostratigraphic"/>	<vs:term_status>unstable</vs:term_status>	</skos:Concept>
<skos:Concept rdf:about="&geotime;Bartonian">	<skos:prefLabel xml:lang="en">Bartonian</skos:prefLabel>	<skos:definition>The Bartonian time period started 40.4  million years (Ma) before present (BP) and ended 37.2 Ma BP.</skos:definition>	<rdfs:seeAlso rdf:resource="http://kos.gbif.org/wiki/geotime:Bartonian"/>	<geotime:rangeType>Stage</geotime:rangeType>	<geotime:rangeTypeURI rdf:resource="&geotime;Stage"/>	<geotime:start>40.4</geotime:start>	<geotime:end>37.2</geotime:end>		<dcterms:created>2011-01-11</dcterms:created>	<dcterms:modified>2012-08-03</dcterms:modified>	<dcterms:hasVersion rdf:resource="&history;20120803/geotime#Bartonian"/>	<rdfs:isDefinedBy rdf:resource="&geotime;"/>	<skos:inScheme rdf:resource="&geotime;"/>	<vann:termGroup rdf:resource="&geotime;Stage"/>	<vann:termGroup rdf:resource="&geotime;Chronostratigraphic"/>	<vs:term_status>unstable</vs:term_status>	</skos:Concept>
<skos:Concept rdf:about="&geotime;Lutetian">	<skos:prefLabel xml:lang="en">Lutetian</skos:prefLabel>	<skos:definition>The Lutetian time period started 48.6  million years (Ma) before present (BP) and ended 40.4 Ma BP.</skos:definition>	<rdfs:seeAlso rdf:resource="http://kos.gbif.org/wiki/geotime:Lutetian"/>	<geotime:rangeType>Stage</geotime:rangeType>	<geotime:rangeTypeURI rdf:resource="&geotime;Stage"/>	<geotime:start>48.6</geotime:start>	<geotime:end>40.4</geotime:end>		<dcterms:created>2011-01-11</dcterms:created>	<dcterms:modified>2012-08-03</dcterms:modified>	<dcterms:hasVersion rdf:resource="&history;20120803/geotime#Lutetian"/>	<rdfs:isDefinedBy rdf:resource="&geotime;"/>	<skos:inScheme rdf:resource="&geotime;"/>	<vann:termGroup rdf:resource="&geotime;Stage"/>	<vann:termGroup rdf:resource="&geotime;Chronostratigraphic"/>	<vs:term_status>unstable</vs:term_status>	</skos:Concept>
<skos:Concept rdf:about="&geotime;Ypresian">	<skos:prefLabel xml:lang="en">Ypresian</skos:prefLabel>	<skos:definition>The Ypresian time period started 55.8  million years (Ma) before present (BP) and ended 48.6 Ma BP.</skos:definition>	<rdfs:seeAlso rdf:resource="http://kos.gbif.org/wiki/geotime:Ypresian"/>	<geotime:rangeType>Stage</geotime:rangeType>	<geotime:rangeTypeURI rdf:resource="&geotime;Stage"/>	<geotime:start>55.8</geotime:start>	<geotime:end>48.6</geotime:end>		<dcterms:created>2011-01-11</dcterms:created>	<dcterms:modified>2012-08-03</dcterms:modified>	<dcterms:hasVersion rdf:resource="&history;20120803/geotime#Ypresian"/>	<rdfs:isDefinedBy rdf:resource="&geotime;"/>	<skos:inScheme rdf:resource="&geotime;"/>	<vann:termGroup rdf:resource="&geotime;Stage"/>	<vann:termGroup rdf:resource="&geotime;Chronostratigraphic"/>	<vs:term_status>unstable</vs:term_status>	</skos:Concept>
<skos:Concept rdf:about="&geotime;Thanetian">	<skos:prefLabel xml:lang="en">Thanetian</skos:prefLabel>	<skos:definition>The Thanetian time period started 58.74  million years (Ma) before present (BP) and ended 55.8 Ma BP.</skos:definition>	<rdfs:seeAlso rdf:resource="http://kos.gbif.org/wiki/geotime:Thanetian"/>	<geotime:rangeType>Stage</geotime:rangeType>	<geotime:rangeTypeURI rdf:resource="&geotime;Stage"/>	<geotime:start>58.74</geotime:start>	<geotime:end>55.8</geotime:end>		<dcterms:created>2011-01-11</dcterms:created>	<dcterms:modified>2012-08-03</dcterms:modified>	<dcterms:hasVersion rdf:resource="&history;20120803/geotime#Thanetian"/>	<rdfs:isDefinedBy rdf:resource="&geotime;"/>	<skos:inScheme rdf:resource="&geotime;"/>	<vann:termGroup rdf:resource="&geotime;Stage"/>	<vann:termGroup rdf:resource="&geotime;Chronostratigraphic"/>	<vs:term_status>unstable</vs:term_status>	</skos:Concept>
<skos:Concept rdf:about="&geotime;Selandian">	<skos:prefLabel xml:lang="en">Selandian</skos:prefLabel>	<skos:definition>The Selandian time period started 61.72  million years (Ma) before present (BP) and ended 58.74 Ma BP.</skos:definition>	<rdfs:seeAlso rdf:resource="http://kos.gbif.org/wiki/geotime:Selandian"/>	<geotime:rangeType>Stage</geotime:rangeType>	<geotime:rangeTypeURI rdf:resource="&geotime;Stage"/>	<geotime:start>61.72</geotime:start>	<geotime:end>58.74</geotime:end>		<dcterms:created>2011-01-11</dcterms:created>	<dcterms:modified>2012-08-03</dcterms:modified>	<dcterms:hasVersion rdf:resource="&history;20120803/geotime#Selandian"/>	<rdfs:isDefinedBy rdf:resource="&geotime;"/>	<skos:inScheme rdf:resource="&geotime;"/>	<vann:termGroup rdf:resource="&geotime;Stage"/>	<vann:termGroup rdf:resource="&geotime;Chronostratigraphic"/>	<vs:term_status>unstable</vs:term_status>	</skos:Concept>
<skos:Concept rdf:about="&geotime;Danian">	<skos:prefLabel xml:lang="en">Danian</skos:prefLabel>	<skos:definition>The Danian time period started 65.5  million years (Ma) before present (BP) and ended 61.72 Ma BP.</skos:definition>	<rdfs:seeAlso rdf:resource="http://kos.gbif.org/wiki/geotime:Danian"/>	<geotime:rangeType>Stage</geotime:rangeType>	<geotime:rangeTypeURI rdf:resource="&geotime;Stage"/>	<geotime:start>65.5</geotime:start>	<geotime:end>61.72</geotime:end>		<dcterms:created>2011-01-11</dcterms:created>	<dcterms:modified>2012-08-03</dcterms:modified>	<dcterms:hasVersion rdf:resource="&history;20120803/geotime#Danian"/>	<rdfs:isDefinedBy rdf:resource="&geotime;"/>	<skos:inScheme rdf:resource="&geotime;"/>	<vann:termGroup rdf:resource="&geotime;Stage"/>	<vann:termGroup rdf:resource="&geotime;Chronostratigraphic"/>	<vs:term_status>unstable</vs:term_status>	</skos:Concept>
<skos:Concept rdf:about="&geotime;Maastrichtian">	<skos:prefLabel xml:lang="en">Maastrichtian</skos:prefLabel>	<skos:definition>The Maastrichtian time period started 70.6  million years (Ma) before present (BP) and ended 65.5 Ma BP.</skos:definition>	<rdfs:seeAlso rdf:resource="http://kos.gbif.org/wiki/geotime:Maastrichtian"/>	<geotime:rangeType>Stage</geotime:rangeType>	<geotime:rangeTypeURI rdf:resource="&geotime;Stage"/>	<geotime:start>70.6</geotime:start>	<geotime:end>65.5</geotime:end>		<dcterms:created>2011-01-11</dcterms:created>	<dcterms:modified>2012-08-03</dcterms:modified>	<dcterms:hasVersion rdf:resource="&history;20120803/geotime#Maastrichtian"/>	<rdfs:isDefinedBy rdf:resource="&geotime;"/>	<skos:inScheme rdf:resource="&geotime;"/>	<vann:termGroup rdf:resource="&geotime;Stage"/>	<vann:termGroup rdf:resource="&geotime;Chronostratigraphic"/>	<vs:term_status>unstable</vs:term_status>	</skos:Concept>
<skos:Concept rdf:about="&geotime;Campanian">	<skos:prefLabel xml:lang="en">Campanian</skos:prefLabel>	<skos:definition>The Campanian time period started 83.5  million years (Ma) before present (BP) and ended 70.6 Ma BP.</skos:definition>	<rdfs:seeAlso rdf:resource="http://kos.gbif.org/wiki/geotime:Campanian"/>	<geotime:rangeType>Stage</geotime:rangeType>	<geotime:rangeTypeURI rdf:resource="&geotime;Stage"/>	<geotime:start>83.5</geotime:start>	<geotime:end>70.6</geotime:end>		<dcterms:created>2011-01-11</dcterms:created>	<dcterms:modified>2012-08-03</dcterms:modified>	<dcterms:hasVersion rdf:resource="&history;20120803/geotime#Campanian"/>	<rdfs:isDefinedBy rdf:resource="&geotime;"/>	<skos:inScheme rdf:resource="&geotime;"/>	<vann:termGroup rdf:resource="&geotime;Stage"/>	<vann:termGroup rdf:resource="&geotime;Chronostratigraphic"/>	<vs:term_status>unstable</vs:term_status>	</skos:Concept>
<skos:Concept rdf:about="&geotime;Santonian">	<skos:prefLabel xml:lang="en">Santonian</skos:prefLabel>	<skos:definition>The Santonian time period started 85.85  million years (Ma) before present (BP) and ended 83.5 Ma BP.</skos:definition>	<rdfs:seeAlso rdf:resource="http://kos.gbif.org/wiki/geotime:Santonian"/>	<geotime:rangeType>Stage</geotime:rangeType>	<geotime:rangeTypeURI rdf:resource="&geotime;Stage"/>	<geotime:start>85.85</geotime:start>	<geotime:end>83.5</geotime:end>		<dcterms:created>2011-01-11</dcterms:created>	<dcterms:modified>2012-08-03</dcterms:modified>	<dcterms:hasVersion rdf:resource="&history;20120803/geotime#Santonian"/>	<rdfs:isDefinedBy rdf:resource="&geotime;"/>	<skos:inScheme rdf:resource="&geotime;"/>	<vann:termGroup rdf:resource="&geotime;Stage"/>	<vann:termGroup rdf:resource="&geotime;Chronostratigraphic"/>	<vs:term_status>unstable</vs:term_status>	</skos:Concept>
<skos:Concept rdf:about="&geotime;Coniacian">	<skos:prefLabel xml:lang="en">Coniacian</skos:prefLabel>	<skos:definition>The Coniacian time period started 89.27  million years (Ma) before present (BP) and ended 85.85 Ma BP.</skos:definition>	<rdfs:seeAlso rdf:resource="http://kos.gbif.org/wiki/geotime:Coniacian"/>	<geotime:rangeType>Stage</geotime:rangeType>	<geotime:rangeTypeURI rdf:resource="&geotime;Stage"/>	<geotime:start>89.27</geotime:start>	<geotime:end>85.85</geotime:end>		<dcterms:created>2011-01-11</dcterms:created>	<dcterms:modified>2012-08-03</dcterms:modified>	<dcterms:hasVersion rdf:resource="&history;20120803/geotime#Coniacian"/>	<rdfs:isDefinedBy rdf:resource="&geotime;"/>	<skos:inScheme rdf:resource="&geotime;"/>	<vann:termGroup rdf:resource="&geotime;Stage"/>	<vann:termGroup rdf:resource="&geotime;Chronostratigraphic"/>	<vs:term_status>unstable</vs:term_status>	</skos:Concept>
<skos:Concept rdf:about="&geotime;Turonian">	<skos:prefLabel xml:lang="en">Turonian</skos:prefLabel>	<skos:definition>The Turonian time period started 93.55  million years (Ma) before present (BP) and ended 89.27 Ma BP.</skos:definition>	<rdfs:seeAlso rdf:resource="http://kos.gbif.org/wiki/geotime:Turonian"/>	<geotime:rangeType>Stage</geotime:rangeType>	<geotime:rangeTypeURI rdf:resource="&geotime;Stage"/>	<geotime:start>93.55</geotime:start>	<geotime:end>89.27</geotime:end>		<dcterms:created>2011-01-11</dcterms:created>	<dcterms:modified>2012-08-03</dcterms:modified>	<dcterms:hasVersion rdf:resource="&history;20120803/geotime#Turonian"/>	<rdfs:isDefinedBy rdf:resource="&geotime;"/>	<skos:inScheme rdf:resource="&geotime;"/>	<vann:termGroup rdf:resource="&geotime;Stage"/>	<vann:termGroup rdf:resource="&geotime;Chronostratigraphic"/>	<vs:term_status>unstable</vs:term_status>	</skos:Concept>
<skos:Concept rdf:about="&geotime;Cenomanian">	<skos:prefLabel xml:lang="en">Cenomanian</skos:prefLabel>	<skos:definition>The Cenomanian time period started 99.6  million years (Ma) before present (BP) and ended 93.55 Ma BP.</skos:definition>	<rdfs:seeAlso rdf:resource="http://kos.gbif.org/wiki/geotime:Cenomanian"/>	<geotime:rangeType>Stage</geotime:rangeType>	<geotime:rangeTypeURI rdf:resource="&geotime;Stage"/>	<geotime:start>99.6</geotime:start>	<geotime:end>93.55</geotime:end>		<dcterms:created>2011-01-11</dcterms:created>	<dcterms:modified>2012-08-03</dcterms:modified>	<dcterms:hasVersion rdf:resource="&history;20120803/geotime#Cenomanian"/>	<rdfs:isDefinedBy rdf:resource="&geotime;"/>	<skos:inScheme rdf:resource="&geotime;"/>	<vann:termGroup rdf:resource="&geotime;Stage"/>	<vann:termGroup rdf:resource="&geotime;Chronostratigraphic"/>	<vs:term_status>unstable</vs:term_status>	</skos:Concept>
<skos:Concept rdf:about="&geotime;Albian">	<skos:prefLabel xml:lang="en">Albian</skos:prefLabel>	<skos:definition>The Albian time period started 112  million years (Ma) before present (BP) and ended 99.6 Ma BP.</skos:definition>	<rdfs:seeAlso rdf:resource="http://kos.gbif.org/wiki/geotime:Albian"/>	<geotime:rangeType>Stage</geotime:rangeType>	<geotime:rangeTypeURI rdf:resource="&geotime;Stage"/>	<geotime:start>112</geotime:start>	<geotime:end>99.6</geotime:end>		<dcterms:created>2011-01-11</dcterms:created>	<dcterms:modified>2012-08-03</dcterms:modified>	<dcterms:hasVersion rdf:resource="&history;20120803/geotime#Albian"/>	<rdfs:isDefinedBy rdf:resource="&geotime;"/>	<skos:inScheme rdf:resource="&geotime;"/>	<vann:termGroup rdf:resource="&geotime;Stage"/>	<vann:termGroup rdf:resource="&geotime;Chronostratigraphic"/>	<vs:term_status>unstable</vs:term_status>	</skos:Concept>
<skos:Concept rdf:about="&geotime;Aptian">	<skos:prefLabel xml:lang="en">Aptian</skos:prefLabel>	<skos:definition>The Aptian time period started 125  million years (Ma) before present (BP) and ended 112 Ma BP.</skos:definition>	<rdfs:seeAlso rdf:resource="http://kos.gbif.org/wiki/geotime:Aptian"/>	<geotime:rangeType>Stage</geotime:rangeType>	<geotime:rangeTypeURI rdf:resource="&geotime;Stage"/>	<geotime:start>125</geotime:start>	<geotime:end>112</geotime:end>		<dcterms:created>2011-01-11</dcterms:created>	<dcterms:modified>2012-08-03</dcterms:modified>	<dcterms:hasVersion rdf:resource="&history;20120803/geotime#Aptian"/>	<rdfs:isDefinedBy rdf:resource="&geotime;"/>	<skos:inScheme rdf:resource="&geotime;"/>	<vann:termGroup rdf:resource="&geotime;Stage"/>	<vann:termGroup rdf:resource="&geotime;Chronostratigraphic"/>	<vs:term_status>unstable</vs:term_status>	</skos:Concept>
<skos:Concept rdf:about="&geotime;Barremian">	<skos:prefLabel xml:lang="en">Barremian</skos:prefLabel>	<skos:definition>The Barremian time period started 129.97  million years (Ma) before present (BP) and ended 125 Ma BP.</skos:definition>	<rdfs:seeAlso rdf:resource="http://kos.gbif.org/wiki/geotime:Barremian"/>	<geotime:rangeType>Stage</geotime:rangeType>	<geotime:rangeTypeURI rdf:resource="&geotime;Stage"/>	<geotime:start>129.97</geotime:start>	<geotime:end>125</geotime:end>		<dcterms:created>2011-01-11</dcterms:created>	<dcterms:modified>2012-08-03</dcterms:modified>	<dcterms:hasVersion rdf:resource="&history;20120803/geotime#Barremian"/>	<rdfs:isDefinedBy rdf:resource="&geotime;"/>	<skos:inScheme rdf:resource="&geotime;"/>	<vann:termGroup rdf:resource="&geotime;Stage"/>	<vann:termGroup rdf:resource="&geotime;Chronostratigraphic"/>	<vs:term_status>unstable</vs:term_status>	</skos:Concept>
<skos:Concept rdf:about="&geotime;Hauterivian">	<skos:prefLabel xml:lang="en">Hauterivian</skos:prefLabel>	<skos:definition>The Hauterivian time period started 136.44  million years (Ma) before present (BP) and ended 129.97 Ma BP.</skos:definition>	<rdfs:seeAlso rdf:resource="http://kos.gbif.org/wiki/geotime:Hauterivian"/>	<geotime:rangeType>Stage</geotime:rangeType>	<geotime:rangeTypeURI rdf:resource="&geotime;Stage"/>	<geotime:start>136.44</geotime:start>	<geotime:end>129.97</geotime:end>		<dcterms:created>2011-01-11</dcterms:created>	<dcterms:modified>2012-08-03</dcterms:modified>	<dcterms:hasVersion rdf:resource="&history;20120803/geotime#Hauterivian"/>	<rdfs:isDefinedBy rdf:resource="&geotime;"/>	<skos:inScheme rdf:resource="&geotime;"/>	<vann:termGroup rdf:resource="&geotime;Stage"/>	<vann:termGroup rdf:resource="&geotime;Chronostratigraphic"/>	<vs:term_status>unstable</vs:term_status>	</skos:Concept>
<skos:Concept rdf:about="&geotime;Valanginian">	<skos:prefLabel xml:lang="en">Valanginian</skos:prefLabel>	<skos:definition>The Valanginian time period started 140.18  million years (Ma) before present (BP) and ended 136.44 Ma BP.</skos:definition>	<rdfs:seeAlso rdf:resource="http://kos.gbif.org/wiki/geotime:Valanginian"/>	<geotime:rangeType>Stage</geotime:rangeType>	<geotime:rangeTypeURI rdf:resource="&geotime;Stage"/>	<geotime:start>140.18</geotime:start>	<geotime:end>136.44</geotime:end>		<dcterms:created>2011-01-11</dcterms:created>	<dcterms:modified>2012-08-03</dcterms:modified>	<dcterms:hasVersion rdf:resource="&history;20120803/geotime#Valanginian"/>	<rdfs:isDefinedBy rdf:resource="&geotime;"/>	<skos:inScheme rdf:resource="&geotime;"/>	<vann:termGroup rdf:resource="&geotime;Stage"/>	<vann:termGroup rdf:resource="&geotime;Chronostratigraphic"/>	<vs:term_status>unstable</vs:term_status>	</skos:Concept>
<skos:Concept rdf:about="&geotime;Berriasian">	<skos:prefLabel xml:lang="en">Berriasian</skos:prefLabel>	<skos:definition>The Berriasian time period started 145.46  million years (Ma) before present (BP) and ended 140.18 Ma BP.</skos:definition>	<rdfs:seeAlso rdf:resource="http://kos.gbif.org/wiki/geotime:Berriasian"/>	<geotime:rangeType>Stage</geotime:rangeType>	<geotime:rangeTypeURI rdf:resource="&geotime;Stage"/>	<geotime:start>145.46</geotime:start>	<geotime:end>140.18</geotime:end>		<dcterms:created>2011-01-11</dcterms:created>	<dcterms:modified>2012-08-03</dcterms:modified>	<dcterms:hasVersion rdf:resource="&history;20120803/geotime#Berriasian"/>	<rdfs:isDefinedBy rdf:resource="&geotime;"/>	<skos:inScheme rdf:resource="&geotime;"/>	<vann:termGroup rdf:resource="&geotime;Stage"/>	<vann:termGroup rdf:resource="&geotime;Chronostratigraphic"/>	<vs:term_status>unstable</vs:term_status>	</skos:Concept>
<skos:Concept rdf:about="&geotime;Tithonian">	<skos:prefLabel xml:lang="en">Tithonian</skos:prefLabel>	<skos:definition>The Tithonian time period started 150.844  million years (Ma) before present (BP) and ended 145.46 Ma BP.</skos:definition>	<rdfs:seeAlso rdf:resource="http://kos.gbif.org/wiki/geotime:Tithonian"/>	<geotime:rangeType>Stage</geotime:rangeType>	<geotime:rangeTypeURI rdf:resource="&geotime;Stage"/>	<geotime:start>150.844</geotime:start>	<geotime:end>145.46</geotime:end>		<dcterms:created>2011-01-11</dcterms:created>	<dcterms:modified>2012-08-03</dcterms:modified>	<dcterms:hasVersion rdf:resource="&history;20120803/geotime#Tithonian"/>	<rdfs:isDefinedBy rdf:resource="&geotime;"/>	<skos:inScheme rdf:resource="&geotime;"/>	<vann:termGroup rdf:resource="&geotime;Stage"/>	<vann:termGroup rdf:resource="&geotime;Chronostratigraphic"/>	<vs:term_status>unstable</vs:term_status>	</skos:Concept>
<skos:Concept rdf:about="&geotime;Kimmeridgian">	<skos:prefLabel xml:lang="en">Kimmeridgian</skos:prefLabel>	<skos:definition>The Kimmeridgian time period started 155.646  million years (Ma) before present (BP) and ended 150.844 Ma BP.</skos:definition>	<rdfs:seeAlso rdf:resource="http://kos.gbif.org/wiki/geotime:Kimmeridgian"/>	<geotime:rangeType>Stage</geotime:rangeType>	<geotime:rangeTypeURI rdf:resource="&geotime;Stage"/>	<geotime:start>155.646</geotime:start>	<geotime:end>150.844</geotime:end>		<dcterms:created>2011-01-11</dcterms:created>	<dcterms:modified>2012-08-03</dcterms:modified>	<dcterms:hasVersion rdf:resource="&history;20120803/geotime#Kimmeridgian"/>	<rdfs:isDefinedBy rdf:resource="&geotime;"/>	<skos:inScheme rdf:resource="&geotime;"/>	<vann:termGroup rdf:resource="&geotime;Stage"/>	<vann:termGroup rdf:resource="&geotime;Chronostratigraphic"/>	<vs:term_status>unstable</vs:term_status>	</skos:Concept>
<skos:Concept rdf:about="&geotime;Oxfordian">	<skos:prefLabel xml:lang="en">Oxfordian</skos:prefLabel>	<skos:definition>The Oxfordian time period started 161.21  million years (Ma) before present (BP) and ended 155.646 Ma BP.</skos:definition>	<rdfs:seeAlso rdf:resource="http://kos.gbif.org/wiki/geotime:Oxfordian"/>	<geotime:rangeType>Stage</geotime:rangeType>	<geotime:rangeTypeURI rdf:resource="&geotime;Stage"/>	<geotime:start>161.21</geotime:start>	<geotime:end>155.646</geotime:end>		<dcterms:created>2011-01-11</dcterms:created>	<dcterms:modified>2012-08-03</dcterms:modified>	<dcterms:hasVersion rdf:resource="&history;20120803/geotime#Oxfordian"/>	<rdfs:isDefinedBy rdf:resource="&geotime;"/>	<skos:inScheme rdf:resource="&geotime;"/>	<vann:termGroup rdf:resource="&geotime;Stage"/>	<vann:termGroup rdf:resource="&geotime;Chronostratigraphic"/>	<vs:term_status>unstable</vs:term_status>	</skos:Concept>
<skos:Concept rdf:about="&geotime;Callovian">	<skos:prefLabel xml:lang="en">Callovian</skos:prefLabel>	<skos:definition>The Callovian time period started 164.74  million years (Ma) before present (BP) and ended 161.21 Ma BP.</skos:definition>	<rdfs:seeAlso rdf:resource="http://kos.gbif.org/wiki/geotime:Callovian"/>	<geotime:rangeType>Stage</geotime:rangeType>	<geotime:rangeTypeURI rdf:resource="&geotime;Stage"/>	<geotime:start>164.74</geotime:start>	<geotime:end>161.21</geotime:end>		<dcterms:created>2011-01-11</dcterms:created>	<dcterms:modified>2012-08-03</dcterms:modified>	<dcterms:hasVersion rdf:resource="&history;20120803/geotime#Callovian"/>	<rdfs:isDefinedBy rdf:resource="&geotime;"/>	<skos:inScheme rdf:resource="&geotime;"/>	<vann:termGroup rdf:resource="&geotime;Stage"/>	<vann:termGroup rdf:resource="&geotime;Chronostratigraphic"/>	<vs:term_status>unstable</vs:term_status>	</skos:Concept>
<skos:Concept rdf:about="&geotime;Bathonian">	<skos:prefLabel xml:lang="en">Bathonian</skos:prefLabel>	<skos:definition>The Bathonian time period started 167.68  million years (Ma) before present (BP) and ended 164.74 Ma BP.</skos:definition>	<rdfs:seeAlso rdf:resource="http://kos.gbif.org/wiki/geotime:Bathonian"/>	<geotime:rangeType>Stage</geotime:rangeType>	<geotime:rangeTypeURI rdf:resource="&geotime;Stage"/>	<geotime:start>167.68</geotime:start>	<geotime:end>164.74</geotime:end>		<dcterms:created>2011-01-11</dcterms:created>	<dcterms:modified>2012-08-03</dcterms:modified>	<dcterms:hasVersion rdf:resource="&history;20120803/geotime#Bathonian"/>	<rdfs:isDefinedBy rdf:resource="&geotime;"/>	<skos:inScheme rdf:resource="&geotime;"/>	<vann:termGroup rdf:resource="&geotime;Stage"/>	<vann:termGroup rdf:resource="&geotime;Chronostratigraphic"/>	<vs:term_status>unstable</vs:term_status>	</skos:Concept>
<skos:Concept rdf:about="&geotime;Bajocian">	<skos:prefLabel xml:lang="en">Bajocian</skos:prefLabel>	<skos:definition>The Bajocian time period started 171.6  million years (Ma) before present (BP) and ended 167.68 Ma BP.</skos:definition>	<rdfs:seeAlso rdf:resource="http://kos.gbif.org/wiki/geotime:Bajocian"/>	<geotime:rangeType>Stage</geotime:rangeType>	<geotime:rangeTypeURI rdf:resource="&geotime;Stage"/>	<geotime:start>171.6</geotime:start>	<geotime:end>167.68</geotime:end>		<dcterms:created>2011-01-11</dcterms:created>	<dcterms:modified>2012-08-03</dcterms:modified>	<dcterms:hasVersion rdf:resource="&history;20120803/geotime#Bajocian"/>	<rdfs:isDefinedBy rdf:resource="&geotime;"/>	<skos:inScheme rdf:resource="&geotime;"/>	<vann:termGroup rdf:resource="&geotime;Stage"/>	<vann:termGroup rdf:resource="&geotime;Chronostratigraphic"/>	<vs:term_status>unstable</vs:term_status>	</skos:Concept>
<skos:Concept rdf:about="&geotime;Aalenian">	<skos:prefLabel xml:lang="en">Aalenian</skos:prefLabel>	<skos:definition>The Aalenian time period started 175.6  million years (Ma) before present (BP) and ended 171.6 Ma BP.</skos:definition>	<rdfs:seeAlso rdf:resource="http://kos.gbif.org/wiki/geotime:Aalenian"/>	<geotime:rangeType>Stage</geotime:rangeType>	<geotime:rangeTypeURI rdf:resource="&geotime;Stage"/>	<geotime:start>175.6</geotime:start>	<geotime:end>171.6</geotime:end>		<dcterms:created>2011-01-11</dcterms:created>	<dcterms:modified>2012-08-03</dcterms:modified>	<dcterms:hasVersion rdf:resource="&history;20120803/geotime#Aalenian"/>	<rdfs:isDefinedBy rdf:resource="&geotime;"/>	<skos:inScheme rdf:resource="&geotime;"/>	<vann:termGroup rdf:resource="&geotime;Stage"/>	<vann:termGroup rdf:resource="&geotime;Chronostratigraphic"/>	<vs:term_status>unstable</vs:term_status>	</skos:Concept>
<skos:Concept rdf:about="&geotime;Toarcian">	<skos:prefLabel xml:lang="en">Toarcian</skos:prefLabel>	<skos:definition>The Toarcian time period started 183  million years (Ma) before present (BP) and ended 175.6 Ma BP.</skos:definition>	<rdfs:seeAlso rdf:resource="http://kos.gbif.org/wiki/geotime:Toarcian"/>	<geotime:rangeType>Stage</geotime:rangeType>	<geotime:rangeTypeURI rdf:resource="&geotime;Stage"/>	<geotime:start>183</geotime:start>	<geotime:end>175.6</geotime:end>		<dcterms:created>2011-01-11</dcterms:created>	<dcterms:modified>2012-08-03</dcterms:modified>	<dcterms:hasVersion rdf:resource="&history;20120803/geotime#Toarcian"/>	<rdfs:isDefinedBy rdf:resource="&geotime;"/>	<skos:inScheme rdf:resource="&geotime;"/>	<vann:termGroup rdf:resource="&geotime;Stage"/>	<vann:termGroup rdf:resource="&geotime;Chronostratigraphic"/>	<vs:term_status>unstable</vs:term_status>	</skos:Concept>
<skos:Concept rdf:about="&geotime;Pliensbachian">	<skos:prefLabel xml:lang="en">Pliensbachian</skos:prefLabel>	<skos:definition>The Pliensbachian time period started 189.6  million years (Ma) before present (BP) and ended 183 Ma BP.</skos:definition>	<rdfs:seeAlso rdf:resource="http://kos.gbif.org/wiki/geotime:Pliensbachian"/>	<geotime:rangeType>Stage</geotime:rangeType>	<geotime:rangeTypeURI rdf:resource="&geotime;Stage"/>	<geotime:start>189.6</geotime:start>	<geotime:end>183</geotime:end>		<dcterms:created>2011-01-11</dcterms:created>	<dcterms:modified>2012-08-03</dcterms:modified>	<dcterms:hasVersion rdf:resource="&history;20120803/geotime#Pliensbachian"/>	<rdfs:isDefinedBy rdf:resource="&geotime;"/>	<skos:inScheme rdf:resource="&geotime;"/>	<vann:termGroup rdf:resource="&geotime;Stage"/>	<vann:termGroup rdf:resource="&geotime;Chronostratigraphic"/>	<vs:term_status>unstable</vs:term_status>	</skos:Concept>
<skos:Concept rdf:about="&geotime;Sinemurian">	<skos:prefLabel xml:lang="en">Sinemurian</skos:prefLabel>	<skos:definition>The Sinemurian time period started 196.5  million years (Ma) before present (BP) and ended 189.6 Ma BP.</skos:definition>	<rdfs:seeAlso rdf:resource="http://kos.gbif.org/wiki/geotime:Sinemurian"/>	<geotime:rangeType>Stage</geotime:rangeType>	<geotime:rangeTypeURI rdf:resource="&geotime;Stage"/>	<geotime:start>196.5</geotime:start>	<geotime:end>189.6</geotime:end>		<dcterms:created>2011-01-11</dcterms:created>	<dcterms:modified>2012-08-03</dcterms:modified>	<dcterms:hasVersion rdf:resource="&history;20120803/geotime#Sinemurian"/>	<rdfs:isDefinedBy rdf:resource="&geotime;"/>	<skos:inScheme rdf:resource="&geotime;"/>	<vann:termGroup rdf:resource="&geotime;Stage"/>	<vann:termGroup rdf:resource="&geotime;Chronostratigraphic"/>	<vs:term_status>unstable</vs:term_status>	</skos:Concept>
<skos:Concept rdf:about="&geotime;Hettangian">	<skos:prefLabel xml:lang="en">Hettangian</skos:prefLabel>	<skos:definition>The Hettangian time period started 199.6  million years (Ma) before present (BP) and ended 196.5 Ma BP.</skos:definition>	<rdfs:seeAlso rdf:resource="http://kos.gbif.org/wiki/geotime:Hettangian"/>	<geotime:rangeType>Stage</geotime:rangeType>	<geotime:rangeTypeURI rdf:resource="&geotime;Stage"/>	<geotime:start>199.6</geotime:start>	<geotime:end>196.5</geotime:end>		<dcterms:created>2011-01-11</dcterms:created>	<dcterms:modified>2012-08-03</dcterms:modified>	<dcterms:hasVersion rdf:resource="&history;20120803/geotime#Hettangian"/>	<rdfs:isDefinedBy rdf:resource="&geotime;"/>	<skos:inScheme rdf:resource="&geotime;"/>	<vann:termGroup rdf:resource="&geotime;Stage"/>	<vann:termGroup rdf:resource="&geotime;Chronostratigraphic"/>	<vs:term_status>unstable</vs:term_status>	</skos:Concept>
<skos:Concept rdf:about="&geotime;Rhaetian">	<skos:prefLabel xml:lang="en">Rhaetian</skos:prefLabel>	<skos:definition>The Rhaetian time period started 203.64  million years (Ma) before present (BP) and ended 199.6 Ma BP.</skos:definition>	<rdfs:seeAlso rdf:resource="http://kos.gbif.org/wiki/geotime:Rhaetian"/>	<geotime:rangeType>Stage</geotime:rangeType>	<geotime:rangeTypeURI rdf:resource="&geotime;Stage"/>	<geotime:start>203.64</geotime:start>	<geotime:end>199.6</geotime:end>		<dcterms:created>2011-01-11</dcterms:created>	<dcterms:modified>2012-08-03</dcterms:modified>	<dcterms:hasVersion rdf:resource="&history;20120803/geotime#Rhaetian"/>	<rdfs:isDefinedBy rdf:resource="&geotime;"/>	<skos:inScheme rdf:resource="&geotime;"/>	<vann:termGroup rdf:resource="&geotime;Stage"/>	<vann:termGroup rdf:resource="&geotime;Chronostratigraphic"/>	<vs:term_status>unstable</vs:term_status>	</skos:Concept>
<skos:Concept rdf:about="&geotime;Norian">	<skos:prefLabel xml:lang="en">Norian</skos:prefLabel>	<skos:definition>The Norian time period started 216.53  million years (Ma) before present (BP) and ended 203.64 Ma BP.</skos:definition>	<rdfs:seeAlso rdf:resource="http://kos.gbif.org/wiki/geotime:Norian"/>	<geotime:rangeType>Stage</geotime:rangeType>	<geotime:rangeTypeURI rdf:resource="&geotime;Stage"/>	<geotime:start>216.53</geotime:start>	<geotime:end>203.64</geotime:end>		<dcterms:created>2011-01-11</dcterms:created>	<dcterms:modified>2012-08-03</dcterms:modified>	<dcterms:hasVersion rdf:resource="&history;20120803/geotime#Norian"/>	<rdfs:isDefinedBy rdf:resource="&geotime;"/>	<skos:inScheme rdf:resource="&geotime;"/>	<vann:termGroup rdf:resource="&geotime;Stage"/>	<vann:termGroup rdf:resource="&geotime;Chronostratigraphic"/>	<vs:term_status>unstable</vs:term_status>	</skos:Concept>
<skos:Concept rdf:about="&geotime;Carnian">	<skos:prefLabel xml:lang="en">Carnian</skos:prefLabel>	<skos:definition>The Carnian time period started 228.01  million years (Ma) before present (BP) and ended 216.53 Ma BP.</skos:definition>	<rdfs:seeAlso rdf:resource="http://kos.gbif.org/wiki/geotime:Carnian"/>	<geotime:rangeType>Stage</geotime:rangeType>	<geotime:rangeTypeURI rdf:resource="&geotime;Stage"/>	<geotime:start>228.01</geotime:start>	<geotime:end>216.53</geotime:end>		<dcterms:created>2011-01-11</dcterms:created>	<dcterms:modified>2012-08-03</dcterms:modified>	<dcterms:hasVersion rdf:resource="&history;20120803/geotime#Carnian"/>	<rdfs:isDefinedBy rdf:resource="&geotime;"/>	<skos:inScheme rdf:resource="&geotime;"/>	<vann:termGroup rdf:resource="&geotime;Stage"/>	<vann:termGroup rdf:resource="&geotime;Chronostratigraphic"/>	<vs:term_status>unstable</vs:term_status>	</skos:Concept>
<skos:Concept rdf:about="&geotime;Ladinian">	<skos:prefLabel xml:lang="en">Ladinian</skos:prefLabel>	<skos:definition>The Ladinian time period started 237  million years (Ma) before present (BP) and ended 228.01 Ma BP.</skos:definition>	<rdfs:seeAlso rdf:resource="http://kos.gbif.org/wiki/geotime:Ladinian"/>	<geotime:rangeType>Stage</geotime:rangeType>	<geotime:rangeTypeURI rdf:resource="&geotime;Stage"/>	<geotime:start>237</geotime:start>	<geotime:end>228.01</geotime:end>		<dcterms:created>2011-01-11</dcterms:created>	<dcterms:modified>2012-08-03</dcterms:modified>	<dcterms:hasVersion rdf:resource="&history;20120803/geotime#Ladinian"/>	<rdfs:isDefinedBy rdf:resource="&geotime;"/>	<skos:inScheme rdf:resource="&geotime;"/>	<vann:termGroup rdf:resource="&geotime;Stage"/>	<vann:termGroup rdf:resource="&geotime;Chronostratigraphic"/>	<vs:term_status>unstable</vs:term_status>	</skos:Concept>
<skos:Concept rdf:about="&geotime;Anisian">	<skos:prefLabel xml:lang="en">Anisian</skos:prefLabel>	<skos:definition>The Anisian time period started 245.17  million years (Ma) before present (BP) and ended 237 Ma BP.</skos:definition>	<rdfs:seeAlso rdf:resource="http://kos.gbif.org/wiki/geotime:Anisian"/>	<geotime:rangeType>Stage</geotime:rangeType>	<geotime:rangeTypeURI rdf:resource="&geotime;Stage"/>	<geotime:start>245.17</geotime:start>	<geotime:end>237</geotime:end>		<dcterms:created>2011-01-11</dcterms:created>	<dcterms:modified>2012-08-03</dcterms:modified>	<dcterms:hasVersion rdf:resource="&history;20120803/geotime#Anisian"/>	<rdfs:isDefinedBy rdf:resource="&geotime;"/>	<skos:inScheme rdf:resource="&geotime;"/>	<vann:termGroup rdf:resource="&geotime;Stage"/>	<vann:termGroup rdf:resource="&geotime;Chronostratigraphic"/>	<vs:term_status>unstable</vs:term_status>	</skos:Concept>
<skos:Concept rdf:about="&geotime;Olenekian">	<skos:prefLabel xml:lang="en">Olenekian</skos:prefLabel>	<skos:definition>The Olenekian time period started 249.75  million years (Ma) before present (BP) and ended 245.17 Ma BP.</skos:definition>	<rdfs:seeAlso rdf:resource="http://kos.gbif.org/wiki/geotime:Olenekian"/>	<geotime:rangeType>Stage</geotime:rangeType>	<geotime:rangeTypeURI rdf:resource="&geotime;Stage"/>	<geotime:start>249.75</geotime:start>	<geotime:end>245.17</geotime:end>		<dcterms:created>2011-01-11</dcterms:created>	<dcterms:modified>2012-08-03</dcterms:modified>	<dcterms:hasVersion rdf:resource="&history;20120803/geotime#Olenekian"/>	<rdfs:isDefinedBy rdf:resource="&geotime;"/>	<skos:inScheme rdf:resource="&geotime;"/>	<vann:termGroup rdf:resource="&geotime;Stage"/>	<vann:termGroup rdf:resource="&geotime;Chronostratigraphic"/>	<vs:term_status>unstable</vs:term_status>	</skos:Concept>
<skos:Concept rdf:about="&geotime;Induan">	<skos:prefLabel xml:lang="en">Induan</skos:prefLabel>	<skos:definition>The Induan time period started 251  million years (Ma) before present (BP) and ended 249.75 Ma BP.</skos:definition>	<rdfs:seeAlso rdf:resource="http://kos.gbif.org/wiki/geotime:Induan"/>	<geotime:rangeType>Stage</geotime:rangeType>	<geotime:rangeTypeURI rdf:resource="&geotime;Stage"/>	<geotime:start>251</geotime:start>	<geotime:end>249.75</geotime:end>		<dcterms:created>2011-01-11</dcterms:created>	<dcterms:modified>2012-08-03</dcterms:modified>	<dcterms:hasVersion rdf:resource="&history;20120803/geotime#Induan"/>	<rdfs:isDefinedBy rdf:resource="&geotime;"/>	<skos:inScheme rdf:resource="&geotime;"/>	<vann:termGroup rdf:resource="&geotime;Stage"/>	<vann:termGroup rdf:resource="&geotime;Chronostratigraphic"/>	<vs:term_status>unstable</vs:term_status>	</skos:Concept>
<skos:Concept rdf:about="&geotime;Changhsingian">	<skos:prefLabel xml:lang="en">Changhsingian</skos:prefLabel>	<skos:definition>The Changhsingian time period started 253.8  million years (Ma) before present (BP) and ended 251 Ma BP.</skos:definition>	<rdfs:seeAlso rdf:resource="http://kos.gbif.org/wiki/geotime:Changhsingian"/>	<geotime:rangeType>Stage</geotime:rangeType>	<geotime:rangeTypeURI rdf:resource="&geotime;Stage"/>	<geotime:start>253.8</geotime:start>	<geotime:end>251</geotime:end>		<dcterms:created>2011-01-11</dcterms:created>	<dcterms:modified>2012-08-03</dcterms:modified>	<dcterms:hasVersion rdf:resource="&history;20120803/geotime#Changhsingian"/>	<rdfs:isDefinedBy rdf:resource="&geotime;"/>	<skos:inScheme rdf:resource="&geotime;"/>	<vann:termGroup rdf:resource="&geotime;Stage"/>	<vann:termGroup rdf:resource="&geotime;Chronostratigraphic"/>	<vs:term_status>unstable</vs:term_status>	</skos:Concept>
<skos:Concept rdf:about="&geotime;Wuchiapingian">	<skos:prefLabel xml:lang="en">Wuchiapingian</skos:prefLabel>	<skos:definition>The Wuchiapingian time period started 260.4  million years (Ma) before present (BP) and ended 253.8 Ma BP.</skos:definition>	<rdfs:seeAlso rdf:resource="http://kos.gbif.org/wiki/geotime:Wuchiapingian"/>	<geotime:rangeType>Stage</geotime:rangeType>	<geotime:rangeTypeURI rdf:resource="&geotime;Stage"/>	<geotime:start>260.4</geotime:start>	<geotime:end>253.8</geotime:end>		<dcterms:created>2011-01-11</dcterms:created>	<dcterms:modified>2012-08-03</dcterms:modified>	<dcterms:hasVersion rdf:resource="&history;20120803/geotime#Wuchiapingian"/>	<rdfs:isDefinedBy rdf:resource="&geotime;"/>	<skos:inScheme rdf:resource="&geotime;"/>	<vann:termGroup rdf:resource="&geotime;Stage"/>	<vann:termGroup rdf:resource="&geotime;Chronostratigraphic"/>	<vs:term_status>unstable</vs:term_status>	</skos:Concept>
<skos:Concept rdf:about="&geotime;Capitanian">	<skos:prefLabel xml:lang="en">Capitanian</skos:prefLabel>	<skos:definition>The Capitanian time period started 265.8  million years (Ma) before present (BP) and ended 260.4 Ma BP.</skos:definition>	<rdfs:seeAlso rdf:resource="http://kos.gbif.org/wiki/geotime:Capitanian"/>	<geotime:rangeType>Stage</geotime:rangeType>	<geotime:rangeTypeURI rdf:resource="&geotime;Stage"/>	<geotime:start>265.8</geotime:start>	<geotime:end>260.4</geotime:end>		<dcterms:created>2011-01-11</dcterms:created>	<dcterms:modified>2012-08-03</dcterms:modified>	<dcterms:hasVersion rdf:resource="&history;20120803/geotime#Capitanian"/>	<rdfs:isDefinedBy rdf:resource="&geotime;"/>	<skos:inScheme rdf:resource="&geotime;"/>	<vann:termGroup rdf:resource="&geotime;Stage"/>	<vann:termGroup rdf:resource="&geotime;Chronostratigraphic"/>	<vs:term_status>unstable</vs:term_status>	</skos:Concept>
<skos:Concept rdf:about="&geotime;Wordian">	<skos:prefLabel xml:lang="en">Wordian</skos:prefLabel>	<skos:definition>The Wordian time period started 268  million years (Ma) before present (BP) and ended 265.8 Ma BP.</skos:definition>	<rdfs:seeAlso rdf:resource="http://kos.gbif.org/wiki/geotime:Wordian"/>	<geotime:rangeType>Stage</geotime:rangeType>	<geotime:rangeTypeURI rdf:resource="&geotime;Stage"/>	<geotime:start>268</geotime:start>	<geotime:end>265.8</geotime:end>		<dcterms:created>2011-01-11</dcterms:created>	<dcterms:modified>2012-08-03</dcterms:modified>	<dcterms:hasVersion rdf:resource="&history;20120803/geotime#Wordian"/>	<rdfs:isDefinedBy rdf:resource="&geotime;"/>	<skos:inScheme rdf:resource="&geotime;"/>	<vann:termGroup rdf:resource="&geotime;Stage"/>	<vann:termGroup rdf:resource="&geotime;Chronostratigraphic"/>	<vs:term_status>unstable</vs:term_status>	</skos:Concept>
<skos:Concept rdf:about="&geotime;Roadian">	<skos:prefLabel xml:lang="en">Roadian</skos:prefLabel>	<skos:definition>The Roadian time period started 270.6  million years (Ma) before present (BP) and ended 268 Ma BP.</skos:definition>	<rdfs:seeAlso rdf:resource="http://kos.gbif.org/wiki/geotime:Roadian"/>	<geotime:rangeType>Stage</geotime:rangeType>	<geotime:rangeTypeURI rdf:resource="&geotime;Stage"/>	<geotime:start>270.6</geotime:start>	<geotime:end>268</geotime:end>		<dcterms:created>2011-01-11</dcterms:created>	<dcterms:modified>2012-08-03</dcterms:modified>	<dcterms:hasVersion rdf:resource="&history;20120803/geotime#Roadian"/>	<rdfs:isDefinedBy rdf:resource="&geotime;"/>	<skos:inScheme rdf:resource="&geotime;"/>	<vann:termGroup rdf:resource="&geotime;Stage"/>	<vann:termGroup rdf:resource="&geotime;Chronostratigraphic"/>	<vs:term_status>unstable</vs:term_status>	</skos:Concept>
<skos:Concept rdf:about="&geotime;Kungurian">	<skos:prefLabel xml:lang="en">Kungurian</skos:prefLabel>	<skos:definition>The Kungurian time period started 275.6  million years (Ma) before present (BP) and ended 270.6 Ma BP.</skos:definition>	<rdfs:seeAlso rdf:resource="http://kos.gbif.org/wiki/geotime:Kungurian"/>	<geotime:rangeType>Stage</geotime:rangeType>	<geotime:rangeTypeURI rdf:resource="&geotime;Stage"/>	<geotime:start>275.6</geotime:start>	<geotime:end>270.6</geotime:end>		<dcterms:created>2011-01-11</dcterms:created>	<dcterms:modified>2012-08-03</dcterms:modified>	<dcterms:hasVersion rdf:resource="&history;20120803/geotime#Kungurian"/>	<rdfs:isDefinedBy rdf:resource="&geotime;"/>	<skos:inScheme rdf:resource="&geotime;"/>	<vann:termGroup rdf:resource="&geotime;Stage"/>	<vann:termGroup rdf:resource="&geotime;Chronostratigraphic"/>	<vs:term_status>unstable</vs:term_status>	</skos:Concept>
<skos:Concept rdf:about="&geotime;Artinskian">	<skos:prefLabel xml:lang="en">Artinskian</skos:prefLabel>	<skos:definition>The Artinskian time period started 284.4  million years (Ma) before present (BP) and ended 275.6 Ma BP.</skos:definition>	<rdfs:seeAlso rdf:resource="http://kos.gbif.org/wiki/geotime:Artinskian"/>	<geotime:rangeType>Stage</geotime:rangeType>	<geotime:rangeTypeURI rdf:resource="&geotime;Stage"/>	<geotime:start>284.4</geotime:start>	<geotime:end>275.6</geotime:end>		<dcterms:created>2011-01-11</dcterms:created>	<dcterms:modified>2012-08-03</dcterms:modified>	<dcterms:hasVersion rdf:resource="&history;20120803/geotime#Artinskian"/>	<rdfs:isDefinedBy rdf:resource="&geotime;"/>	<skos:inScheme rdf:resource="&geotime;"/>	<vann:termGroup rdf:resource="&geotime;Stage"/>	<vann:termGroup rdf:resource="&geotime;Chronostratigraphic"/>	<vs:term_status>unstable</vs:term_status>	</skos:Concept>
<skos:Concept rdf:about="&geotime;Sakmarian">	<skos:prefLabel xml:lang="en">Sakmarian</skos:prefLabel>	<skos:definition>The Sakmarian time period started 294.6  million years (Ma) before present (BP) and ended 284.4 Ma BP.</skos:definition>	<rdfs:seeAlso rdf:resource="http://kos.gbif.org/wiki/geotime:Sakmarian"/>	<geotime:rangeType>Stage</geotime:rangeType>	<geotime:rangeTypeURI rdf:resource="&geotime;Stage"/>	<geotime:start>294.6</geotime:start>	<geotime:end>284.4</geotime:end>		<dcterms:created>2011-01-11</dcterms:created>	<dcterms:modified>2012-08-03</dcterms:modified>	<dcterms:hasVersion rdf:resource="&history;20120803/geotime#Sakmarian"/>	<rdfs:isDefinedBy rdf:resource="&geotime;"/>	<skos:inScheme rdf:resource="&geotime;"/>	<vann:termGroup rdf:resource="&geotime;Stage"/>	<vann:termGroup rdf:resource="&geotime;Chronostratigraphic"/>	<vs:term_status>unstable</vs:term_status>	</skos:Concept>
<skos:Concept rdf:about="&geotime;Asselian">	<skos:prefLabel xml:lang="en">Asselian</skos:prefLabel>	<skos:definition>The Asselian time period started 299  million years (Ma) before present (BP) and ended 294.6 Ma BP.</skos:definition>	<rdfs:seeAlso rdf:resource="http://kos.gbif.org/wiki/geotime:Asselian"/>	<geotime:rangeType>Stage</geotime:rangeType>	<geotime:rangeTypeURI rdf:resource="&geotime;Stage"/>	<geotime:start>299</geotime:start>	<geotime:end>294.6</geotime:end>		<dcterms:created>2011-01-11</dcterms:created>	<dcterms:modified>2012-08-03</dcterms:modified>	<dcterms:hasVersion rdf:resource="&history;20120803/geotime#Asselian"/>	<rdfs:isDefinedBy rdf:resource="&geotime;"/>	<skos:inScheme rdf:resource="&geotime;"/>	<vann:termGroup rdf:resource="&geotime;Stage"/>	<vann:termGroup rdf:resource="&geotime;Chronostratigraphic"/>	<vs:term_status>unstable</vs:term_status>	</skos:Concept>
<skos:Concept rdf:about="&geotime;Gzhelian">	<skos:prefLabel xml:lang="en">Gzhelian</skos:prefLabel>	<skos:definition>The Gzhelian time period started 303.9  million years (Ma) before present (BP) and ended 299 Ma BP.</skos:definition>	<rdfs:seeAlso rdf:resource="http://kos.gbif.org/wiki/geotime:Gzhelian"/>	<geotime:rangeType>Stage</geotime:rangeType>	<geotime:rangeTypeURI rdf:resource="&geotime;Stage"/>	<geotime:start>303.9</geotime:start>	<geotime:end>299</geotime:end>		<dcterms:created>2011-01-11</dcterms:created>	<dcterms:modified>2012-08-03</dcterms:modified>	<dcterms:hasVersion rdf:resource="&history;20120803/geotime#Gzhelian"/>	<rdfs:isDefinedBy rdf:resource="&geotime;"/>	<skos:inScheme rdf:resource="&geotime;"/>	<vann:termGroup rdf:resource="&geotime;Stage"/>	<vann:termGroup rdf:resource="&geotime;Chronostratigraphic"/>	<vs:term_status>unstable</vs:term_status>	</skos:Concept>
<skos:Concept rdf:about="&geotime;Kasimovian">	<skos:prefLabel xml:lang="en">Kasimovian</skos:prefLabel>	<skos:definition>The Kasimovian time period started 306.5  million years (Ma) before present (BP) and ended 303.9 Ma BP.</skos:definition>	<rdfs:seeAlso rdf:resource="http://kos.gbif.org/wiki/geotime:Kasimovian"/>	<geotime:rangeType>Stage</geotime:rangeType>	<geotime:rangeTypeURI rdf:resource="&geotime;Stage"/>	<geotime:start>306.5</geotime:start>	<geotime:end>303.9</geotime:end>		<dcterms:created>2011-01-11</dcterms:created>	<dcterms:modified>2012-08-03</dcterms:modified>	<dcterms:hasVersion rdf:resource="&history;20120803/geotime#Kasimovian"/>	<rdfs:isDefinedBy rdf:resource="&geotime;"/>	<skos:inScheme rdf:resource="&geotime;"/>	<vann:termGroup rdf:resource="&geotime;Stage"/>	<vann:termGroup rdf:resource="&geotime;Chronostratigraphic"/>	<vs:term_status>unstable</vs:term_status>	</skos:Concept>
<skos:Concept rdf:about="&geotime;Moscovian">	<skos:prefLabel xml:lang="en">Moscovian</skos:prefLabel>	<skos:definition>The Moscovian time period started 311.7  million years (Ma) before present (BP) and ended 306.5 Ma BP.</skos:definition>	<rdfs:seeAlso rdf:resource="http://kos.gbif.org/wiki/geotime:Moscovian"/>	<geotime:rangeType>Stage</geotime:rangeType>	<geotime:rangeTypeURI rdf:resource="&geotime;Stage"/>	<geotime:start>311.7</geotime:start>	<geotime:end>306.5</geotime:end>		<dcterms:created>2011-01-11</dcterms:created>	<dcterms:modified>2012-08-03</dcterms:modified>	<dcterms:hasVersion rdf:resource="&history;20120803/geotime#Moscovian"/>	<rdfs:isDefinedBy rdf:resource="&geotime;"/>	<skos:inScheme rdf:resource="&geotime;"/>	<vann:termGroup rdf:resource="&geotime;Stage"/>	<vann:termGroup rdf:resource="&geotime;Chronostratigraphic"/>	<vs:term_status>unstable</vs:term_status>	</skos:Concept>
<skos:Concept rdf:about="&geotime;Bashkirian">	<skos:prefLabel xml:lang="en">Bashkirian</skos:prefLabel>	<skos:definition>The Bashkirian time period started 318.1  million years (Ma) before present (BP) and ended 311.7 Ma BP.</skos:definition>	<rdfs:seeAlso rdf:resource="http://kos.gbif.org/wiki/geotime:Bashkirian"/>	<geotime:rangeType>Stage</geotime:rangeType>	<geotime:rangeTypeURI rdf:resource="&geotime;Stage"/>	<geotime:start>318.1</geotime:start>	<geotime:end>311.7</geotime:end>		<dcterms:created>2011-01-11</dcterms:created>	<dcterms:modified>2012-08-03</dcterms:modified>	<dcterms:hasVersion rdf:resource="&history;20120803/geotime#Bashkirian"/>	<rdfs:isDefinedBy rdf:resource="&geotime;"/>	<skos:inScheme rdf:resource="&geotime;"/>	<vann:termGroup rdf:resource="&geotime;Stage"/>	<vann:termGroup rdf:resource="&geotime;Chronostratigraphic"/>	<vs:term_status>unstable</vs:term_status>	</skos:Concept>
<skos:Concept rdf:about="&geotime;Serpukhovian">	<skos:prefLabel xml:lang="en">Serpukhovian</skos:prefLabel>	<skos:definition>The Serpukhovian time period started 326.4  million years (Ma) before present (BP) and ended 318.1 Ma BP.</skos:definition>	<rdfs:seeAlso rdf:resource="http://kos.gbif.org/wiki/geotime:Serpukhovian"/>	<geotime:rangeType>Stage</geotime:rangeType>	<geotime:rangeTypeURI rdf:resource="&geotime;Stage"/>	<geotime:start>326.4</geotime:start>	<geotime:end>318.1</geotime:end>		<dcterms:created>2011-01-11</dcterms:created>	<dcterms:modified>2012-08-03</dcterms:modified>	<dcterms:hasVersion rdf:resource="&history;20120803/geotime#Serpukhovian"/>	<rdfs:isDefinedBy rdf:resource="&geotime;"/>	<skos:inScheme rdf:resource="&geotime;"/>	<vann:termGroup rdf:resource="&geotime;Stage"/>	<vann:termGroup rdf:resource="&geotime;Chronostratigraphic"/>	<vs:term_status>unstable</vs:term_status>	</skos:Concept>
<skos:Concept rdf:about="&geotime;Visean">	<skos:prefLabel xml:lang="en">Visean</skos:prefLabel>	<skos:definition>The Visean time period started 345.3  million years (Ma) before present (BP) and ended 326.4 Ma BP.</skos:definition>	<rdfs:seeAlso rdf:resource="http://kos.gbif.org/wiki/geotime:Visean"/>	<geotime:rangeType>Stage</geotime:rangeType>	<geotime:rangeTypeURI rdf:resource="&geotime;Stage"/>	<geotime:start>345.3</geotime:start>	<geotime:end>326.4</geotime:end>		<dcterms:created>2011-01-11</dcterms:created>	<dcterms:modified>2012-08-03</dcterms:modified>	<dcterms:hasVersion rdf:resource="&history;20120803/geotime#Visean"/>	<rdfs:isDefinedBy rdf:resource="&geotime;"/>	<skos:inScheme rdf:resource="&geotime;"/>	<vann:termGroup rdf:resource="&geotime;Stage"/>	<vann:termGroup rdf:resource="&geotime;Chronostratigraphic"/>	<vs:term_status>unstable</vs:term_status>	</skos:Concept>
<skos:Concept rdf:about="&geotime;Tournaisian">	<skos:prefLabel xml:lang="en">Tournaisian</skos:prefLabel>	<skos:definition>The Tournaisian time period started 359.2  million years (Ma) before present (BP) and ended 345.3 Ma BP.</skos:definition>	<rdfs:seeAlso rdf:resource="http://kos.gbif.org/wiki/geotime:Tournaisian"/>	<geotime:rangeType>Stage</geotime:rangeType>	<geotime:rangeTypeURI rdf:resource="&geotime;Stage"/>	<geotime:start>359.2</geotime:start>	<geotime:end>345.3</geotime:end>		<dcterms:created>2011-01-11</dcterms:created>	<dcterms:modified>2012-08-03</dcterms:modified>	<dcterms:hasVersion rdf:resource="&history;20120803/geotime#Tournaisian"/>	<rdfs:isDefinedBy rdf:resource="&geotime;"/>	<skos:inScheme rdf:resource="&geotime;"/>	<vann:termGroup rdf:resource="&geotime;Stage"/>	<vann:termGroup rdf:resource="&geotime;Chronostratigraphic"/>	<vs:term_status>unstable</vs:term_status>	</skos:Concept>
<skos:Concept rdf:about="&geotime;Famennian">	<skos:prefLabel xml:lang="en">Famennian</skos:prefLabel>	<skos:definition>The Famennian time period started 374.5  million years (Ma) before present (BP) and ended 359.2 Ma BP.</skos:definition>	<rdfs:seeAlso rdf:resource="http://kos.gbif.org/wiki/geotime:Famennian"/>	<geotime:rangeType>Stage</geotime:rangeType>	<geotime:rangeTypeURI rdf:resource="&geotime;Stage"/>	<geotime:start>374.5</geotime:start>	<geotime:end>359.2</geotime:end>		<dcterms:created>2011-01-11</dcterms:created>	<dcterms:modified>2012-08-03</dcterms:modified>	<dcterms:hasVersion rdf:resource="&history;20120803/geotime#Famennian"/>	<rdfs:isDefinedBy rdf:resource="&geotime;"/>	<skos:inScheme rdf:resource="&geotime;"/>	<vann:termGroup rdf:resource="&geotime;Stage"/>	<vann:termGroup rdf:resource="&geotime;Chronostratigraphic"/>	<vs:term_status>unstable</vs:term_status>	</skos:Concept>
<skos:Concept rdf:about="&geotime;Frasnian">	<skos:prefLabel xml:lang="en">Frasnian</skos:prefLabel>	<skos:definition>The Frasnian time period started 385.3  million years (Ma) before present (BP) and ended 374.5 Ma BP.</skos:definition>	<rdfs:seeAlso rdf:resource="http://kos.gbif.org/wiki/geotime:Frasnian"/>	<geotime:rangeType>Stage</geotime:rangeType>	<geotime:rangeTypeURI rdf:resource="&geotime;Stage"/>	<geotime:start>385.3</geotime:start>	<geotime:end>374.5</geotime:end>		<dcterms:created>2011-01-11</dcterms:created>	<dcterms:modified>2012-08-03</dcterms:modified>	<dcterms:hasVersion rdf:resource="&history;20120803/geotime#Frasnian"/>	<rdfs:isDefinedBy rdf:resource="&geotime;"/>	<skos:inScheme rdf:resource="&geotime;"/>	<vann:termGroup rdf:resource="&geotime;Stage"/>	<vann:termGroup rdf:resource="&geotime;Chronostratigraphic"/>	<vs:term_status>unstable</vs:term_status>	</skos:Concept>
<skos:Concept rdf:about="&geotime;Givetian">	<skos:prefLabel xml:lang="en">Givetian</skos:prefLabel>	<skos:definition>The Givetian time period started 391.8  million years (Ma) before present (BP) and ended 385.3 Ma BP.</skos:definition>	<rdfs:seeAlso rdf:resource="http://kos.gbif.org/wiki/geotime:Givetian"/>	<geotime:rangeType>Stage</geotime:rangeType>	<geotime:rangeTypeURI rdf:resource="&geotime;Stage"/>	<geotime:start>391.8</geotime:start>	<geotime:end>385.3</geotime:end>		<dcterms:created>2011-01-11</dcterms:created>	<dcterms:modified>2012-08-03</dcterms:modified>	<dcterms:hasVersion rdf:resource="&history;20120803/geotime#Givetian"/>	<rdfs:isDefinedBy rdf:resource="&geotime;"/>	<skos:inScheme rdf:resource="&geotime;"/>	<vann:termGroup rdf:resource="&geotime;Stage"/>	<vann:termGroup rdf:resource="&geotime;Chronostratigraphic"/>	<vs:term_status>unstable</vs:term_status>	</skos:Concept>
<skos:Concept rdf:about="&geotime;Eifelian">	<skos:prefLabel xml:lang="en">Eifelian</skos:prefLabel>	<skos:definition>The Eifelian time period started 397.5  million years (Ma) before present (BP) and ended 391.8 Ma BP.</skos:definition>	<rdfs:seeAlso rdf:resource="http://kos.gbif.org/wiki/geotime:Eifelian"/>	<geotime:rangeType>Stage</geotime:rangeType>	<geotime:rangeTypeURI rdf:resource="&geotime;Stage"/>	<geotime:start>397.5</geotime:start>	<geotime:end>391.8</geotime:end>		<dcterms:created>2011-01-11</dcterms:created>	<dcterms:modified>2012-08-03</dcterms:modified>	<dcterms:hasVersion rdf:resource="&history;20120803/geotime#Eifelian"/>	<rdfs:isDefinedBy rdf:resource="&geotime;"/>	<skos:inScheme rdf:resource="&geotime;"/>	<vann:termGroup rdf:resource="&geotime;Stage"/>	<vann:termGroup rdf:resource="&geotime;Chronostratigraphic"/>	<vs:term_status>unstable</vs:term_status>	</skos:Concept>
<skos:Concept rdf:about="&geotime;Emsian">	<skos:prefLabel xml:lang="en">Emsian</skos:prefLabel>	<skos:definition>The Emsian time period started 407  million years (Ma) before present (BP) and ended 397.5 Ma BP.</skos:definition>	<rdfs:seeAlso rdf:resource="http://kos.gbif.org/wiki/geotime:Emsian"/>	<geotime:rangeType>Stage</geotime:rangeType>	<geotime:rangeTypeURI rdf:resource="&geotime;Stage"/>	<geotime:start>407</geotime:start>	<geotime:end>397.5</geotime:end>		<dcterms:created>2011-01-11</dcterms:created>	<dcterms:modified>2012-08-03</dcterms:modified>	<dcterms:hasVersion rdf:resource="&history;20120803/geotime#Emsian"/>	<rdfs:isDefinedBy rdf:resource="&geotime;"/>	<skos:inScheme rdf:resource="&geotime;"/>	<vann:termGroup rdf:resource="&geotime;Stage"/>	<vann:termGroup rdf:resource="&geotime;Chronostratigraphic"/>	<vs:term_status>unstable</vs:term_status>	</skos:Concept>
<skos:Concept rdf:about="&geotime;Pragian">	<skos:prefLabel xml:lang="en">Pragian</skos:prefLabel>	<skos:definition>The Pragian time period started 411.2  million years (Ma) before present (BP) and ended 407 Ma BP.</skos:definition>	<rdfs:seeAlso rdf:resource="http://kos.gbif.org/wiki/geotime:Pragian"/>	<geotime:rangeType>Stage</geotime:rangeType>	<geotime:rangeTypeURI rdf:resource="&geotime;Stage"/>	<geotime:start>411.2</geotime:start>	<geotime:end>407</geotime:end>		<dcterms:created>2011-01-11</dcterms:created>	<dcterms:modified>2012-08-03</dcterms:modified>	<dcterms:hasVersion rdf:resource="&history;20120803/geotime#Pragian"/>	<rdfs:isDefinedBy rdf:resource="&geotime;"/>	<skos:inScheme rdf:resource="&geotime;"/>	<vann:termGroup rdf:resource="&geotime;Stage"/>	<vann:termGroup rdf:resource="&geotime;Chronostratigraphic"/>	<vs:term_status>unstable</vs:term_status>	</skos:Concept>
<skos:Concept rdf:about="&geotime;Lochkovian">	<skos:prefLabel xml:lang="en">Lochkovian</skos:prefLabel>	<skos:definition>The Lochkovian time period started 416  million years (Ma) before present (BP) and ended 411.2 Ma BP.</skos:definition>	<rdfs:seeAlso rdf:resource="http://kos.gbif.org/wiki/geotime:Lochkovian"/>	<geotime:rangeType>Stage</geotime:rangeType>	<geotime:rangeTypeURI rdf:resource="&geotime;Stage"/>	<geotime:start>416</geotime:start>	<geotime:end>411.2</geotime:end>		<dcterms:created>2011-01-11</dcterms:created>	<dcterms:modified>2012-08-03</dcterms:modified>	<dcterms:hasVersion rdf:resource="&history;20120803/geotime#Lochkovian"/>	<rdfs:isDefinedBy rdf:resource="&geotime;"/>	<skos:inScheme rdf:resource="&geotime;"/>	<vann:termGroup rdf:resource="&geotime;Stage"/>	<vann:termGroup rdf:resource="&geotime;Chronostratigraphic"/>	<vs:term_status>unstable</vs:term_status>	</skos:Concept>
<skos:Concept rdf:about="&geotime;Pridoli_not_divided">	<skos:prefLabel xml:lang="en">Pridoli not divided</skos:prefLabel>	<skos:definition>The Pridoli not divided time period started 418.7  million years (Ma) before present (BP) and ended 416 Ma BP.</skos:definition>	<rdfs:seeAlso rdf:resource="http://kos.gbif.org/wiki/geotime:Pridoli_not_divided"/>	<geotime:rangeType>Stage</geotime:rangeType>	<geotime:rangeTypeURI rdf:resource="&geotime;Stage"/>	<geotime:start>418.7</geotime:start>	<geotime:end>416</geotime:end>		<dcterms:created>2011-01-11</dcterms:created>	<dcterms:modified>2012-08-03</dcterms:modified>	<dcterms:hasVersion rdf:resource="&history;20120803/geotime#Pridoli_not_divided"/>	<rdfs:isDefinedBy rdf:resource="&geotime;"/>	<skos:inScheme rdf:resource="&geotime;"/>	<vann:termGroup rdf:resource="&geotime;Stage"/>	<vann:termGroup rdf:resource="&geotime;Chronostratigraphic"/>	<vs:term_status>unstable</vs:term_status>	</skos:Concept>
<skos:Concept rdf:about="&geotime;Ludfordian">	<skos:prefLabel xml:lang="en">Ludfordian</skos:prefLabel>	<skos:definition>The Ludfordian time period started 421.3  million years (Ma) before present (BP) and ended 418.7 Ma BP.</skos:definition>	<rdfs:seeAlso rdf:resource="http://kos.gbif.org/wiki/geotime:Ludfordian"/>	<geotime:rangeType>Stage</geotime:rangeType>	<geotime:rangeTypeURI rdf:resource="&geotime;Stage"/>	<geotime:start>421.3</geotime:start>	<geotime:end>418.7</geotime:end>		<dcterms:created>2011-01-11</dcterms:created>	<dcterms:modified>2012-08-03</dcterms:modified>	<dcterms:hasVersion rdf:resource="&history;20120803/geotime#Ludfordian"/>	<rdfs:isDefinedBy rdf:resource="&geotime;"/>	<skos:inScheme rdf:resource="&geotime;"/>	<vann:termGroup rdf:resource="&geotime;Stage"/>	<vann:termGroup rdf:resource="&geotime;Chronostratigraphic"/>	<vs:term_status>unstable</vs:term_status>	</skos:Concept>
<skos:Concept rdf:about="&geotime;Gorstian">	<skos:prefLabel xml:lang="en">Gorstian</skos:prefLabel>	<skos:definition>The Gorstian time period started 422.9  million years (Ma) before present (BP) and ended 421.3 Ma BP.</skos:definition>	<rdfs:seeAlso rdf:resource="http://kos.gbif.org/wiki/geotime:Gorstian"/>	<geotime:rangeType>Stage</geotime:rangeType>	<geotime:rangeTypeURI rdf:resource="&geotime;Stage"/>	<geotime:start>422.9</geotime:start>	<geotime:end>421.3</geotime:end>		<dcterms:created>2011-01-11</dcterms:created>	<dcterms:modified>2012-08-03</dcterms:modified>	<dcterms:hasVersion rdf:resource="&history;20120803/geotime#Gorstian"/>	<rdfs:isDefinedBy rdf:resource="&geotime;"/>	<skos:inScheme rdf:resource="&geotime;"/>	<vann:termGroup rdf:resource="&geotime;Stage"/>	<vann:termGroup rdf:resource="&geotime;Chronostratigraphic"/>	<vs:term_status>unstable</vs:term_status>	</skos:Concept>
<skos:Concept rdf:about="&geotime;Homerian">	<skos:prefLabel xml:lang="en">Homerian</skos:prefLabel>	<skos:definition>The Homerian time period started 426.2  million years (Ma) before present (BP) and ended 422.9 Ma BP.</skos:definition>	<rdfs:seeAlso rdf:resource="http://kos.gbif.org/wiki/geotime:Homerian"/>	<geotime:rangeType>Stage</geotime:rangeType>	<geotime:rangeTypeURI rdf:resource="&geotime;Stage"/>	<geotime:start>426.2</geotime:start>	<geotime:end>422.9</geotime:end>		<dcterms:created>2011-01-11</dcterms:created>	<dcterms:modified>2012-08-03</dcterms:modified>	<dcterms:hasVersion rdf:resource="&history;20120803/geotime#Homerian"/>	<rdfs:isDefinedBy rdf:resource="&geotime;"/>	<skos:inScheme rdf:resource="&geotime;"/>	<vann:termGroup rdf:resource="&geotime;Stage"/>	<vann:termGroup rdf:resource="&geotime;Chronostratigraphic"/>	<vs:term_status>unstable</vs:term_status>	</skos:Concept>
<skos:Concept rdf:about="&geotime;Sheinwoodian">	<skos:prefLabel xml:lang="en">Sheinwoodian</skos:prefLabel>	<skos:definition>The Sheinwoodian time period started 428.2  million years (Ma) before present (BP) and ended 426.2 Ma BP.</skos:definition>	<rdfs:seeAlso rdf:resource="http://kos.gbif.org/wiki/geotime:Sheinwoodian"/>	<geotime:rangeType>Stage</geotime:rangeType>	<geotime:rangeTypeURI rdf:resource="&geotime;Stage"/>	<geotime:start>428.2</geotime:start>	<geotime:end>426.2</geotime:end>		<dcterms:created>2011-01-11</dcterms:created>	<dcterms:modified>2012-08-03</dcterms:modified>	<dcterms:hasVersion rdf:resource="&history;20120803/geotime#Sheinwoodian"/>	<rdfs:isDefinedBy rdf:resource="&geotime;"/>	<skos:inScheme rdf:resource="&geotime;"/>	<vann:termGroup rdf:resource="&geotime;Stage"/>	<vann:termGroup rdf:resource="&geotime;Chronostratigraphic"/>	<vs:term_status>unstable</vs:term_status>	</skos:Concept>
<skos:Concept rdf:about="&geotime;Telychian">	<skos:prefLabel xml:lang="en">Telychian</skos:prefLabel>	<skos:definition>The Telychian time period started 436.1  million years (Ma) before present (BP) and ended 428.2 Ma BP.</skos:definition>	<rdfs:seeAlso rdf:resource="http://kos.gbif.org/wiki/geotime:Telychian"/>	<geotime:rangeType>Stage</geotime:rangeType>	<geotime:rangeTypeURI rdf:resource="&geotime;Stage"/>	<geotime:start>436.1</geotime:start>	<geotime:end>428.2</geotime:end>		<dcterms:created>2011-01-11</dcterms:created>	<dcterms:modified>2012-08-03</dcterms:modified>	<dcterms:hasVersion rdf:resource="&history;20120803/geotime#Telychian"/>	<rdfs:isDefinedBy rdf:resource="&geotime;"/>	<skos:inScheme rdf:resource="&geotime;"/>	<vann:termGroup rdf:resource="&geotime;Stage"/>	<vann:termGroup rdf:resource="&geotime;Chronostratigraphic"/>	<vs:term_status>unstable</vs:term_status>	</skos:Concept>
<skos:Concept rdf:about="&geotime;Aeronian">	<skos:prefLabel xml:lang="en">Aeronian</skos:prefLabel>	<skos:definition>The Aeronian time period started 439  million years (Ma) before present (BP) and ended 436.1 Ma BP.</skos:definition>	<rdfs:seeAlso rdf:resource="http://kos.gbif.org/wiki/geotime:Aeronian"/>	<geotime:rangeType>Stage</geotime:rangeType>	<geotime:rangeTypeURI rdf:resource="&geotime;Stage"/>	<geotime:start>439</geotime:start>	<geotime:end>436.1</geotime:end>		<dcterms:created>2011-01-11</dcterms:created>	<dcterms:modified>2012-08-03</dcterms:modified>	<dcterms:hasVersion rdf:resource="&history;20120803/geotime#Aeronian"/>	<rdfs:isDefinedBy rdf:resource="&geotime;"/>	<skos:inScheme rdf:resource="&geotime;"/>	<vann:termGroup rdf:resource="&geotime;Stage"/>	<vann:termGroup rdf:resource="&geotime;Chronostratigraphic"/>	<vs:term_status>unstable</vs:term_status>	</skos:Concept>
<skos:Concept rdf:about="&geotime;Rhuddanian">	<skos:prefLabel xml:lang="en">Rhuddanian</skos:prefLabel>	<skos:definition>The Rhuddanian time period started 443.7  million years (Ma) before present (BP) and ended 439 Ma BP.</skos:definition>	<rdfs:seeAlso rdf:resource="http://kos.gbif.org/wiki/geotime:Rhuddanian"/>	<geotime:rangeType>Stage</geotime:rangeType>	<geotime:rangeTypeURI rdf:resource="&geotime;Stage"/>	<geotime:start>443.7</geotime:start>	<geotime:end>439</geotime:end>		<dcterms:created>2011-01-11</dcterms:created>	<dcterms:modified>2012-08-03</dcterms:modified>	<dcterms:hasVersion rdf:resource="&history;20120803/geotime#Rhuddanian"/>	<rdfs:isDefinedBy rdf:resource="&geotime;"/>	<skos:inScheme rdf:resource="&geotime;"/>	<vann:termGroup rdf:resource="&geotime;Stage"/>	<vann:termGroup rdf:resource="&geotime;Chronostratigraphic"/>	<vs:term_status>unstable</vs:term_status>	</skos:Concept>
<skos:Concept rdf:about="&geotime;Hirnantian">	<skos:prefLabel xml:lang="en">Hirnantian</skos:prefLabel>	<skos:definition>The Hirnantian time period started 445.6  million years (Ma) before present (BP) and ended 443.7 Ma BP.</skos:definition>	<rdfs:seeAlso rdf:resource="http://kos.gbif.org/wiki/geotime:Hirnantian"/>	<geotime:rangeType>Stage</geotime:rangeType>	<geotime:rangeTypeURI rdf:resource="&geotime;Stage"/>	<geotime:start>445.6</geotime:start>	<geotime:end>443.7</geotime:end>		<dcterms:created>2011-01-11</dcterms:created>	<dcterms:modified>2012-08-03</dcterms:modified>	<dcterms:hasVersion rdf:resource="&history;20120803/geotime#Hirnantian"/>	<rdfs:isDefinedBy rdf:resource="&geotime;"/>	<skos:inScheme rdf:resource="&geotime;"/>	<vann:termGroup rdf:resource="&geotime;Stage"/>	<vann:termGroup rdf:resource="&geotime;Chronostratigraphic"/>	<vs:term_status>unstable</vs:term_status>	</skos:Concept>
<skos:Concept rdf:about="&geotime;Sixth">	<skos:prefLabel xml:lang="en">Sixth</skos:prefLabel>	<skos:definition>The Sixth time period started 455.8  million years (Ma) before present (BP) and ended 445.6 Ma BP.</skos:definition>	<rdfs:seeAlso rdf:resource="http://kos.gbif.org/wiki/geotime:Sixth"/>	<geotime:rangeType>Stage</geotime:rangeType>	<geotime:rangeTypeURI rdf:resource="&geotime;Stage"/>	<geotime:start>455.8</geotime:start>	<geotime:end>445.6</geotime:end>		<dcterms:created>2011-01-11</dcterms:created>	<dcterms:modified>2012-08-03</dcterms:modified>	<dcterms:hasVersion rdf:resource="&history;20120803/geotime#Sixth"/>	<rdfs:isDefinedBy rdf:resource="&geotime;"/>	<skos:inScheme rdf:resource="&geotime;"/>	<vann:termGroup rdf:resource="&geotime;Stage"/>	<vann:termGroup rdf:resource="&geotime;Chronostratigraphic"/>	<vs:term_status>unstable</vs:term_status>	</skos:Concept>
<skos:Concept rdf:about="&geotime;Fifth">	<skos:prefLabel xml:lang="en">Fifth</skos:prefLabel>	<skos:definition>The Fifth time period started 460.9  million years (Ma) before present (BP) and ended 455.8 Ma BP.</skos:definition>	<rdfs:seeAlso rdf:resource="http://kos.gbif.org/wiki/geotime:Fifth"/>	<geotime:rangeType>Stage</geotime:rangeType>	<geotime:rangeTypeURI rdf:resource="&geotime;Stage"/>	<geotime:start>460.9</geotime:start>	<geotime:end>455.8</geotime:end>		<dcterms:created>2011-01-11</dcterms:created>	<dcterms:modified>2012-08-03</dcterms:modified>	<dcterms:hasVersion rdf:resource="&history;20120803/geotime#Fifth"/>	<rdfs:isDefinedBy rdf:resource="&geotime;"/>	<skos:inScheme rdf:resource="&geotime;"/>	<vann:termGroup rdf:resource="&geotime;Stage"/>	<vann:termGroup rdf:resource="&geotime;Chronostratigraphic"/>	<vs:term_status>unstable</vs:term_status>	</skos:Concept>
<skos:Concept rdf:about="&geotime;Darriwillian">	<skos:prefLabel xml:lang="en">Darriwillian</skos:prefLabel>	<skos:definition>The Darriwillian time period started 468.1  million years (Ma) before present (BP) and ended 460.9 Ma BP.</skos:definition>	<rdfs:seeAlso rdf:resource="http://kos.gbif.org/wiki/geotime:Darriwillian"/>	<geotime:rangeType>Stage</geotime:rangeType>	<geotime:rangeTypeURI rdf:resource="&geotime;Stage"/>	<geotime:start>468.1</geotime:start>	<geotime:end>460.9</geotime:end>		<dcterms:created>2011-01-11</dcterms:created>	<dcterms:modified>2012-08-03</dcterms:modified>	<dcterms:hasVersion rdf:resource="&history;20120803/geotime#Darriwillian"/>	<rdfs:isDefinedBy rdf:resource="&geotime;"/>	<skos:inScheme rdf:resource="&geotime;"/>	<vann:termGroup rdf:resource="&geotime;Stage"/>	<vann:termGroup rdf:resource="&geotime;Chronostratigraphic"/>	<vs:term_status>unstable</vs:term_status>	</skos:Concept>
<skos:Concept rdf:about="&geotime;Third">	<skos:prefLabel xml:lang="en">Third</skos:prefLabel>	<skos:definition>The Third time period started 471.8  million years (Ma) before present (BP) and ended 468.1 Ma BP.</skos:definition>	<rdfs:seeAlso rdf:resource="http://kos.gbif.org/wiki/geotime:Third"/>	<geotime:rangeType>Stage</geotime:rangeType>	<geotime:rangeTypeURI rdf:resource="&geotime;Stage"/>	<geotime:start>471.8</geotime:start>	<geotime:end>468.1</geotime:end>		<dcterms:created>2011-01-11</dcterms:created>	<dcterms:modified>2012-08-03</dcterms:modified>	<dcterms:hasVersion rdf:resource="&history;20120803/geotime#Third"/>	<rdfs:isDefinedBy rdf:resource="&geotime;"/>	<skos:inScheme rdf:resource="&geotime;"/>	<vann:termGroup rdf:resource="&geotime;Stage"/>	<vann:termGroup rdf:resource="&geotime;Chronostratigraphic"/>	<vs:term_status>unstable</vs:term_status>	</skos:Concept>
<skos:Concept rdf:about="&geotime;Second">	<skos:prefLabel xml:lang="en">Second</skos:prefLabel>	<skos:definition>The Second time period started 478.6  million years (Ma) before present (BP) and ended 471.8 Ma BP.</skos:definition>	<rdfs:seeAlso rdf:resource="http://kos.gbif.org/wiki/geotime:Second"/>	<geotime:rangeType>Stage</geotime:rangeType>	<geotime:rangeTypeURI rdf:resource="&geotime;Stage"/>	<geotime:start>478.6</geotime:start>	<geotime:end>471.8</geotime:end>		<dcterms:created>2011-01-11</dcterms:created>	<dcterms:modified>2012-08-03</dcterms:modified>	<dcterms:hasVersion rdf:resource="&history;20120803/geotime#Second"/>	<rdfs:isDefinedBy rdf:resource="&geotime;"/>	<skos:inScheme rdf:resource="&geotime;"/>	<vann:termGroup rdf:resource="&geotime;Stage"/>	<vann:termGroup rdf:resource="&geotime;Chronostratigraphic"/>	<vs:term_status>unstable</vs:term_status>	</skos:Concept>
<skos:Concept rdf:about="&geotime;Tremadocian">	<skos:prefLabel xml:lang="en">Tremadocian</skos:prefLabel>	<skos:definition>The Tremadocian time period started 488.3  million years (Ma) before present (BP) and ended 478.6 Ma BP.</skos:definition>	<rdfs:seeAlso rdf:resource="http://kos.gbif.org/wiki/geotime:Tremadocian"/>	<geotime:rangeType>Stage</geotime:rangeType>	<geotime:rangeTypeURI rdf:resource="&geotime;Stage"/>	<geotime:start>488.3</geotime:start>	<geotime:end>478.6</geotime:end>		<dcterms:created>2011-01-11</dcterms:created>	<dcterms:modified>2012-08-03</dcterms:modified>	<dcterms:hasVersion rdf:resource="&history;20120803/geotime#Tremadocian"/>	<rdfs:isDefinedBy rdf:resource="&geotime;"/>	<skos:inScheme rdf:resource="&geotime;"/>	<vann:termGroup rdf:resource="&geotime;Stage"/>	<vann:termGroup rdf:resource="&geotime;Chronostratigraphic"/>	<vs:term_status>unstable</vs:term_status>	</skos:Concept>
<skos:Concept rdf:about="&geotime;UppermostCambrian_not_named">	<skos:prefLabel xml:lang="en">Uppermost Cambrian not named</skos:prefLabel>	<skos:definition>The Uppermost Cambrian not named time period started 496  million years (Ma) before present (BP) and ended 488.3 Ma BP.</skos:definition>	<rdfs:seeAlso rdf:resource="http://kos.gbif.org/wiki/geotime:UppermostCambrian_not_named"/>	<geotime:rangeType>Stage</geotime:rangeType>	<geotime:rangeTypeURI rdf:resource="&geotime;Stage"/>	<geotime:start>496</geotime:start>	<geotime:end>488.3</geotime:end>		<dcterms:created>2011-01-11</dcterms:created>	<dcterms:modified>2012-08-03</dcterms:modified>	<dcterms:hasVersion rdf:resource="&history;20120803/geotime#UppermostCambrian_not_named"/>	<rdfs:isDefinedBy rdf:resource="&geotime;"/>	<skos:inScheme rdf:resource="&geotime;"/>	<vann:termGroup rdf:resource="&geotime;Stage"/>	<vann:termGroup rdf:resource="&geotime;Chronostratigraphic"/>	<vs:term_status>unstable</vs:term_status>	</skos:Concept>
<skos:Concept rdf:about="&geotime;Paibian">	<skos:prefLabel xml:lang="en">Paibian</skos:prefLabel>	<skos:definition>The Paibian time period started 501  million years (Ma) before present (BP) and ended 496 Ma BP.</skos:definition>	<rdfs:seeAlso rdf:resource="http://kos.gbif.org/wiki/geotime:Paibian"/>	<geotime:rangeType>Stage</geotime:rangeType>	<geotime:rangeTypeURI rdf:resource="&geotime;Stage"/>	<geotime:start>501</geotime:start>	<geotime:end>496</geotime:end>		<dcterms:created>2011-01-11</dcterms:created>	<dcterms:modified>2012-08-03</dcterms:modified>	<dcterms:hasVersion rdf:resource="&history;20120803/geotime#Paibian"/>	<rdfs:isDefinedBy rdf:resource="&geotime;"/>	<skos:inScheme rdf:resource="&geotime;"/>	<vann:termGroup rdf:resource="&geotime;Stage"/>	<vann:termGroup rdf:resource="&geotime;Chronostratigraphic"/>	<vs:term_status>unstable</vs:term_status>	</skos:Concept>
<skos:Concept rdf:about="&geotime;Quaternary">	<skos:prefLabel xml:lang="en">Quaternary</skos:prefLabel>	<skos:definition>The Quaternary time period started 2.6  million years (Ma) before present (BP) and ended 0 Ma BP.</skos:definition>	<rdfs:seeAlso rdf:resource="http://kos.gbif.org/wiki/geotime:Quaternary"/>	<geotime:rangeType>Sub-Era</geotime:rangeType>	<geotime:rangeTypeURI rdf:resource="&geotime;Sub-Era"/>	<geotime:start>2.6</geotime:start>	<geotime:end>0</geotime:end>	<skos:narrower>Cenozoic</skos:narrower>	<dcterms:created>2011-01-11</dcterms:created>	<dcterms:modified>2012-08-03</dcterms:modified>	<dcterms:hasVersion rdf:resource="&history;20120803/geotime#Quaternary"/>	<rdfs:isDefinedBy rdf:resource="&geotime;"/>	<skos:inScheme rdf:resource="&geotime;"/>	<vann:termGroup rdf:resource="&geotime;Sub-Era"/>	<vann:termGroup rdf:resource="&geotime;Chronostratigraphic"/>	<vs:term_status>unstable</vs:term_status>	</skos:Concept>
<skos:Concept rdf:about="&geotime;Tertiary">	<skos:prefLabel xml:lang="en">Tertiary</skos:prefLabel>	<skos:definition>The Tertiary time period started 65.5  million years (Ma) before present (BP) and ended 2.6 Ma BP.</skos:definition>	<rdfs:seeAlso rdf:resource="http://kos.gbif.org/wiki/geotime:Tertiary"/>	<geotime:rangeType>Sub-Era</geotime:rangeType>	<geotime:rangeTypeURI rdf:resource="&geotime;Sub-Era"/>	<geotime:start>65.5</geotime:start>	<geotime:end>2.6</geotime:end>	<skos:narrower>Cenozoic</skos:narrower>	<dcterms:created>2011-01-11</dcterms:created>	<dcterms:modified>2012-08-03</dcterms:modified>	<dcterms:hasVersion rdf:resource="&history;20120803/geotime#Tertiary"/>	<rdfs:isDefinedBy rdf:resource="&geotime;"/>	<skos:inScheme rdf:resource="&geotime;"/>	<vann:termGroup rdf:resource="&geotime;Sub-Era"/>	<vann:termGroup rdf:resource="&geotime;Chronostratigraphic"/>	<vs:term_status>unstable</vs:term_status>	</skos:Concept>
<skos:Concept rdf:about="&geotime;Pennsylvanian">	<skos:prefLabel xml:lang="en">Pennsylvanian</skos:prefLabel>	<skos:definition>The Pennsylvanian time period started 318.1  million years (Ma) before present (BP) and ended 299 Ma BP.</skos:definition>	<rdfs:seeAlso rdf:resource="http://kos.gbif.org/wiki/geotime:Pennsylvanian"/>	<geotime:rangeType>Sub-Period</geotime:rangeType>	<geotime:rangeTypeURI rdf:resource="&geotime;Sub-Period"/>	<geotime:start>318.1</geotime:start>	<geotime:end>299</geotime:end>	<skos:narrower>Carboniferous</skos:narrower>	<dcterms:created>2011-01-11</dcterms:created>	<dcterms:modified>2012-08-03</dcterms:modified>	<dcterms:hasVersion rdf:resource="&history;20120803/geotime#Pennsylvanian"/>	<rdfs:isDefinedBy rdf:resource="&geotime;"/>	<skos:inScheme rdf:resource="&geotime;"/>	<vann:termGroup rdf:resource="&geotime;Sub-Period"/>	<vann:termGroup rdf:resource="&geotime;Chronostratigraphic"/>	<vs:term_status>unstable</vs:term_status>	</skos:Concept>
<skos:Concept rdf:about="&geotime;Mississippian">	<skos:prefLabel xml:lang="en">Mississippian</skos:prefLabel>	<skos:definition>The Mississippian time period started 359.2  million years (Ma) before present (BP) and ended 318.1 Ma BP.</skos:definition>	<rdfs:seeAlso rdf:resource="http://kos.gbif.org/wiki/geotime:Mississippian"/>	<geotime:rangeType>Sub-Period</geotime:rangeType>	<geotime:rangeTypeURI rdf:resource="&geotime;Sub-Period"/>	<geotime:start>359.2</geotime:start>	<geotime:end>318.1</geotime:end>	<skos:narrower>Carboniferous</skos:narrower>	<dcterms:created>2011-01-11</dcterms:created>	<dcterms:modified>2012-08-03</dcterms:modified>	<dcterms:hasVersion rdf:resource="&history;20120803/geotime#Mississippian"/>	<rdfs:isDefinedBy rdf:resource="&geotime;"/>	<skos:inScheme rdf:resource="&geotime;"/>	<vann:termGroup rdf:resource="&geotime;Sub-Period"/>	<vann:termGroup rdf:resource="&geotime;Chronostratigraphic"/>	<vs:term_status>unstable</vs:term_status>	</skos:Concept>
<skos:Concept rdf:about="&geotime;LateMaastrichtian">	<skos:prefLabel xml:lang="en">Late Maastrichtian</skos:prefLabel>	<skos:definition>The Late Maastrichtian time period started 69.23  million years (Ma) before present (BP) and ended 65.5 Ma BP.</skos:definition>	<rdfs:seeAlso rdf:resource="http://kos.gbif.org/wiki/geotime:LateMaastrichtian"/>	<geotime:rangeType>Substage</geotime:rangeType>	<geotime:rangeTypeURI rdf:resource="&geotime;Substage"/>	<geotime:start>69.23</geotime:start>	<geotime:end>65.5</geotime:end>		<dcterms:created>2011-01-11</dcterms:created>	<dcterms:modified>2012-08-03</dcterms:modified>	<dcterms:hasVersion rdf:resource="&history;20120803/geotime#LateMaastrichtian"/>	<rdfs:isDefinedBy rdf:resource="&geotime;"/>	<skos:inScheme rdf:resource="&geotime;"/>	<vann:termGroup rdf:resource="&geotime;Substage"/>	<vann:termGroup rdf:resource="&geotime;Chronostratigraphic"/>	<vs:term_status>unstable</vs:term_status>	</skos:Concept>
<skos:Concept rdf:about="&geotime;EarlyMaastrichtian">	<skos:prefLabel xml:lang="en">Early Maastrichtian</skos:prefLabel>	<skos:definition>The Early Maastrichtian time period started 70.6  million years (Ma) before present (BP) and ended 69.23 Ma BP.</skos:definition>	<rdfs:seeAlso rdf:resource="http://kos.gbif.org/wiki/geotime:EarlyMaastrichtian"/>	<geotime:rangeType>Substage</geotime:rangeType>	<geotime:rangeTypeURI rdf:resource="&geotime;Substage"/>	<geotime:start>70.6</geotime:start>	<geotime:end>69.23</geotime:end>		<dcterms:created>2011-01-11</dcterms:created>	<dcterms:modified>2012-08-03</dcterms:modified>	<dcterms:hasVersion rdf:resource="&history;20120803/geotime#EarlyMaastrichtian"/>	<rdfs:isDefinedBy rdf:resource="&geotime;"/>	<skos:inScheme rdf:resource="&geotime;"/>	<vann:termGroup rdf:resource="&geotime;Substage"/>	<vann:termGroup rdf:resource="&geotime;Chronostratigraphic"/>	<vs:term_status>unstable</vs:term_status>	</skos:Concept>
<skos:Concept rdf:about="&geotime;LateCampanian">	<skos:prefLabel xml:lang="en">Late Campanian</skos:prefLabel>	<skos:definition>The Late Campanian time period started 76.38  million years (Ma) before present (BP) and ended 70.6 Ma BP.</skos:definition>	<rdfs:seeAlso rdf:resource="http://kos.gbif.org/wiki/geotime:LateCampanian"/>	<geotime:rangeType>Substage</geotime:rangeType>	<geotime:rangeTypeURI rdf:resource="&geotime;Substage"/>	<geotime:start>76.38</geotime:start>	<geotime:end>70.6</geotime:end>		<dcterms:created>2011-01-11</dcterms:created>	<dcterms:modified>2012-08-03</dcterms:modified>	<dcterms:hasVersion rdf:resource="&history;20120803/geotime#LateCampanian"/>	<rdfs:isDefinedBy rdf:resource="&geotime;"/>	<skos:inScheme rdf:resource="&geotime;"/>	<vann:termGroup rdf:resource="&geotime;Substage"/>	<vann:termGroup rdf:resource="&geotime;Chronostratigraphic"/>	<vs:term_status>unstable</vs:term_status>	</skos:Concept>
<skos:Concept rdf:about="&geotime;MiddleCampanian">	<skos:prefLabel xml:lang="en">Middle Campanian</skos:prefLabel>	<skos:definition>The Middle Campanian time period started 80.64  million years (Ma) before present (BP) and ended 76.38 Ma BP.</skos:definition>	<rdfs:seeAlso rdf:resource="http://kos.gbif.org/wiki/geotime:MiddleCampanian"/>	<geotime:rangeType>Substage</geotime:rangeType>	<geotime:rangeTypeURI rdf:resource="&geotime;Substage"/>	<geotime:start>80.64</geotime:start>	<geotime:end>76.38</geotime:end>		<dcterms:created>2011-01-11</dcterms:created>	<dcterms:modified>2012-08-03</dcterms:modified>	<dcterms:hasVersion rdf:resource="&history;20120803/geotime#MiddleCampanian"/>	<rdfs:isDefinedBy rdf:resource="&geotime;"/>	<skos:inScheme rdf:resource="&geotime;"/>	<vann:termGroup rdf:resource="&geotime;Substage"/>	<vann:termGroup rdf:resource="&geotime;Chronostratigraphic"/>	<vs:term_status>unstable</vs:term_status>	</skos:Concept>
<skos:Concept rdf:about="&geotime;EarlyCampanian">	<skos:prefLabel xml:lang="en">Early Campanian</skos:prefLabel>	<skos:definition>The Early Campanian time period started 83.53  million years (Ma) before present (BP) and ended 80.64 Ma BP.</skos:definition>	<rdfs:seeAlso rdf:resource="http://kos.gbif.org/wiki/geotime:EarlyCampanian"/>	<geotime:rangeType>Substage</geotime:rangeType>	<geotime:rangeTypeURI rdf:resource="&geotime;Substage"/>	<geotime:start>83.53</geotime:start>	<geotime:end>80.64</geotime:end>		<dcterms:created>2011-01-11</dcterms:created>	<dcterms:modified>2012-08-03</dcterms:modified>	<dcterms:hasVersion rdf:resource="&history;20120803/geotime#EarlyCampanian"/>	<rdfs:isDefinedBy rdf:resource="&geotime;"/>	<skos:inScheme rdf:resource="&geotime;"/>	<vann:termGroup rdf:resource="&geotime;Substage"/>	<vann:termGroup rdf:resource="&geotime;Chronostratigraphic"/>	<vs:term_status>unstable</vs:term_status>	</skos:Concept>
<skos:Concept rdf:about="&geotime;LateSantonian">	<skos:prefLabel xml:lang="en">Late Santonian</skos:prefLabel>	<skos:definition>The Late Santonian time period started 83.99  million years (Ma) before present (BP) and ended 83.53 Ma BP.</skos:definition>	<rdfs:seeAlso rdf:resource="http://kos.gbif.org/wiki/geotime:LateSantonian"/>	<geotime:rangeType>Substage</geotime:rangeType>	<geotime:rangeTypeURI rdf:resource="&geotime;Substage"/>	<geotime:start>83.99</geotime:start>	<geotime:end>83.53</geotime:end>		<dcterms:created>2011-01-11</dcterms:created>	<dcterms:modified>2012-08-03</dcterms:modified>	<dcterms:hasVersion rdf:resource="&history;20120803/geotime#LateSantonian"/>	<rdfs:isDefinedBy rdf:resource="&geotime;"/>	<skos:inScheme rdf:resource="&geotime;"/>	<vann:termGroup rdf:resource="&geotime;Substage"/>	<vann:termGroup rdf:resource="&geotime;Chronostratigraphic"/>	<vs:term_status>unstable</vs:term_status>	</skos:Concept>
<skos:Concept rdf:about="&geotime;MiddleSantonian">	<skos:prefLabel xml:lang="en">Middle Santonian</skos:prefLabel>	<skos:definition>The Middle Santonian time period started 84.94  million years (Ma) before present (BP) and ended 83.99 Ma BP.</skos:definition>	<rdfs:seeAlso rdf:resource="http://kos.gbif.org/wiki/geotime:MiddleSantonian"/>	<geotime:rangeType>Substage</geotime:rangeType>	<geotime:rangeTypeURI rdf:resource="&geotime;Substage"/>	<geotime:start>84.94</geotime:start>	<geotime:end>83.99</geotime:end>		<dcterms:created>2011-01-11</dcterms:created>	<dcterms:modified>2012-08-03</dcterms:modified>	<dcterms:hasVersion rdf:resource="&history;20120803/geotime#MiddleSantonian"/>	<rdfs:isDefinedBy rdf:resource="&geotime;"/>	<skos:inScheme rdf:resource="&geotime;"/>	<vann:termGroup rdf:resource="&geotime;Substage"/>	<vann:termGroup rdf:resource="&geotime;Chronostratigraphic"/>	<vs:term_status>unstable</vs:term_status>	</skos:Concept>
<skos:Concept rdf:about="&geotime;EarlySantonian">	<skos:prefLabel xml:lang="en">Early Santonian</skos:prefLabel>	<skos:definition>The Early Santonian time period started 85.85  million years (Ma) before present (BP) and ended 84.94 Ma BP.</skos:definition>	<rdfs:seeAlso rdf:resource="http://kos.gbif.org/wiki/geotime:EarlySantonian"/>	<geotime:rangeType>Substage</geotime:rangeType>	<geotime:rangeTypeURI rdf:resource="&geotime;Substage"/>	<geotime:start>85.85</geotime:start>	<geotime:end>84.94</geotime:end>		<dcterms:created>2011-01-11</dcterms:created>	<dcterms:modified>2012-08-03</dcterms:modified>	<dcterms:hasVersion rdf:resource="&history;20120803/geotime#EarlySantonian"/>	<rdfs:isDefinedBy rdf:resource="&geotime;"/>	<skos:inScheme rdf:resource="&geotime;"/>	<vann:termGroup rdf:resource="&geotime;Substage"/>	<vann:termGroup rdf:resource="&geotime;Chronostratigraphic"/>	<vs:term_status>unstable</vs:term_status>	</skos:Concept>
<skos:Concept rdf:about="&geotime;LateConiacian">	<skos:prefLabel xml:lang="en">Late Coniacian</skos:prefLabel>	<skos:definition>The Late Coniacian time period started 86.96  million years (Ma) before present (BP) and ended 85.85 Ma BP.</skos:definition>	<rdfs:seeAlso rdf:resource="http://kos.gbif.org/wiki/geotime:LateConiacian"/>	<geotime:rangeType>Substage</geotime:rangeType>	<geotime:rangeTypeURI rdf:resource="&geotime;Substage"/>	<geotime:start>86.96</geotime:start>	<geotime:end>85.85</geotime:end>		<dcterms:created>2011-01-11</dcterms:created>	<dcterms:modified>2012-08-03</dcterms:modified>	<dcterms:hasVersion rdf:resource="&history;20120803/geotime#LateConiacian"/>	<rdfs:isDefinedBy rdf:resource="&geotime;"/>	<skos:inScheme rdf:resource="&geotime;"/>	<vann:termGroup rdf:resource="&geotime;Substage"/>	<vann:termGroup rdf:resource="&geotime;Chronostratigraphic"/>	<vs:term_status>unstable</vs:term_status>	</skos:Concept>
<skos:Concept rdf:about="&geotime;MiddleConiacian">	<skos:prefLabel xml:lang="en">Middle Coniacian</skos:prefLabel>	<skos:definition>The Middle Coniacian time period started 88.58  million years (Ma) before present (BP) and ended 86.96 Ma BP.</skos:definition>	<rdfs:seeAlso rdf:resource="http://kos.gbif.org/wiki/geotime:MiddleConiacian"/>	<geotime:rangeType>Substage</geotime:rangeType>	<geotime:rangeTypeURI rdf:resource="&geotime;Substage"/>	<geotime:start>88.58</geotime:start>	<geotime:end>86.96</geotime:end>		<dcterms:created>2011-01-11</dcterms:created>	<dcterms:modified>2012-08-03</dcterms:modified>	<dcterms:hasVersion rdf:resource="&history;20120803/geotime#MiddleConiacian"/>	<rdfs:isDefinedBy rdf:resource="&geotime;"/>	<skos:inScheme rdf:resource="&geotime;"/>	<vann:termGroup rdf:resource="&geotime;Substage"/>	<vann:termGroup rdf:resource="&geotime;Chronostratigraphic"/>	<vs:term_status>unstable</vs:term_status>	</skos:Concept>
<skos:Concept rdf:about="&geotime;EarlyConiacian">	<skos:prefLabel xml:lang="en">Early Coniacian</skos:prefLabel>	<skos:definition>The Early Coniacian time period started 89.27  million years (Ma) before present (BP) and ended 88.58 Ma BP.</skos:definition>	<rdfs:seeAlso rdf:resource="http://kos.gbif.org/wiki/geotime:EarlyConiacian"/>	<geotime:rangeType>Substage</geotime:rangeType>	<geotime:rangeTypeURI rdf:resource="&geotime;Substage"/>	<geotime:start>89.27</geotime:start>	<geotime:end>88.58</geotime:end>		<dcterms:created>2011-01-11</dcterms:created>	<dcterms:modified>2012-08-03</dcterms:modified>	<dcterms:hasVersion rdf:resource="&history;20120803/geotime#EarlyConiacian"/>	<rdfs:isDefinedBy rdf:resource="&geotime;"/>	<skos:inScheme rdf:resource="&geotime;"/>	<vann:termGroup rdf:resource="&geotime;Substage"/>	<vann:termGroup rdf:resource="&geotime;Chronostratigraphic"/>	<vs:term_status>unstable</vs:term_status>	</skos:Concept>
<skos:Concept rdf:about="&geotime;LateTuronian">	<skos:prefLabel xml:lang="en">Late Turonian</skos:prefLabel>	<skos:definition>The Late Turonian time period started 90.48  million years (Ma) before present (BP) and ended 89.27 Ma BP.</skos:definition>	<rdfs:seeAlso rdf:resource="http://kos.gbif.org/wiki/geotime:LateTuronian"/>	<geotime:rangeType>Substage</geotime:rangeType>	<geotime:rangeTypeURI rdf:resource="&geotime;Substage"/>	<geotime:start>90.48</geotime:start>	<geotime:end>89.27</geotime:end>		<dcterms:created>2011-01-11</dcterms:created>	<dcterms:modified>2012-08-03</dcterms:modified>	<dcterms:hasVersion rdf:resource="&history;20120803/geotime#LateTuronian"/>	<rdfs:isDefinedBy rdf:resource="&geotime;"/>	<skos:inScheme rdf:resource="&geotime;"/>	<vann:termGroup rdf:resource="&geotime;Substage"/>	<vann:termGroup rdf:resource="&geotime;Chronostratigraphic"/>	<vs:term_status>unstable</vs:term_status>	</skos:Concept>
<skos:Concept rdf:about="&geotime;MiddleTuronian">	<skos:prefLabel xml:lang="en">Middle Turonian</skos:prefLabel>	<skos:definition>The Middle Turonian time period started 92.13  million years (Ma) before present (BP) and ended 90.48 Ma BP.</skos:definition>	<rdfs:seeAlso rdf:resource="http://kos.gbif.org/wiki/geotime:MiddleTuronian"/>	<geotime:rangeType>Substage</geotime:rangeType>	<geotime:rangeTypeURI rdf:resource="&geotime;Substage"/>	<geotime:start>92.13</geotime:start>	<geotime:end>90.48</geotime:end>		<dcterms:created>2011-01-11</dcterms:created>	<dcterms:modified>2012-08-03</dcterms:modified>	<dcterms:hasVersion rdf:resource="&history;20120803/geotime#MiddleTuronian"/>	<rdfs:isDefinedBy rdf:resource="&geotime;"/>	<skos:inScheme rdf:resource="&geotime;"/>	<vann:termGroup rdf:resource="&geotime;Substage"/>	<vann:termGroup rdf:resource="&geotime;Chronostratigraphic"/>	<vs:term_status>unstable</vs:term_status>	</skos:Concept>
<skos:Concept rdf:about="&geotime;EarlyTuronian">	<skos:prefLabel xml:lang="en">Early Turonian</skos:prefLabel>	<skos:definition>The Early Turonian time period started 93.55  million years (Ma) before present (BP) and ended 92.13 Ma BP.</skos:definition>	<rdfs:seeAlso rdf:resource="http://kos.gbif.org/wiki/geotime:EarlyTuronian"/>	<geotime:rangeType>Substage</geotime:rangeType>	<geotime:rangeTypeURI rdf:resource="&geotime;Substage"/>	<geotime:start>93.55</geotime:start>	<geotime:end>92.13</geotime:end>		<dcterms:created>2011-01-11</dcterms:created>	<dcterms:modified>2012-08-03</dcterms:modified>	<dcterms:hasVersion rdf:resource="&history;20120803/geotime#EarlyTuronian"/>	<rdfs:isDefinedBy rdf:resource="&geotime;"/>	<skos:inScheme rdf:resource="&geotime;"/>	<vann:termGroup rdf:resource="&geotime;Substage"/>	<vann:termGroup rdf:resource="&geotime;Chronostratigraphic"/>	<vs:term_status>unstable</vs:term_status>	</skos:Concept>
<skos:Concept rdf:about="&geotime;LateCenomanian">	<skos:prefLabel xml:lang="en">Late Cenomanian</skos:prefLabel>	<skos:definition>The Late Cenomanian time period started 94.75  million years (Ma) before present (BP) and ended 93.55 Ma BP.</skos:definition>	<rdfs:seeAlso rdf:resource="http://kos.gbif.org/wiki/geotime:LateCenomanian"/>	<geotime:rangeType>Substage</geotime:rangeType>	<geotime:rangeTypeURI rdf:resource="&geotime;Substage"/>	<geotime:start>94.75</geotime:start>	<geotime:end>93.55</geotime:end>		<dcterms:created>2011-01-11</dcterms:created>	<dcterms:modified>2012-08-03</dcterms:modified>	<dcterms:hasVersion rdf:resource="&history;20120803/geotime#LateCenomanian"/>	<rdfs:isDefinedBy rdf:resource="&geotime;"/>	<skos:inScheme rdf:resource="&geotime;"/>	<vann:termGroup rdf:resource="&geotime;Substage"/>	<vann:termGroup rdf:resource="&geotime;Chronostratigraphic"/>	<vs:term_status>unstable</vs:term_status>	</skos:Concept>
<skos:Concept rdf:about="&geotime;MiddleCenomanian">	<skos:prefLabel xml:lang="en">Middle Cenomanian</skos:prefLabel>	<skos:definition>The Middle Cenomanian time period started 96.01  million years (Ma) before present (BP) and ended 94.75 Ma BP.</skos:definition>	<rdfs:seeAlso rdf:resource="http://kos.gbif.org/wiki/geotime:MiddleCenomanian"/>	<geotime:rangeType>Substage</geotime:rangeType>	<geotime:rangeTypeURI rdf:resource="&geotime;Substage"/>	<geotime:start>96.01</geotime:start>	<geotime:end>94.75</geotime:end>		<dcterms:created>2011-01-11</dcterms:created>	<dcterms:modified>2012-08-03</dcterms:modified>	<dcterms:hasVersion rdf:resource="&history;20120803/geotime#MiddleCenomanian"/>	<rdfs:isDefinedBy rdf:resource="&geotime;"/>	<skos:inScheme rdf:resource="&geotime;"/>	<vann:termGroup rdf:resource="&geotime;Substage"/>	<vann:termGroup rdf:resource="&geotime;Chronostratigraphic"/>	<vs:term_status>unstable</vs:term_status>	</skos:Concept>
<skos:Concept rdf:about="&geotime;EarlyCenomanian">	<skos:prefLabel xml:lang="en">Early Cenomanian</skos:prefLabel>	<skos:definition>The Early Cenomanian time period started 99.6  million years (Ma) before present (BP) and ended 96.01 Ma BP.</skos:definition>	<rdfs:seeAlso rdf:resource="http://kos.gbif.org/wiki/geotime:EarlyCenomanian"/>	<geotime:rangeType>Substage</geotime:rangeType>	<geotime:rangeTypeURI rdf:resource="&geotime;Substage"/>	<geotime:start>99.6</geotime:start>	<geotime:end>96.01</geotime:end>		<dcterms:created>2011-01-11</dcterms:created>	<dcterms:modified>2012-08-03</dcterms:modified>	<dcterms:hasVersion rdf:resource="&history;20120803/geotime#EarlyCenomanian"/>	<rdfs:isDefinedBy rdf:resource="&geotime;"/>	<skos:inScheme rdf:resource="&geotime;"/>	<vann:termGroup rdf:resource="&geotime;Substage"/>	<vann:termGroup rdf:resource="&geotime;Chronostratigraphic"/>	<vs:term_status>unstable</vs:term_status>	</skos:Concept>
<skos:Concept rdf:about="&geotime;LateAlbian">	<skos:prefLabel xml:lang="en">Late Albian</skos:prefLabel>	<skos:definition>The Late Albian time period started 106.42  million years (Ma) before present (BP) and ended 99.6 Ma BP.</skos:definition>	<rdfs:seeAlso rdf:resource="http://kos.gbif.org/wiki/geotime:LateAlbian"/>	<geotime:rangeType>Substage</geotime:rangeType>	<geotime:rangeTypeURI rdf:resource="&geotime;Substage"/>	<geotime:start>106.42</geotime:start>	<geotime:end>99.6</geotime:end>		<dcterms:created>2011-01-11</dcterms:created>	<dcterms:modified>2012-08-03</dcterms:modified>	<dcterms:hasVersion rdf:resource="&history;20120803/geotime#LateAlbian"/>	<rdfs:isDefinedBy rdf:resource="&geotime;"/>	<skos:inScheme rdf:resource="&geotime;"/>	<vann:termGroup rdf:resource="&geotime;Substage"/>	<vann:termGroup rdf:resource="&geotime;Chronostratigraphic"/>	<vs:term_status>unstable</vs:term_status>	</skos:Concept>
<skos:Concept rdf:about="&geotime;MiddleAlbian">	<skos:prefLabel xml:lang="en">Middle Albian</skos:prefLabel>	<skos:definition>The Middle Albian time period started 108.77  million years (Ma) before present (BP) and ended 106.42 Ma BP.</skos:definition>	<rdfs:seeAlso rdf:resource="http://kos.gbif.org/wiki/geotime:MiddleAlbian"/>	<geotime:rangeType>Substage</geotime:rangeType>	<geotime:rangeTypeURI rdf:resource="&geotime;Substage"/>	<geotime:start>108.77</geotime:start>	<geotime:end>106.42</geotime:end>		<dcterms:created>2011-01-11</dcterms:created>	<dcterms:modified>2012-08-03</dcterms:modified>	<dcterms:hasVersion rdf:resource="&history;20120803/geotime#MiddleAlbian"/>	<rdfs:isDefinedBy rdf:resource="&geotime;"/>	<skos:inScheme rdf:resource="&geotime;"/>	<vann:termGroup rdf:resource="&geotime;Substage"/>	<vann:termGroup rdf:resource="&geotime;Chronostratigraphic"/>	<vs:term_status>unstable</vs:term_status>	</skos:Concept>
<skos:Concept rdf:about="&geotime;EarlyAlbian">	<skos:prefLabel xml:lang="en">Early Albian</skos:prefLabel>	<skos:definition>The Early Albian time period started 112  million years (Ma) before present (BP) and ended 108.77 Ma BP.</skos:definition>	<rdfs:seeAlso rdf:resource="http://kos.gbif.org/wiki/geotime:EarlyAlbian"/>	<geotime:rangeType>Substage</geotime:rangeType>	<geotime:rangeTypeURI rdf:resource="&geotime;Substage"/>	<geotime:start>112</geotime:start>	<geotime:end>108.77</geotime:end>		<dcterms:created>2011-01-11</dcterms:created>	<dcterms:modified>2012-08-03</dcterms:modified>	<dcterms:hasVersion rdf:resource="&history;20120803/geotime#EarlyAlbian"/>	<rdfs:isDefinedBy rdf:resource="&geotime;"/>	<skos:inScheme rdf:resource="&geotime;"/>	<vann:termGroup rdf:resource="&geotime;Substage"/>	<vann:termGroup rdf:resource="&geotime;Chronostratigraphic"/>	<vs:term_status>unstable</vs:term_status>	</skos:Concept>
<skos:Concept rdf:about="&geotime;LateAptian">	<skos:prefLabel xml:lang="en">Late Aptian</skos:prefLabel>	<skos:definition>The Late Aptian time period started 115  million years (Ma) before present (BP) and ended 112 Ma BP.</skos:definition>	<rdfs:seeAlso rdf:resource="http://kos.gbif.org/wiki/geotime:LateAptian"/>	<geotime:rangeType>Substage</geotime:rangeType>	<geotime:rangeTypeURI rdf:resource="&geotime;Substage"/>	<geotime:start>115</geotime:start>	<geotime:end>112</geotime:end>		<dcterms:created>2011-01-11</dcterms:created>	<dcterms:modified>2012-08-03</dcterms:modified>	<dcterms:hasVersion rdf:resource="&history;20120803/geotime#LateAptian"/>	<rdfs:isDefinedBy rdf:resource="&geotime;"/>	<skos:inScheme rdf:resource="&geotime;"/>	<vann:termGroup rdf:resource="&geotime;Substage"/>	<vann:termGroup rdf:resource="&geotime;Chronostratigraphic"/>	<vs:term_status>unstable</vs:term_status>	</skos:Concept>
<skos:Concept rdf:about="&geotime;EarlyAptian">	<skos:prefLabel xml:lang="en">Early Aptian</skos:prefLabel>	<skos:definition>The Early Aptian time period started 125  million years (Ma) before present (BP) and ended 121 Ma BP.</skos:definition>	<rdfs:seeAlso rdf:resource="http://kos.gbif.org/wiki/geotime:EarlyAptian"/>	<geotime:rangeType>Substage</geotime:rangeType>	<geotime:rangeTypeURI rdf:resource="&geotime;Substage"/>	<geotime:start>125</geotime:start>	<geotime:end>121</geotime:end>		<dcterms:created>2011-01-11</dcterms:created>	<dcterms:modified>2012-08-03</dcterms:modified>	<dcterms:hasVersion rdf:resource="&history;20120803/geotime#EarlyAptian"/>	<rdfs:isDefinedBy rdf:resource="&geotime;"/>	<skos:inScheme rdf:resource="&geotime;"/>	<vann:termGroup rdf:resource="&geotime;Substage"/>	<vann:termGroup rdf:resource="&geotime;Chronostratigraphic"/>	<vs:term_status>unstable</vs:term_status>	</skos:Concept>
<skos:Concept rdf:about="&geotime;LateBarremian">	<skos:prefLabel xml:lang="en">Late Barremian</skos:prefLabel>	<skos:definition>The Late Barremian time period started 128.3  million years (Ma) before present (BP) and ended 125 Ma BP.</skos:definition>	<rdfs:seeAlso rdf:resource="http://kos.gbif.org/wiki/geotime:LateBarremian"/>	<geotime:rangeType>Substage</geotime:rangeType>	<geotime:rangeTypeURI rdf:resource="&geotime;Substage"/>	<geotime:start>128.3</geotime:start>	<geotime:end>125</geotime:end>		<dcterms:created>2011-01-11</dcterms:created>	<dcterms:modified>2012-08-03</dcterms:modified>	<dcterms:hasVersion rdf:resource="&history;20120803/geotime#LateBarremian"/>	<rdfs:isDefinedBy rdf:resource="&geotime;"/>	<skos:inScheme rdf:resource="&geotime;"/>	<vann:termGroup rdf:resource="&geotime;Substage"/>	<vann:termGroup rdf:resource="&geotime;Chronostratigraphic"/>	<vs:term_status>unstable</vs:term_status>	</skos:Concept>
<skos:Concept rdf:about="&geotime;EarlyBarremian">	<skos:prefLabel xml:lang="en">Early Barremian</skos:prefLabel>	<skos:definition>The Early Barremian time period started 129.97  million years (Ma) before present (BP) and ended 128.3 Ma BP.</skos:definition>	<rdfs:seeAlso rdf:resource="http://kos.gbif.org/wiki/geotime:EarlyBarremian"/>	<geotime:rangeType>Substage</geotime:rangeType>	<geotime:rangeTypeURI rdf:resource="&geotime;Substage"/>	<geotime:start>129.97</geotime:start>	<geotime:end>128.3</geotime:end>		<dcterms:created>2011-01-11</dcterms:created>	<dcterms:modified>2012-08-03</dcterms:modified>	<dcterms:hasVersion rdf:resource="&history;20120803/geotime#EarlyBarremian"/>	<rdfs:isDefinedBy rdf:resource="&geotime;"/>	<skos:inScheme rdf:resource="&geotime;"/>	<vann:termGroup rdf:resource="&geotime;Substage"/>	<vann:termGroup rdf:resource="&geotime;Chronostratigraphic"/>	<vs:term_status>unstable</vs:term_status>	</skos:Concept>
<skos:Concept rdf:about="&geotime;LateHauterivian">	<skos:prefLabel xml:lang="en">Late Hauterivian</skos:prefLabel>	<skos:definition>The Late Hauterivian time period started 133.85  million years (Ma) before present (BP) and ended 129.97 Ma BP.</skos:definition>	<rdfs:seeAlso rdf:resource="http://kos.gbif.org/wiki/geotime:LateHauterivian"/>	<geotime:rangeType>Substage</geotime:rangeType>	<geotime:rangeTypeURI rdf:resource="&geotime;Substage"/>	<geotime:start>133.85</geotime:start>	<geotime:end>129.97</geotime:end>		<dcterms:created>2011-01-11</dcterms:created>	<dcterms:modified>2012-08-03</dcterms:modified>	<dcterms:hasVersion rdf:resource="&history;20120803/geotime#LateHauterivian"/>	<rdfs:isDefinedBy rdf:resource="&geotime;"/>	<skos:inScheme rdf:resource="&geotime;"/>	<vann:termGroup rdf:resource="&geotime;Substage"/>	<vann:termGroup rdf:resource="&geotime;Chronostratigraphic"/>	<vs:term_status>unstable</vs:term_status>	</skos:Concept>
<skos:Concept rdf:about="&geotime;EarlyHauterivian">	<skos:prefLabel xml:lang="en">Early Hauterivian</skos:prefLabel>	<skos:definition>The Early Hauterivian time period started 136.44  million years (Ma) before present (BP) and ended 133.85 Ma BP.</skos:definition>	<rdfs:seeAlso rdf:resource="http://kos.gbif.org/wiki/geotime:EarlyHauterivian"/>	<geotime:rangeType>Substage</geotime:rangeType>	<geotime:rangeTypeURI rdf:resource="&geotime;Substage"/>	<geotime:start>136.44</geotime:start>	<geotime:end>133.85</geotime:end>		<dcterms:created>2011-01-11</dcterms:created>	<dcterms:modified>2012-08-03</dcterms:modified>	<dcterms:hasVersion rdf:resource="&history;20120803/geotime#EarlyHauterivian"/>	<rdfs:isDefinedBy rdf:resource="&geotime;"/>	<skos:inScheme rdf:resource="&geotime;"/>	<vann:termGroup rdf:resource="&geotime;Substage"/>	<vann:termGroup rdf:resource="&geotime;Chronostratigraphic"/>	<vs:term_status>unstable</vs:term_status>	</skos:Concept>
<skos:Concept rdf:about="&geotime;LateValanginian">	<skos:prefLabel xml:lang="en">Late Valanginian</skos:prefLabel>	<skos:definition>The Late Valanginian time period started 138.94  million years (Ma) before present (BP) and ended 136.44 Ma BP.</skos:definition>	<rdfs:seeAlso rdf:resource="http://kos.gbif.org/wiki/geotime:LateValanginian"/>	<geotime:rangeType>Substage</geotime:rangeType>	<geotime:rangeTypeURI rdf:resource="&geotime;Substage"/>	<geotime:start>138.94</geotime:start>	<geotime:end>136.44</geotime:end>		<dcterms:created>2011-01-11</dcterms:created>	<dcterms:modified>2012-08-03</dcterms:modified>	<dcterms:hasVersion rdf:resource="&history;20120803/geotime#LateValanginian"/>	<rdfs:isDefinedBy rdf:resource="&geotime;"/>	<skos:inScheme rdf:resource="&geotime;"/>	<vann:termGroup rdf:resource="&geotime;Substage"/>	<vann:termGroup rdf:resource="&geotime;Chronostratigraphic"/>	<vs:term_status>unstable</vs:term_status>	</skos:Concept>
<skos:Concept rdf:about="&geotime;EarlyValanginian">	<skos:prefLabel xml:lang="en">Early Valanginian</skos:prefLabel>	<skos:definition>The Early Valanginian time period started 140.18  million years (Ma) before present (BP) and ended 138.94 Ma BP.</skos:definition>	<rdfs:seeAlso rdf:resource="http://kos.gbif.org/wiki/geotime:EarlyValanginian"/>	<geotime:rangeType>Substage</geotime:rangeType>	<geotime:rangeTypeURI rdf:resource="&geotime;Substage"/>	<geotime:start>140.18</geotime:start>	<geotime:end>138.94</geotime:end>		<dcterms:created>2011-01-11</dcterms:created>	<dcterms:modified>2012-08-03</dcterms:modified>	<dcterms:hasVersion rdf:resource="&history;20120803/geotime#EarlyValanginian"/>	<rdfs:isDefinedBy rdf:resource="&geotime;"/>	<skos:inScheme rdf:resource="&geotime;"/>	<vann:termGroup rdf:resource="&geotime;Substage"/>	<vann:termGroup rdf:resource="&geotime;Chronostratigraphic"/>	<vs:term_status>unstable</vs:term_status>	</skos:Concept>
<skos:Concept rdf:about="&geotime;LateBerriasian">	<skos:prefLabel xml:lang="en">Late Berriasian</skos:prefLabel>	<skos:definition>The Late Berriasian time period started 142.3  million years (Ma) before present (BP) and ended 140.18 Ma BP.</skos:definition>	<rdfs:seeAlso rdf:resource="http://kos.gbif.org/wiki/geotime:LateBerriasian"/>	<geotime:rangeType>Substage</geotime:rangeType>	<geotime:rangeTypeURI rdf:resource="&geotime;Substage"/>	<geotime:start>142.3</geotime:start>	<geotime:end>140.18</geotime:end>		<dcterms:created>2011-01-11</dcterms:created>	<dcterms:modified>2012-08-03</dcterms:modified>	<dcterms:hasVersion rdf:resource="&history;20120803/geotime#LateBerriasian"/>	<rdfs:isDefinedBy rdf:resource="&geotime;"/>	<skos:inScheme rdf:resource="&geotime;"/>	<vann:termGroup rdf:resource="&geotime;Substage"/>	<vann:termGroup rdf:resource="&geotime;Chronostratigraphic"/>	<vs:term_status>unstable</vs:term_status>	</skos:Concept>
<skos:Concept rdf:about="&geotime;EarlyBerriasian">	<skos:prefLabel xml:lang="en">Early Berriasian</skos:prefLabel>	<skos:definition>The Early Berriasian time period started 145.46  million years (Ma) before present (BP) and ended 142.3 Ma BP.</skos:definition>	<rdfs:seeAlso rdf:resource="http://kos.gbif.org/wiki/geotime:EarlyBerriasian"/>	<geotime:rangeType>Substage</geotime:rangeType>	<geotime:rangeTypeURI rdf:resource="&geotime;Substage"/>	<geotime:start>145.46</geotime:start>	<geotime:end>142.3</geotime:end>		<dcterms:created>2011-01-11</dcterms:created>	<dcterms:modified>2012-08-03</dcterms:modified>	<dcterms:hasVersion rdf:resource="&history;20120803/geotime#EarlyBerriasian"/>	<rdfs:isDefinedBy rdf:resource="&geotime;"/>	<skos:inScheme rdf:resource="&geotime;"/>	<vann:termGroup rdf:resource="&geotime;Substage"/>	<vann:termGroup rdf:resource="&geotime;Chronostratigraphic"/>	<vs:term_status>unstable</vs:term_status>	</skos:Concept>
<skos:Concept rdf:about="&geotime;LateTithonian">	<skos:prefLabel xml:lang="en">Late Tithonian</skos:prefLabel>	<skos:definition>The Late Tithonian time period started 147.16  million years (Ma) before present (BP) and ended 145.46 Ma BP.</skos:definition>	<rdfs:seeAlso rdf:resource="http://kos.gbif.org/wiki/geotime:LateTithonian"/>	<geotime:rangeType>Substage</geotime:rangeType>	<geotime:rangeTypeURI rdf:resource="&geotime;Substage"/>	<geotime:start>147.16</geotime:start>	<geotime:end>145.46</geotime:end>		<dcterms:created>2011-01-11</dcterms:created>	<dcterms:modified>2012-08-03</dcterms:modified>	<dcterms:hasVersion rdf:resource="&history;20120803/geotime#LateTithonian"/>	<rdfs:isDefinedBy rdf:resource="&geotime;"/>	<skos:inScheme rdf:resource="&geotime;"/>	<vann:termGroup rdf:resource="&geotime;Substage"/>	<vann:termGroup rdf:resource="&geotime;Chronostratigraphic"/>	<vs:term_status>unstable</vs:term_status>	</skos:Concept>
<skos:Concept rdf:about="&geotime;EarlyTithonian">	<skos:prefLabel xml:lang="en">Early Tithonian</skos:prefLabel>	<skos:definition>The Early Tithonian time period started 150.844  million years (Ma) before present (BP) and ended 147.16 Ma BP.</skos:definition>	<rdfs:seeAlso rdf:resource="http://kos.gbif.org/wiki/geotime:EarlyTithonian"/>	<geotime:rangeType>Substage</geotime:rangeType>	<geotime:rangeTypeURI rdf:resource="&geotime;Substage"/>	<geotime:start>150.844</geotime:start>	<geotime:end>147.16</geotime:end>		<dcterms:created>2011-01-11</dcterms:created>	<dcterms:modified>2012-08-03</dcterms:modified>	<dcterms:hasVersion rdf:resource="&history;20120803/geotime#EarlyTithonian"/>	<rdfs:isDefinedBy rdf:resource="&geotime;"/>	<skos:inScheme rdf:resource="&geotime;"/>	<vann:termGroup rdf:resource="&geotime;Substage"/>	<vann:termGroup rdf:resource="&geotime;Chronostratigraphic"/>	<vs:term_status>unstable</vs:term_status>	</skos:Concept>
<skos:Concept rdf:about="&geotime;LateKimmeridgian">	<skos:prefLabel xml:lang="en">Late Kimmeridgian</skos:prefLabel>	<skos:definition>The Late Kimmeridgian time period started 153.06  million years (Ma) before present (BP) and ended 150.844 Ma BP.</skos:definition>	<rdfs:seeAlso rdf:resource="http://kos.gbif.org/wiki/geotime:LateKimmeridgian"/>	<geotime:rangeType>Substage</geotime:rangeType>	<geotime:rangeTypeURI rdf:resource="&geotime;Substage"/>	<geotime:start>153.06</geotime:start>	<geotime:end>150.844</geotime:end>		<dcterms:created>2011-01-11</dcterms:created>	<dcterms:modified>2012-08-03</dcterms:modified>	<dcterms:hasVersion rdf:resource="&history;20120803/geotime#LateKimmeridgian"/>	<rdfs:isDefinedBy rdf:resource="&geotime;"/>	<skos:inScheme rdf:resource="&geotime;"/>	<vann:termGroup rdf:resource="&geotime;Substage"/>	<vann:termGroup rdf:resource="&geotime;Chronostratigraphic"/>	<vs:term_status>unstable</vs:term_status>	</skos:Concept>
<skos:Concept rdf:about="&geotime;EarlyKimmeridgian">	<skos:prefLabel xml:lang="en">Early Kimmeridgian</skos:prefLabel>	<skos:definition>The Early Kimmeridgian time period started 155.646  million years (Ma) before present (BP) and ended 153.06 Ma BP.</skos:definition>	<rdfs:seeAlso rdf:resource="http://kos.gbif.org/wiki/geotime:EarlyKimmeridgian"/>	<geotime:rangeType>Substage</geotime:rangeType>	<geotime:rangeTypeURI rdf:resource="&geotime;Substage"/>	<geotime:start>155.646</geotime:start>	<geotime:end>153.06</geotime:end>		<dcterms:created>2011-01-11</dcterms:created>	<dcterms:modified>2012-08-03</dcterms:modified>	<dcterms:hasVersion rdf:resource="&history;20120803/geotime#EarlyKimmeridgian"/>	<rdfs:isDefinedBy rdf:resource="&geotime;"/>	<skos:inScheme rdf:resource="&geotime;"/>	<vann:termGroup rdf:resource="&geotime;Substage"/>	<vann:termGroup rdf:resource="&geotime;Chronostratigraphic"/>	<vs:term_status>unstable</vs:term_status>	</skos:Concept>
<skos:Concept rdf:about="&geotime;MiddleAptian">	<skos:prefLabel xml:lang="en">Middle Aptian</skos:prefLabel>	<skos:definition>The Middle Aptian time period started 121  million years (Ma) before present (BP) and ended 155 Ma BP.</skos:definition>	<rdfs:seeAlso rdf:resource="http://kos.gbif.org/wiki/geotime:MiddleAptian"/>	<geotime:rangeType>Substage</geotime:rangeType>	<geotime:rangeTypeURI rdf:resource="&geotime;Substage"/>	<geotime:start>121</geotime:start>	<geotime:end>155</geotime:end>		<dcterms:created>2011-01-11</dcterms:created>	<dcterms:modified>2012-08-03</dcterms:modified>	<dcterms:hasVersion rdf:resource="&history;20120803/geotime#MiddleAptian"/>	<rdfs:isDefinedBy rdf:resource="&geotime;"/>	<skos:inScheme rdf:resource="&geotime;"/>	<vann:termGroup rdf:resource="&geotime;Substage"/>	<vann:termGroup rdf:resource="&geotime;Chronostratigraphic"/>	<vs:term_status>unstable</vs:term_status>	</skos:Concept>
<skos:Concept rdf:about="&geotime;LateOxfordian">	<skos:prefLabel xml:lang="en">Late Oxfordian</skos:prefLabel>	<skos:definition>The Late Oxfordian time period started 157.4  million years (Ma) before present (BP) and ended 155.646 Ma BP.</skos:definition>	<rdfs:seeAlso rdf:resource="http://kos.gbif.org/wiki/geotime:LateOxfordian"/>	<geotime:rangeType>Substage</geotime:rangeType>	<geotime:rangeTypeURI rdf:resource="&geotime;Substage"/>	<geotime:start>157.4</geotime:start>	<geotime:end>155.646</geotime:end>		<dcterms:created>2011-01-11</dcterms:created>	<dcterms:modified>2012-08-03</dcterms:modified>	<dcterms:hasVersion rdf:resource="&history;20120803/geotime#LateOxfordian"/>	<rdfs:isDefinedBy rdf:resource="&geotime;"/>	<skos:inScheme rdf:resource="&geotime;"/>	<vann:termGroup rdf:resource="&geotime;Substage"/>	<vann:termGroup rdf:resource="&geotime;Chronostratigraphic"/>	<vs:term_status>unstable</vs:term_status>	</skos:Concept>
<skos:Concept rdf:about="&geotime;MiddleOxfordian">	<skos:prefLabel xml:lang="en">Middle Oxfordian</skos:prefLabel>	<skos:definition>The Middle Oxfordian time period started 159.61  million years (Ma) before present (BP) and ended 157.4 Ma BP.</skos:definition>	<rdfs:seeAlso rdf:resource="http://kos.gbif.org/wiki/geotime:MiddleOxfordian"/>	<geotime:rangeType>Substage</geotime:rangeType>	<geotime:rangeTypeURI rdf:resource="&geotime;Substage"/>	<geotime:start>159.61</geotime:start>	<geotime:end>157.4</geotime:end>		<dcterms:created>2011-01-11</dcterms:created>	<dcterms:modified>2012-08-03</dcterms:modified>	<dcterms:hasVersion rdf:resource="&history;20120803/geotime#MiddleOxfordian"/>	<rdfs:isDefinedBy rdf:resource="&geotime;"/>	<skos:inScheme rdf:resource="&geotime;"/>	<vann:termGroup rdf:resource="&geotime;Substage"/>	<vann:termGroup rdf:resource="&geotime;Chronostratigraphic"/>	<vs:term_status>unstable</vs:term_status>	</skos:Concept>
<skos:Concept rdf:about="&geotime;EarlyOxfordian">	<skos:prefLabel xml:lang="en">Early Oxfordian</skos:prefLabel>	<skos:definition>The Early Oxfordian time period started 161.21  million years (Ma) before present (BP) and ended 159.61 Ma BP.</skos:definition>	<rdfs:seeAlso rdf:resource="http://kos.gbif.org/wiki/geotime:EarlyOxfordian"/>	<geotime:rangeType>Substage</geotime:rangeType>	<geotime:rangeTypeURI rdf:resource="&geotime;Substage"/>	<geotime:start>161.21</geotime:start>	<geotime:end>159.61</geotime:end>		<dcterms:created>2011-01-11</dcterms:created>	<dcterms:modified>2012-08-03</dcterms:modified>	<dcterms:hasVersion rdf:resource="&history;20120803/geotime#EarlyOxfordian"/>	<rdfs:isDefinedBy rdf:resource="&geotime;"/>	<skos:inScheme rdf:resource="&geotime;"/>	<vann:termGroup rdf:resource="&geotime;Substage"/>	<vann:termGroup rdf:resource="&geotime;Chronostratigraphic"/>	<vs:term_status>unstable</vs:term_status>	</skos:Concept>
<skos:Concept rdf:about="&geotime;LateCallovian">	<skos:prefLabel xml:lang="en">Late Callovian</skos:prefLabel>	<skos:definition>The Late Callovian time period started 162.52  million years (Ma) before present (BP) and ended 161.21 Ma BP.</skos:definition>	<rdfs:seeAlso rdf:resource="http://kos.gbif.org/wiki/geotime:LateCallovian"/>	<geotime:rangeType>Substage</geotime:rangeType>	<geotime:rangeTypeURI rdf:resource="&geotime;Substage"/>	<geotime:start>162.52</geotime:start>	<geotime:end>161.21</geotime:end>		<dcterms:created>2011-01-11</dcterms:created>	<dcterms:modified>2012-08-03</dcterms:modified>	<dcterms:hasVersion rdf:resource="&history;20120803/geotime#LateCallovian"/>	<rdfs:isDefinedBy rdf:resource="&geotime;"/>	<skos:inScheme rdf:resource="&geotime;"/>	<vann:termGroup rdf:resource="&geotime;Substage"/>	<vann:termGroup rdf:resource="&geotime;Chronostratigraphic"/>	<vs:term_status>unstable</vs:term_status>	</skos:Concept>
<skos:Concept rdf:about="&geotime;MiddleCallovian">	<skos:prefLabel xml:lang="en">Middle Callovian</skos:prefLabel>	<skos:definition>The Middle Callovian time period started 163.2  million years (Ma) before present (BP) and ended 162.52 Ma BP.</skos:definition>	<rdfs:seeAlso rdf:resource="http://kos.gbif.org/wiki/geotime:MiddleCallovian"/>	<geotime:rangeType>Substage</geotime:rangeType>	<geotime:rangeTypeURI rdf:resource="&geotime;Substage"/>	<geotime:start>163.2</geotime:start>	<geotime:end>162.52</geotime:end>		<dcterms:created>2011-01-11</dcterms:created>	<dcterms:modified>2012-08-03</dcterms:modified>	<dcterms:hasVersion rdf:resource="&history;20120803/geotime#MiddleCallovian"/>	<rdfs:isDefinedBy rdf:resource="&geotime;"/>	<skos:inScheme rdf:resource="&geotime;"/>	<vann:termGroup rdf:resource="&geotime;Substage"/>	<vann:termGroup rdf:resource="&geotime;Chronostratigraphic"/>	<vs:term_status>unstable</vs:term_status>	</skos:Concept>
<skos:Concept rdf:about="&geotime;EarlyCallovian">	<skos:prefLabel xml:lang="en">Early Callovian</skos:prefLabel>	<skos:definition>The Early Callovian time period started 164.74  million years (Ma) before present (BP) and ended 163.2 Ma BP.</skos:definition>	<rdfs:seeAlso rdf:resource="http://kos.gbif.org/wiki/geotime:EarlyCallovian"/>	<geotime:rangeType>Substage</geotime:rangeType>	<geotime:rangeTypeURI rdf:resource="&geotime;Substage"/>	<geotime:start>164.74</geotime:start>	<geotime:end>163.2</geotime:end>		<dcterms:created>2011-01-11</dcterms:created>	<dcterms:modified>2012-08-03</dcterms:modified>	<dcterms:hasVersion rdf:resource="&history;20120803/geotime#EarlyCallovian"/>	<rdfs:isDefinedBy rdf:resource="&geotime;"/>	<skos:inScheme rdf:resource="&geotime;"/>	<vann:termGroup rdf:resource="&geotime;Substage"/>	<vann:termGroup rdf:resource="&geotime;Chronostratigraphic"/>	<vs:term_status>unstable</vs:term_status>	</skos:Concept>
<skos:Concept rdf:about="&geotime;LateBathonian">	<skos:prefLabel xml:lang="en">Late Bathonian</skos:prefLabel>	<skos:definition>The Late Bathonian time period started 165.72  million years (Ma) before present (BP) and ended 164.74 Ma BP.</skos:definition>	<rdfs:seeAlso rdf:resource="http://kos.gbif.org/wiki/geotime:LateBathonian"/>	<geotime:rangeType>Substage</geotime:rangeType>	<geotime:rangeTypeURI rdf:resource="&geotime;Substage"/>	<geotime:start>165.72</geotime:start>	<geotime:end>164.74</geotime:end>		<dcterms:created>2011-01-11</dcterms:created>	<dcterms:modified>2012-08-03</dcterms:modified>	<dcterms:hasVersion rdf:resource="&history;20120803/geotime#LateBathonian"/>	<rdfs:isDefinedBy rdf:resource="&geotime;"/>	<skos:inScheme rdf:resource="&geotime;"/>	<vann:termGroup rdf:resource="&geotime;Substage"/>	<vann:termGroup rdf:resource="&geotime;Chronostratigraphic"/>	<vs:term_status>unstable</vs:term_status>	</skos:Concept>
<skos:Concept rdf:about="&geotime;MiddleBathonian">	<skos:prefLabel xml:lang="en">Middle Bathonian</skos:prefLabel>	<skos:definition>The Middle Bathonian time period started 166.89  million years (Ma) before present (BP) and ended 165.72 Ma BP.</skos:definition>	<rdfs:seeAlso rdf:resource="http://kos.gbif.org/wiki/geotime:MiddleBathonian"/>	<geotime:rangeType>Substage</geotime:rangeType>	<geotime:rangeTypeURI rdf:resource="&geotime;Substage"/>	<geotime:start>166.89</geotime:start>	<geotime:end>165.72</geotime:end>		<dcterms:created>2011-01-11</dcterms:created>	<dcterms:modified>2012-08-03</dcterms:modified>	<dcterms:hasVersion rdf:resource="&history;20120803/geotime#MiddleBathonian"/>	<rdfs:isDefinedBy rdf:resource="&geotime;"/>	<skos:inScheme rdf:resource="&geotime;"/>	<vann:termGroup rdf:resource="&geotime;Substage"/>	<vann:termGroup rdf:resource="&geotime;Chronostratigraphic"/>	<vs:term_status>unstable</vs:term_status>	</skos:Concept>
<skos:Concept rdf:about="&geotime;EarlyBathonian">	<skos:prefLabel xml:lang="en">Early Bathonian</skos:prefLabel>	<skos:definition>The Early Bathonian time period started 167.68  million years (Ma) before present (BP) and ended 166.89 Ma BP.</skos:definition>	<rdfs:seeAlso rdf:resource="http://kos.gbif.org/wiki/geotime:EarlyBathonian"/>	<geotime:rangeType>Substage</geotime:rangeType>	<geotime:rangeTypeURI rdf:resource="&geotime;Substage"/>	<geotime:start>167.68</geotime:start>	<geotime:end>166.89</geotime:end>		<dcterms:created>2011-01-11</dcterms:created>	<dcterms:modified>2012-08-03</dcterms:modified>	<dcterms:hasVersion rdf:resource="&history;20120803/geotime#EarlyBathonian"/>	<rdfs:isDefinedBy rdf:resource="&geotime;"/>	<skos:inScheme rdf:resource="&geotime;"/>	<vann:termGroup rdf:resource="&geotime;Substage"/>	<vann:termGroup rdf:resource="&geotime;Chronostratigraphic"/>	<vs:term_status>unstable</vs:term_status>	</skos:Concept>
<skos:Concept rdf:about="&geotime;LateBajocian">	<skos:prefLabel xml:lang="en">Late Bajocian</skos:prefLabel>	<skos:definition>The Late Bajocian time period started 169.64  million years (Ma) before present (BP) and ended 167.68 Ma BP.</skos:definition>	<rdfs:seeAlso rdf:resource="http://kos.gbif.org/wiki/geotime:LateBajocian"/>	<geotime:rangeType>Substage</geotime:rangeType>	<geotime:rangeTypeURI rdf:resource="&geotime;Substage"/>	<geotime:start>169.64</geotime:start>	<geotime:end>167.68</geotime:end>		<dcterms:created>2011-01-11</dcterms:created>	<dcterms:modified>2012-08-03</dcterms:modified>	<dcterms:hasVersion rdf:resource="&history;20120803/geotime#LateBajocian"/>	<rdfs:isDefinedBy rdf:resource="&geotime;"/>	<skos:inScheme rdf:resource="&geotime;"/>	<vann:termGroup rdf:resource="&geotime;Substage"/>	<vann:termGroup rdf:resource="&geotime;Chronostratigraphic"/>	<vs:term_status>unstable</vs:term_status>	</skos:Concept>
<skos:Concept rdf:about="&geotime;EarlyBajocian">	<skos:prefLabel xml:lang="en">Early Bajocian</skos:prefLabel>	<skos:definition>The Early Bajocian time period started 171.6  million years (Ma) before present (BP) and ended 169.64 Ma BP.</skos:definition>	<rdfs:seeAlso rdf:resource="http://kos.gbif.org/wiki/geotime:EarlyBajocian"/>	<geotime:rangeType>Substage</geotime:rangeType>	<geotime:rangeTypeURI rdf:resource="&geotime;Substage"/>	<geotime:start>171.6</geotime:start>	<geotime:end>169.64</geotime:end>		<dcterms:created>2011-01-11</dcterms:created>	<dcterms:modified>2012-08-03</dcterms:modified>	<dcterms:hasVersion rdf:resource="&history;20120803/geotime#EarlyBajocian"/>	<rdfs:isDefinedBy rdf:resource="&geotime;"/>	<skos:inScheme rdf:resource="&geotime;"/>	<vann:termGroup rdf:resource="&geotime;Substage"/>	<vann:termGroup rdf:resource="&geotime;Chronostratigraphic"/>	<vs:term_status>unstable</vs:term_status>	</skos:Concept>
<skos:Concept rdf:about="&geotime;LateAalenian">	<skos:prefLabel xml:lang="en">Late Aalenian</skos:prefLabel>	<skos:definition>The Late Aalenian time period started 172.49  million years (Ma) before present (BP) and ended 171.6 Ma BP.</skos:definition>	<rdfs:seeAlso rdf:resource="http://kos.gbif.org/wiki/geotime:LateAalenian"/>	<geotime:rangeType>Substage</geotime:rangeType>	<geotime:rangeTypeURI rdf:resource="&geotime;Substage"/>	<geotime:start>172.49</geotime:start>	<geotime:end>171.6</geotime:end>		<dcterms:created>2011-01-11</dcterms:created>	<dcterms:modified>2012-08-03</dcterms:modified>	<dcterms:hasVersion rdf:resource="&history;20120803/geotime#LateAalenian"/>	<rdfs:isDefinedBy rdf:resource="&geotime;"/>	<skos:inScheme rdf:resource="&geotime;"/>	<vann:termGroup rdf:resource="&geotime;Substage"/>	<vann:termGroup rdf:resource="&geotime;Chronostratigraphic"/>	<vs:term_status>unstable</vs:term_status>	</skos:Concept>
<skos:Concept rdf:about="&geotime;MiddleAalenian">	<skos:prefLabel xml:lang="en">Middle Aalenian</skos:prefLabel>	<skos:definition>The Middle Aalenian time period started 174.71  million years (Ma) before present (BP) and ended 172.49 Ma BP.</skos:definition>	<rdfs:seeAlso rdf:resource="http://kos.gbif.org/wiki/geotime:MiddleAalenian"/>	<geotime:rangeType>Substage</geotime:rangeType>	<geotime:rangeTypeURI rdf:resource="&geotime;Substage"/>	<geotime:start>174.71</geotime:start>	<geotime:end>172.49</geotime:end>		<dcterms:created>2011-01-11</dcterms:created>	<dcterms:modified>2012-08-03</dcterms:modified>	<dcterms:hasVersion rdf:resource="&history;20120803/geotime#MiddleAalenian"/>	<rdfs:isDefinedBy rdf:resource="&geotime;"/>	<skos:inScheme rdf:resource="&geotime;"/>	<vann:termGroup rdf:resource="&geotime;Substage"/>	<vann:termGroup rdf:resource="&geotime;Chronostratigraphic"/>	<vs:term_status>unstable</vs:term_status>	</skos:Concept>
<skos:Concept rdf:about="&geotime;EarlyAalenian">	<skos:prefLabel xml:lang="en">Early Aalenian</skos:prefLabel>	<skos:definition>The Early Aalenian time period started 175.6  million years (Ma) before present (BP) and ended 174.71 Ma BP.</skos:definition>	<rdfs:seeAlso rdf:resource="http://kos.gbif.org/wiki/geotime:EarlyAalenian"/>	<geotime:rangeType>Substage</geotime:rangeType>	<geotime:rangeTypeURI rdf:resource="&geotime;Substage"/>	<geotime:start>175.6</geotime:start>	<geotime:end>174.71</geotime:end>		<dcterms:created>2011-01-11</dcterms:created>	<dcterms:modified>2012-08-03</dcterms:modified>	<dcterms:hasVersion rdf:resource="&history;20120803/geotime#EarlyAalenian"/>	<rdfs:isDefinedBy rdf:resource="&geotime;"/>	<skos:inScheme rdf:resource="&geotime;"/>	<vann:termGroup rdf:resource="&geotime;Substage"/>	<vann:termGroup rdf:resource="&geotime;Chronostratigraphic"/>	<vs:term_status>unstable</vs:term_status>	</skos:Concept>
<skos:Concept rdf:about="&geotime;LateToarcian">	<skos:prefLabel xml:lang="en">Late Toarcian</skos:prefLabel>	<skos:definition>The Late Toarcian time period started 180.5  million years (Ma) before present (BP) and ended 175.6 Ma BP.</skos:definition>	<rdfs:seeAlso rdf:resource="http://kos.gbif.org/wiki/geotime:LateToarcian"/>	<geotime:rangeType>Substage</geotime:rangeType>	<geotime:rangeTypeURI rdf:resource="&geotime;Substage"/>	<geotime:start>180.5</geotime:start>	<geotime:end>175.6</geotime:end>		<dcterms:created>2011-01-11</dcterms:created>	<dcterms:modified>2012-08-03</dcterms:modified>	<dcterms:hasVersion rdf:resource="&history;20120803/geotime#LateToarcian"/>	<rdfs:isDefinedBy rdf:resource="&geotime;"/>	<skos:inScheme rdf:resource="&geotime;"/>	<vann:termGroup rdf:resource="&geotime;Substage"/>	<vann:termGroup rdf:resource="&geotime;Chronostratigraphic"/>	<vs:term_status>unstable</vs:term_status>	</skos:Concept>
<skos:Concept rdf:about="&geotime;MiddleToarcian">	<skos:prefLabel xml:lang="en">Middle Toarcian</skos:prefLabel>	<skos:definition>The Middle Toarcian time period started 181.2  million years (Ma) before present (BP) and ended 180.5 Ma BP.</skos:definition>	<rdfs:seeAlso rdf:resource="http://kos.gbif.org/wiki/geotime:MiddleToarcian"/>	<geotime:rangeType>Substage</geotime:rangeType>	<geotime:rangeTypeURI rdf:resource="&geotime;Substage"/>	<geotime:start>181.2</geotime:start>	<geotime:end>180.5</geotime:end>		<dcterms:created>2011-01-11</dcterms:created>	<dcterms:modified>2012-08-03</dcterms:modified>	<dcterms:hasVersion rdf:resource="&history;20120803/geotime#MiddleToarcian"/>	<rdfs:isDefinedBy rdf:resource="&geotime;"/>	<skos:inScheme rdf:resource="&geotime;"/>	<vann:termGroup rdf:resource="&geotime;Substage"/>	<vann:termGroup rdf:resource="&geotime;Chronostratigraphic"/>	<vs:term_status>unstable</vs:term_status>	</skos:Concept>
<skos:Concept rdf:about="&geotime;EarlyToarcian">	<skos:prefLabel xml:lang="en">Early Toarcian</skos:prefLabel>	<skos:definition>The Early Toarcian time period started 183  million years (Ma) before present (BP) and ended 181.2 Ma BP.</skos:definition>	<rdfs:seeAlso rdf:resource="http://kos.gbif.org/wiki/geotime:EarlyToarcian"/>	<geotime:rangeType>Substage</geotime:rangeType>	<geotime:rangeTypeURI rdf:resource="&geotime;Substage"/>	<geotime:start>183</geotime:start>	<geotime:end>181.2</geotime:end>		<dcterms:created>2011-01-11</dcterms:created>	<dcterms:modified>2012-08-03</dcterms:modified>	<dcterms:hasVersion rdf:resource="&history;20120803/geotime#EarlyToarcian"/>	<rdfs:isDefinedBy rdf:resource="&geotime;"/>	<skos:inScheme rdf:resource="&geotime;"/>	<vann:termGroup rdf:resource="&geotime;Substage"/>	<vann:termGroup rdf:resource="&geotime;Chronostratigraphic"/>	<vs:term_status>unstable</vs:term_status>	</skos:Concept>
<skos:Concept rdf:about="&geotime;LatePliensbachian">	<skos:prefLabel xml:lang="en">Late Pliensbachian</skos:prefLabel>	<skos:definition>The Late Pliensbachian time period started 186.95  million years (Ma) before present (BP) and ended 183 Ma BP.</skos:definition>	<rdfs:seeAlso rdf:resource="http://kos.gbif.org/wiki/geotime:LatePliensbachian"/>	<geotime:rangeType>Substage</geotime:rangeType>	<geotime:rangeTypeURI rdf:resource="&geotime;Substage"/>	<geotime:start>186.95</geotime:start>	<geotime:end>183</geotime:end>		<dcterms:created>2011-01-11</dcterms:created>	<dcterms:modified>2012-08-03</dcterms:modified>	<dcterms:hasVersion rdf:resource="&history;20120803/geotime#LatePliensbachian"/>	<rdfs:isDefinedBy rdf:resource="&geotime;"/>	<skos:inScheme rdf:resource="&geotime;"/>	<vann:termGroup rdf:resource="&geotime;Substage"/>	<vann:termGroup rdf:resource="&geotime;Chronostratigraphic"/>	<vs:term_status>unstable</vs:term_status>	</skos:Concept>
<skos:Concept rdf:about="&geotime;EarlyPliensbachian">	<skos:prefLabel xml:lang="en">Early Pliensbachian</skos:prefLabel>	<skos:definition>The Early Pliensbachian time period started 189.6  million years (Ma) before present (BP) and ended 186.95 Ma BP.</skos:definition>	<rdfs:seeAlso rdf:resource="http://kos.gbif.org/wiki/geotime:EarlyPliensbachian"/>	<geotime:rangeType>Substage</geotime:rangeType>	<geotime:rangeTypeURI rdf:resource="&geotime;Substage"/>	<geotime:start>189.6</geotime:start>	<geotime:end>186.95</geotime:end>		<dcterms:created>2011-01-11</dcterms:created>	<dcterms:modified>2012-08-03</dcterms:modified>	<dcterms:hasVersion rdf:resource="&history;20120803/geotime#EarlyPliensbachian"/>	<rdfs:isDefinedBy rdf:resource="&geotime;"/>	<skos:inScheme rdf:resource="&geotime;"/>	<vann:termGroup rdf:resource="&geotime;Substage"/>	<vann:termGroup rdf:resource="&geotime;Chronostratigraphic"/>	<vs:term_status>unstable</vs:term_status>	</skos:Concept>
<skos:Concept rdf:about="&geotime;LateSinemurian">	<skos:prefLabel xml:lang="en">Late Sinemurian</skos:prefLabel>	<skos:definition>The Late Sinemurian time period started 193.25  million years (Ma) before present (BP) and ended 189.6 Ma BP.</skos:definition>	<rdfs:seeAlso rdf:resource="http://kos.gbif.org/wiki/geotime:LateSinemurian"/>	<geotime:rangeType>Substage</geotime:rangeType>	<geotime:rangeTypeURI rdf:resource="&geotime;Substage"/>	<geotime:start>193.25</geotime:start>	<geotime:end>189.6</geotime:end>		<dcterms:created>2011-01-11</dcterms:created>	<dcterms:modified>2012-08-03</dcterms:modified>	<dcterms:hasVersion rdf:resource="&history;20120803/geotime#LateSinemurian"/>	<rdfs:isDefinedBy rdf:resource="&geotime;"/>	<skos:inScheme rdf:resource="&geotime;"/>	<vann:termGroup rdf:resource="&geotime;Substage"/>	<vann:termGroup rdf:resource="&geotime;Chronostratigraphic"/>	<vs:term_status>unstable</vs:term_status>	</skos:Concept>
<skos:Concept rdf:about="&geotime;EarlySinemurian">	<skos:prefLabel xml:lang="en">Early Sinemurian</skos:prefLabel>	<skos:definition>The Early Sinemurian time period started 196.5  million years (Ma) before present (BP) and ended 193.25 Ma BP.</skos:definition>	<rdfs:seeAlso rdf:resource="http://kos.gbif.org/wiki/geotime:EarlySinemurian"/>	<geotime:rangeType>Substage</geotime:rangeType>	<geotime:rangeTypeURI rdf:resource="&geotime;Substage"/>	<geotime:start>196.5</geotime:start>	<geotime:end>193.25</geotime:end>		<dcterms:created>2011-01-11</dcterms:created>	<dcterms:modified>2012-08-03</dcterms:modified>	<dcterms:hasVersion rdf:resource="&history;20120803/geotime#EarlySinemurian"/>	<rdfs:isDefinedBy rdf:resource="&geotime;"/>	<skos:inScheme rdf:resource="&geotime;"/>	<vann:termGroup rdf:resource="&geotime;Substage"/>	<vann:termGroup rdf:resource="&geotime;Chronostratigraphic"/>	<vs:term_status>unstable</vs:term_status>	</skos:Concept>
<skos:Concept rdf:about="&geotime;Unnamed">	<skos:prefLabel xml:lang="en">Unnamed</skos:prefLabel>	<skos:definition>The Unnamed time period started 199.6  million years (Ma) before present (BP) and ended 196.5 Ma BP.</skos:definition>	<rdfs:seeAlso rdf:resource="http://kos.gbif.org/wiki/geotime:Unnamed"/>	<geotime:rangeType>Substage</geotime:rangeType>	<geotime:rangeTypeURI rdf:resource="&geotime;Substage"/>	<geotime:start>199.6</geotime:start>	<geotime:end>196.5</geotime:end>		<dcterms:created>2011-01-11</dcterms:created>	<dcterms:modified>2012-08-03</dcterms:modified>	<dcterms:hasVersion rdf:resource="&history;20120803/geotime#Unnamed"/>	<rdfs:isDefinedBy rdf:resource="&geotime;"/>	<skos:inScheme rdf:resource="&geotime;"/>	<vann:termGroup rdf:resource="&geotime;Substage"/>	<vann:termGroup rdf:resource="&geotime;Chronostratigraphic"/>	<vs:term_status>unstable</vs:term_status>	</skos:Concept>
<skos:Concept rdf:about="&geotime;LateNorian">	<skos:prefLabel xml:lang="en">Late Norian</skos:prefLabel>	<skos:definition>The Late Norian time period started 205.71  million years (Ma) before present (BP) and ended 203.64 Ma BP.</skos:definition>	<rdfs:seeAlso rdf:resource="http://kos.gbif.org/wiki/geotime:LateNorian"/>	<geotime:rangeType>Substage</geotime:rangeType>	<geotime:rangeTypeURI rdf:resource="&geotime;Substage"/>	<geotime:start>205.71</geotime:start>	<geotime:end>203.64</geotime:end>		<dcterms:created>2011-01-11</dcterms:created>	<dcterms:modified>2012-08-03</dcterms:modified>	<dcterms:hasVersion rdf:resource="&history;20120803/geotime#LateNorian"/>	<rdfs:isDefinedBy rdf:resource="&geotime;"/>	<skos:inScheme rdf:resource="&geotime;"/>	<vann:termGroup rdf:resource="&geotime;Substage"/>	<vann:termGroup rdf:resource="&geotime;Chronostratigraphic"/>	<vs:term_status>unstable</vs:term_status>	</skos:Concept>
<skos:Concept rdf:about="&geotime;MiddleNorian">	<skos:prefLabel xml:lang="en">Middle Norian</skos:prefLabel>	<skos:definition>The Middle Norian time period started 211.3  million years (Ma) before present (BP) and ended 205.71 Ma BP.</skos:definition>	<rdfs:seeAlso rdf:resource="http://kos.gbif.org/wiki/geotime:MiddleNorian"/>	<geotime:rangeType>Substage</geotime:rangeType>	<geotime:rangeTypeURI rdf:resource="&geotime;Substage"/>	<geotime:start>211.3</geotime:start>	<geotime:end>205.71</geotime:end>		<dcterms:created>2011-01-11</dcterms:created>	<dcterms:modified>2012-08-03</dcterms:modified>	<dcterms:hasVersion rdf:resource="&history;20120803/geotime#MiddleNorian"/>	<rdfs:isDefinedBy rdf:resource="&geotime;"/>	<skos:inScheme rdf:resource="&geotime;"/>	<vann:termGroup rdf:resource="&geotime;Substage"/>	<vann:termGroup rdf:resource="&geotime;Chronostratigraphic"/>	<vs:term_status>unstable</vs:term_status>	</skos:Concept>
<skos:Concept rdf:about="&geotime;EarlyNorian">	<skos:prefLabel xml:lang="en">Early Norian</skos:prefLabel>	<skos:definition>The Early Norian time period started 216.53  million years (Ma) before present (BP) and ended 211.3 Ma BP.</skos:definition>	<rdfs:seeAlso rdf:resource="http://kos.gbif.org/wiki/geotime:EarlyNorian"/>	<geotime:rangeType>Substage</geotime:rangeType>	<geotime:rangeTypeURI rdf:resource="&geotime;Substage"/>	<geotime:start>216.53</geotime:start>	<geotime:end>211.3</geotime:end>		<dcterms:created>2011-01-11</dcterms:created>	<dcterms:modified>2012-08-03</dcterms:modified>	<dcterms:hasVersion rdf:resource="&history;20120803/geotime#EarlyNorian"/>	<rdfs:isDefinedBy rdf:resource="&geotime;"/>	<skos:inScheme rdf:resource="&geotime;"/>	<vann:termGroup rdf:resource="&geotime;Substage"/>	<vann:termGroup rdf:resource="&geotime;Chronostratigraphic"/>	<vs:term_status>unstable</vs:term_status>	</skos:Concept>
<skos:Concept rdf:about="&geotime;LateCarnian">	<skos:prefLabel xml:lang="en">Late Carnian</skos:prefLabel>	<skos:definition>The Late Carnian time period started 222.7  million years (Ma) before present (BP) and ended 216.53 Ma BP.</skos:definition>	<rdfs:seeAlso rdf:resource="http://kos.gbif.org/wiki/geotime:LateCarnian"/>	<geotime:rangeType>Substage</geotime:rangeType>	<geotime:rangeTypeURI rdf:resource="&geotime;Substage"/>	<geotime:start>222.7</geotime:start>	<geotime:end>216.53</geotime:end>		<dcterms:created>2011-01-11</dcterms:created>	<dcterms:modified>2012-08-03</dcterms:modified>	<dcterms:hasVersion rdf:resource="&history;20120803/geotime#LateCarnian"/>	<rdfs:isDefinedBy rdf:resource="&geotime;"/>	<skos:inScheme rdf:resource="&geotime;"/>	<vann:termGroup rdf:resource="&geotime;Substage"/>	<vann:termGroup rdf:resource="&geotime;Chronostratigraphic"/>	<vs:term_status>unstable</vs:term_status>	</skos:Concept>
<skos:Concept rdf:about="&geotime;EarlyCarnian">	<skos:prefLabel xml:lang="en">Early Carnian</skos:prefLabel>	<skos:definition>The Early Carnian time period started 228.01  million years (Ma) before present (BP) and ended 222.7 Ma BP.</skos:definition>	<rdfs:seeAlso rdf:resource="http://kos.gbif.org/wiki/geotime:EarlyCarnian"/>	<geotime:rangeType>Substage</geotime:rangeType>	<geotime:rangeTypeURI rdf:resource="&geotime;Substage"/>	<geotime:start>228.01</geotime:start>	<geotime:end>222.7</geotime:end>		<dcterms:created>2011-01-11</dcterms:created>	<dcterms:modified>2012-08-03</dcterms:modified>	<dcterms:hasVersion rdf:resource="&history;20120803/geotime#EarlyCarnian"/>	<rdfs:isDefinedBy rdf:resource="&geotime;"/>	<skos:inScheme rdf:resource="&geotime;"/>	<vann:termGroup rdf:resource="&geotime;Substage"/>	<vann:termGroup rdf:resource="&geotime;Chronostratigraphic"/>	<vs:term_status>unstable</vs:term_status>	</skos:Concept>
<skos:Concept rdf:about="&geotime;LateLadinian">	<skos:prefLabel xml:lang="en">Late Ladinian</skos:prefLabel>	<skos:definition>The Late Ladinian time period started 233.34  million years (Ma) before present (BP) and ended 228.01 Ma BP.</skos:definition>	<rdfs:seeAlso rdf:resource="http://kos.gbif.org/wiki/geotime:LateLadinian"/>	<geotime:rangeType>Substage</geotime:rangeType>	<geotime:rangeTypeURI rdf:resource="&geotime;Substage"/>	<geotime:start>233.34</geotime:start>	<geotime:end>228.01</geotime:end>		<dcterms:created>2011-01-11</dcterms:created>	<dcterms:modified>2012-08-03</dcterms:modified>	<dcterms:hasVersion rdf:resource="&history;20120803/geotime#LateLadinian"/>	<rdfs:isDefinedBy rdf:resource="&geotime;"/>	<skos:inScheme rdf:resource="&geotime;"/>	<vann:termGroup rdf:resource="&geotime;Substage"/>	<vann:termGroup rdf:resource="&geotime;Chronostratigraphic"/>	<vs:term_status>unstable</vs:term_status>	</skos:Concept>
<skos:Concept rdf:about="&geotime;EarlyLadinian">	<skos:prefLabel xml:lang="en">Early Ladinian</skos:prefLabel>	<skos:definition>The Early Ladinian time period started 237  million years (Ma) before present (BP) and ended 233.34 Ma BP.</skos:definition>	<rdfs:seeAlso rdf:resource="http://kos.gbif.org/wiki/geotime:EarlyLadinian"/>	<geotime:rangeType>Substage</geotime:rangeType>	<geotime:rangeTypeURI rdf:resource="&geotime;Substage"/>	<geotime:start>237</geotime:start>	<geotime:end>233.34</geotime:end>		<dcterms:created>2011-01-11</dcterms:created>	<dcterms:modified>2012-08-03</dcterms:modified>	<dcterms:hasVersion rdf:resource="&history;20120803/geotime#EarlyLadinian"/>	<rdfs:isDefinedBy rdf:resource="&geotime;"/>	<skos:inScheme rdf:resource="&geotime;"/>	<vann:termGroup rdf:resource="&geotime;Substage"/>	<vann:termGroup rdf:resource="&geotime;Chronostratigraphic"/>	<vs:term_status>unstable</vs:term_status>	</skos:Concept>
<skos:Concept rdf:about="&geotime;LateAnisian">	<skos:prefLabel xml:lang="en">Late Anisian</skos:prefLabel>	<skos:definition>The Late Anisian time period started 241.6  million years (Ma) before present (BP) and ended 237 Ma BP.</skos:definition>	<rdfs:seeAlso rdf:resource="http://kos.gbif.org/wiki/geotime:LateAnisian"/>	<geotime:rangeType>Substage</geotime:rangeType>	<geotime:rangeTypeURI rdf:resource="&geotime;Substage"/>	<geotime:start>241.6</geotime:start>	<geotime:end>237</geotime:end>		<dcterms:created>2011-01-11</dcterms:created>	<dcterms:modified>2012-08-03</dcterms:modified>	<dcterms:hasVersion rdf:resource="&history;20120803/geotime#LateAnisian"/>	<rdfs:isDefinedBy rdf:resource="&geotime;"/>	<skos:inScheme rdf:resource="&geotime;"/>	<vann:termGroup rdf:resource="&geotime;Substage"/>	<vann:termGroup rdf:resource="&geotime;Chronostratigraphic"/>	<vs:term_status>unstable</vs:term_status>	</skos:Concept>
<skos:Concept rdf:about="&geotime;EarlyAnisian">	<skos:prefLabel xml:lang="en">Early Anisian</skos:prefLabel>	<skos:definition>The Early Anisian time period started 243.68  million years (Ma) before present (BP) and ended 242.49 Ma BP.</skos:definition>	<rdfs:seeAlso rdf:resource="http://kos.gbif.org/wiki/geotime:EarlyAnisian"/>	<geotime:rangeType>Substage</geotime:rangeType>	<geotime:rangeTypeURI rdf:resource="&geotime;Substage"/>	<geotime:start>243.68</geotime:start>	<geotime:end>242.49</geotime:end>		<dcterms:created>2011-01-11</dcterms:created>	<dcterms:modified>2012-08-03</dcterms:modified>	<dcterms:hasVersion rdf:resource="&history;20120803/geotime#EarlyAnisian"/>	<rdfs:isDefinedBy rdf:resource="&geotime;"/>	<skos:inScheme rdf:resource="&geotime;"/>	<vann:termGroup rdf:resource="&geotime;Substage"/>	<vann:termGroup rdf:resource="&geotime;Chronostratigraphic"/>	<vs:term_status>unstable</vs:term_status>	</skos:Concept>
<skos:Concept rdf:about="&geotime;LateOlenekian">	<skos:prefLabel xml:lang="en">Late Olenekian</skos:prefLabel>	<skos:definition>The Late Olenekian time period started 248.08  million years (Ma) before present (BP) and ended 245.17 Ma BP.</skos:definition>	<rdfs:seeAlso rdf:resource="http://kos.gbif.org/wiki/geotime:LateOlenekian"/>	<geotime:rangeType>Substage</geotime:rangeType>	<geotime:rangeTypeURI rdf:resource="&geotime;Substage"/>	<geotime:start>248.08</geotime:start>	<geotime:end>245.17</geotime:end>		<dcterms:created>2011-01-11</dcterms:created>	<dcterms:modified>2012-08-03</dcterms:modified>	<dcterms:hasVersion rdf:resource="&history;20120803/geotime#LateOlenekian"/>	<rdfs:isDefinedBy rdf:resource="&geotime;"/>	<skos:inScheme rdf:resource="&geotime;"/>	<vann:termGroup rdf:resource="&geotime;Substage"/>	<vann:termGroup rdf:resource="&geotime;Chronostratigraphic"/>	<vs:term_status>unstable</vs:term_status>	</skos:Concept>
<skos:Concept rdf:about="&geotime;EarlyOlenekian">	<skos:prefLabel xml:lang="en">Early Olenekian</skos:prefLabel>	<skos:definition>The Early Olenekian time period started 249.75  million years (Ma) before present (BP) and ended 248.08 Ma BP.</skos:definition>	<rdfs:seeAlso rdf:resource="http://kos.gbif.org/wiki/geotime:EarlyOlenekian"/>	<geotime:rangeType>Substage</geotime:rangeType>	<geotime:rangeTypeURI rdf:resource="&geotime;Substage"/>	<geotime:start>249.75</geotime:start>	<geotime:end>248.08</geotime:end>		<dcterms:created>2011-01-11</dcterms:created>	<dcterms:modified>2012-08-03</dcterms:modified>	<dcterms:hasVersion rdf:resource="&history;20120803/geotime#EarlyOlenekian"/>	<rdfs:isDefinedBy rdf:resource="&geotime;"/>	<skos:inScheme rdf:resource="&geotime;"/>	<vann:termGroup rdf:resource="&geotime;Substage"/>	<vann:termGroup rdf:resource="&geotime;Chronostratigraphic"/>	<vs:term_status>unstable</vs:term_status>	</skos:Concept>
<skos:Concept rdf:about="&geotime;LateInduan">	<skos:prefLabel xml:lang="en">Late Induan</skos:prefLabel>	<skos:definition>The Late Induan time period started 250.38  million years (Ma) before present (BP) and ended 249.75 Ma BP.</skos:definition>	<rdfs:seeAlso rdf:resource="http://kos.gbif.org/wiki/geotime:LateInduan"/>	<geotime:rangeType>Substage</geotime:rangeType>	<geotime:rangeTypeURI rdf:resource="&geotime;Substage"/>	<geotime:start>250.38</geotime:start>	<geotime:end>249.75</geotime:end>		<dcterms:created>2011-01-11</dcterms:created>	<dcterms:modified>2012-08-03</dcterms:modified>	<dcterms:hasVersion rdf:resource="&history;20120803/geotime#LateInduan"/>	<rdfs:isDefinedBy rdf:resource="&geotime;"/>	<skos:inScheme rdf:resource="&geotime;"/>	<vann:termGroup rdf:resource="&geotime;Substage"/>	<vann:termGroup rdf:resource="&geotime;Chronostratigraphic"/>	<vs:term_status>unstable</vs:term_status>	</skos:Concept>
<skos:Concept rdf:about="&geotime;EarlyInduan">	<skos:prefLabel xml:lang="en">Early Induan</skos:prefLabel>	<skos:definition>The Early Induan time period started 251  million years (Ma) before present (BP) and ended 250.38 Ma BP.</skos:definition>	<rdfs:seeAlso rdf:resource="http://kos.gbif.org/wiki/geotime:EarlyInduan"/>	<geotime:rangeType>Substage</geotime:rangeType>	<geotime:rangeTypeURI rdf:resource="&geotime;Substage"/>	<geotime:start>251</geotime:start>	<geotime:end>250.38</geotime:end>		<dcterms:created>2011-01-11</dcterms:created>	<dcterms:modified>2012-08-03</dcterms:modified>	<dcterms:hasVersion rdf:resource="&history;20120803/geotime#EarlyInduan"/>	<rdfs:isDefinedBy rdf:resource="&geotime;"/>	<skos:inScheme rdf:resource="&geotime;"/>	<vann:termGroup rdf:resource="&geotime;Substage"/>	<vann:termGroup rdf:resource="&geotime;Chronostratigraphic"/>	<vs:term_status>unstable</vs:term_status>	</skos:Concept>




<!-- Magnetostratigraphic scale -->

<skos:Concept rdf:about="http://rs.gbif.org/terms/geotime#C1n">	<skos:prefLabel xml:lang="en">C1n</skos:prefLabel>	<skos:definition>The C1n magnetostratographic time period started 0.781 million years (Ma) before present (BP) and ended 0 Ma BP.</skos:definition>	<rdfs:seeAlso rdf:resource="http://kos.gbif.org/wiki/geotime:C1n"/>	<dcterms:created>2011-01-11</dcterms:created>	<dcterms:modified>2012-08-03</dcterms:modified>	<geotime:start>0.781</geotime:start>	<geotime:end>0</geotime:end>	<geotime:polarity>N</geotime:polarity>	<geotime:regionName>Brunhes</geotime:regionName>	<dcterms:hasVersion rdf:resource="&history;20120803/geotime#C1n"/>	<rdfs:isDefinedBy rdf:resource="&geotime;"/>	<skos:inScheme rdf:resource="&geotime;"/>	<vann:termGroup rdf:resource="&geotime;Magnetostratigraphic"/>	<vs:term_status>unstable</vs:term_status>	</skos:Concept>
<skos:Concept rdf:about="http://rs.gbif.org/terms/geotime#C1rvvv1r">	<skos:prefLabel xml:lang="en">C1rvvv1r</skos:prefLabel>	<skos:definition>The C1rvvv1r magnetostratographic time period started 0.988 million years (Ma) before present (BP) and ended 0.781 Ma BP.</skos:definition>	<rdfs:seeAlso rdf:resource="http://kos.gbif.org/wiki/geotime:C1rvvv1r"/>	<dcterms:created>2011-01-11</dcterms:created>	<dcterms:modified>2012-08-03</dcterms:modified>	<geotime:start>0.988</geotime:start>	<geotime:end>0.781</geotime:end>	<geotime:polarity>R</geotime:polarity>	<geotime:regionName>Matuyama</geotime:regionName>	<dcterms:hasVersion rdf:resource="&history;20120803/geotime#C1rvvv1r"/>	<rdfs:isDefinedBy rdf:resource="&geotime;"/>	<skos:inScheme rdf:resource="&geotime;"/>	<vann:termGroup rdf:resource="&geotime;Magnetostratigraphic"/>	<vs:term_status>unstable</vs:term_status>	</skos:Concept>
<skos:Concept rdf:about="http://rs.gbif.org/terms/geotime#C1rvvv1n">	<skos:prefLabel xml:lang="en">C1rvvv1n</skos:prefLabel>	<skos:definition>The C1rvvv1n magnetostratographic time period started 1.072 million years (Ma) before present (BP) and ended 0.988 Ma BP.</skos:definition>	<rdfs:seeAlso rdf:resource="http://kos.gbif.org/wiki/geotime:C1rvvv1n"/>	<dcterms:created>2011-01-11</dcterms:created>	<dcterms:modified>2012-08-03</dcterms:modified>	<geotime:start>1.072</geotime:start>	<geotime:end>0.988</geotime:end>	<geotime:polarity>N</geotime:polarity>	<geotime:regionName>Jaramillo</geotime:regionName>	<dcterms:hasVersion rdf:resource="&history;20120803/geotime#C1rvvv1n"/>	<rdfs:isDefinedBy rdf:resource="&geotime;"/>	<skos:inScheme rdf:resource="&geotime;"/>	<vann:termGroup rdf:resource="&geotime;Magnetostratigraphic"/>	<vs:term_status>unstable</vs:term_status>	</skos:Concept>
<skos:Concept rdf:about="http://rs.gbif.org/terms/geotime#C1rvvv2r">	<skos:prefLabel xml:lang="en">C1rvvv2r</skos:prefLabel>	<skos:definition>The C1rvvv2r magnetostratographic time period started 1.173 million years (Ma) before present (BP) and ended 1.072 Ma BP.</skos:definition>	<rdfs:seeAlso rdf:resource="http://kos.gbif.org/wiki/geotime:C1rvvv2r"/>	<dcterms:created>2011-01-11</dcterms:created>	<dcterms:modified>2012-08-03</dcterms:modified>	<geotime:start>1.173</geotime:start>	<geotime:end>1.072</geotime:end>	<geotime:polarity>R</geotime:polarity>	<geotime:regionName></geotime:regionName>	<dcterms:hasVersion rdf:resource="&history;20120803/geotime#C1rvvv2r"/>	<rdfs:isDefinedBy rdf:resource="&geotime;"/>	<skos:inScheme rdf:resource="&geotime;"/>	<vann:termGroup rdf:resource="&geotime;Magnetostratigraphic"/>	<vs:term_status>unstable</vs:term_status>	</skos:Concept>
<skos:Concept rdf:about="http://rs.gbif.org/terms/geotime#C1rvvv2n">	<skos:prefLabel xml:lang="en">C1rvvv2n</skos:prefLabel>	<skos:definition>The C1rvvv2n magnetostratographic time period started 1.185 million years (Ma) before present (BP) and ended 1.173 Ma BP.</skos:definition>	<rdfs:seeAlso rdf:resource="http://kos.gbif.org/wiki/geotime:C1rvvv2n"/>	<dcterms:created>2011-01-11</dcterms:created>	<dcterms:modified>2012-08-03</dcterms:modified>	<geotime:start>1.185</geotime:start>	<geotime:end>1.173</geotime:end>	<geotime:polarity>N</geotime:polarity>	<geotime:regionName>Cobb Mountain</geotime:regionName>	<dcterms:hasVersion rdf:resource="&history;20120803/geotime#C1rvvv2n"/>	<rdfs:isDefinedBy rdf:resource="&geotime;"/>	<skos:inScheme rdf:resource="&geotime;"/>	<vann:termGroup rdf:resource="&geotime;Magnetostratigraphic"/>	<vs:term_status>unstable</vs:term_status>	</skos:Concept>
<skos:Concept rdf:about="http://rs.gbif.org/terms/geotime#C1">	<skos:prefLabel xml:lang="en">C1</skos:prefLabel>	<skos:definition>The C1 magnetostratographic time period started 1.778 million years (Ma) before present (BP) and ended 0 Ma BP.</skos:definition>	<rdfs:seeAlso rdf:resource="http://kos.gbif.org/wiki/geotime:C1"/>	<dcterms:created>2011-01-11</dcterms:created>	<dcterms:modified>2012-08-03</dcterms:modified>	<geotime:start>1.778</geotime:start>	<geotime:end>0</geotime:end>	<geotime:polarity></geotime:polarity>	<geotime:regionName></geotime:regionName>	<dcterms:hasVersion rdf:resource="&history;20120803/geotime#C1"/>	<rdfs:isDefinedBy rdf:resource="&geotime;"/>	<skos:inScheme rdf:resource="&geotime;"/>	<vann:termGroup rdf:resource="&geotime;Magnetostratigraphic"/>	<vs:term_status>unstable</vs:term_status>	</skos:Concept>
<skos:Concept rdf:about="http://rs.gbif.org/terms/geotime#C1rvvv3r">	<skos:prefLabel xml:lang="en">C1rvvv3r</skos:prefLabel>	<skos:definition>The C1rvvv3r magnetostratographic time period started 1.778 million years (Ma) before present (BP) and ended 1.185 Ma BP.</skos:definition>	<rdfs:seeAlso rdf:resource="http://kos.gbif.org/wiki/geotime:C1rvvv3r"/>	<dcterms:created>2011-01-11</dcterms:created>	<dcterms:modified>2012-08-03</dcterms:modified>	<geotime:start>1.778</geotime:start>	<geotime:end>1.185</geotime:end>	<geotime:polarity>R</geotime:polarity>	<geotime:regionName></geotime:regionName>	<dcterms:hasVersion rdf:resource="&history;20120803/geotime#C1rvvv3r"/>	<rdfs:isDefinedBy rdf:resource="&geotime;"/>	<skos:inScheme rdf:resource="&geotime;"/>	<vann:termGroup rdf:resource="&geotime;Magnetostratigraphic"/>	<vs:term_status>unstable</vs:term_status>	</skos:Concept>
<skos:Concept rdf:about="http://rs.gbif.org/terms/geotime#C2n">	<skos:prefLabel xml:lang="en">C2n</skos:prefLabel>	<skos:definition>The C2n magnetostratographic time period started 1.945 million years (Ma) before present (BP) and ended 1.778 Ma BP.</skos:definition>	<rdfs:seeAlso rdf:resource="http://kos.gbif.org/wiki/geotime:C2n"/>	<dcterms:created>2011-01-11</dcterms:created>	<dcterms:modified>2012-08-03</dcterms:modified>	<geotime:start>1.945</geotime:start>	<geotime:end>1.778</geotime:end>	<geotime:polarity>N</geotime:polarity>	<geotime:regionName>Olduvai</geotime:regionName>	<dcterms:hasVersion rdf:resource="&history;20120803/geotime#C2n"/>	<rdfs:isDefinedBy rdf:resource="&geotime;"/>	<skos:inScheme rdf:resource="&geotime;"/>	<vann:termGroup rdf:resource="&geotime;Magnetostratigraphic"/>	<vs:term_status>unstable</vs:term_status>	</skos:Concept>
<skos:Concept rdf:about="http://rs.gbif.org/terms/geotime#C5nvvv2n">	<skos:prefLabel xml:lang="en">C5nvvv2n</skos:prefLabel>	<skos:definition>The C5nvvv2n magnetostratographic time period started 11.04 million years (Ma) before present (BP) and ended 9.987 Ma BP.</skos:definition>	<rdfs:seeAlso rdf:resource="http://kos.gbif.org/wiki/geotime:C5nvvv2n"/>	<dcterms:created>2011-01-11</dcterms:created>	<dcterms:modified>2012-08-03</dcterms:modified>	<geotime:start>11.04</geotime:start>	<geotime:end>9.987</geotime:end>	<geotime:polarity>N</geotime:polarity>	<geotime:regionName></geotime:regionName>	<dcterms:hasVersion rdf:resource="&history;20120803/geotime#C5nvvv2n"/>	<rdfs:isDefinedBy rdf:resource="&geotime;"/>	<skos:inScheme rdf:resource="&geotime;"/>	<vann:termGroup rdf:resource="&geotime;Magnetostratigraphic"/>	<vs:term_status>unstable</vs:term_status>	</skos:Concept>
<skos:Concept rdf:about="http://rs.gbif.org/terms/geotime#C5rvvv1r">	<skos:prefLabel xml:lang="en">C5rvvv1r</skos:prefLabel>	<skos:definition>The C5rvvv1r magnetostratographic time period started 11.118 million years (Ma) before present (BP) and ended 11.04 Ma BP.</skos:definition>	<rdfs:seeAlso rdf:resource="http://kos.gbif.org/wiki/geotime:C5rvvv1r"/>	<dcterms:created>2011-01-11</dcterms:created>	<dcterms:modified>2012-08-03</dcterms:modified>	<geotime:start>11.118</geotime:start>	<geotime:end>11.04</geotime:end>	<geotime:polarity>R</geotime:polarity>	<geotime:regionName></geotime:regionName>	<dcterms:hasVersion rdf:resource="&history;20120803/geotime#C5rvvv1r"/>	<rdfs:isDefinedBy rdf:resource="&geotime;"/>	<skos:inScheme rdf:resource="&geotime;"/>	<vann:termGroup rdf:resource="&geotime;Magnetostratigraphic"/>	<vs:term_status>unstable</vs:term_status>	</skos:Concept>
<skos:Concept rdf:about="http://rs.gbif.org/terms/geotime#C5rvvv1n">	<skos:prefLabel xml:lang="en">C5rvvv1n</skos:prefLabel>	<skos:definition>The C5rvvv1n magnetostratographic time period started 11.154 million years (Ma) before present (BP) and ended 11.118 Ma BP.</skos:definition>	<rdfs:seeAlso rdf:resource="http://kos.gbif.org/wiki/geotime:C5rvvv1n"/>	<dcterms:created>2011-01-11</dcterms:created>	<dcterms:modified>2012-08-03</dcterms:modified>	<geotime:start>11.154</geotime:start>	<geotime:end>11.118</geotime:end>	<geotime:polarity>N</geotime:polarity>	<geotime:regionName></geotime:regionName>	<dcterms:hasVersion rdf:resource="&history;20120803/geotime#C5rvvv1n"/>	<rdfs:isDefinedBy rdf:resource="&geotime;"/>	<skos:inScheme rdf:resource="&geotime;"/>	<vann:termGroup rdf:resource="&geotime;Magnetostratigraphic"/>	<vs:term_status>unstable</vs:term_status>	</skos:Concept>
<skos:Concept rdf:about="http://rs.gbif.org/terms/geotime#C5rvvv2r">	<skos:prefLabel xml:lang="en">C5rvvv2r</skos:prefLabel>	<skos:definition>The C5rvvv2r magnetostratographic time period started 11.554 million years (Ma) before present (BP) and ended 11.154 Ma BP.</skos:definition>	<rdfs:seeAlso rdf:resource="http://kos.gbif.org/wiki/geotime:C5rvvv2r"/>	<dcterms:created>2011-01-11</dcterms:created>	<dcterms:modified>2012-08-03</dcterms:modified>	<geotime:start>11.554</geotime:start>	<geotime:end>11.154</geotime:end>	<geotime:polarity>R</geotime:polarity>	<geotime:regionName></geotime:regionName>	<dcterms:hasVersion rdf:resource="&history;20120803/geotime#C5rvvv2r"/>	<rdfs:isDefinedBy rdf:resource="&geotime;"/>	<skos:inScheme rdf:resource="&geotime;"/>	<vann:termGroup rdf:resource="&geotime;Magnetostratigraphic"/>	<vs:term_status>unstable</vs:term_status>	</skos:Concept>
<skos:Concept rdf:about="http://rs.gbif.org/terms/geotime#C5rvvv2n">	<skos:prefLabel xml:lang="en">C5rvvv2n</skos:prefLabel>	<skos:definition>The C5rvvv2n magnetostratographic time period started 11.614 million years (Ma) before present (BP) and ended 11.554 Ma BP.</skos:definition>	<rdfs:seeAlso rdf:resource="http://kos.gbif.org/wiki/geotime:C5rvvv2n"/>	<dcterms:created>2011-01-11</dcterms:created>	<dcterms:modified>2012-08-03</dcterms:modified>	<geotime:start>11.614</geotime:start>	<geotime:end>11.554</geotime:end>	<geotime:polarity>N</geotime:polarity>	<geotime:regionName></geotime:regionName>	<dcterms:hasVersion rdf:resource="&history;20120803/geotime#C5rvvv2n"/>	<rdfs:isDefinedBy rdf:resource="&geotime;"/>	<skos:inScheme rdf:resource="&geotime;"/>	<vann:termGroup rdf:resource="&geotime;Magnetostratigraphic"/>	<vs:term_status>unstable</vs:term_status>	</skos:Concept>
<skos:Concept rdf:about="http://rs.gbif.org/terms/geotime#C5rvvv3r">	<skos:prefLabel xml:lang="en">C5rvvv3r</skos:prefLabel>	<skos:definition>The C5rvvv3r magnetostratographic time period started 12.014 million years (Ma) before present (BP) and ended 11.614 Ma BP.</skos:definition>	<rdfs:seeAlso rdf:resource="http://kos.gbif.org/wiki/geotime:C5rvvv3r"/>	<dcterms:created>2011-01-11</dcterms:created>	<dcterms:modified>2012-08-03</dcterms:modified>	<geotime:start>12.014</geotime:start>	<geotime:end>11.614</geotime:end>	<geotime:polarity>R</geotime:polarity>	<geotime:regionName></geotime:regionName>	<dcterms:hasVersion rdf:resource="&history;20120803/geotime#C5rvvv3r"/>	<rdfs:isDefinedBy rdf:resource="&geotime;"/>	<skos:inScheme rdf:resource="&geotime;"/>	<vann:termGroup rdf:resource="&geotime;Magnetostratigraphic"/>	<vs:term_status>unstable</vs:term_status>	</skos:Concept>
<skos:Concept rdf:about="http://rs.gbif.org/terms/geotime#C5">	<skos:prefLabel xml:lang="en">C5</skos:prefLabel>	<skos:definition>The C5 magnetostratographic time period started 12.014 million years (Ma) before present (BP) and ended 9.779 Ma BP.</skos:definition>	<rdfs:seeAlso rdf:resource="http://kos.gbif.org/wiki/geotime:C5"/>	<dcterms:created>2011-01-11</dcterms:created>	<dcterms:modified>2012-08-03</dcterms:modified>	<geotime:start>12.014</geotime:start>	<geotime:end>9.779</geotime:end>	<geotime:polarity></geotime:polarity>	<geotime:regionName></geotime:regionName>	<dcterms:hasVersion rdf:resource="&history;20120803/geotime#C5"/>	<rdfs:isDefinedBy rdf:resource="&geotime;"/>	<skos:inScheme rdf:resource="&geotime;"/>	<vann:termGroup rdf:resource="&geotime;Magnetostratigraphic"/>	<vs:term_status>unstable</vs:term_status>	</skos:Concept>
<skos:Concept rdf:about="http://rs.gbif.org/terms/geotime#C5Anvvv1n">	<skos:prefLabel xml:lang="en">C5Anvvv1n</skos:prefLabel>	<skos:definition>The C5Anvvv1n magnetostratographic time period started 12.116 million years (Ma) before present (BP) and ended 12.014 Ma BP.</skos:definition>	<rdfs:seeAlso rdf:resource="http://kos.gbif.org/wiki/geotime:C5Anvvv1n"/>	<dcterms:created>2011-01-11</dcterms:created>	<dcterms:modified>2012-08-03</dcterms:modified>	<geotime:start>12.116</geotime:start>	<geotime:end>12.014</geotime:end>	<geotime:polarity>N</geotime:polarity>	<geotime:regionName></geotime:regionName>	<dcterms:hasVersion rdf:resource="&history;20120803/geotime#C5Anvvv1n"/>	<rdfs:isDefinedBy rdf:resource="&geotime;"/>	<skos:inScheme rdf:resource="&geotime;"/>	<vann:termGroup rdf:resource="&geotime;Magnetostratigraphic"/>	<vs:term_status>unstable</vs:term_status>	</skos:Concept>
<skos:Concept rdf:about="http://rs.gbif.org/terms/geotime#C5Anvvv1r">	<skos:prefLabel xml:lang="en">C5Anvvv1r</skos:prefLabel>	<skos:definition>The C5Anvvv1r magnetostratographic time period started 12.207 million years (Ma) before present (BP) and ended 12.116 Ma BP.</skos:definition>	<rdfs:seeAlso rdf:resource="http://kos.gbif.org/wiki/geotime:C5Anvvv1r"/>	<dcterms:created>2011-01-11</dcterms:created>	<dcterms:modified>2012-08-03</dcterms:modified>	<geotime:start>12.207</geotime:start>	<geotime:end>12.116</geotime:end>	<geotime:polarity>R</geotime:polarity>	<geotime:regionName></geotime:regionName>	<dcterms:hasVersion rdf:resource="&history;20120803/geotime#C5Anvvv1r"/>	<rdfs:isDefinedBy rdf:resource="&geotime;"/>	<skos:inScheme rdf:resource="&geotime;"/>	<vann:termGroup rdf:resource="&geotime;Magnetostratigraphic"/>	<vs:term_status>unstable</vs:term_status>	</skos:Concept>
<skos:Concept rdf:about="http://rs.gbif.org/terms/geotime#C5Anvvv2n">	<skos:prefLabel xml:lang="en">C5Anvvv2n</skos:prefLabel>	<skos:definition>The C5Anvvv2n magnetostratographic time period started 12.415 million years (Ma) before present (BP) and ended 12.207 Ma BP.</skos:definition>	<rdfs:seeAlso rdf:resource="http://kos.gbif.org/wiki/geotime:C5Anvvv2n"/>	<dcterms:created>2011-01-11</dcterms:created>	<dcterms:modified>2012-08-03</dcterms:modified>	<geotime:start>12.415</geotime:start>	<geotime:end>12.207</geotime:end>	<geotime:polarity>N</geotime:polarity>	<geotime:regionName></geotime:regionName>	<dcterms:hasVersion rdf:resource="&history;20120803/geotime#C5Anvvv2n"/>	<rdfs:isDefinedBy rdf:resource="&geotime;"/>	<skos:inScheme rdf:resource="&geotime;"/>	<vann:termGroup rdf:resource="&geotime;Magnetostratigraphic"/>	<vs:term_status>unstable</vs:term_status>	</skos:Concept>
<skos:Concept rdf:about="http://rs.gbif.org/terms/geotime#C5Arvvv1r">	<skos:prefLabel xml:lang="en">C5Arvvv1r</skos:prefLabel>	<skos:definition>The C5Arvvv1r magnetostratographic time period started 12.73 million years (Ma) before present (BP) and ended 12.415 Ma BP.</skos:definition>	<rdfs:seeAlso rdf:resource="http://kos.gbif.org/wiki/geotime:C5Arvvv1r"/>	<dcterms:created>2011-01-11</dcterms:created>	<dcterms:modified>2012-08-03</dcterms:modified>	<geotime:start>12.73</geotime:start>	<geotime:end>12.415</geotime:end>	<geotime:polarity>R</geotime:polarity>	<geotime:regionName></geotime:regionName>	<dcterms:hasVersion rdf:resource="&history;20120803/geotime#C5Arvvv1r"/>	<rdfs:isDefinedBy rdf:resource="&geotime;"/>	<skos:inScheme rdf:resource="&geotime;"/>	<vann:termGroup rdf:resource="&geotime;Magnetostratigraphic"/>	<vs:term_status>unstable</vs:term_status>	</skos:Concept>
<skos:Concept rdf:about="http://rs.gbif.org/terms/geotime#C5Arvvv1n">	<skos:prefLabel xml:lang="en">C5Arvvv1n</skos:prefLabel>	<skos:definition>The C5Arvvv1n magnetostratographic time period started 12.765 million years (Ma) before present (BP) and ended 12.73 Ma BP.</skos:definition>	<rdfs:seeAlso rdf:resource="http://kos.gbif.org/wiki/geotime:C5Arvvv1n"/>	<dcterms:created>2011-01-11</dcterms:created>	<dcterms:modified>2012-08-03</dcterms:modified>	<geotime:start>12.765</geotime:start>	<geotime:end>12.73</geotime:end>	<geotime:polarity>N</geotime:polarity>	<geotime:regionName></geotime:regionName>	<dcterms:hasVersion rdf:resource="&history;20120803/geotime#C5Arvvv1n"/>	<rdfs:isDefinedBy rdf:resource="&geotime;"/>	<skos:inScheme rdf:resource="&geotime;"/>	<vann:termGroup rdf:resource="&geotime;Magnetostratigraphic"/>	<vs:term_status>unstable</vs:term_status>	</skos:Concept>
<skos:Concept rdf:about="http://rs.gbif.org/terms/geotime#C5Arvvv2r">	<skos:prefLabel xml:lang="en">C5Arvvv2r</skos:prefLabel>	<skos:definition>The C5Arvvv2r magnetostratographic time period started 12.82 million years (Ma) before present (BP) and ended 12.765 Ma BP.</skos:definition>	<rdfs:seeAlso rdf:resource="http://kos.gbif.org/wiki/geotime:C5Arvvv2r"/>	<dcterms:created>2011-01-11</dcterms:created>	<dcterms:modified>2012-08-03</dcterms:modified>	<geotime:start>12.82</geotime:start>	<geotime:end>12.765</geotime:end>	<geotime:polarity>R</geotime:polarity>	<geotime:regionName></geotime:regionName>	<dcterms:hasVersion rdf:resource="&history;20120803/geotime#C5Arvvv2r"/>	<rdfs:isDefinedBy rdf:resource="&geotime;"/>	<skos:inScheme rdf:resource="&geotime;"/>	<vann:termGroup rdf:resource="&geotime;Magnetostratigraphic"/>	<vs:term_status>unstable</vs:term_status>	</skos:Concept>
<skos:Concept rdf:about="http://rs.gbif.org/terms/geotime#C5Arvvv2n">	<skos:prefLabel xml:lang="en">C5Arvvv2n</skos:prefLabel>	<skos:definition>The C5Arvvv2n magnetostratographic time period started 12.878 million years (Ma) before present (BP) and ended 12.82 Ma BP.</skos:definition>	<rdfs:seeAlso rdf:resource="http://kos.gbif.org/wiki/geotime:C5Arvvv2n"/>	<dcterms:created>2011-01-11</dcterms:created>	<dcterms:modified>2012-08-03</dcterms:modified>	<geotime:start>12.878</geotime:start>	<geotime:end>12.82</geotime:end>	<geotime:polarity>N</geotime:polarity>	<geotime:regionName></geotime:regionName>	<dcterms:hasVersion rdf:resource="&history;20120803/geotime#C5Arvvv2n"/>	<rdfs:isDefinedBy rdf:resource="&geotime;"/>	<skos:inScheme rdf:resource="&geotime;"/>	<vann:termGroup rdf:resource="&geotime;Magnetostratigraphic"/>	<vs:term_status>unstable</vs:term_status>	</skos:Concept>
<skos:Concept rdf:about="http://rs.gbif.org/terms/geotime#C5A">	<skos:prefLabel xml:lang="en">C5A</skos:prefLabel>	<skos:definition>The C5A magnetostratographic time period started 13.015 million years (Ma) before present (BP) and ended 12.014 Ma BP.</skos:definition>	<rdfs:seeAlso rdf:resource="http://kos.gbif.org/wiki/geotime:C5A"/>	<dcterms:created>2011-01-11</dcterms:created>	<dcterms:modified>2012-08-03</dcterms:modified>	<geotime:start>13.015</geotime:start>	<geotime:end>12.014</geotime:end>	<geotime:polarity></geotime:polarity>	<geotime:regionName></geotime:regionName>	<dcterms:hasVersion rdf:resource="&history;20120803/geotime#C5A"/>	<rdfs:isDefinedBy rdf:resource="&geotime;"/>	<skos:inScheme rdf:resource="&geotime;"/>	<vann:termGroup rdf:resource="&geotime;Magnetostratigraphic"/>	<vs:term_status>unstable</vs:term_status>	</skos:Concept>
<skos:Concept rdf:about="http://rs.gbif.org/terms/geotime#C5Arvvv3r">	<skos:prefLabel xml:lang="en">C5Arvvv3r</skos:prefLabel>	<skos:definition>The C5Arvvv3r magnetostratographic time period started 13.015 million years (Ma) before present (BP) and ended 12.878 Ma BP.</skos:definition>	<rdfs:seeAlso rdf:resource="http://kos.gbif.org/wiki/geotime:C5Arvvv3r"/>	<dcterms:created>2011-01-11</dcterms:created>	<dcterms:modified>2012-08-03</dcterms:modified>	<geotime:start>13.015</geotime:start>	<geotime:end>12.878</geotime:end>	<geotime:polarity>R</geotime:polarity>	<geotime:regionName></geotime:regionName>	<dcterms:hasVersion rdf:resource="&history;20120803/geotime#C5Arvvv3r"/>	<rdfs:isDefinedBy rdf:resource="&geotime;"/>	<skos:inScheme rdf:resource="&geotime;"/>	<vann:termGroup rdf:resource="&geotime;Magnetostratigraphic"/>	<vs:term_status>unstable</vs:term_status>	</skos:Concept>
<skos:Concept rdf:about="http://rs.gbif.org/terms/geotime#C5AAn">	<skos:prefLabel xml:lang="en">C5AAn</skos:prefLabel>	<skos:definition>The C5AAn magnetostratographic time period started 13.183 million years (Ma) before present (BP) and ended 13.015 Ma BP.</skos:definition>	<rdfs:seeAlso rdf:resource="http://kos.gbif.org/wiki/geotime:C5AAn"/>	<dcterms:created>2011-01-11</dcterms:created>	<dcterms:modified>2012-08-03</dcterms:modified>	<geotime:start>13.183</geotime:start>	<geotime:end>13.015</geotime:end>	<geotime:polarity>N</geotime:polarity>	<geotime:regionName></geotime:regionName>	<dcterms:hasVersion rdf:resource="&history;20120803/geotime#C5AAn"/>	<rdfs:isDefinedBy rdf:resource="&geotime;"/>	<skos:inScheme rdf:resource="&geotime;"/>	<vann:termGroup rdf:resource="&geotime;Magnetostratigraphic"/>	<vs:term_status>unstable</vs:term_status>	</skos:Concept>
<skos:Concept rdf:about="http://rs.gbif.org/terms/geotime#C5AA">	<skos:prefLabel xml:lang="en">C5AA</skos:prefLabel>	<skos:definition>The C5AA magnetostratographic time period started 13.369 million years (Ma) before present (BP) and ended 13.015 Ma BP.</skos:definition>	<rdfs:seeAlso rdf:resource="http://kos.gbif.org/wiki/geotime:C5AA"/>	<dcterms:created>2011-01-11</dcterms:created>	<dcterms:modified>2012-08-03</dcterms:modified>	<geotime:start>13.369</geotime:start>	<geotime:end>13.015</geotime:end>	<geotime:polarity></geotime:polarity>	<geotime:regionName></geotime:regionName>	<dcterms:hasVersion rdf:resource="&history;20120803/geotime#C5AA"/>	<rdfs:isDefinedBy rdf:resource="&geotime;"/>	<skos:inScheme rdf:resource="&geotime;"/>	<vann:termGroup rdf:resource="&geotime;Magnetostratigraphic"/>	<vs:term_status>unstable</vs:term_status>	</skos:Concept>
<skos:Concept rdf:about="http://rs.gbif.org/terms/geotime#C5AAr">	<skos:prefLabel xml:lang="en">C5AAr</skos:prefLabel>	<skos:definition>The C5AAr magnetostratographic time period started 13.369 million years (Ma) before present (BP) and ended 13.183 Ma BP.</skos:definition>	<rdfs:seeAlso rdf:resource="http://kos.gbif.org/wiki/geotime:C5AAr"/>	<dcterms:created>2011-01-11</dcterms:created>	<dcterms:modified>2012-08-03</dcterms:modified>	<geotime:start>13.369</geotime:start>	<geotime:end>13.183</geotime:end>	<geotime:polarity>R</geotime:polarity>	<geotime:regionName></geotime:regionName>	<dcterms:hasVersion rdf:resource="&history;20120803/geotime#C5AAr"/>	<rdfs:isDefinedBy rdf:resource="&geotime;"/>	<skos:inScheme rdf:resource="&geotime;"/>	<vann:termGroup rdf:resource="&geotime;Magnetostratigraphic"/>	<vs:term_status>unstable</vs:term_status>	</skos:Concept>
<skos:Concept rdf:about="http://rs.gbif.org/terms/geotime#C5ABn">	<skos:prefLabel xml:lang="en">C5ABn</skos:prefLabel>	<skos:definition>The C5ABn magnetostratographic time period started 13.605 million years (Ma) before present (BP) and ended 13.369 Ma BP.</skos:definition>	<rdfs:seeAlso rdf:resource="http://kos.gbif.org/wiki/geotime:C5ABn"/>	<dcterms:created>2011-01-11</dcterms:created>	<dcterms:modified>2012-08-03</dcterms:modified>	<geotime:start>13.605</geotime:start>	<geotime:end>13.369</geotime:end>	<geotime:polarity>N</geotime:polarity>	<geotime:regionName></geotime:regionName>	<dcterms:hasVersion rdf:resource="&history;20120803/geotime#C5ABn"/>	<rdfs:isDefinedBy rdf:resource="&geotime;"/>	<skos:inScheme rdf:resource="&geotime;"/>	<vann:termGroup rdf:resource="&geotime;Magnetostratigraphic"/>	<vs:term_status>unstable</vs:term_status>	</skos:Concept>
<skos:Concept rdf:about="http://rs.gbif.org/terms/geotime#C5AB">	<skos:prefLabel xml:lang="en">C5AB</skos:prefLabel>	<skos:definition>The C5AB magnetostratographic time period started 13.734 million years (Ma) before present (BP) and ended 13.369 Ma BP.</skos:definition>	<rdfs:seeAlso rdf:resource="http://kos.gbif.org/wiki/geotime:C5AB"/>	<dcterms:created>2011-01-11</dcterms:created>	<dcterms:modified>2012-08-03</dcterms:modified>	<geotime:start>13.734</geotime:start>	<geotime:end>13.369</geotime:end>	<geotime:polarity></geotime:polarity>	<geotime:regionName></geotime:regionName>	<dcterms:hasVersion rdf:resource="&history;20120803/geotime#C5AB"/>	<rdfs:isDefinedBy rdf:resource="&geotime;"/>	<skos:inScheme rdf:resource="&geotime;"/>	<vann:termGroup rdf:resource="&geotime;Magnetostratigraphic"/>	<vs:term_status>unstable</vs:term_status>	</skos:Concept>
<skos:Concept rdf:about="http://rs.gbif.org/terms/geotime#C5ABr">	<skos:prefLabel xml:lang="en">C5ABr</skos:prefLabel>	<skos:definition>The C5ABr magnetostratographic time period started 13.734 million years (Ma) before present (BP) and ended 13.605 Ma BP.</skos:definition>	<rdfs:seeAlso rdf:resource="http://kos.gbif.org/wiki/geotime:C5ABr"/>	<dcterms:created>2011-01-11</dcterms:created>	<dcterms:modified>2012-08-03</dcterms:modified>	<geotime:start>13.734</geotime:start>	<geotime:end>13.605</geotime:end>	<geotime:polarity>R</geotime:polarity>	<geotime:regionName></geotime:regionName>	<dcterms:hasVersion rdf:resource="&history;20120803/geotime#C5ABr"/>	<rdfs:isDefinedBy rdf:resource="&geotime;"/>	<skos:inScheme rdf:resource="&geotime;"/>	<vann:termGroup rdf:resource="&geotime;Magnetostratigraphic"/>	<vs:term_status>unstable</vs:term_status>	</skos:Concept>
<skos:Concept rdf:about="http://rs.gbif.org/terms/geotime#C5ACn">	<skos:prefLabel xml:lang="en">C5ACn</skos:prefLabel>	<skos:definition>The C5ACn magnetostratographic time period started 14.095 million years (Ma) before present (BP) and ended 13.734 Ma BP.</skos:definition>	<rdfs:seeAlso rdf:resource="http://kos.gbif.org/wiki/geotime:C5ACn"/>	<dcterms:created>2011-01-11</dcterms:created>	<dcterms:modified>2012-08-03</dcterms:modified>	<geotime:start>14.095</geotime:start>	<geotime:end>13.734</geotime:end>	<geotime:polarity>N</geotime:polarity>	<geotime:regionName></geotime:regionName>	<dcterms:hasVersion rdf:resource="&history;20120803/geotime#C5ACn"/>	<rdfs:isDefinedBy rdf:resource="&geotime;"/>	<skos:inScheme rdf:resource="&geotime;"/>	<vann:termGroup rdf:resource="&geotime;Magnetostratigraphic"/>	<vs:term_status>unstable</vs:term_status>	</skos:Concept>
<skos:Concept rdf:about="http://rs.gbif.org/terms/geotime#C5AC">	<skos:prefLabel xml:lang="en">C5AC</skos:prefLabel>	<skos:definition>The C5AC magnetostratographic time period started 14.194 million years (Ma) before present (BP) and ended 13.734 Ma BP.</skos:definition>	<rdfs:seeAlso rdf:resource="http://kos.gbif.org/wiki/geotime:C5AC"/>	<dcterms:created>2011-01-11</dcterms:created>	<dcterms:modified>2012-08-03</dcterms:modified>	<geotime:start>14.194</geotime:start>	<geotime:end>13.734</geotime:end>	<geotime:polarity></geotime:polarity>	<geotime:regionName></geotime:regionName>	<dcterms:hasVersion rdf:resource="&history;20120803/geotime#C5AC"/>	<rdfs:isDefinedBy rdf:resource="&geotime;"/>	<skos:inScheme rdf:resource="&geotime;"/>	<vann:termGroup rdf:resource="&geotime;Magnetostratigraphic"/>	<vs:term_status>unstable</vs:term_status>	</skos:Concept>
<skos:Concept rdf:about="http://rs.gbif.org/terms/geotime#C5ACr">	<skos:prefLabel xml:lang="en">C5ACr</skos:prefLabel>	<skos:definition>The C5ACr magnetostratographic time period started 14.194 million years (Ma) before present (BP) and ended 14.095 Ma BP.</skos:definition>	<rdfs:seeAlso rdf:resource="http://kos.gbif.org/wiki/geotime:C5ACr"/>	<dcterms:created>2011-01-11</dcterms:created>	<dcterms:modified>2012-08-03</dcterms:modified>	<geotime:start>14.194</geotime:start>	<geotime:end>14.095</geotime:end>	<geotime:polarity>R</geotime:polarity>	<geotime:regionName></geotime:regionName>	<dcterms:hasVersion rdf:resource="&history;20120803/geotime#C5ACr"/>	<rdfs:isDefinedBy rdf:resource="&geotime;"/>	<skos:inScheme rdf:resource="&geotime;"/>	<vann:termGroup rdf:resource="&geotime;Magnetostratigraphic"/>	<vs:term_status>unstable</vs:term_status>	</skos:Concept>
<skos:Concept rdf:about="http://rs.gbif.org/terms/geotime#C5ADn">	<skos:prefLabel xml:lang="en">C5ADn</skos:prefLabel>	<skos:definition>The C5ADn magnetostratographic time period started 14.581 million years (Ma) before present (BP) and ended 14.194 Ma BP.</skos:definition>	<rdfs:seeAlso rdf:resource="http://kos.gbif.org/wiki/geotime:C5ADn"/>	<dcterms:created>2011-01-11</dcterms:created>	<dcterms:modified>2012-08-03</dcterms:modified>	<geotime:start>14.581</geotime:start>	<geotime:end>14.194</geotime:end>	<geotime:polarity>N</geotime:polarity>	<geotime:regionName></geotime:regionName>	<dcterms:hasVersion rdf:resource="&history;20120803/geotime#C5ADn"/>	<rdfs:isDefinedBy rdf:resource="&geotime;"/>	<skos:inScheme rdf:resource="&geotime;"/>	<vann:termGroup rdf:resource="&geotime;Magnetostratigraphic"/>	<vs:term_status>unstable</vs:term_status>	</skos:Concept>
<skos:Concept rdf:about="http://rs.gbif.org/terms/geotime#C5AD">	<skos:prefLabel xml:lang="en">C5AD</skos:prefLabel>	<skos:definition>The C5AD magnetostratographic time period started 14.784 million years (Ma) before present (BP) and ended 14.194 Ma BP.</skos:definition>	<rdfs:seeAlso rdf:resource="http://kos.gbif.org/wiki/geotime:C5AD"/>	<dcterms:created>2011-01-11</dcterms:created>	<dcterms:modified>2012-08-03</dcterms:modified>	<geotime:start>14.784</geotime:start>	<geotime:end>14.194</geotime:end>	<geotime:polarity></geotime:polarity>	<geotime:regionName></geotime:regionName>	<dcterms:hasVersion rdf:resource="&history;20120803/geotime#C5AD"/>	<rdfs:isDefinedBy rdf:resource="&geotime;"/>	<skos:inScheme rdf:resource="&geotime;"/>	<vann:termGroup rdf:resource="&geotime;Magnetostratigraphic"/>	<vs:term_status>unstable</vs:term_status>	</skos:Concept>
<skos:Concept rdf:about="http://rs.gbif.org/terms/geotime#C5ADr">	<skos:prefLabel xml:lang="en">C5ADr</skos:prefLabel>	<skos:definition>The C5ADr magnetostratographic time period started 14.784 million years (Ma) before present (BP) and ended 14.581 Ma BP.</skos:definition>	<rdfs:seeAlso rdf:resource="http://kos.gbif.org/wiki/geotime:C5ADr"/>	<dcterms:created>2011-01-11</dcterms:created>	<dcterms:modified>2012-08-03</dcterms:modified>	<geotime:start>14.784</geotime:start>	<geotime:end>14.581</geotime:end>	<geotime:polarity>R</geotime:polarity>	<geotime:regionName></geotime:regionName>	<dcterms:hasVersion rdf:resource="&history;20120803/geotime#C5ADr"/>	<rdfs:isDefinedBy rdf:resource="&geotime;"/>	<skos:inScheme rdf:resource="&geotime;"/>	<vann:termGroup rdf:resource="&geotime;Magnetostratigraphic"/>	<vs:term_status>unstable</vs:term_status>	</skos:Concept>
<skos:Concept rdf:about="http://rs.gbif.org/terms/geotime#C5Bnvvv1n">	<skos:prefLabel xml:lang="en">C5Bnvvv1n</skos:prefLabel>	<skos:definition>The C5Bnvvv1n magnetostratographic time period started 14.877 million years (Ma) before present (BP) and ended 14.784 Ma BP.</skos:definition>	<rdfs:seeAlso rdf:resource="http://kos.gbif.org/wiki/geotime:C5Bnvvv1n"/>	<dcterms:created>2011-01-11</dcterms:created>	<dcterms:modified>2012-08-03</dcterms:modified>	<geotime:start>14.877</geotime:start>	<geotime:end>14.784</geotime:end>	<geotime:polarity>N</geotime:polarity>	<geotime:regionName></geotime:regionName>	<dcterms:hasVersion rdf:resource="&history;20120803/geotime#C5Bnvvv1n"/>	<rdfs:isDefinedBy rdf:resource="&geotime;"/>	<skos:inScheme rdf:resource="&geotime;"/>	<vann:termGroup rdf:resource="&geotime;Magnetostratigraphic"/>	<vs:term_status>unstable</vs:term_status>	</skos:Concept>
<skos:Concept rdf:about="http://rs.gbif.org/terms/geotime#C5Bnvvv1r">	<skos:prefLabel xml:lang="en">C5Bnvvv1r</skos:prefLabel>	<skos:definition>The C5Bnvvv1r magnetostratographic time period started 15.032 million years (Ma) before present (BP) and ended 14.877 Ma BP.</skos:definition>	<rdfs:seeAlso rdf:resource="http://kos.gbif.org/wiki/geotime:C5Bnvvv1r"/>	<dcterms:created>2011-01-11</dcterms:created>	<dcterms:modified>2012-08-03</dcterms:modified>	<geotime:start>15.032</geotime:start>	<geotime:end>14.877</geotime:end>	<geotime:polarity>R</geotime:polarity>	<geotime:regionName></geotime:regionName>	<dcterms:hasVersion rdf:resource="&history;20120803/geotime#C5Bnvvv1r"/>	<rdfs:isDefinedBy rdf:resource="&geotime;"/>	<skos:inScheme rdf:resource="&geotime;"/>	<vann:termGroup rdf:resource="&geotime;Magnetostratigraphic"/>	<vs:term_status>unstable</vs:term_status>	</skos:Concept>
<skos:Concept rdf:about="http://rs.gbif.org/terms/geotime#C5Bnvvv2n">	<skos:prefLabel xml:lang="en">C5Bnvvv2n</skos:prefLabel>	<skos:definition>The C5Bnvvv2n magnetostratographic time period started 15.16 million years (Ma) before present (BP) and ended 15.032 Ma BP.</skos:definition>	<rdfs:seeAlso rdf:resource="http://kos.gbif.org/wiki/geotime:C5Bnvvv2n"/>	<dcterms:created>2011-01-11</dcterms:created>	<dcterms:modified>2012-08-03</dcterms:modified>	<geotime:start>15.16</geotime:start>	<geotime:end>15.032</geotime:end>	<geotime:polarity>N</geotime:polarity>	<geotime:regionName></geotime:regionName>	<dcterms:hasVersion rdf:resource="&history;20120803/geotime#C5Bnvvv2n"/>	<rdfs:isDefinedBy rdf:resource="&geotime;"/>	<skos:inScheme rdf:resource="&geotime;"/>	<vann:termGroup rdf:resource="&geotime;Magnetostratigraphic"/>	<vs:term_status>unstable</vs:term_status>	</skos:Concept>
<skos:Concept rdf:about="http://rs.gbif.org/terms/geotime#C5B">	<skos:prefLabel xml:lang="en">C5B</skos:prefLabel>	<skos:definition>The C5B magnetostratographic time period started 15.974 million years (Ma) before present (BP) and ended 14.784 Ma BP.</skos:definition>	<rdfs:seeAlso rdf:resource="http://kos.gbif.org/wiki/geotime:C5B"/>	<dcterms:created>2011-01-11</dcterms:created>	<dcterms:modified>2012-08-03</dcterms:modified>	<geotime:start>15.974</geotime:start>	<geotime:end>14.784</geotime:end>	<geotime:polarity></geotime:polarity>	<geotime:regionName></geotime:regionName>	<dcterms:hasVersion rdf:resource="&history;20120803/geotime#C5B"/>	<rdfs:isDefinedBy rdf:resource="&geotime;"/>	<skos:inScheme rdf:resource="&geotime;"/>	<vann:termGroup rdf:resource="&geotime;Magnetostratigraphic"/>	<vs:term_status>unstable</vs:term_status>	</skos:Concept>
<skos:Concept rdf:about="http://rs.gbif.org/terms/geotime#C5Br">	<skos:prefLabel xml:lang="en">C5Br</skos:prefLabel>	<skos:definition>The C5Br magnetostratographic time period started 15.974 million years (Ma) before present (BP) and ended 15.16 Ma BP.</skos:definition>	<rdfs:seeAlso rdf:resource="http://kos.gbif.org/wiki/geotime:C5Br"/>	<dcterms:created>2011-01-11</dcterms:created>	<dcterms:modified>2012-08-03</dcterms:modified>	<geotime:start>15.974</geotime:start>	<geotime:end>15.16</geotime:end>	<geotime:polarity>R</geotime:polarity>	<geotime:regionName></geotime:regionName>	<dcterms:hasVersion rdf:resource="&history;20120803/geotime#C5Br"/>	<rdfs:isDefinedBy rdf:resource="&geotime;"/>	<skos:inScheme rdf:resource="&geotime;"/>	<vann:termGroup rdf:resource="&geotime;Magnetostratigraphic"/>	<vs:term_status>unstable</vs:term_status>	</skos:Concept>
<skos:Concept rdf:about="http://rs.gbif.org/terms/geotime#C5Cnvvv1n">	<skos:prefLabel xml:lang="en">C5Cnvvv1n</skos:prefLabel>	<skos:definition>The C5Cnvvv1n magnetostratographic time period started 16.268 million years (Ma) before present (BP) and ended 15.974 Ma BP.</skos:definition>	<rdfs:seeAlso rdf:resource="http://kos.gbif.org/wiki/geotime:C5Cnvvv1n"/>	<dcterms:created>2011-01-11</dcterms:created>	<dcterms:modified>2012-08-03</dcterms:modified>	<geotime:start>16.268</geotime:start>	<geotime:end>15.974</geotime:end>	<geotime:polarity>N</geotime:polarity>	<geotime:regionName></geotime:regionName>	<dcterms:hasVersion rdf:resource="&history;20120803/geotime#C5Cnvvv1n"/>	<rdfs:isDefinedBy rdf:resource="&geotime;"/>	<skos:inScheme rdf:resource="&geotime;"/>	<vann:termGroup rdf:resource="&geotime;Magnetostratigraphic"/>	<vs:term_status>unstable</vs:term_status>	</skos:Concept>
<skos:Concept rdf:about="http://rs.gbif.org/terms/geotime#C5Cnvvv1r">	<skos:prefLabel xml:lang="en">C5Cnvvv1r</skos:prefLabel>	<skos:definition>The C5Cnvvv1r magnetostratographic time period started 16.303 million years (Ma) before present (BP) and ended 16.268 Ma BP.</skos:definition>	<rdfs:seeAlso rdf:resource="http://kos.gbif.org/wiki/geotime:C5Cnvvv1r"/>	<dcterms:created>2011-01-11</dcterms:created>	<dcterms:modified>2012-08-03</dcterms:modified>	<geotime:start>16.303</geotime:start>	<geotime:end>16.268</geotime:end>	<geotime:polarity>R</geotime:polarity>	<geotime:regionName></geotime:regionName>	<dcterms:hasVersion rdf:resource="&history;20120803/geotime#C5Cnvvv1r"/>	<rdfs:isDefinedBy rdf:resource="&geotime;"/>	<skos:inScheme rdf:resource="&geotime;"/>	<vann:termGroup rdf:resource="&geotime;Magnetostratigraphic"/>	<vs:term_status>unstable</vs:term_status>	</skos:Concept>
<skos:Concept rdf:about="http://rs.gbif.org/terms/geotime#C5Cnvvv2n">	<skos:prefLabel xml:lang="en">C5Cnvvv2n</skos:prefLabel>	<skos:definition>The C5Cnvvv2n magnetostratographic time period started 16.472 million years (Ma) before present (BP) and ended 16.303 Ma BP.</skos:definition>	<rdfs:seeAlso rdf:resource="http://kos.gbif.org/wiki/geotime:C5Cnvvv2n"/>	<dcterms:created>2011-01-11</dcterms:created>	<dcterms:modified>2012-08-03</dcterms:modified>	<geotime:start>16.472</geotime:start>	<geotime:end>16.303</geotime:end>	<geotime:polarity>N</geotime:polarity>	<geotime:regionName></geotime:regionName>	<dcterms:hasVersion rdf:resource="&history;20120803/geotime#C5Cnvvv2n"/>	<rdfs:isDefinedBy rdf:resource="&geotime;"/>	<skos:inScheme rdf:resource="&geotime;"/>	<vann:termGroup rdf:resource="&geotime;Magnetostratigraphic"/>	<vs:term_status>unstable</vs:term_status>	</skos:Concept>
<skos:Concept rdf:about="http://rs.gbif.org/terms/geotime#C5Cnvvv2r">	<skos:prefLabel xml:lang="en">C5Cnvvv2r</skos:prefLabel>	<skos:definition>The C5Cnvvv2r magnetostratographic time period started 16.543 million years (Ma) before present (BP) and ended 16.472 Ma BP.</skos:definition>	<rdfs:seeAlso rdf:resource="http://kos.gbif.org/wiki/geotime:C5Cnvvv2r"/>	<dcterms:created>2011-01-11</dcterms:created>	<dcterms:modified>2012-08-03</dcterms:modified>	<geotime:start>16.543</geotime:start>	<geotime:end>16.472</geotime:end>	<geotime:polarity>R</geotime:polarity>	<geotime:regionName></geotime:regionName>	<dcterms:hasVersion rdf:resource="&history;20120803/geotime#C5Cnvvv2r"/>	<rdfs:isDefinedBy rdf:resource="&geotime;"/>	<skos:inScheme rdf:resource="&geotime;"/>	<vann:termGroup rdf:resource="&geotime;Magnetostratigraphic"/>	<vs:term_status>unstable</vs:term_status>	</skos:Concept>
<skos:Concept rdf:about="http://rs.gbif.org/terms/geotime#C5Cnvvv3n">	<skos:prefLabel xml:lang="en">C5Cnvvv3n</skos:prefLabel>	<skos:definition>The C5Cnvvv3n magnetostratographic time period started 16.721 million years (Ma) before present (BP) and ended 16.543 Ma BP.</skos:definition>	<rdfs:seeAlso rdf:resource="http://kos.gbif.org/wiki/geotime:C5Cnvvv3n"/>	<dcterms:created>2011-01-11</dcterms:created>	<dcterms:modified>2012-08-03</dcterms:modified>	<geotime:start>16.721</geotime:start>	<geotime:end>16.543</geotime:end>	<geotime:polarity>N</geotime:polarity>	<geotime:regionName></geotime:regionName>	<dcterms:hasVersion rdf:resource="&history;20120803/geotime#C5Cnvvv3n"/>	<rdfs:isDefinedBy rdf:resource="&geotime;"/>	<skos:inScheme rdf:resource="&geotime;"/>	<vann:termGroup rdf:resource="&geotime;Magnetostratigraphic"/>	<vs:term_status>unstable</vs:term_status>	</skos:Concept>
<skos:Concept rdf:about="http://rs.gbif.org/terms/geotime#C5C">	<skos:prefLabel xml:lang="en">C5C</skos:prefLabel>	<skos:definition>The C5C magnetostratographic time period started 17.235 million years (Ma) before present (BP) and ended 15.974 Ma BP.</skos:definition>	<rdfs:seeAlso rdf:resource="http://kos.gbif.org/wiki/geotime:C5C"/>	<dcterms:created>2011-01-11</dcterms:created>	<dcterms:modified>2012-08-03</dcterms:modified>	<geotime:start>17.235</geotime:start>	<geotime:end>15.974</geotime:end>	<geotime:polarity></geotime:polarity>	<geotime:regionName></geotime:regionName>	<dcterms:hasVersion rdf:resource="&history;20120803/geotime#C5C"/>	<rdfs:isDefinedBy rdf:resource="&geotime;"/>	<skos:inScheme rdf:resource="&geotime;"/>	<vann:termGroup rdf:resource="&geotime;Magnetostratigraphic"/>	<vs:term_status>unstable</vs:term_status>	</skos:Concept>
<skos:Concept rdf:about="http://rs.gbif.org/terms/geotime#C5Cr">	<skos:prefLabel xml:lang="en">C5Cr</skos:prefLabel>	<skos:definition>The C5Cr magnetostratographic time period started 17.235 million years (Ma) before present (BP) and ended 16.721 Ma BP.</skos:definition>	<rdfs:seeAlso rdf:resource="http://kos.gbif.org/wiki/geotime:C5Cr"/>	<dcterms:created>2011-01-11</dcterms:created>	<dcterms:modified>2012-08-03</dcterms:modified>	<geotime:start>17.235</geotime:start>	<geotime:end>16.721</geotime:end>	<geotime:polarity>R</geotime:polarity>	<geotime:regionName></geotime:regionName>	<dcterms:hasVersion rdf:resource="&history;20120803/geotime#C5Cr"/>	<rdfs:isDefinedBy rdf:resource="&geotime;"/>	<skos:inScheme rdf:resource="&geotime;"/>	<vann:termGroup rdf:resource="&geotime;Magnetostratigraphic"/>	<vs:term_status>unstable</vs:term_status>	</skos:Concept>
<skos:Concept rdf:about="http://rs.gbif.org/terms/geotime#C5Dn">	<skos:prefLabel xml:lang="en">C5Dn</skos:prefLabel>	<skos:definition>The C5Dn magnetostratographic time period started 17.533 million years (Ma) before present (BP) and ended 17.235 Ma BP.</skos:definition>	<rdfs:seeAlso rdf:resource="http://kos.gbif.org/wiki/geotime:C5Dn"/>	<dcterms:created>2011-01-11</dcterms:created>	<dcterms:modified>2012-08-03</dcterms:modified>	<geotime:start>17.533</geotime:start>	<geotime:end>17.235</geotime:end>	<geotime:polarity>N</geotime:polarity>	<geotime:regionName></geotime:regionName>	<dcterms:hasVersion rdf:resource="&history;20120803/geotime#C5Dn"/>	<rdfs:isDefinedBy rdf:resource="&geotime;"/>	<skos:inScheme rdf:resource="&geotime;"/>	<vann:termGroup rdf:resource="&geotime;Magnetostratigraphic"/>	<vs:term_status>unstable</vs:term_status>	</skos:Concept>
<skos:Concept rdf:about="http://rs.gbif.org/terms/geotime#C5Drvvv1r">	<skos:prefLabel xml:lang="en">C5Drvvv1r</skos:prefLabel>	<skos:definition>The C5Drvvv1r magnetostratographic time period started 17.717 million years (Ma) before present (BP) and ended 17.533 Ma BP.</skos:definition>	<rdfs:seeAlso rdf:resource="http://kos.gbif.org/wiki/geotime:C5Drvvv1r"/>	<dcterms:created>2011-01-11</dcterms:created>	<dcterms:modified>2012-08-03</dcterms:modified>	<geotime:start>17.717</geotime:start>	<geotime:end>17.533</geotime:end>	<geotime:polarity>R</geotime:polarity>	<geotime:regionName></geotime:regionName>	<dcterms:hasVersion rdf:resource="&history;20120803/geotime#C5Drvvv1r"/>	<rdfs:isDefinedBy rdf:resource="&geotime;"/>	<skos:inScheme rdf:resource="&geotime;"/>	<vann:termGroup rdf:resource="&geotime;Magnetostratigraphic"/>	<vs:term_status>unstable</vs:term_status>	</skos:Concept>
<skos:Concept rdf:about="http://rs.gbif.org/terms/geotime#C5Drvvv1n">	<skos:prefLabel xml:lang="en">C5Drvvv1n</skos:prefLabel>	<skos:definition>The C5Drvvv1n magnetostratographic time period started 17.74 million years (Ma) before present (BP) and ended 17.717 Ma BP.</skos:definition>	<rdfs:seeAlso rdf:resource="http://kos.gbif.org/wiki/geotime:C5Drvvv1n"/>	<dcterms:created>2011-01-11</dcterms:created>	<dcterms:modified>2012-08-03</dcterms:modified>	<geotime:start>17.74</geotime:start>	<geotime:end>17.717</geotime:end>	<geotime:polarity>N</geotime:polarity>	<geotime:regionName></geotime:regionName>	<dcterms:hasVersion rdf:resource="&history;20120803/geotime#C5Drvvv1n"/>	<rdfs:isDefinedBy rdf:resource="&geotime;"/>	<skos:inScheme rdf:resource="&geotime;"/>	<vann:termGroup rdf:resource="&geotime;Magnetostratigraphic"/>	<vs:term_status>unstable</vs:term_status>	</skos:Concept>
<skos:Concept rdf:about="http://rs.gbif.org/terms/geotime#C5D">	<skos:prefLabel xml:lang="en">C5D</skos:prefLabel>	<skos:definition>The C5D magnetostratographic time period started 18.056 million years (Ma) before present (BP) and ended 17.235 Ma BP.</skos:definition>	<rdfs:seeAlso rdf:resource="http://kos.gbif.org/wiki/geotime:C5D"/>	<dcterms:created>2011-01-11</dcterms:created>	<dcterms:modified>2012-08-03</dcterms:modified>	<geotime:start>18.056</geotime:start>	<geotime:end>17.235</geotime:end>	<geotime:polarity></geotime:polarity>	<geotime:regionName></geotime:regionName>	<dcterms:hasVersion rdf:resource="&history;20120803/geotime#C5D"/>	<rdfs:isDefinedBy rdf:resource="&geotime;"/>	<skos:inScheme rdf:resource="&geotime;"/>	<vann:termGroup rdf:resource="&geotime;Magnetostratigraphic"/>	<vs:term_status>unstable</vs:term_status>	</skos:Concept>
<skos:Concept rdf:about="http://rs.gbif.org/terms/geotime#C5Drvvv2r">	<skos:prefLabel xml:lang="en">C5Drvvv2r</skos:prefLabel>	<skos:definition>The C5Drvvv2r magnetostratographic time period started 18.056 million years (Ma) before present (BP) and ended 17.74 Ma BP.</skos:definition>	<rdfs:seeAlso rdf:resource="http://kos.gbif.org/wiki/geotime:C5Drvvv2r"/>	<dcterms:created>2011-01-11</dcterms:created>	<dcterms:modified>2012-08-03</dcterms:modified>	<geotime:start>18.056</geotime:start>	<geotime:end>17.74</geotime:end>	<geotime:polarity>R</geotime:polarity>	<geotime:regionName></geotime:regionName>	<dcterms:hasVersion rdf:resource="&history;20120803/geotime#C5Drvvv2r"/>	<rdfs:isDefinedBy rdf:resource="&geotime;"/>	<skos:inScheme rdf:resource="&geotime;"/>	<vann:termGroup rdf:resource="&geotime;Magnetostratigraphic"/>	<vs:term_status>unstable</vs:term_status>	</skos:Concept>
<skos:Concept rdf:about="http://rs.gbif.org/terms/geotime#C5En">	<skos:prefLabel xml:lang="en">C5En</skos:prefLabel>	<skos:definition>The C5En magnetostratographic time period started 18.524 million years (Ma) before present (BP) and ended 18.056 Ma BP.</skos:definition>	<rdfs:seeAlso rdf:resource="http://kos.gbif.org/wiki/geotime:C5En"/>	<dcterms:created>2011-01-11</dcterms:created>	<dcterms:modified>2012-08-03</dcterms:modified>	<geotime:start>18.524</geotime:start>	<geotime:end>18.056</geotime:end>	<geotime:polarity>N</geotime:polarity>	<geotime:regionName></geotime:regionName>	<dcterms:hasVersion rdf:resource="&history;20120803/geotime#C5En"/>	<rdfs:isDefinedBy rdf:resource="&geotime;"/>	<skos:inScheme rdf:resource="&geotime;"/>	<vann:termGroup rdf:resource="&geotime;Magnetostratigraphic"/>	<vs:term_status>unstable</vs:term_status>	</skos:Concept>
<skos:Concept rdf:about="http://rs.gbif.org/terms/geotime#C5Er">	<skos:prefLabel xml:lang="en">C5Er</skos:prefLabel>	<skos:definition>The C5Er magnetostratographic time period started 18.748 million years (Ma) before present (BP) and ended 18.524 Ma BP.</skos:definition>	<rdfs:seeAlso rdf:resource="http://kos.gbif.org/wiki/geotime:C5Er"/>	<dcterms:created>2011-01-11</dcterms:created>	<dcterms:modified>2012-08-03</dcterms:modified>	<geotime:start>18.748</geotime:start>	<geotime:end>18.524</geotime:end>	<geotime:polarity>R</geotime:polarity>	<geotime:regionName></geotime:regionName>	<dcterms:hasVersion rdf:resource="&history;20120803/geotime#C5Er"/>	<rdfs:isDefinedBy rdf:resource="&geotime;"/>	<skos:inScheme rdf:resource="&geotime;"/>	<vann:termGroup rdf:resource="&geotime;Magnetostratigraphic"/>	<vs:term_status>unstable</vs:term_status>	</skos:Concept>
<skos:Concept rdf:about="http://rs.gbif.org/terms/geotime#C6n">	<skos:prefLabel xml:lang="en">C6n</skos:prefLabel>	<skos:definition>The C6n magnetostratographic time period started 19.722 million years (Ma) before present (BP) and ended 18.748 Ma BP.</skos:definition>	<rdfs:seeAlso rdf:resource="http://kos.gbif.org/wiki/geotime:C6n"/>	<dcterms:created>2011-01-11</dcterms:created>	<dcterms:modified>2012-08-03</dcterms:modified>	<geotime:start>19.722</geotime:start>	<geotime:end>18.748</geotime:end>	<geotime:polarity>N</geotime:polarity>	<geotime:regionName></geotime:regionName>	<dcterms:hasVersion rdf:resource="&history;20120803/geotime#C6n"/>	<rdfs:isDefinedBy rdf:resource="&geotime;"/>	<skos:inScheme rdf:resource="&geotime;"/>	<vann:termGroup rdf:resource="&geotime;Magnetostratigraphic"/>	<vs:term_status>unstable</vs:term_status>	</skos:Concept>
<skos:Concept rdf:about="http://rs.gbif.org/terms/geotime#C2rvvv1r">	<skos:prefLabel xml:lang="en">C2rvvv1r</skos:prefLabel>	<skos:definition>The C2rvvv1r magnetostratographic time period started 2.128 million years (Ma) before present (BP) and ended 1.945 Ma BP.</skos:definition>	<rdfs:seeAlso rdf:resource="http://kos.gbif.org/wiki/geotime:C2rvvv1r"/>	<dcterms:created>2011-01-11</dcterms:created>	<dcterms:modified>2012-08-03</dcterms:modified>	<geotime:start>2.128</geotime:start>	<geotime:end>1.945</geotime:end>	<geotime:polarity>R</geotime:polarity>	<geotime:regionName></geotime:regionName>	<dcterms:hasVersion rdf:resource="&history;20120803/geotime#C2rvvv1r"/>	<rdfs:isDefinedBy rdf:resource="&geotime;"/>	<skos:inScheme rdf:resource="&geotime;"/>	<vann:termGroup rdf:resource="&geotime;Magnetostratigraphic"/>	<vs:term_status>unstable</vs:term_status>	</skos:Concept>
<skos:Concept rdf:about="http://rs.gbif.org/terms/geotime#C2rvvv1n">	<skos:prefLabel xml:lang="en">C2rvvv1n</skos:prefLabel>	<skos:definition>The C2rvvv1n magnetostratographic time period started 2.148 million years (Ma) before present (BP) and ended 2.128 Ma BP.</skos:definition>	<rdfs:seeAlso rdf:resource="http://kos.gbif.org/wiki/geotime:C2rvvv1n"/>	<dcterms:created>2011-01-11</dcterms:created>	<dcterms:modified>2012-08-03</dcterms:modified>	<geotime:start>2.148</geotime:start>	<geotime:end>2.128</geotime:end>	<geotime:polarity>N</geotime:polarity>	<geotime:regionName>Reunion</geotime:regionName>	<dcterms:hasVersion rdf:resource="&history;20120803/geotime#C2rvvv1n"/>	<rdfs:isDefinedBy rdf:resource="&geotime;"/>	<skos:inScheme rdf:resource="&geotime;"/>	<vann:termGroup rdf:resource="&geotime;Magnetostratigraphic"/>	<vs:term_status>unstable</vs:term_status>	</skos:Concept>
<skos:Concept rdf:about="http://rs.gbif.org/terms/geotime#C2">	<skos:prefLabel xml:lang="en">C2</skos:prefLabel>	<skos:definition>The C2 magnetostratographic time period started 2.581 million years (Ma) before present (BP) and ended 1.778 Ma BP.</skos:definition>	<rdfs:seeAlso rdf:resource="http://kos.gbif.org/wiki/geotime:C2"/>	<dcterms:created>2011-01-11</dcterms:created>	<dcterms:modified>2012-08-03</dcterms:modified>	<geotime:start>2.581</geotime:start>	<geotime:end>1.778</geotime:end>	<geotime:polarity></geotime:polarity>	<geotime:regionName></geotime:regionName>	<dcterms:hasVersion rdf:resource="&history;20120803/geotime#C2"/>	<rdfs:isDefinedBy rdf:resource="&geotime;"/>	<skos:inScheme rdf:resource="&geotime;"/>	<vann:termGroup rdf:resource="&geotime;Magnetostratigraphic"/>	<vs:term_status>unstable</vs:term_status>	</skos:Concept>
<skos:Concept rdf:about="http://rs.gbif.org/terms/geotime#C2rvvv2r">	<skos:prefLabel xml:lang="en">C2rvvv2r</skos:prefLabel>	<skos:definition>The C2rvvv2r magnetostratographic time period started 2.581 million years (Ma) before present (BP) and ended 2.148 Ma BP.</skos:definition>	<rdfs:seeAlso rdf:resource="http://kos.gbif.org/wiki/geotime:C2rvvv2r"/>	<dcterms:created>2011-01-11</dcterms:created>	<dcterms:modified>2012-08-03</dcterms:modified>	<geotime:start>2.581</geotime:start>	<geotime:end>2.148</geotime:end>	<geotime:polarity>R</geotime:polarity>	<geotime:regionName>Matuyama continued</geotime:regionName>	<dcterms:hasVersion rdf:resource="&history;20120803/geotime#C2rvvv2r"/>	<rdfs:isDefinedBy rdf:resource="&geotime;"/>	<skos:inScheme rdf:resource="&geotime;"/>	<vann:termGroup rdf:resource="&geotime;Magnetostratigraphic"/>	<vs:term_status>unstable</vs:term_status>	</skos:Concept>
<skos:Concept rdf:about="http://rs.gbif.org/terms/geotime#C5E">	<skos:prefLabel xml:lang="en">C5E</skos:prefLabel>	<skos:definition>The C5E magnetostratographic time period started 20.04 million years (Ma) before present (BP) and ended 18.056 Ma BP.</skos:definition>	<rdfs:seeAlso rdf:resource="http://kos.gbif.org/wiki/geotime:C5E"/>	<dcterms:created>2011-01-11</dcterms:created>	<dcterms:modified>2012-08-03</dcterms:modified>	<geotime:start>20.04</geotime:start>	<geotime:end>18.056</geotime:end>	<geotime:polarity></geotime:polarity>	<geotime:regionName></geotime:regionName>	<dcterms:hasVersion rdf:resource="&history;20120803/geotime#C5E"/>	<rdfs:isDefinedBy rdf:resource="&geotime;"/>	<skos:inScheme rdf:resource="&geotime;"/>	<vann:termGroup rdf:resource="&geotime;Magnetostratigraphic"/>	<vs:term_status>unstable</vs:term_status>	</skos:Concept>
<skos:Concept rdf:about="http://rs.gbif.org/terms/geotime#C6r">	<skos:prefLabel xml:lang="en">C6r</skos:prefLabel>	<skos:definition>The C6r magnetostratographic time period started 20.04 million years (Ma) before present (BP) and ended 19.722 Ma BP.</skos:definition>	<rdfs:seeAlso rdf:resource="http://kos.gbif.org/wiki/geotime:C6r"/>	<dcterms:created>2011-01-11</dcterms:created>	<dcterms:modified>2012-08-03</dcterms:modified>	<geotime:start>20.04</geotime:start>	<geotime:end>19.722</geotime:end>	<geotime:polarity>R</geotime:polarity>	<geotime:regionName></geotime:regionName>	<dcterms:hasVersion rdf:resource="&history;20120803/geotime#C6r"/>	<rdfs:isDefinedBy rdf:resource="&geotime;"/>	<skos:inScheme rdf:resource="&geotime;"/>	<vann:termGroup rdf:resource="&geotime;Magnetostratigraphic"/>	<vs:term_status>unstable</vs:term_status>	</skos:Concept>
<skos:Concept rdf:about="http://rs.gbif.org/terms/geotime#C6Anvvv1n">	<skos:prefLabel xml:lang="en">C6Anvvv1n</skos:prefLabel>	<skos:definition>The C6Anvvv1n magnetostratographic time period started 20.213 million years (Ma) before present (BP) and ended 20.04 Ma BP.</skos:definition>	<rdfs:seeAlso rdf:resource="http://kos.gbif.org/wiki/geotime:C6Anvvv1n"/>	<dcterms:created>2011-01-11</dcterms:created>	<dcterms:modified>2012-08-03</dcterms:modified>	<geotime:start>20.213</geotime:start>	<geotime:end>20.04</geotime:end>	<geotime:polarity>N</geotime:polarity>	<geotime:regionName></geotime:regionName>	<dcterms:hasVersion rdf:resource="&history;20120803/geotime#C6Anvvv1n"/>	<rdfs:isDefinedBy rdf:resource="&geotime;"/>	<skos:inScheme rdf:resource="&geotime;"/>	<vann:termGroup rdf:resource="&geotime;Magnetostratigraphic"/>	<vs:term_status>unstable</vs:term_status>	</skos:Concept>
<skos:Concept rdf:about="http://rs.gbif.org/terms/geotime#C6Anvvv1r">	<skos:prefLabel xml:lang="en">C6Anvvv1r</skos:prefLabel>	<skos:definition>The C6Anvvv1r magnetostratographic time period started 20.439 million years (Ma) before present (BP) and ended 20.213 Ma BP.</skos:definition>	<rdfs:seeAlso rdf:resource="http://kos.gbif.org/wiki/geotime:C6Anvvv1r"/>	<dcterms:created>2011-01-11</dcterms:created>	<dcterms:modified>2012-08-03</dcterms:modified>	<geotime:start>20.439</geotime:start>	<geotime:end>20.213</geotime:end>	<geotime:polarity>R</geotime:polarity>	<geotime:regionName></geotime:regionName>	<dcterms:hasVersion rdf:resource="&history;20120803/geotime#C6Anvvv1r"/>	<rdfs:isDefinedBy rdf:resource="&geotime;"/>	<skos:inScheme rdf:resource="&geotime;"/>	<vann:termGroup rdf:resource="&geotime;Magnetostratigraphic"/>	<vs:term_status>unstable</vs:term_status>	</skos:Concept>
<skos:Concept rdf:about="http://rs.gbif.org/terms/geotime#C6Anvvv2n">	<skos:prefLabel xml:lang="en">C6Anvvv2n</skos:prefLabel>	<skos:definition>The C6Anvvv2n magnetostratographic time period started 20.709 million years (Ma) before present (BP) and ended 20.439 Ma BP.</skos:definition>	<rdfs:seeAlso rdf:resource="http://kos.gbif.org/wiki/geotime:C6Anvvv2n"/>	<dcterms:created>2011-01-11</dcterms:created>	<dcterms:modified>2012-08-03</dcterms:modified>	<geotime:start>20.709</geotime:start>	<geotime:end>20.439</geotime:end>	<geotime:polarity>N</geotime:polarity>	<geotime:regionName></geotime:regionName>	<dcterms:hasVersion rdf:resource="&history;20120803/geotime#C6Anvvv2n"/>	<rdfs:isDefinedBy rdf:resource="&geotime;"/>	<skos:inScheme rdf:resource="&geotime;"/>	<vann:termGroup rdf:resource="&geotime;Magnetostratigraphic"/>	<vs:term_status>unstable</vs:term_status>	</skos:Concept>
<skos:Concept rdf:about="http://rs.gbif.org/terms/geotime#C6A">	<skos:prefLabel xml:lang="en">C6A</skos:prefLabel>	<skos:definition>The C6A magnetostratographic time period started 21.083 million years (Ma) before present (BP) and ended 20.4 Ma BP.</skos:definition>	<rdfs:seeAlso rdf:resource="http://kos.gbif.org/wiki/geotime:C6A"/>	<dcterms:created>2011-01-11</dcterms:created>	<dcterms:modified>2012-08-03</dcterms:modified>	<geotime:start>21.083</geotime:start>	<geotime:end>20.4</geotime:end>	<geotime:polarity></geotime:polarity>	<geotime:regionName></geotime:regionName>	<dcterms:hasVersion rdf:resource="&history;20120803/geotime#C6A"/>	<rdfs:isDefinedBy rdf:resource="&geotime;"/>	<skos:inScheme rdf:resource="&geotime;"/>	<vann:termGroup rdf:resource="&geotime;Magnetostratigraphic"/>	<vs:term_status>unstable</vs:term_status>	</skos:Concept>
<skos:Concept rdf:about="http://rs.gbif.org/terms/geotime#C6Ar">	<skos:prefLabel xml:lang="en">C6Ar</skos:prefLabel>	<skos:definition>The C6Ar magnetostratographic time period started 21.083 million years (Ma) before present (BP) and ended 20.709 Ma BP.</skos:definition>	<rdfs:seeAlso rdf:resource="http://kos.gbif.org/wiki/geotime:C6Ar"/>	<dcterms:created>2011-01-11</dcterms:created>	<dcterms:modified>2012-08-03</dcterms:modified>	<geotime:start>21.083</geotime:start>	<geotime:end>20.709</geotime:end>	<geotime:polarity>R</geotime:polarity>	<geotime:regionName></geotime:regionName>	<dcterms:hasVersion rdf:resource="&history;20120803/geotime#C6Ar"/>	<rdfs:isDefinedBy rdf:resource="&geotime;"/>	<skos:inScheme rdf:resource="&geotime;"/>	<vann:termGroup rdf:resource="&geotime;Magnetostratigraphic"/>	<vs:term_status>unstable</vs:term_status>	</skos:Concept>
<skos:Concept rdf:about="http://rs.gbif.org/terms/geotime#C6AAn">	<skos:prefLabel xml:lang="en">C6AAn</skos:prefLabel>	<skos:definition>The C6AAn magnetostratographic time period started 21.159 million years (Ma) before present (BP) and ended 21.083 Ma BP.</skos:definition>	<rdfs:seeAlso rdf:resource="http://kos.gbif.org/wiki/geotime:C6AAn"/>	<dcterms:created>2011-01-11</dcterms:created>	<dcterms:modified>2012-08-03</dcterms:modified>	<geotime:start>21.159</geotime:start>	<geotime:end>21.083</geotime:end>	<geotime:polarity>N</geotime:polarity>	<geotime:regionName></geotime:regionName>	<dcterms:hasVersion rdf:resource="&history;20120803/geotime#C6AAn"/>	<rdfs:isDefinedBy rdf:resource="&geotime;"/>	<skos:inScheme rdf:resource="&geotime;"/>	<vann:termGroup rdf:resource="&geotime;Magnetostratigraphic"/>	<vs:term_status>unstable</vs:term_status>	</skos:Concept>
<skos:Concept rdf:about="http://rs.gbif.org/terms/geotime#C6AArvvv1r">	<skos:prefLabel xml:lang="en">C6AArvvv1r</skos:prefLabel>	<skos:definition>The C6AArvvv1r magnetostratographic time period started 21.403 million years (Ma) before present (BP) and ended 21.159 Ma BP.</skos:definition>	<rdfs:seeAlso rdf:resource="http://kos.gbif.org/wiki/geotime:C6AArvvv1r"/>	<dcterms:created>2011-01-11</dcterms:created>	<dcterms:modified>2012-08-03</dcterms:modified>	<geotime:start>21.403</geotime:start>	<geotime:end>21.159</geotime:end>	<geotime:polarity>R</geotime:polarity>	<geotime:regionName></geotime:regionName>	<dcterms:hasVersion rdf:resource="&history;20120803/geotime#C6AArvvv1r"/>	<rdfs:isDefinedBy rdf:resource="&geotime;"/>	<skos:inScheme rdf:resource="&geotime;"/>	<vann:termGroup rdf:resource="&geotime;Magnetostratigraphic"/>	<vs:term_status>unstable</vs:term_status>	</skos:Concept>
<skos:Concept rdf:about="http://rs.gbif.org/terms/geotime#C6AArvvv1n">	<skos:prefLabel xml:lang="en">C6AArvvv1n</skos:prefLabel>	<skos:definition>The C6AArvvv1n magnetostratographic time period started 21.483 million years (Ma) before present (BP) and ended 21.403 Ma BP.</skos:definition>	<rdfs:seeAlso rdf:resource="http://kos.gbif.org/wiki/geotime:C6AArvvv1n"/>	<dcterms:created>2011-01-11</dcterms:created>	<dcterms:modified>2012-08-03</dcterms:modified>	<geotime:start>21.483</geotime:start>	<geotime:end>21.403</geotime:end>	<geotime:polarity>N</geotime:polarity>	<geotime:regionName></geotime:regionName>	<dcterms:hasVersion rdf:resource="&history;20120803/geotime#C6AArvvv1n"/>	<rdfs:isDefinedBy rdf:resource="&geotime;"/>	<skos:inScheme rdf:resource="&geotime;"/>	<vann:termGroup rdf:resource="&geotime;Magnetostratigraphic"/>	<vs:term_status>unstable</vs:term_status>	</skos:Concept>
<skos:Concept rdf:about="http://rs.gbif.org/terms/geotime#C6AArvvv2r">	<skos:prefLabel xml:lang="en">C6AArvvv2r</skos:prefLabel>	<skos:definition>The C6AArvvv2r magnetostratographic time period started 21.659 million years (Ma) before present (BP) and ended 21.483 Ma BP.</skos:definition>	<rdfs:seeAlso rdf:resource="http://kos.gbif.org/wiki/geotime:C6AArvvv2r"/>	<dcterms:created>2011-01-11</dcterms:created>	<dcterms:modified>2012-08-03</dcterms:modified>	<geotime:start>21.659</geotime:start>	<geotime:end>21.483</geotime:end>	<geotime:polarity>R</geotime:polarity>	<geotime:regionName></geotime:regionName>	<dcterms:hasVersion rdf:resource="&history;20120803/geotime#C6AArvvv2r"/>	<rdfs:isDefinedBy rdf:resource="&geotime;"/>	<skos:inScheme rdf:resource="&geotime;"/>	<vann:termGroup rdf:resource="&geotime;Magnetostratigraphic"/>	<vs:term_status>unstable</vs:term_status>	</skos:Concept>
<skos:Concept rdf:about="http://rs.gbif.org/terms/geotime#C6AArvvv2n">	<skos:prefLabel xml:lang="en">C6AArvvv2n</skos:prefLabel>	<skos:definition>The C6AArvvv2n magnetostratographic time period started 21.688 million years (Ma) before present (BP) and ended 21.659 Ma BP.</skos:definition>	<rdfs:seeAlso rdf:resource="http://kos.gbif.org/wiki/geotime:C6AArvvv2n"/>	<dcterms:created>2011-01-11</dcterms:created>	<dcterms:modified>2012-08-03</dcterms:modified>	<geotime:start>21.688</geotime:start>	<geotime:end>21.659</geotime:end>	<geotime:polarity>N</geotime:polarity>	<geotime:regionName></geotime:regionName>	<dcterms:hasVersion rdf:resource="&history;20120803/geotime#C6AArvvv2n"/>	<rdfs:isDefinedBy rdf:resource="&geotime;"/>	<skos:inScheme rdf:resource="&geotime;"/>	<vann:termGroup rdf:resource="&geotime;Magnetostratigraphic"/>	<vs:term_status>unstable</vs:term_status>	</skos:Concept>
<skos:Concept rdf:about="http://rs.gbif.org/terms/geotime#C6AA">	<skos:prefLabel xml:lang="en">C6AA</skos:prefLabel>	<skos:definition>The C6AA magnetostratographic time period started 21.767 million years (Ma) before present (BP) and ended 21.083 Ma BP.</skos:definition>	<rdfs:seeAlso rdf:resource="http://kos.gbif.org/wiki/geotime:C6AA"/>	<dcterms:created>2011-01-11</dcterms:created>	<dcterms:modified>2012-08-03</dcterms:modified>	<geotime:start>21.767</geotime:start>	<geotime:end>21.083</geotime:end>	<geotime:polarity></geotime:polarity>	<geotime:regionName></geotime:regionName>	<dcterms:hasVersion rdf:resource="&history;20120803/geotime#C6AA"/>	<rdfs:isDefinedBy rdf:resource="&geotime;"/>	<skos:inScheme rdf:resource="&geotime;"/>	<vann:termGroup rdf:resource="&geotime;Magnetostratigraphic"/>	<vs:term_status>unstable</vs:term_status>	</skos:Concept>
<skos:Concept rdf:about="http://rs.gbif.org/terms/geotime#C6AArvvv3r">	<skos:prefLabel xml:lang="en">C6AArvvv3r</skos:prefLabel>	<skos:definition>The C6AArvvv3r magnetostratographic time period started 21.767 million years (Ma) before present (BP) and ended 21.688 Ma BP.</skos:definition>	<rdfs:seeAlso rdf:resource="http://kos.gbif.org/wiki/geotime:C6AArvvv3r"/>	<dcterms:created>2011-01-11</dcterms:created>	<dcterms:modified>2012-08-03</dcterms:modified>	<geotime:start>21.767</geotime:start>	<geotime:end>21.688</geotime:end>	<geotime:polarity>R</geotime:polarity>	<geotime:regionName></geotime:regionName>	<dcterms:hasVersion rdf:resource="&history;20120803/geotime#C6AArvvv3r"/>	<rdfs:isDefinedBy rdf:resource="&geotime;"/>	<skos:inScheme rdf:resource="&geotime;"/>	<vann:termGroup rdf:resource="&geotime;Magnetostratigraphic"/>	<vs:term_status>unstable</vs:term_status>	</skos:Concept>
<skos:Concept rdf:about="http://rs.gbif.org/terms/geotime#C6Bnvvv1n">	<skos:prefLabel xml:lang="en">C6Bnvvv1n</skos:prefLabel>	<skos:definition>The C6Bnvvv1n magnetostratographic time period started 21.936 million years (Ma) before present (BP) and ended 21.767 Ma BP.</skos:definition>	<rdfs:seeAlso rdf:resource="http://kos.gbif.org/wiki/geotime:C6Bnvvv1n"/>	<dcterms:created>2011-01-11</dcterms:created>	<dcterms:modified>2012-08-03</dcterms:modified>	<geotime:start>21.936</geotime:start>	<geotime:end>21.767</geotime:end>	<geotime:polarity>N</geotime:polarity>	<geotime:regionName></geotime:regionName>	<dcterms:hasVersion rdf:resource="&history;20120803/geotime#C6Bnvvv1n"/>	<rdfs:isDefinedBy rdf:resource="&geotime;"/>	<skos:inScheme rdf:resource="&geotime;"/>	<vann:termGroup rdf:resource="&geotime;Magnetostratigraphic"/>	<vs:term_status>unstable</vs:term_status>	</skos:Concept>
<skos:Concept rdf:about="http://rs.gbif.org/terms/geotime#C6Bnvvv1r">	<skos:prefLabel xml:lang="en">C6Bnvvv1r</skos:prefLabel>	<skos:definition>The C6Bnvvv1r magnetostratographic time period started 21.992 million years (Ma) before present (BP) and ended 21.936 Ma BP.</skos:definition>	<rdfs:seeAlso rdf:resource="http://kos.gbif.org/wiki/geotime:C6Bnvvv1r"/>	<dcterms:created>2011-01-11</dcterms:created>	<dcterms:modified>2012-08-03</dcterms:modified>	<geotime:start>21.992</geotime:start>	<geotime:end>21.936</geotime:end>	<geotime:polarity>R</geotime:polarity>	<geotime:regionName></geotime:regionName>	<dcterms:hasVersion rdf:resource="&history;20120803/geotime#C6Bnvvv1r"/>	<rdfs:isDefinedBy rdf:resource="&geotime;"/>	<skos:inScheme rdf:resource="&geotime;"/>	<vann:termGroup rdf:resource="&geotime;Magnetostratigraphic"/>	<vs:term_status>unstable</vs:term_status>	</skos:Concept>
<skos:Concept rdf:about="http://rs.gbif.org/terms/geotime#C6Bnvvv2n">	<skos:prefLabel xml:lang="en">C6Bnvvv2n</skos:prefLabel>	<skos:definition>The C6Bnvvv2n magnetostratographic time period started 22.268 million years (Ma) before present (BP) and ended 21.992 Ma BP.</skos:definition>	<rdfs:seeAlso rdf:resource="http://kos.gbif.org/wiki/geotime:C6Bnvvv2n"/>	<dcterms:created>2011-01-11</dcterms:created>	<dcterms:modified>2012-08-03</dcterms:modified>	<geotime:start>22.268</geotime:start>	<geotime:end>21.992</geotime:end>	<geotime:polarity>N</geotime:polarity>	<geotime:regionName></geotime:regionName>	<dcterms:hasVersion rdf:resource="&history;20120803/geotime#C6Bnvvv2n"/>	<rdfs:isDefinedBy rdf:resource="&geotime;"/>	<skos:inScheme rdf:resource="&geotime;"/>	<vann:termGroup rdf:resource="&geotime;Magnetostratigraphic"/>	<vs:term_status>unstable</vs:term_status>	</skos:Concept>
<skos:Concept rdf:about="http://rs.gbif.org/terms/geotime#C6B">	<skos:prefLabel xml:lang="en">C6B</skos:prefLabel>	<skos:definition>The C6B magnetostratographic time period started 22.487 million years (Ma) before present (BP) and ended 21.767 Ma BP.</skos:definition>	<rdfs:seeAlso rdf:resource="http://kos.gbif.org/wiki/geotime:C6B"/>	<dcterms:created>2011-01-11</dcterms:created>	<dcterms:modified>2012-08-03</dcterms:modified>	<geotime:start>22.487</geotime:start>	<geotime:end>21.767</geotime:end>	<geotime:polarity></geotime:polarity>	<geotime:regionName></geotime:regionName>	<dcterms:hasVersion rdf:resource="&history;20120803/geotime#C6B"/>	<rdfs:isDefinedBy rdf:resource="&geotime;"/>	<skos:inScheme rdf:resource="&geotime;"/>	<vann:termGroup rdf:resource="&geotime;Magnetostratigraphic"/>	<vs:term_status>unstable</vs:term_status>	</skos:Concept>
<skos:Concept rdf:about="http://rs.gbif.org/terms/geotime#C6Br">	<skos:prefLabel xml:lang="en">C6Br</skos:prefLabel>	<skos:definition>The C6Br magnetostratographic time period started 22.487 million years (Ma) before present (BP) and ended 22.268 Ma BP.</skos:definition>	<rdfs:seeAlso rdf:resource="http://kos.gbif.org/wiki/geotime:C6Br"/>	<dcterms:created>2011-01-11</dcterms:created>	<dcterms:modified>2012-08-03</dcterms:modified>	<geotime:start>22.487</geotime:start>	<geotime:end>22.268</geotime:end>	<geotime:polarity>R</geotime:polarity>	<geotime:regionName></geotime:regionName>	<dcterms:hasVersion rdf:resource="&history;20120803/geotime#C6Br"/>	<rdfs:isDefinedBy rdf:resource="&geotime;"/>	<skos:inScheme rdf:resource="&geotime;"/>	<vann:termGroup rdf:resource="&geotime;Magnetostratigraphic"/>	<vs:term_status>unstable</vs:term_status>	</skos:Concept>
<skos:Concept rdf:about="http://rs.gbif.org/terms/geotime#C6Cnvvv1n">	<skos:prefLabel xml:lang="en">C6Cnvvv1n</skos:prefLabel>	<skos:definition>The C6Cnvvv1n magnetostratographic time period started 22.754 million years (Ma) before present (BP) and ended 22.487 Ma BP.</skos:definition>	<rdfs:seeAlso rdf:resource="http://kos.gbif.org/wiki/geotime:C6Cnvvv1n"/>	<dcterms:created>2011-01-11</dcterms:created>	<dcterms:modified>2012-08-03</dcterms:modified>	<geotime:start>22.754</geotime:start>	<geotime:end>22.487</geotime:end>	<geotime:polarity>N</geotime:polarity>	<geotime:regionName></geotime:regionName>	<dcterms:hasVersion rdf:resource="&history;20120803/geotime#C6Cnvvv1n"/>	<rdfs:isDefinedBy rdf:resource="&geotime;"/>	<skos:inScheme rdf:resource="&geotime;"/>	<vann:termGroup rdf:resource="&geotime;Magnetostratigraphic"/>	<vs:term_status>unstable</vs:term_status>	</skos:Concept>
<skos:Concept rdf:about="http://rs.gbif.org/terms/geotime#C6Cnvvv1r">	<skos:prefLabel xml:lang="en">C6Cnvvv1r</skos:prefLabel>	<skos:definition>The C6Cnvvv1r magnetostratographic time period started 22.902 million years (Ma) before present (BP) and ended 22.754 Ma BP.</skos:definition>	<rdfs:seeAlso rdf:resource="http://kos.gbif.org/wiki/geotime:C6Cnvvv1r"/>	<dcterms:created>2011-01-11</dcterms:created>	<dcterms:modified>2012-08-03</dcterms:modified>	<geotime:start>22.902</geotime:start>	<geotime:end>22.754</geotime:end>	<geotime:polarity>R</geotime:polarity>	<geotime:regionName></geotime:regionName>	<dcterms:hasVersion rdf:resource="&history;20120803/geotime#C6Cnvvv1r"/>	<rdfs:isDefinedBy rdf:resource="&geotime;"/>	<skos:inScheme rdf:resource="&geotime;"/>	<vann:termGroup rdf:resource="&geotime;Magnetostratigraphic"/>	<vs:term_status>unstable</vs:term_status>	</skos:Concept>
<skos:Concept rdf:about="http://rs.gbif.org/terms/geotime#C6Cnvvv2n">	<skos:prefLabel xml:lang="en">C6Cnvvv2n</skos:prefLabel>	<skos:definition>The C6Cnvvv2n magnetostratographic time period started 23.03 million years (Ma) before present (BP) and ended 22.902 Ma BP.</skos:definition>	<rdfs:seeAlso rdf:resource="http://kos.gbif.org/wiki/geotime:C6Cnvvv2n"/>	<dcterms:created>2011-01-11</dcterms:created>	<dcterms:modified>2012-08-03</dcterms:modified>	<geotime:start>23.03</geotime:start>	<geotime:end>22.902</geotime:end>	<geotime:polarity>N</geotime:polarity>	<geotime:regionName></geotime:regionName>	<dcterms:hasVersion rdf:resource="&history;20120803/geotime#C6Cnvvv2n"/>	<rdfs:isDefinedBy rdf:resource="&geotime;"/>	<skos:inScheme rdf:resource="&geotime;"/>	<vann:termGroup rdf:resource="&geotime;Magnetostratigraphic"/>	<vs:term_status>unstable</vs:term_status>	</skos:Concept>
<skos:Concept rdf:about="http://rs.gbif.org/terms/geotime#C6Cnvvv2r">	<skos:prefLabel xml:lang="en">C6Cnvvv2r</skos:prefLabel>	<skos:definition>The C6Cnvvv2r magnetostratographic time period started 23.249 million years (Ma) before present (BP) and ended 23.03 Ma BP.</skos:definition>	<rdfs:seeAlso rdf:resource="http://kos.gbif.org/wiki/geotime:C6Cnvvv2r"/>	<dcterms:created>2011-01-11</dcterms:created>	<dcterms:modified>2012-08-03</dcterms:modified>	<geotime:start>23.249</geotime:start>	<geotime:end>23.03</geotime:end>	<geotime:polarity>R</geotime:polarity>	<geotime:regionName></geotime:regionName>	<dcterms:hasVersion rdf:resource="&history;20120803/geotime#C6Cnvvv2r"/>	<rdfs:isDefinedBy rdf:resource="&geotime;"/>	<skos:inScheme rdf:resource="&geotime;"/>	<vann:termGroup rdf:resource="&geotime;Magnetostratigraphic"/>	<vs:term_status>unstable</vs:term_status>	</skos:Concept>
<skos:Concept rdf:about="http://rs.gbif.org/terms/geotime#C6Cnvvv3n">	<skos:prefLabel xml:lang="en">C6Cnvvv3n</skos:prefLabel>	<skos:definition>The C6Cnvvv3n magnetostratographic time period started 23.375 million years (Ma) before present (BP) and ended 23.249 Ma BP.</skos:definition>	<rdfs:seeAlso rdf:resource="http://kos.gbif.org/wiki/geotime:C6Cnvvv3n"/>	<dcterms:created>2011-01-11</dcterms:created>	<dcterms:modified>2012-08-03</dcterms:modified>	<geotime:start>23.375</geotime:start>	<geotime:end>23.249</geotime:end>	<geotime:polarity>N</geotime:polarity>	<geotime:regionName></geotime:regionName>	<dcterms:hasVersion rdf:resource="&history;20120803/geotime#C6Cnvvv3n"/>	<rdfs:isDefinedBy rdf:resource="&geotime;"/>	<skos:inScheme rdf:resource="&geotime;"/>	<vann:termGroup rdf:resource="&geotime;Magnetostratigraphic"/>	<vs:term_status>unstable</vs:term_status>	</skos:Concept>
<skos:Concept rdf:about="http://rs.gbif.org/terms/geotime#C6C">	<skos:prefLabel xml:lang="en">C6C</skos:prefLabel>	<skos:definition>The C6C magnetostratographic time period started 24.044 million years (Ma) before present (BP) and ended 22.487 Ma BP.</skos:definition>	<rdfs:seeAlso rdf:resource="http://kos.gbif.org/wiki/geotime:C6C"/>	<dcterms:created>2011-01-11</dcterms:created>	<dcterms:modified>2012-08-03</dcterms:modified>	<geotime:start>24.044</geotime:start>	<geotime:end>22.487</geotime:end>	<geotime:polarity></geotime:polarity>	<geotime:regionName></geotime:regionName>	<dcterms:hasVersion rdf:resource="&history;20120803/geotime#C6C"/>	<rdfs:isDefinedBy rdf:resource="&geotime;"/>	<skos:inScheme rdf:resource="&geotime;"/>	<vann:termGroup rdf:resource="&geotime;Magnetostratigraphic"/>	<vs:term_status>unstable</vs:term_status>	</skos:Concept>
<skos:Concept rdf:about="http://rs.gbif.org/terms/geotime#C6Cr">	<skos:prefLabel xml:lang="en">C6Cr</skos:prefLabel>	<skos:definition>The C6Cr magnetostratographic time period started 24.044 million years (Ma) before present (BP) and ended 23.375 Ma BP.</skos:definition>	<rdfs:seeAlso rdf:resource="http://kos.gbif.org/wiki/geotime:C6Cr"/>	<dcterms:created>2011-01-11</dcterms:created>	<dcterms:modified>2012-08-03</dcterms:modified>	<geotime:start>24.044</geotime:start>	<geotime:end>23.375</geotime:end>	<geotime:polarity>R</geotime:polarity>	<geotime:regionName></geotime:regionName>	<dcterms:hasVersion rdf:resource="&history;20120803/geotime#C6Cr"/>	<rdfs:isDefinedBy rdf:resource="&geotime;"/>	<skos:inScheme rdf:resource="&geotime;"/>	<vann:termGroup rdf:resource="&geotime;Magnetostratigraphic"/>	<vs:term_status>unstable</vs:term_status>	</skos:Concept>
<skos:Concept rdf:about="http://rs.gbif.org/terms/geotime#C7nvvv1n">	<skos:prefLabel xml:lang="en">C7nvvv1n</skos:prefLabel>	<skos:definition>The C7nvvv1n magnetostratographic time period started 24.102 million years (Ma) before present (BP) and ended 24.044 Ma BP.</skos:definition>	<rdfs:seeAlso rdf:resource="http://kos.gbif.org/wiki/geotime:C7nvvv1n"/>	<dcterms:created>2011-01-11</dcterms:created>	<dcterms:modified>2012-08-03</dcterms:modified>	<geotime:start>24.102</geotime:start>	<geotime:end>24.044</geotime:end>	<geotime:polarity>N</geotime:polarity>	<geotime:regionName></geotime:regionName>	<dcterms:hasVersion rdf:resource="&history;20120803/geotime#C7nvvv1n"/>	<rdfs:isDefinedBy rdf:resource="&geotime;"/>	<skos:inScheme rdf:resource="&geotime;"/>	<vann:termGroup rdf:resource="&geotime;Magnetostratigraphic"/>	<vs:term_status>unstable</vs:term_status>	</skos:Concept>
<skos:Concept rdf:about="http://rs.gbif.org/terms/geotime#C7nvvv1r">	<skos:prefLabel xml:lang="en">C7nvvv1r</skos:prefLabel>	<skos:definition>The C7nvvv1r magnetostratographic time period started 24.163 million years (Ma) before present (BP) and ended 24.102 Ma BP.</skos:definition>	<rdfs:seeAlso rdf:resource="http://kos.gbif.org/wiki/geotime:C7nvvv1r"/>	<dcterms:created>2011-01-11</dcterms:created>	<dcterms:modified>2012-08-03</dcterms:modified>	<geotime:start>24.163</geotime:start>	<geotime:end>24.102</geotime:end>	<geotime:polarity>R</geotime:polarity>	<geotime:regionName></geotime:regionName>	<dcterms:hasVersion rdf:resource="&history;20120803/geotime#C7nvvv1r"/>	<rdfs:isDefinedBy rdf:resource="&geotime;"/>	<skos:inScheme rdf:resource="&geotime;"/>	<vann:termGroup rdf:resource="&geotime;Magnetostratigraphic"/>	<vs:term_status>unstable</vs:term_status>	</skos:Concept>
<skos:Concept rdf:about="http://rs.gbif.org/terms/geotime#C7nvvv2n">	<skos:prefLabel xml:lang="en">C7nvvv2n</skos:prefLabel>	<skos:definition>The C7nvvv2n magnetostratographic time period started 24.556 million years (Ma) before present (BP) and ended 24.163 Ma BP.</skos:definition>	<rdfs:seeAlso rdf:resource="http://kos.gbif.org/wiki/geotime:C7nvvv2n"/>	<dcterms:created>2011-01-11</dcterms:created>	<dcterms:modified>2012-08-03</dcterms:modified>	<geotime:start>24.556</geotime:start>	<geotime:end>24.163</geotime:end>	<geotime:polarity>N</geotime:polarity>	<geotime:regionName></geotime:regionName>	<dcterms:hasVersion rdf:resource="&history;20120803/geotime#C7nvvv2n"/>	<rdfs:isDefinedBy rdf:resource="&geotime;"/>	<skos:inScheme rdf:resource="&geotime;"/>	<vann:termGroup rdf:resource="&geotime;Magnetostratigraphic"/>	<vs:term_status>unstable</vs:term_status>	</skos:Concept>
<skos:Concept rdf:about="http://rs.gbif.org/terms/geotime#C7">	<skos:prefLabel xml:lang="en">C7</skos:prefLabel>	<skos:definition>The C7 magnetostratographic time period started 24.915 million years (Ma) before present (BP) and ended 24.044 Ma BP.</skos:definition>	<rdfs:seeAlso rdf:resource="http://kos.gbif.org/wiki/geotime:C7"/>	<dcterms:created>2011-01-11</dcterms:created>	<dcterms:modified>2012-08-03</dcterms:modified>	<geotime:start>24.915</geotime:start>	<geotime:end>24.044</geotime:end>	<geotime:polarity></geotime:polarity>	<geotime:regionName></geotime:regionName>	<dcterms:hasVersion rdf:resource="&history;20120803/geotime#C7"/>	<rdfs:isDefinedBy rdf:resource="&geotime;"/>	<skos:inScheme rdf:resource="&geotime;"/>	<vann:termGroup rdf:resource="&geotime;Magnetostratigraphic"/>	<vs:term_status>unstable</vs:term_status>	</skos:Concept>
<skos:Concept rdf:about="http://rs.gbif.org/terms/geotime#C7r">	<skos:prefLabel xml:lang="en">C7r</skos:prefLabel>	<skos:definition>The C7r magnetostratographic time period started 24.915 million years (Ma) before present (BP) and ended 24.556 Ma BP.</skos:definition>	<rdfs:seeAlso rdf:resource="http://kos.gbif.org/wiki/geotime:C7r"/>	<dcterms:created>2011-01-11</dcterms:created>	<dcterms:modified>2012-08-03</dcterms:modified>	<geotime:start>24.915</geotime:start>	<geotime:end>24.556</geotime:end>	<geotime:polarity>R</geotime:polarity>	<geotime:regionName></geotime:regionName>	<dcterms:hasVersion rdf:resource="&history;20120803/geotime#C7r"/>	<rdfs:isDefinedBy rdf:resource="&geotime;"/>	<skos:inScheme rdf:resource="&geotime;"/>	<vann:termGroup rdf:resource="&geotime;Magnetostratigraphic"/>	<vs:term_status>unstable</vs:term_status>	</skos:Concept>
<skos:Concept rdf:about="http://rs.gbif.org/terms/geotime#C7An">	<skos:prefLabel xml:lang="en">C7An</skos:prefLabel>	<skos:definition>The C7An magnetostratographic time period started 25.091 million years (Ma) before present (BP) and ended 24.915 Ma BP.</skos:definition>	<rdfs:seeAlso rdf:resource="http://kos.gbif.org/wiki/geotime:C7An"/>	<dcterms:created>2011-01-11</dcterms:created>	<dcterms:modified>2012-08-03</dcterms:modified>	<geotime:start>25.091</geotime:start>	<geotime:end>24.915</geotime:end>	<geotime:polarity>N</geotime:polarity>	<geotime:regionName></geotime:regionName>	<dcterms:hasVersion rdf:resource="&history;20120803/geotime#C7An"/>	<rdfs:isDefinedBy rdf:resource="&geotime;"/>	<skos:inScheme rdf:resource="&geotime;"/>	<vann:termGroup rdf:resource="&geotime;Magnetostratigraphic"/>	<vs:term_status>unstable</vs:term_status>	</skos:Concept>
<skos:Concept rdf:about="http://rs.gbif.org/terms/geotime#C7A">	<skos:prefLabel xml:lang="en">C7A</skos:prefLabel>	<skos:definition>The C7A magnetostratographic time period started 25.295 million years (Ma) before present (BP) and ended 24.915 Ma BP.</skos:definition>	<rdfs:seeAlso rdf:resource="http://kos.gbif.org/wiki/geotime:C7A"/>	<dcterms:created>2011-01-11</dcterms:created>	<dcterms:modified>2012-08-03</dcterms:modified>	<geotime:start>25.295</geotime:start>	<geotime:end>24.915</geotime:end>	<geotime:polarity></geotime:polarity>	<geotime:regionName></geotime:regionName>	<dcterms:hasVersion rdf:resource="&history;20120803/geotime#C7A"/>	<rdfs:isDefinedBy rdf:resource="&geotime;"/>	<skos:inScheme rdf:resource="&geotime;"/>	<vann:termGroup rdf:resource="&geotime;Magnetostratigraphic"/>	<vs:term_status>unstable</vs:term_status>	</skos:Concept>
<skos:Concept rdf:about="http://rs.gbif.org/terms/geotime#C7Ar">	<skos:prefLabel xml:lang="en">C7Ar</skos:prefLabel>	<skos:definition>The C7Ar magnetostratographic time period started 25.295 million years (Ma) before present (BP) and ended 25.091 Ma BP.</skos:definition>	<rdfs:seeAlso rdf:resource="http://kos.gbif.org/wiki/geotime:C7Ar"/>	<dcterms:created>2011-01-11</dcterms:created>	<dcterms:modified>2012-08-03</dcterms:modified>	<geotime:start>25.295</geotime:start>	<geotime:end>25.091</geotime:end>	<geotime:polarity>R</geotime:polarity>	<geotime:regionName></geotime:regionName>	<dcterms:hasVersion rdf:resource="&history;20120803/geotime#C7Ar"/>	<rdfs:isDefinedBy rdf:resource="&geotime;"/>	<skos:inScheme rdf:resource="&geotime;"/>	<vann:termGroup rdf:resource="&geotime;Magnetostratigraphic"/>	<vs:term_status>unstable</vs:term_status>	</skos:Concept>
<skos:Concept rdf:about="http://rs.gbif.org/terms/geotime#C8nvvv1n">	<skos:prefLabel xml:lang="en">C8nvvv1n</skos:prefLabel>	<skos:definition>The C8nvvv1n magnetostratographic time period started 25.444 million years (Ma) before present (BP) and ended 25.295 Ma BP.</skos:definition>	<rdfs:seeAlso rdf:resource="http://kos.gbif.org/wiki/geotime:C8nvvv1n"/>	<dcterms:created>2011-01-11</dcterms:created>	<dcterms:modified>2012-08-03</dcterms:modified>	<geotime:start>25.444</geotime:start>	<geotime:end>25.295</geotime:end>	<geotime:polarity>N</geotime:polarity>	<geotime:regionName></geotime:regionName>	<dcterms:hasVersion rdf:resource="&history;20120803/geotime#C8nvvv1n"/>	<rdfs:isDefinedBy rdf:resource="&geotime;"/>	<skos:inScheme rdf:resource="&geotime;"/>	<vann:termGroup rdf:resource="&geotime;Magnetostratigraphic"/>	<vs:term_status>unstable</vs:term_status>	</skos:Concept>
<skos:Concept rdf:about="http://rs.gbif.org/terms/geotime#C8nvvv1r">	<skos:prefLabel xml:lang="en">C8nvvv1r</skos:prefLabel>	<skos:definition>The C8nvvv1r magnetostratographic time period started 25.492 million years (Ma) before present (BP) and ended 25.444 Ma BP.</skos:definition>	<rdfs:seeAlso rdf:resource="http://kos.gbif.org/wiki/geotime:C8nvvv1r"/>	<dcterms:created>2011-01-11</dcterms:created>	<dcterms:modified>2012-08-03</dcterms:modified>	<geotime:start>25.492</geotime:start>	<geotime:end>25.444</geotime:end>	<geotime:polarity>R</geotime:polarity>	<geotime:regionName></geotime:regionName>	<dcterms:hasVersion rdf:resource="&history;20120803/geotime#C8nvvv1r"/>	<rdfs:isDefinedBy rdf:resource="&geotime;"/>	<skos:inScheme rdf:resource="&geotime;"/>	<vann:termGroup rdf:resource="&geotime;Magnetostratigraphic"/>	<vs:term_status>unstable</vs:term_status>	</skos:Concept>
<skos:Concept rdf:about="http://rs.gbif.org/terms/geotime#C8nvvv2n">	<skos:prefLabel xml:lang="en">C8nvvv2n</skos:prefLabel>	<skos:definition>The C8nvvv2n magnetostratographic time period started 26.154 million years (Ma) before present (BP) and ended 25.492 Ma BP.</skos:definition>	<rdfs:seeAlso rdf:resource="http://kos.gbif.org/wiki/geotime:C8nvvv2n"/>	<dcterms:created>2011-01-11</dcterms:created>	<dcterms:modified>2012-08-03</dcterms:modified>	<geotime:start>26.154</geotime:start>	<geotime:end>25.492</geotime:end>	<geotime:polarity>N</geotime:polarity>	<geotime:regionName></geotime:regionName>	<dcterms:hasVersion rdf:resource="&history;20120803/geotime#C8nvvv2n"/>	<rdfs:isDefinedBy rdf:resource="&geotime;"/>	<skos:inScheme rdf:resource="&geotime;"/>	<vann:termGroup rdf:resource="&geotime;Magnetostratigraphic"/>	<vs:term_status>unstable</vs:term_status>	</skos:Concept>
<skos:Concept rdf:about="http://rs.gbif.org/terms/geotime#C8">	<skos:prefLabel xml:lang="en">C8</skos:prefLabel>	<skos:definition>The C8 magnetostratographic time period started 26.714 million years (Ma) before present (BP) and ended 25.295 Ma BP.</skos:definition>	<rdfs:seeAlso rdf:resource="http://kos.gbif.org/wiki/geotime:C8"/>	<dcterms:created>2011-01-11</dcterms:created>	<dcterms:modified>2012-08-03</dcterms:modified>	<geotime:start>26.714</geotime:start>	<geotime:end>25.295</geotime:end>	<geotime:polarity></geotime:polarity>	<geotime:regionName></geotime:regionName>	<dcterms:hasVersion rdf:resource="&history;20120803/geotime#C8"/>	<rdfs:isDefinedBy rdf:resource="&geotime;"/>	<skos:inScheme rdf:resource="&geotime;"/>	<vann:termGroup rdf:resource="&geotime;Magnetostratigraphic"/>	<vs:term_status>unstable</vs:term_status>	</skos:Concept>
<skos:Concept rdf:about="http://rs.gbif.org/terms/geotime#C8r">	<skos:prefLabel xml:lang="en">C8r</skos:prefLabel>	<skos:definition>The C8r magnetostratographic time period started 26.714 million years (Ma) before present (BP) and ended 26.154 Ma BP.</skos:definition>	<rdfs:seeAlso rdf:resource="http://kos.gbif.org/wiki/geotime:C8r"/>	<dcterms:created>2011-01-11</dcterms:created>	<dcterms:modified>2012-08-03</dcterms:modified>	<geotime:start>26.714</geotime:start>	<geotime:end>26.154</geotime:end>	<geotime:polarity>R</geotime:polarity>	<geotime:regionName></geotime:regionName>	<dcterms:hasVersion rdf:resource="&history;20120803/geotime#C8r"/>	<rdfs:isDefinedBy rdf:resource="&geotime;"/>	<skos:inScheme rdf:resource="&geotime;"/>	<vann:termGroup rdf:resource="&geotime;Magnetostratigraphic"/>	<vs:term_status>unstable</vs:term_status>	</skos:Concept>
<skos:Concept rdf:about="http://rs.gbif.org/terms/geotime#C9n">	<skos:prefLabel xml:lang="en">C9n</skos:prefLabel>	<skos:definition>The C9n magnetostratographic time period started 27.826 million years (Ma) before present (BP) and ended 26.714 Ma BP.</skos:definition>	<rdfs:seeAlso rdf:resource="http://kos.gbif.org/wiki/geotime:C9n"/>	<dcterms:created>2011-01-11</dcterms:created>	<dcterms:modified>2012-08-03</dcterms:modified>	<geotime:start>27.826</geotime:start>	<geotime:end>26.714</geotime:end>	<geotime:polarity>N</geotime:polarity>	<geotime:regionName></geotime:regionName>	<dcterms:hasVersion rdf:resource="&history;20120803/geotime#C9n"/>	<rdfs:isDefinedBy rdf:resource="&geotime;"/>	<skos:inScheme rdf:resource="&geotime;"/>	<vann:termGroup rdf:resource="&geotime;Magnetostratigraphic"/>	<vs:term_status>unstable</vs:term_status>	</skos:Concept>
<skos:Concept rdf:about="http://rs.gbif.org/terms/geotime#C9">	<skos:prefLabel xml:lang="en">C9</skos:prefLabel>	<skos:definition>The C9 magnetostratographic time period started 28.186 million years (Ma) before present (BP) and ended 26.714 Ma BP.</skos:definition>	<rdfs:seeAlso rdf:resource="http://kos.gbif.org/wiki/geotime:C9"/>	<dcterms:created>2011-01-11</dcterms:created>	<dcterms:modified>2012-08-03</dcterms:modified>	<geotime:start>28.186</geotime:start>	<geotime:end>26.714</geotime:end>	<geotime:polarity></geotime:polarity>	<geotime:regionName></geotime:regionName>	<dcterms:hasVersion rdf:resource="&history;20120803/geotime#C9"/>	<rdfs:isDefinedBy rdf:resource="&geotime;"/>	<skos:inScheme rdf:resource="&geotime;"/>	<vann:termGroup rdf:resource="&geotime;Magnetostratigraphic"/>	<vs:term_status>unstable</vs:term_status>	</skos:Concept>
<skos:Concept rdf:about="http://rs.gbif.org/terms/geotime#C9r">	<skos:prefLabel xml:lang="en">C9r</skos:prefLabel>	<skos:definition>The C9r magnetostratographic time period started 28.186 million years (Ma) before present (BP) and ended 27.826 Ma BP.</skos:definition>	<rdfs:seeAlso rdf:resource="http://kos.gbif.org/wiki/geotime:C9r"/>	<dcterms:created>2011-01-11</dcterms:created>	<dcterms:modified>2012-08-03</dcterms:modified>	<geotime:start>28.186</geotime:start>	<geotime:end>27.826</geotime:end>	<geotime:polarity>R</geotime:polarity>	<geotime:regionName></geotime:regionName>	<dcterms:hasVersion rdf:resource="&history;20120803/geotime#C9r"/>	<rdfs:isDefinedBy rdf:resource="&geotime;"/>	<skos:inScheme rdf:resource="&geotime;"/>	<vann:termGroup rdf:resource="&geotime;Magnetostratigraphic"/>	<vs:term_status>unstable</vs:term_status>	</skos:Concept>
<skos:Concept rdf:about="http://rs.gbif.org/terms/geotime#C10nvvv1n">	<skos:prefLabel xml:lang="en">C10nvvv1n</skos:prefLabel>	<skos:definition>The C10nvvv1n magnetostratographic time period started 28.45 million years (Ma) before present (BP) and ended 28.186 Ma BP.</skos:definition>	<rdfs:seeAlso rdf:resource="http://kos.gbif.org/wiki/geotime:C10nvvv1n"/>	<dcterms:created>2011-01-11</dcterms:created>	<dcterms:modified>2012-08-03</dcterms:modified>	<geotime:start>28.45</geotime:start>	<geotime:end>28.186</geotime:end>	<geotime:polarity>N</geotime:polarity>	<geotime:regionName></geotime:regionName>	<dcterms:hasVersion rdf:resource="&history;20120803/geotime#C10nvvv1n"/>	<rdfs:isDefinedBy rdf:resource="&geotime;"/>	<skos:inScheme rdf:resource="&geotime;"/>	<vann:termGroup rdf:resource="&geotime;Magnetostratigraphic"/>	<vs:term_status>unstable</vs:term_status>	</skos:Concept>
<skos:Concept rdf:about="http://rs.gbif.org/terms/geotime#C10nvvv1r">	<skos:prefLabel xml:lang="en">C10nvvv1r</skos:prefLabel>	<skos:definition>The C10nvvv1r magnetostratographic time period started 28.525 million years (Ma) before present (BP) and ended 28.45 Ma BP.</skos:definition>	<rdfs:seeAlso rdf:resource="http://kos.gbif.org/wiki/geotime:C10nvvv1r"/>	<dcterms:created>2011-01-11</dcterms:created>	<dcterms:modified>2012-08-03</dcterms:modified>	<geotime:start>28.525</geotime:start>	<geotime:end>28.45</geotime:end>	<geotime:polarity>R</geotime:polarity>	<geotime:regionName></geotime:regionName>	<dcterms:hasVersion rdf:resource="&history;20120803/geotime#C10nvvv1r"/>	<rdfs:isDefinedBy rdf:resource="&geotime;"/>	<skos:inScheme rdf:resource="&geotime;"/>	<vann:termGroup rdf:resource="&geotime;Magnetostratigraphic"/>	<vs:term_status>unstable</vs:term_status>	</skos:Concept>
<skos:Concept rdf:about="http://rs.gbif.org/terms/geotime#C10nvvv2n">	<skos:prefLabel xml:lang="en">C10nvvv2n</skos:prefLabel>	<skos:definition>The C10nvvv2n magnetostratographic time period started 28.715 million years (Ma) before present (BP) and ended 28.525 Ma BP.</skos:definition>	<rdfs:seeAlso rdf:resource="http://kos.gbif.org/wiki/geotime:C10nvvv2n"/>	<dcterms:created>2011-01-11</dcterms:created>	<dcterms:modified>2012-08-03</dcterms:modified>	<geotime:start>28.715</geotime:start>	<geotime:end>28.525</geotime:end>	<geotime:polarity>N</geotime:polarity>	<geotime:regionName></geotime:regionName>	<dcterms:hasVersion rdf:resource="&history;20120803/geotime#C10nvvv2n"/>	<rdfs:isDefinedBy rdf:resource="&geotime;"/>	<skos:inScheme rdf:resource="&geotime;"/>	<vann:termGroup rdf:resource="&geotime;Magnetostratigraphic"/>	<vs:term_status>unstable</vs:term_status>	</skos:Concept>
<skos:Concept rdf:about="http://rs.gbif.org/terms/geotime#C10">	<skos:prefLabel xml:lang="en">C10</skos:prefLabel>	<skos:definition>The C10 magnetostratographic time period started 29.451 million years (Ma) before present (BP) and ended 28.186 Ma BP.</skos:definition>	<rdfs:seeAlso rdf:resource="http://kos.gbif.org/wiki/geotime:C10"/>	<dcterms:created>2011-01-11</dcterms:created>	<dcterms:modified>2012-08-03</dcterms:modified>	<geotime:start>29.451</geotime:start>	<geotime:end>28.186</geotime:end>	<geotime:polarity></geotime:polarity>	<geotime:regionName></geotime:regionName>	<dcterms:hasVersion rdf:resource="&history;20120803/geotime#C10"/>	<rdfs:isDefinedBy rdf:resource="&geotime;"/>	<skos:inScheme rdf:resource="&geotime;"/>	<vann:termGroup rdf:resource="&geotime;Magnetostratigraphic"/>	<vs:term_status>unstable</vs:term_status>	</skos:Concept>
<skos:Concept rdf:about="http://rs.gbif.org/terms/geotime#C10r">	<skos:prefLabel xml:lang="en">C10r</skos:prefLabel>	<skos:definition>The C10r magnetostratographic time period started 29.451 million years (Ma) before present (BP) and ended 28.715 Ma BP.</skos:definition>	<rdfs:seeAlso rdf:resource="http://kos.gbif.org/wiki/geotime:C10r"/>	<dcterms:created>2011-01-11</dcterms:created>	<dcterms:modified>2012-08-03</dcterms:modified>	<geotime:start>29.451</geotime:start>	<geotime:end>28.715</geotime:end>	<geotime:polarity>R</geotime:polarity>	<geotime:regionName></geotime:regionName>	<dcterms:hasVersion rdf:resource="&history;20120803/geotime#C10r"/>	<rdfs:isDefinedBy rdf:resource="&geotime;"/>	<skos:inScheme rdf:resource="&geotime;"/>	<vann:termGroup rdf:resource="&geotime;Magnetostratigraphic"/>	<vs:term_status>unstable</vs:term_status>	</skos:Concept>
<skos:Concept rdf:about="http://rs.gbif.org/terms/geotime#C11nvvv1n">	<skos:prefLabel xml:lang="en">C11nvvv1n</skos:prefLabel>	<skos:definition>The C11nvvv1n magnetostratographic time period started 29.74 million years (Ma) before present (BP) and ended 29.451 Ma BP.</skos:definition>	<rdfs:seeAlso rdf:resource="http://kos.gbif.org/wiki/geotime:C11nvvv1n"/>	<dcterms:created>2011-01-11</dcterms:created>	<dcterms:modified>2012-08-03</dcterms:modified>	<geotime:start>29.74</geotime:start>	<geotime:end>29.451</geotime:end>	<geotime:polarity>N</geotime:polarity>	<geotime:regionName></geotime:regionName>	<dcterms:hasVersion rdf:resource="&history;20120803/geotime#C11nvvv1n"/>	<rdfs:isDefinedBy rdf:resource="&geotime;"/>	<skos:inScheme rdf:resource="&geotime;"/>	<vann:termGroup rdf:resource="&geotime;Magnetostratigraphic"/>	<vs:term_status>unstable</vs:term_status>	</skos:Concept>
<skos:Concept rdf:about="http://rs.gbif.org/terms/geotime#C11nvvv1r">	<skos:prefLabel xml:lang="en">C11nvvv1r</skos:prefLabel>	<skos:definition>The C11nvvv1r magnetostratographic time period started 29.853 million years (Ma) before present (BP) and ended 29.74 Ma BP.</skos:definition>	<rdfs:seeAlso rdf:resource="http://kos.gbif.org/wiki/geotime:C11nvvv1r"/>	<dcterms:created>2011-01-11</dcterms:created>	<dcterms:modified>2012-08-03</dcterms:modified>	<geotime:start>29.853</geotime:start>	<geotime:end>29.74</geotime:end>	<geotime:polarity>R</geotime:polarity>	<geotime:regionName></geotime:regionName>	<dcterms:hasVersion rdf:resource="&history;20120803/geotime#C11nvvv1r"/>	<rdfs:isDefinedBy rdf:resource="&geotime;"/>	<skos:inScheme rdf:resource="&geotime;"/>	<vann:termGroup rdf:resource="&geotime;Magnetostratigraphic"/>	<vs:term_status>unstable</vs:term_status>	</skos:Concept>
<skos:Concept rdf:about="http://rs.gbif.org/terms/geotime#C2Anvvv1n">	<skos:prefLabel xml:lang="en">C2Anvvv1n</skos:prefLabel>	<skos:definition>The C2Anvvv1n magnetostratographic time period started 3.032 million years (Ma) before present (BP) and ended 2.581 Ma BP.</skos:definition>	<rdfs:seeAlso rdf:resource="http://kos.gbif.org/wiki/geotime:C2Anvvv1n"/>	<dcterms:created>2011-01-11</dcterms:created>	<dcterms:modified>2012-08-03</dcterms:modified>	<geotime:start>3.032</geotime:start>	<geotime:end>2.581</geotime:end>	<geotime:polarity>N</geotime:polarity>	<geotime:regionName>Gauss</geotime:regionName>	<dcterms:hasVersion rdf:resource="&history;20120803/geotime#C2Anvvv1n"/>	<rdfs:isDefinedBy rdf:resource="&geotime;"/>	<skos:inScheme rdf:resource="&geotime;"/>	<vann:termGroup rdf:resource="&geotime;Magnetostratigraphic"/>	<vs:term_status>unstable</vs:term_status>	</skos:Concept>
<skos:Concept rdf:about="http://rs.gbif.org/terms/geotime#C2Anvvv1r">	<skos:prefLabel xml:lang="en">C2Anvvv1r</skos:prefLabel>	<skos:definition>The C2Anvvv1r magnetostratographic time period started 3.116 million years (Ma) before present (BP) and ended 3.032 Ma BP.</skos:definition>	<rdfs:seeAlso rdf:resource="http://kos.gbif.org/wiki/geotime:C2Anvvv1r"/>	<dcterms:created>2011-01-11</dcterms:created>	<dcterms:modified>2012-08-03</dcterms:modified>	<geotime:start>3.116</geotime:start>	<geotime:end>3.032</geotime:end>	<geotime:polarity>R</geotime:polarity>	<geotime:regionName>Keana</geotime:regionName>	<dcterms:hasVersion rdf:resource="&history;20120803/geotime#C2Anvvv1r"/>	<rdfs:isDefinedBy rdf:resource="&geotime;"/>	<skos:inScheme rdf:resource="&geotime;"/>	<vann:termGroup rdf:resource="&geotime;Magnetostratigraphic"/>	<vs:term_status>unstable</vs:term_status>	</skos:Concept>
<skos:Concept rdf:about="http://rs.gbif.org/terms/geotime#C2Anvvv2n">	<skos:prefLabel xml:lang="en">C2Anvvv2n</skos:prefLabel>	<skos:definition>The C2Anvvv2n magnetostratographic time period started 3.207 million years (Ma) before present (BP) and ended 3.116 Ma BP.</skos:definition>	<rdfs:seeAlso rdf:resource="http://kos.gbif.org/wiki/geotime:C2Anvvv2n"/>	<dcterms:created>2011-01-11</dcterms:created>	<dcterms:modified>2012-08-03</dcterms:modified>	<geotime:start>3.207</geotime:start>	<geotime:end>3.116</geotime:end>	<geotime:polarity>N</geotime:polarity>	<geotime:regionName></geotime:regionName>	<dcterms:hasVersion rdf:resource="&history;20120803/geotime#C2Anvvv2n"/>	<rdfs:isDefinedBy rdf:resource="&geotime;"/>	<skos:inScheme rdf:resource="&geotime;"/>	<vann:termGroup rdf:resource="&geotime;Magnetostratigraphic"/>	<vs:term_status>unstable</vs:term_status>	</skos:Concept>
<skos:Concept rdf:about="http://rs.gbif.org/terms/geotime#C2Anvvv2r">	<skos:prefLabel xml:lang="en">C2Anvvv2r</skos:prefLabel>	<skos:definition>The C2Anvvv2r magnetostratographic time period started 3.33 million years (Ma) before present (BP) and ended 3.207 Ma BP.</skos:definition>	<rdfs:seeAlso rdf:resource="http://kos.gbif.org/wiki/geotime:C2Anvvv2r"/>	<dcterms:created>2011-01-11</dcterms:created>	<dcterms:modified>2012-08-03</dcterms:modified>	<geotime:start>3.33</geotime:start>	<geotime:end>3.207</geotime:end>	<geotime:polarity>R</geotime:polarity>	<geotime:regionName>Mammoth</geotime:regionName>	<dcterms:hasVersion rdf:resource="&history;20120803/geotime#C2Anvvv2r"/>	<rdfs:isDefinedBy rdf:resource="&geotime;"/>	<skos:inScheme rdf:resource="&geotime;"/>	<vann:termGroup rdf:resource="&geotime;Magnetostratigraphic"/>	<vs:term_status>unstable</vs:term_status>	</skos:Concept>
<skos:Concept rdf:about="http://rs.gbif.org/terms/geotime#C2Anvvv3n">	<skos:prefLabel xml:lang="en">C2Anvvv3n</skos:prefLabel>	<skos:definition>The C2Anvvv3n magnetostratographic time period started 3.596 million years (Ma) before present (BP) and ended 3.33 Ma BP.</skos:definition>	<rdfs:seeAlso rdf:resource="http://kos.gbif.org/wiki/geotime:C2Anvvv3n"/>	<dcterms:created>2011-01-11</dcterms:created>	<dcterms:modified>2012-08-03</dcterms:modified>	<geotime:start>3.596</geotime:start>	<geotime:end>3.33</geotime:end>	<geotime:polarity>N</geotime:polarity>	<geotime:regionName>Gauss continued</geotime:regionName>	<dcterms:hasVersion rdf:resource="&history;20120803/geotime#C2Anvvv3n"/>	<rdfs:isDefinedBy rdf:resource="&geotime;"/>	<skos:inScheme rdf:resource="&geotime;"/>	<vann:termGroup rdf:resource="&geotime;Magnetostratigraphic"/>	<vs:term_status>unstable</vs:term_status>	</skos:Concept>
<skos:Concept rdf:about="http://rs.gbif.org/terms/geotime#C11nvvv2n">	<skos:prefLabel xml:lang="en">C11nvvv2n</skos:prefLabel>	<skos:definition>The C11nvvv2n magnetostratographic time period started 30.217 million years (Ma) before present (BP) and ended 29.853 Ma BP.</skos:definition>	<rdfs:seeAlso rdf:resource="http://kos.gbif.org/wiki/geotime:C11nvvv2n"/>	<dcterms:created>2011-01-11</dcterms:created>	<dcterms:modified>2012-08-03</dcterms:modified>	<geotime:start>30.217</geotime:start>	<geotime:end>29.853</geotime:end>	<geotime:polarity>N</geotime:polarity>	<geotime:regionName></geotime:regionName>	<dcterms:hasVersion rdf:resource="&history;20120803/geotime#C11nvvv2n"/>	<rdfs:isDefinedBy rdf:resource="&geotime;"/>	<skos:inScheme rdf:resource="&geotime;"/>	<vann:termGroup rdf:resource="&geotime;Magnetostratigraphic"/>	<vs:term_status>unstable</vs:term_status>	</skos:Concept>
<skos:Concept rdf:about="http://rs.gbif.org/terms/geotime#C11">	<skos:prefLabel xml:lang="en">C11</skos:prefLabel>	<skos:definition>The C11 magnetostratographic time period started 30.627 million years (Ma) before present (BP) and ended 29.451 Ma BP.</skos:definition>	<rdfs:seeAlso rdf:resource="http://kos.gbif.org/wiki/geotime:C11"/>	<dcterms:created>2011-01-11</dcterms:created>	<dcterms:modified>2012-08-03</dcterms:modified>	<geotime:start>30.627</geotime:start>	<geotime:end>29.451</geotime:end>	<geotime:polarity></geotime:polarity>	<geotime:regionName></geotime:regionName>	<dcterms:hasVersion rdf:resource="&history;20120803/geotime#C11"/>	<rdfs:isDefinedBy rdf:resource="&geotime;"/>	<skos:inScheme rdf:resource="&geotime;"/>	<vann:termGroup rdf:resource="&geotime;Magnetostratigraphic"/>	<vs:term_status>unstable</vs:term_status>	</skos:Concept>
<skos:Concept rdf:about="http://rs.gbif.org/terms/geotime#C11r">	<skos:prefLabel xml:lang="en">C11r</skos:prefLabel>	<skos:definition>The C11r magnetostratographic time period started 30.627 million years (Ma) before present (BP) and ended 30.217 Ma BP.</skos:definition>	<rdfs:seeAlso rdf:resource="http://kos.gbif.org/wiki/geotime:C11r"/>	<dcterms:created>2011-01-11</dcterms:created>	<dcterms:modified>2012-08-03</dcterms:modified>	<geotime:start>30.627</geotime:start>	<geotime:end>30.217</geotime:end>	<geotime:polarity>R</geotime:polarity>	<geotime:regionName></geotime:regionName>	<dcterms:hasVersion rdf:resource="&history;20120803/geotime#C11r"/>	<rdfs:isDefinedBy rdf:resource="&geotime;"/>	<skos:inScheme rdf:resource="&geotime;"/>	<vann:termGroup rdf:resource="&geotime;Magnetostratigraphic"/>	<vs:term_status>unstable</vs:term_status>	</skos:Concept>
<skos:Concept rdf:about="http://rs.gbif.org/terms/geotime#C12n">	<skos:prefLabel xml:lang="en">C12n</skos:prefLabel>	<skos:definition>The C12n magnetostratographic time period started 31.116 million years (Ma) before present (BP) and ended 30.627 Ma BP.</skos:definition>	<rdfs:seeAlso rdf:resource="http://kos.gbif.org/wiki/geotime:C12n"/>	<dcterms:created>2011-01-11</dcterms:created>	<dcterms:modified>2012-08-03</dcterms:modified>	<geotime:start>31.116</geotime:start>	<geotime:end>30.627</geotime:end>	<geotime:polarity>N</geotime:polarity>	<geotime:regionName></geotime:regionName>	<dcterms:hasVersion rdf:resource="&history;20120803/geotime#C12n"/>	<rdfs:isDefinedBy rdf:resource="&geotime;"/>	<skos:inScheme rdf:resource="&geotime;"/>	<vann:termGroup rdf:resource="&geotime;Magnetostratigraphic"/>	<vs:term_status>unstable</vs:term_status>	</skos:Concept>
<skos:Concept rdf:about="http://rs.gbif.org/terms/geotime#C12">	<skos:prefLabel xml:lang="en">C12</skos:prefLabel>	<skos:definition>The C12 magnetostratographic time period started 33.266 million years (Ma) before present (BP) and ended 30.627 Ma BP.</skos:definition>	<rdfs:seeAlso rdf:resource="http://kos.gbif.org/wiki/geotime:C12"/>	<dcterms:created>2011-01-11</dcterms:created>	<dcterms:modified>2012-08-03</dcterms:modified>	<geotime:start>33.266</geotime:start>	<geotime:end>30.627</geotime:end>	<geotime:polarity></geotime:polarity>	<geotime:regionName></geotime:regionName>	<dcterms:hasVersion rdf:resource="&history;20120803/geotime#C12"/>	<rdfs:isDefinedBy rdf:resource="&geotime;"/>	<skos:inScheme rdf:resource="&geotime;"/>	<vann:termGroup rdf:resource="&geotime;Magnetostratigraphic"/>	<vs:term_status>unstable</vs:term_status>	</skos:Concept>
<skos:Concept rdf:about="http://rs.gbif.org/terms/geotime#C12r">	<skos:prefLabel xml:lang="en">C12r</skos:prefLabel>	<skos:definition>The C12r magnetostratographic time period started 33.266 million years (Ma) before present (BP) and ended 31.116 Ma BP.</skos:definition>	<rdfs:seeAlso rdf:resource="http://kos.gbif.org/wiki/geotime:C12r"/>	<dcterms:created>2011-01-11</dcterms:created>	<dcterms:modified>2012-08-03</dcterms:modified>	<geotime:start>33.266</geotime:start>	<geotime:end>31.116</geotime:end>	<geotime:polarity>R</geotime:polarity>	<geotime:regionName></geotime:regionName>	<dcterms:hasVersion rdf:resource="&history;20120803/geotime#C12r"/>	<rdfs:isDefinedBy rdf:resource="&geotime;"/>	<skos:inScheme rdf:resource="&geotime;"/>	<vann:termGroup rdf:resource="&geotime;Magnetostratigraphic"/>	<vs:term_status>unstable</vs:term_status>	</skos:Concept>
<skos:Concept rdf:about="http://rs.gbif.org/terms/geotime#C13n">	<skos:prefLabel xml:lang="en">C13n</skos:prefLabel>	<skos:definition>The C13n magnetostratographic time period started 33.738 million years (Ma) before present (BP) and ended 33.266 Ma BP.</skos:definition>	<rdfs:seeAlso rdf:resource="http://kos.gbif.org/wiki/geotime:C13n"/>	<dcterms:created>2011-01-11</dcterms:created>	<dcterms:modified>2012-08-03</dcterms:modified>	<geotime:start>33.738</geotime:start>	<geotime:end>33.266</geotime:end>	<geotime:polarity>N</geotime:polarity>	<geotime:regionName></geotime:regionName>	<dcterms:hasVersion rdf:resource="&history;20120803/geotime#C13n"/>	<rdfs:isDefinedBy rdf:resource="&geotime;"/>	<skos:inScheme rdf:resource="&geotime;"/>	<vann:termGroup rdf:resource="&geotime;Magnetostratigraphic"/>	<vs:term_status>unstable</vs:term_status>	</skos:Concept>
<skos:Concept rdf:about="http://rs.gbif.org/terms/geotime#C13">	<skos:prefLabel xml:lang="en">C13</skos:prefLabel>	<skos:definition>The C13 magnetostratographic time period started 34.782 million years (Ma) before present (BP) and ended 33.266 Ma BP.</skos:definition>	<rdfs:seeAlso rdf:resource="http://kos.gbif.org/wiki/geotime:C13"/>	<dcterms:created>2011-01-11</dcterms:created>	<dcterms:modified>2012-08-03</dcterms:modified>	<geotime:start>34.782</geotime:start>	<geotime:end>33.266</geotime:end>	<geotime:polarity></geotime:polarity>	<geotime:regionName></geotime:regionName>	<dcterms:hasVersion rdf:resource="&history;20120803/geotime#C13"/>	<rdfs:isDefinedBy rdf:resource="&geotime;"/>	<skos:inScheme rdf:resource="&geotime;"/>	<vann:termGroup rdf:resource="&geotime;Magnetostratigraphic"/>	<vs:term_status>unstable</vs:term_status>	</skos:Concept>
<skos:Concept rdf:about="http://rs.gbif.org/terms/geotime#C13r">	<skos:prefLabel xml:lang="en">C13r</skos:prefLabel>	<skos:definition>The C13r magnetostratographic time period started 34.782 million years (Ma) before present (BP) and ended 33.738 Ma BP.</skos:definition>	<rdfs:seeAlso rdf:resource="http://kos.gbif.org/wiki/geotime:C13r"/>	<dcterms:created>2011-01-11</dcterms:created>	<dcterms:modified>2012-08-03</dcterms:modified>	<geotime:start>34.782</geotime:start>	<geotime:end>33.738</geotime:end>	<geotime:polarity>R</geotime:polarity>	<geotime:regionName></geotime:regionName>	<dcterms:hasVersion rdf:resource="&history;20120803/geotime#C13r"/>	<rdfs:isDefinedBy rdf:resource="&geotime;"/>	<skos:inScheme rdf:resource="&geotime;"/>	<vann:termGroup rdf:resource="&geotime;Magnetostratigraphic"/>	<vs:term_status>unstable</vs:term_status>	</skos:Concept>
<skos:Concept rdf:about="http://rs.gbif.org/terms/geotime#C15n">	<skos:prefLabel xml:lang="en">C15n</skos:prefLabel>	<skos:definition>The C15n magnetostratographic time period started 35.043 million years (Ma) before present (BP) and ended 34.782 Ma BP.</skos:definition>	<rdfs:seeAlso rdf:resource="http://kos.gbif.org/wiki/geotime:C15n"/>	<dcterms:created>2011-01-11</dcterms:created>	<dcterms:modified>2012-08-03</dcterms:modified>	<geotime:start>35.043</geotime:start>	<geotime:end>34.782</geotime:end>	<geotime:polarity>N</geotime:polarity>	<geotime:regionName></geotime:regionName>	<dcterms:hasVersion rdf:resource="&history;20120803/geotime#C15n"/>	<rdfs:isDefinedBy rdf:resource="&geotime;"/>	<skos:inScheme rdf:resource="&geotime;"/>	<vann:termGroup rdf:resource="&geotime;Magnetostratigraphic"/>	<vs:term_status>unstable</vs:term_status>	</skos:Concept>
<skos:Concept rdf:about="http://rs.gbif.org/terms/geotime#C15">	<skos:prefLabel xml:lang="en">C15</skos:prefLabel>	<skos:definition>The C15 magnetostratographic time period started 35.404 million years (Ma) before present (BP) and ended 34.782 Ma BP.</skos:definition>	<rdfs:seeAlso rdf:resource="http://kos.gbif.org/wiki/geotime:C15"/>	<dcterms:created>2011-01-11</dcterms:created>	<dcterms:modified>2012-08-03</dcterms:modified>	<geotime:start>35.404</geotime:start>	<geotime:end>34.782</geotime:end>	<geotime:polarity></geotime:polarity>	<geotime:regionName></geotime:regionName>	<dcterms:hasVersion rdf:resource="&history;20120803/geotime#C15"/>	<rdfs:isDefinedBy rdf:resource="&geotime;"/>	<skos:inScheme rdf:resource="&geotime;"/>	<vann:termGroup rdf:resource="&geotime;Magnetostratigraphic"/>	<vs:term_status>unstable</vs:term_status>	</skos:Concept>
<skos:Concept rdf:about="http://rs.gbif.org/terms/geotime#C15r">	<skos:prefLabel xml:lang="en">C15r</skos:prefLabel>	<skos:definition>The C15r magnetostratographic time period started 35.404 million years (Ma) before present (BP) and ended 35.043 Ma BP.</skos:definition>	<rdfs:seeAlso rdf:resource="http://kos.gbif.org/wiki/geotime:C15r"/>	<dcterms:created>2011-01-11</dcterms:created>	<dcterms:modified>2012-08-03</dcterms:modified>	<geotime:start>35.404</geotime:start>	<geotime:end>35.043</geotime:end>	<geotime:polarity>R</geotime:polarity>	<geotime:regionName></geotime:regionName>	<dcterms:hasVersion rdf:resource="&history;20120803/geotime#C15r"/>	<rdfs:isDefinedBy rdf:resource="&geotime;"/>	<skos:inScheme rdf:resource="&geotime;"/>	<vann:termGroup rdf:resource="&geotime;Magnetostratigraphic"/>	<vs:term_status>unstable</vs:term_status>	</skos:Concept>
<skos:Concept rdf:about="http://rs.gbif.org/terms/geotime#C16nvvv1n">	<skos:prefLabel xml:lang="en">C16nvvv1n</skos:prefLabel>	<skos:definition>The C16nvvv1n magnetostratographic time period started 35.567 million years (Ma) before present (BP) and ended 35.404 Ma BP.</skos:definition>	<rdfs:seeAlso rdf:resource="http://kos.gbif.org/wiki/geotime:C16nvvv1n"/>	<dcterms:created>2011-01-11</dcterms:created>	<dcterms:modified>2012-08-03</dcterms:modified>	<geotime:start>35.567</geotime:start>	<geotime:end>35.404</geotime:end>	<geotime:polarity>N</geotime:polarity>	<geotime:regionName></geotime:regionName>	<dcterms:hasVersion rdf:resource="&history;20120803/geotime#C16nvvv1n"/>	<rdfs:isDefinedBy rdf:resource="&geotime;"/>	<skos:inScheme rdf:resource="&geotime;"/>	<vann:termGroup rdf:resource="&geotime;Magnetostratigraphic"/>	<vs:term_status>unstable</vs:term_status>	</skos:Concept>
<skos:Concept rdf:about="http://rs.gbif.org/terms/geotime#C16nvvv1r">	<skos:prefLabel xml:lang="en">C16nvvv1r</skos:prefLabel>	<skos:definition>The C16nvvv1r magnetostratographic time period started 35.707 million years (Ma) before present (BP) and ended 35.567 Ma BP.</skos:definition>	<rdfs:seeAlso rdf:resource="http://kos.gbif.org/wiki/geotime:C16nvvv1r"/>	<dcterms:created>2011-01-11</dcterms:created>	<dcterms:modified>2012-08-03</dcterms:modified>	<geotime:start>35.707</geotime:start>	<geotime:end>35.567</geotime:end>	<geotime:polarity>R</geotime:polarity>	<geotime:regionName></geotime:regionName>	<dcterms:hasVersion rdf:resource="&history;20120803/geotime#C16nvvv1r"/>	<rdfs:isDefinedBy rdf:resource="&geotime;"/>	<skos:inScheme rdf:resource="&geotime;"/>	<vann:termGroup rdf:resource="&geotime;Magnetostratigraphic"/>	<vs:term_status>unstable</vs:term_status>	</skos:Concept>
<skos:Concept rdf:about="http://rs.gbif.org/terms/geotime#C16nvvv2n">	<skos:prefLabel xml:lang="en">C16nvvv2n</skos:prefLabel>	<skos:definition>The C16nvvv2n magnetostratographic time period started 36.276 million years (Ma) before present (BP) and ended 35.707 Ma BP.</skos:definition>	<rdfs:seeAlso rdf:resource="http://kos.gbif.org/wiki/geotime:C16nvvv2n"/>	<dcterms:created>2011-01-11</dcterms:created>	<dcterms:modified>2012-08-03</dcterms:modified>	<geotime:start>36.276</geotime:start>	<geotime:end>35.707</geotime:end>	<geotime:polarity>N</geotime:polarity>	<geotime:regionName></geotime:regionName>	<dcterms:hasVersion rdf:resource="&history;20120803/geotime#C16nvvv2n"/>	<rdfs:isDefinedBy rdf:resource="&geotime;"/>	<skos:inScheme rdf:resource="&geotime;"/>	<vann:termGroup rdf:resource="&geotime;Magnetostratigraphic"/>	<vs:term_status>unstable</vs:term_status>	</skos:Concept>
<skos:Concept rdf:about="http://rs.gbif.org/terms/geotime#C16">	<skos:prefLabel xml:lang="en">C16</skos:prefLabel>	<skos:definition>The C16 magnetostratographic time period started 36.512 million years (Ma) before present (BP) and ended 35.404 Ma BP.</skos:definition>	<rdfs:seeAlso rdf:resource="http://kos.gbif.org/wiki/geotime:C16"/>	<dcterms:created>2011-01-11</dcterms:created>	<dcterms:modified>2012-08-03</dcterms:modified>	<geotime:start>36.512</geotime:start>	<geotime:end>35.404</geotime:end>	<geotime:polarity></geotime:polarity>	<geotime:regionName></geotime:regionName>	<dcterms:hasVersion rdf:resource="&history;20120803/geotime#C16"/>	<rdfs:isDefinedBy rdf:resource="&geotime;"/>	<skos:inScheme rdf:resource="&geotime;"/>	<vann:termGroup rdf:resource="&geotime;Magnetostratigraphic"/>	<vs:term_status>unstable</vs:term_status>	</skos:Concept>
<skos:Concept rdf:about="http://rs.gbif.org/terms/geotime#C16r">	<skos:prefLabel xml:lang="en">C16r</skos:prefLabel>	<skos:definition>The C16r magnetostratographic time period started 36.512 million years (Ma) before present (BP) and ended 36.276 Ma BP.</skos:definition>	<rdfs:seeAlso rdf:resource="http://kos.gbif.org/wiki/geotime:C16r"/>	<dcterms:created>2011-01-11</dcterms:created>	<dcterms:modified>2012-08-03</dcterms:modified>	<geotime:start>36.512</geotime:start>	<geotime:end>36.276</geotime:end>	<geotime:polarity>R</geotime:polarity>	<geotime:regionName></geotime:regionName>	<dcterms:hasVersion rdf:resource="&history;20120803/geotime#C16r"/>	<rdfs:isDefinedBy rdf:resource="&geotime;"/>	<skos:inScheme rdf:resource="&geotime;"/>	<vann:termGroup rdf:resource="&geotime;Magnetostratigraphic"/>	<vs:term_status>unstable</vs:term_status>	</skos:Concept>
<skos:Concept rdf:about="http://rs.gbif.org/terms/geotime#C17nvvv1n">	<skos:prefLabel xml:lang="en">C17nvvv1n</skos:prefLabel>	<skos:definition>The C17nvvv1n magnetostratographic time period started 37.235 million years (Ma) before present (BP) and ended 36.512 Ma BP.</skos:definition>	<rdfs:seeAlso rdf:resource="http://kos.gbif.org/wiki/geotime:C17nvvv1n"/>	<dcterms:created>2011-01-11</dcterms:created>	<dcterms:modified>2012-08-03</dcterms:modified>	<geotime:start>37.235</geotime:start>	<geotime:end>36.512</geotime:end>	<geotime:polarity>N</geotime:polarity>	<geotime:regionName></geotime:regionName>	<dcterms:hasVersion rdf:resource="&history;20120803/geotime#C17nvvv1n"/>	<rdfs:isDefinedBy rdf:resource="&geotime;"/>	<skos:inScheme rdf:resource="&geotime;"/>	<vann:termGroup rdf:resource="&geotime;Magnetostratigraphic"/>	<vs:term_status>unstable</vs:term_status>	</skos:Concept>
<skos:Concept rdf:about="http://rs.gbif.org/terms/geotime#C17nvvv1r">	<skos:prefLabel xml:lang="en">C17nvvv1r</skos:prefLabel>	<skos:definition>The C17nvvv1r magnetostratographic time period started 37.345 million years (Ma) before present (BP) and ended 37.235 Ma BP.</skos:definition>	<rdfs:seeAlso rdf:resource="http://kos.gbif.org/wiki/geotime:C17nvvv1r"/>	<dcterms:created>2011-01-11</dcterms:created>	<dcterms:modified>2012-08-03</dcterms:modified>	<geotime:start>37.345</geotime:start>	<geotime:end>37.235</geotime:end>	<geotime:polarity>R</geotime:polarity>	<geotime:regionName></geotime:regionName>	<dcterms:hasVersion rdf:resource="&history;20120803/geotime#C17nvvv1r"/>	<rdfs:isDefinedBy rdf:resource="&geotime;"/>	<skos:inScheme rdf:resource="&geotime;"/>	<vann:termGroup rdf:resource="&geotime;Magnetostratigraphic"/>	<vs:term_status>unstable</vs:term_status>	</skos:Concept>
<skos:Concept rdf:about="http://rs.gbif.org/terms/geotime#C17nvvv2n">	<skos:prefLabel xml:lang="en">C17nvvv2n</skos:prefLabel>	<skos:definition>The C17nvvv2n magnetostratographic time period started 37.549 million years (Ma) before present (BP) and ended 37.345 Ma BP.</skos:definition>	<rdfs:seeAlso rdf:resource="http://kos.gbif.org/wiki/geotime:C17nvvv2n"/>	<dcterms:created>2011-01-11</dcterms:created>	<dcterms:modified>2012-08-03</dcterms:modified>	<geotime:start>37.549</geotime:start>	<geotime:end>37.345</geotime:end>	<geotime:polarity>N</geotime:polarity>	<geotime:regionName></geotime:regionName>	<dcterms:hasVersion rdf:resource="&history;20120803/geotime#C17nvvv2n"/>	<rdfs:isDefinedBy rdf:resource="&geotime;"/>	<skos:inScheme rdf:resource="&geotime;"/>	<vann:termGroup rdf:resource="&geotime;Magnetostratigraphic"/>	<vs:term_status>unstable</vs:term_status>	</skos:Concept>
<skos:Concept rdf:about="http://rs.gbif.org/terms/geotime#C17nvvv2r">	<skos:prefLabel xml:lang="en">C17nvvv2r</skos:prefLabel>	<skos:definition>The C17nvvv2r magnetostratographic time period started 37.61 million years (Ma) before present (BP) and ended 37.549 Ma BP.</skos:definition>	<rdfs:seeAlso rdf:resource="http://kos.gbif.org/wiki/geotime:C17nvvv2r"/>	<dcterms:created>2011-01-11</dcterms:created>	<dcterms:modified>2012-08-03</dcterms:modified>	<geotime:start>37.61</geotime:start>	<geotime:end>37.549</geotime:end>	<geotime:polarity>R</geotime:polarity>	<geotime:regionName></geotime:regionName>	<dcterms:hasVersion rdf:resource="&history;20120803/geotime#C17nvvv2r"/>	<rdfs:isDefinedBy rdf:resource="&geotime;"/>	<skos:inScheme rdf:resource="&geotime;"/>	<vann:termGroup rdf:resource="&geotime;Magnetostratigraphic"/>	<vs:term_status>unstable</vs:term_status>	</skos:Concept>
<skos:Concept rdf:about="http://rs.gbif.org/terms/geotime#C17nvvv3n">	<skos:prefLabel xml:lang="en">C17nvvv3n</skos:prefLabel>	<skos:definition>The C17nvvv3n magnetostratographic time period started 37.771 million years (Ma) before present (BP) and ended 37.61 Ma BP.</skos:definition>	<rdfs:seeAlso rdf:resource="http://kos.gbif.org/wiki/geotime:C17nvvv3n"/>	<dcterms:created>2011-01-11</dcterms:created>	<dcterms:modified>2012-08-03</dcterms:modified>	<geotime:start>37.771</geotime:start>	<geotime:end>37.61</geotime:end>	<geotime:polarity>N</geotime:polarity>	<geotime:regionName></geotime:regionName>	<dcterms:hasVersion rdf:resource="&history;20120803/geotime#C17nvvv3n"/>	<rdfs:isDefinedBy rdf:resource="&geotime;"/>	<skos:inScheme rdf:resource="&geotime;"/>	<vann:termGroup rdf:resource="&geotime;Magnetostratigraphic"/>	<vs:term_status>unstable</vs:term_status>	</skos:Concept>
<skos:Concept rdf:about="http://rs.gbif.org/terms/geotime#C17">	<skos:prefLabel xml:lang="en">C17</skos:prefLabel>	<skos:definition>The C17 magnetostratographic time period started 38.032 million years (Ma) before present (BP) and ended 36.512 Ma BP.</skos:definition>	<rdfs:seeAlso rdf:resource="http://kos.gbif.org/wiki/geotime:C17"/>	<dcterms:created>2011-01-11</dcterms:created>	<dcterms:modified>2012-08-03</dcterms:modified>	<geotime:start>38.032</geotime:start>	<geotime:end>36.512</geotime:end>	<geotime:polarity></geotime:polarity>	<geotime:regionName></geotime:regionName>	<dcterms:hasVersion rdf:resource="&history;20120803/geotime#C17"/>	<rdfs:isDefinedBy rdf:resource="&geotime;"/>	<skos:inScheme rdf:resource="&geotime;"/>	<vann:termGroup rdf:resource="&geotime;Magnetostratigraphic"/>	<vs:term_status>unstable</vs:term_status>	</skos:Concept>
<skos:Concept rdf:about="http://rs.gbif.org/terms/geotime#C17r">	<skos:prefLabel xml:lang="en">C17r</skos:prefLabel>	<skos:definition>The C17r magnetostratographic time period started 38.032 million years (Ma) before present (BP) and ended 37.771 Ma BP.</skos:definition>	<rdfs:seeAlso rdf:resource="http://kos.gbif.org/wiki/geotime:C17r"/>	<dcterms:created>2011-01-11</dcterms:created>	<dcterms:modified>2012-08-03</dcterms:modified>	<geotime:start>38.032</geotime:start>	<geotime:end>37.771</geotime:end>	<geotime:polarity>R</geotime:polarity>	<geotime:regionName></geotime:regionName>	<dcterms:hasVersion rdf:resource="&history;20120803/geotime#C17r"/>	<rdfs:isDefinedBy rdf:resource="&geotime;"/>	<skos:inScheme rdf:resource="&geotime;"/>	<vann:termGroup rdf:resource="&geotime;Magnetostratigraphic"/>	<vs:term_status>unstable</vs:term_status>	</skos:Concept>
<skos:Concept rdf:about="http://rs.gbif.org/terms/geotime#C18nvvv1n">	<skos:prefLabel xml:lang="en">C18nvvv1n</skos:prefLabel>	<skos:definition>The C18nvvv1n magnetostratographic time period started 38.975 million years (Ma) before present (BP) and ended 38.032 Ma BP.</skos:definition>	<rdfs:seeAlso rdf:resource="http://kos.gbif.org/wiki/geotime:C18nvvv1n"/>	<dcterms:created>2011-01-11</dcterms:created>	<dcterms:modified>2012-08-03</dcterms:modified>	<geotime:start>38.975</geotime:start>	<geotime:end>38.032</geotime:end>	<geotime:polarity>N</geotime:polarity>	<geotime:regionName></geotime:regionName>	<dcterms:hasVersion rdf:resource="&history;20120803/geotime#C18nvvv1n"/>	<rdfs:isDefinedBy rdf:resource="&geotime;"/>	<skos:inScheme rdf:resource="&geotime;"/>	<vann:termGroup rdf:resource="&geotime;Magnetostratigraphic"/>	<vs:term_status>unstable</vs:term_status>	</skos:Concept>
<skos:Concept rdf:about="http://rs.gbif.org/terms/geotime#C18nvvv1r">	<skos:prefLabel xml:lang="en">C18nvvv1r</skos:prefLabel>	<skos:definition>The C18nvvv1r magnetostratographic time period started 39.041 million years (Ma) before present (BP) and ended 38.975 Ma BP.</skos:definition>	<rdfs:seeAlso rdf:resource="http://kos.gbif.org/wiki/geotime:C18nvvv1r"/>	<dcterms:created>2011-01-11</dcterms:created>	<dcterms:modified>2012-08-03</dcterms:modified>	<geotime:start>39.041</geotime:start>	<geotime:end>38.975</geotime:end>	<geotime:polarity>R</geotime:polarity>	<geotime:regionName></geotime:regionName>	<dcterms:hasVersion rdf:resource="&history;20120803/geotime#C18nvvv1r"/>	<rdfs:isDefinedBy rdf:resource="&geotime;"/>	<skos:inScheme rdf:resource="&geotime;"/>	<vann:termGroup rdf:resource="&geotime;Magnetostratigraphic"/>	<vs:term_status>unstable</vs:term_status>	</skos:Concept>
<skos:Concept rdf:about="http://rs.gbif.org/terms/geotime#C18nvvv2n">	<skos:prefLabel xml:lang="en">C18nvvv2n</skos:prefLabel>	<skos:definition>The C18nvvv2n magnetostratographic time period started 39.464 million years (Ma) before present (BP) and ended 39.041 Ma BP.</skos:definition>	<rdfs:seeAlso rdf:resource="http://kos.gbif.org/wiki/geotime:C18nvvv2n"/>	<dcterms:created>2011-01-11</dcterms:created>	<dcterms:modified>2012-08-03</dcterms:modified>	<geotime:start>39.464</geotime:start>	<geotime:end>39.041</geotime:end>	<geotime:polarity>N</geotime:polarity>	<geotime:regionName></geotime:regionName>	<dcterms:hasVersion rdf:resource="&history;20120803/geotime#C18nvvv2n"/>	<rdfs:isDefinedBy rdf:resource="&geotime;"/>	<skos:inScheme rdf:resource="&geotime;"/>	<vann:termGroup rdf:resource="&geotime;Magnetostratigraphic"/>	<vs:term_status>unstable</vs:term_status>	</skos:Concept>
<skos:Concept rdf:about="http://rs.gbif.org/terms/geotime#C2A">	<skos:prefLabel xml:lang="en">C2A</skos:prefLabel>	<skos:definition>The C2A magnetostratographic time period started 4.187 million years (Ma) before present (BP) and ended 2.581 Ma BP.</skos:definition>	<rdfs:seeAlso rdf:resource="http://kos.gbif.org/wiki/geotime:C2A"/>	<dcterms:created>2011-01-11</dcterms:created>	<dcterms:modified>2012-08-03</dcterms:modified>	<geotime:start>4.187</geotime:start>	<geotime:end>2.581</geotime:end>	<geotime:polarity></geotime:polarity>	<geotime:regionName></geotime:regionName>	<dcterms:hasVersion rdf:resource="&history;20120803/geotime#C2A"/>	<rdfs:isDefinedBy rdf:resource="&geotime;"/>	<skos:inScheme rdf:resource="&geotime;"/>	<vann:termGroup rdf:resource="&geotime;Magnetostratigraphic"/>	<vs:term_status>unstable</vs:term_status>	</skos:Concept>
<skos:Concept rdf:about="http://rs.gbif.org/terms/geotime#C2Ar">	<skos:prefLabel xml:lang="en">C2Ar</skos:prefLabel>	<skos:definition>The C2Ar magnetostratographic time period started 4.187 million years (Ma) before present (BP) and ended 3.596 Ma BP.</skos:definition>	<rdfs:seeAlso rdf:resource="http://kos.gbif.org/wiki/geotime:C2Ar"/>	<dcterms:created>2011-01-11</dcterms:created>	<dcterms:modified>2012-08-03</dcterms:modified>	<geotime:start>4.187</geotime:start>	<geotime:end>3.596</geotime:end>	<geotime:polarity>R</geotime:polarity>	<geotime:regionName>Gilbert</geotime:regionName>	<dcterms:hasVersion rdf:resource="&history;20120803/geotime#C2Ar"/>	<rdfs:isDefinedBy rdf:resource="&geotime;"/>	<skos:inScheme rdf:resource="&geotime;"/>	<vann:termGroup rdf:resource="&geotime;Magnetostratigraphic"/>	<vs:term_status>unstable</vs:term_status>	</skos:Concept>
<skos:Concept rdf:about="http://rs.gbif.org/terms/geotime#C3nvvv1n">	<skos:prefLabel xml:lang="en">C3nvvv1n</skos:prefLabel>	<skos:definition>The C3nvvv1n magnetostratographic time period started 4.3 million years (Ma) before present (BP) and ended 4.187 Ma BP.</skos:definition>	<rdfs:seeAlso rdf:resource="http://kos.gbif.org/wiki/geotime:C3nvvv1n"/>	<dcterms:created>2011-01-11</dcterms:created>	<dcterms:modified>2012-08-03</dcterms:modified>	<geotime:start>4.3</geotime:start>	<geotime:end>4.187</geotime:end>	<geotime:polarity>N</geotime:polarity>	<geotime:regionName>Cochiti</geotime:regionName>	<dcterms:hasVersion rdf:resource="&history;20120803/geotime#C3nvvv1n"/>	<rdfs:isDefinedBy rdf:resource="&geotime;"/>	<skos:inScheme rdf:resource="&geotime;"/>	<vann:termGroup rdf:resource="&geotime;Magnetostratigraphic"/>	<vs:term_status>unstable</vs:term_status>	</skos:Concept>
<skos:Concept rdf:about="http://rs.gbif.org/terms/geotime#C3nvvv1r">	<skos:prefLabel xml:lang="en">C3nvvv1r</skos:prefLabel>	<skos:definition>The C3nvvv1r magnetostratographic time period started 4.493 million years (Ma) before present (BP) and ended 4.3 Ma BP.</skos:definition>	<rdfs:seeAlso rdf:resource="http://kos.gbif.org/wiki/geotime:C3nvvv1r"/>	<dcterms:created>2011-01-11</dcterms:created>	<dcterms:modified>2012-08-03</dcterms:modified>	<geotime:start>4.493</geotime:start>	<geotime:end>4.3</geotime:end>	<geotime:polarity>R</geotime:polarity>	<geotime:regionName></geotime:regionName>	<dcterms:hasVersion rdf:resource="&history;20120803/geotime#C3nvvv1r"/>	<rdfs:isDefinedBy rdf:resource="&geotime;"/>	<skos:inScheme rdf:resource="&geotime;"/>	<vann:termGroup rdf:resource="&geotime;Magnetostratigraphic"/>	<vs:term_status>unstable</vs:term_status>	</skos:Concept>
<skos:Concept rdf:about="http://rs.gbif.org/terms/geotime#C3nvvv2n">	<skos:prefLabel xml:lang="en">C3nvvv2n</skos:prefLabel>	<skos:definition>The C3nvvv2n magnetostratographic time period started 4.631 million years (Ma) before present (BP) and ended 4.493 Ma BP.</skos:definition>	<rdfs:seeAlso rdf:resource="http://kos.gbif.org/wiki/geotime:C3nvvv2n"/>	<dcterms:created>2011-01-11</dcterms:created>	<dcterms:modified>2012-08-03</dcterms:modified>	<geotime:start>4.631</geotime:start>	<geotime:end>4.493</geotime:end>	<geotime:polarity>N</geotime:polarity>	<geotime:regionName>Nunivak</geotime:regionName>	<dcterms:hasVersion rdf:resource="&history;20120803/geotime#C3nvvv2n"/>	<rdfs:isDefinedBy rdf:resource="&geotime;"/>	<skos:inScheme rdf:resource="&geotime;"/>	<vann:termGroup rdf:resource="&geotime;Magnetostratigraphic"/>	<vs:term_status>unstable</vs:term_status>	</skos:Concept>
<skos:Concept rdf:about="http://rs.gbif.org/terms/geotime#C3nvvv2r">	<skos:prefLabel xml:lang="en">C3nvvv2r</skos:prefLabel>	<skos:definition>The C3nvvv2r magnetostratographic time period started 4.799 million years (Ma) before present (BP) and ended 4.631 Ma BP.</skos:definition>	<rdfs:seeAlso rdf:resource="http://kos.gbif.org/wiki/geotime:C3nvvv2r"/>	<dcterms:created>2011-01-11</dcterms:created>	<dcterms:modified>2012-08-03</dcterms:modified>	<geotime:start>4.799</geotime:start>	<geotime:end>4.631</geotime:end>	<geotime:polarity>R</geotime:polarity>	<geotime:regionName></geotime:regionName>	<dcterms:hasVersion rdf:resource="&history;20120803/geotime#C3nvvv2r"/>	<rdfs:isDefinedBy rdf:resource="&geotime;"/>	<skos:inScheme rdf:resource="&geotime;"/>	<vann:termGroup rdf:resource="&geotime;Magnetostratigraphic"/>	<vs:term_status>unstable</vs:term_status>	</skos:Concept>
<skos:Concept rdf:about="http://rs.gbif.org/terms/geotime#C3nvvv3n">	<skos:prefLabel xml:lang="en">C3nvvv3n</skos:prefLabel>	<skos:definition>The C3nvvv3n magnetostratographic time period started 4.896 million years (Ma) before present (BP) and ended 4.799 Ma BP.</skos:definition>	<rdfs:seeAlso rdf:resource="http://kos.gbif.org/wiki/geotime:C3nvvv3n"/>	<dcterms:created>2011-01-11</dcterms:created>	<dcterms:modified>2012-08-03</dcterms:modified>	<geotime:start>4.896</geotime:start>	<geotime:end>4.799</geotime:end>	<geotime:polarity>N</geotime:polarity>	<geotime:regionName>Sidufjall</geotime:regionName>	<dcterms:hasVersion rdf:resource="&history;20120803/geotime#C3nvvv3n"/>	<rdfs:isDefinedBy rdf:resource="&geotime;"/>	<skos:inScheme rdf:resource="&geotime;"/>	<vann:termGroup rdf:resource="&geotime;Magnetostratigraphic"/>	<vs:term_status>unstable</vs:term_status>	</skos:Concept>
<skos:Concept rdf:about="http://rs.gbif.org/terms/geotime#C3nvvv3r">	<skos:prefLabel xml:lang="en">C3nvvv3r</skos:prefLabel>	<skos:definition>The C3nvvv3r magnetostratographic time period started 4.997 million years (Ma) before present (BP) and ended 4.896 Ma BP.</skos:definition>	<rdfs:seeAlso rdf:resource="http://kos.gbif.org/wiki/geotime:C3nvvv3r"/>	<dcterms:created>2011-01-11</dcterms:created>	<dcterms:modified>2012-08-03</dcterms:modified>	<geotime:start>4.997</geotime:start>	<geotime:end>4.896</geotime:end>	<geotime:polarity>R</geotime:polarity>	<geotime:regionName></geotime:regionName>	<dcterms:hasVersion rdf:resource="&history;20120803/geotime#C3nvvv3r"/>	<rdfs:isDefinedBy rdf:resource="&geotime;"/>	<skos:inScheme rdf:resource="&geotime;"/>	<vann:termGroup rdf:resource="&geotime;Magnetostratigraphic"/>	<vs:term_status>unstable</vs:term_status>	</skos:Concept>
<skos:Concept rdf:about="http://rs.gbif.org/terms/geotime#C18">	<skos:prefLabel xml:lang="en">C18</skos:prefLabel>	<skos:definition>The C18 magnetostratographic time period started 40.439 million years (Ma) before present (BP) and ended 38.032 Ma BP.</skos:definition>	<rdfs:seeAlso rdf:resource="http://kos.gbif.org/wiki/geotime:C18"/>	<dcterms:created>2011-01-11</dcterms:created>	<dcterms:modified>2012-08-03</dcterms:modified>	<geotime:start>40.439</geotime:start>	<geotime:end>38.032</geotime:end>	<geotime:polarity></geotime:polarity>	<geotime:regionName></geotime:regionName>	<dcterms:hasVersion rdf:resource="&history;20120803/geotime#C18"/>	<rdfs:isDefinedBy rdf:resource="&geotime;"/>	<skos:inScheme rdf:resource="&geotime;"/>	<vann:termGroup rdf:resource="&geotime;Magnetostratigraphic"/>	<vs:term_status>unstable</vs:term_status>	</skos:Concept>
<skos:Concept rdf:about="http://rs.gbif.org/terms/geotime#C18r">	<skos:prefLabel xml:lang="en">C18r</skos:prefLabel>	<skos:definition>The C18r magnetostratographic time period started 40.439 million years (Ma) before present (BP) and ended 39.464 Ma BP.</skos:definition>	<rdfs:seeAlso rdf:resource="http://kos.gbif.org/wiki/geotime:C18r"/>	<dcterms:created>2011-01-11</dcterms:created>	<dcterms:modified>2012-08-03</dcterms:modified>	<geotime:start>40.439</geotime:start>	<geotime:end>39.464</geotime:end>	<geotime:polarity>R</geotime:polarity>	<geotime:regionName></geotime:regionName>	<dcterms:hasVersion rdf:resource="&history;20120803/geotime#C18r"/>	<rdfs:isDefinedBy rdf:resource="&geotime;"/>	<skos:inScheme rdf:resource="&geotime;"/>	<vann:termGroup rdf:resource="&geotime;Magnetostratigraphic"/>	<vs:term_status>unstable</vs:term_status>	</skos:Concept>
<skos:Concept rdf:about="http://rs.gbif.org/terms/geotime#C19n">	<skos:prefLabel xml:lang="en">C19n</skos:prefLabel>	<skos:definition>The C19n magnetostratographic time period started 40.671 million years (Ma) before present (BP) and ended 40.439 Ma BP.</skos:definition>	<rdfs:seeAlso rdf:resource="http://kos.gbif.org/wiki/geotime:C19n"/>	<dcterms:created>2011-01-11</dcterms:created>	<dcterms:modified>2012-08-03</dcterms:modified>	<geotime:start>40.671</geotime:start>	<geotime:end>40.439</geotime:end>	<geotime:polarity>N</geotime:polarity>	<geotime:regionName></geotime:regionName>	<dcterms:hasVersion rdf:resource="&history;20120803/geotime#C19n"/>	<rdfs:isDefinedBy rdf:resource="&geotime;"/>	<skos:inScheme rdf:resource="&geotime;"/>	<vann:termGroup rdf:resource="&geotime;Magnetostratigraphic"/>	<vs:term_status>unstable</vs:term_status>	</skos:Concept>
<skos:Concept rdf:about="http://rs.gbif.org/terms/geotime#C19">	<skos:prefLabel xml:lang="en">C19</skos:prefLabel>	<skos:definition>The C19 magnetostratographic time period started 41.59 million years (Ma) before present (BP) and ended 40.439 Ma BP.</skos:definition>	<rdfs:seeAlso rdf:resource="http://kos.gbif.org/wiki/geotime:C19"/>	<dcterms:created>2011-01-11</dcterms:created>	<dcterms:modified>2012-08-03</dcterms:modified>	<geotime:start>41.59</geotime:start>	<geotime:end>40.439</geotime:end>	<geotime:polarity></geotime:polarity>	<geotime:regionName></geotime:regionName>	<dcterms:hasVersion rdf:resource="&history;20120803/geotime#C19"/>	<rdfs:isDefinedBy rdf:resource="&geotime;"/>	<skos:inScheme rdf:resource="&geotime;"/>	<vann:termGroup rdf:resource="&geotime;Magnetostratigraphic"/>	<vs:term_status>unstable</vs:term_status>	</skos:Concept>
<skos:Concept rdf:about="http://rs.gbif.org/terms/geotime#C19r">	<skos:prefLabel xml:lang="en">C19r</skos:prefLabel>	<skos:definition>The C19r magnetostratographic time period started 41.59 million years (Ma) before present (BP) and ended 40.671 Ma BP.</skos:definition>	<rdfs:seeAlso rdf:resource="http://kos.gbif.org/wiki/geotime:C19r"/>	<dcterms:created>2011-01-11</dcterms:created>	<dcterms:modified>2012-08-03</dcterms:modified>	<geotime:start>41.59</geotime:start>	<geotime:end>40.671</geotime:end>	<geotime:polarity>R</geotime:polarity>	<geotime:regionName></geotime:regionName>	<dcterms:hasVersion rdf:resource="&history;20120803/geotime#C19r"/>	<rdfs:isDefinedBy rdf:resource="&geotime;"/>	<skos:inScheme rdf:resource="&geotime;"/>	<vann:termGroup rdf:resource="&geotime;Magnetostratigraphic"/>	<vs:term_status>unstable</vs:term_status>	</skos:Concept>
<skos:Concept rdf:about="http://rs.gbif.org/terms/geotime#C20n">	<skos:prefLabel xml:lang="en">C20n</skos:prefLabel>	<skos:definition>The C20n magnetostratographic time period started 42.774 million years (Ma) before present (BP) and ended 41.59 Ma BP.</skos:definition>	<rdfs:seeAlso rdf:resource="http://kos.gbif.org/wiki/geotime:C20n"/>	<dcterms:created>2011-01-11</dcterms:created>	<dcterms:modified>2012-08-03</dcterms:modified>	<geotime:start>42.774</geotime:start>	<geotime:end>41.59</geotime:end>	<geotime:polarity>N</geotime:polarity>	<geotime:regionName></geotime:regionName>	<dcterms:hasVersion rdf:resource="&history;20120803/geotime#C20n"/>	<rdfs:isDefinedBy rdf:resource="&geotime;"/>	<skos:inScheme rdf:resource="&geotime;"/>	<vann:termGroup rdf:resource="&geotime;Magnetostratigraphic"/>	<vs:term_status>unstable</vs:term_status>	</skos:Concept>
<skos:Concept rdf:about="http://rs.gbif.org/terms/geotime#C20">	<skos:prefLabel xml:lang="en">C20</skos:prefLabel>	<skos:definition>The C20 magnetostratographic time period started 45.346 million years (Ma) before present (BP) and ended 41.59 Ma BP.</skos:definition>	<rdfs:seeAlso rdf:resource="http://kos.gbif.org/wiki/geotime:C20"/>	<dcterms:created>2011-01-11</dcterms:created>	<dcterms:modified>2012-08-03</dcterms:modified>	<geotime:start>45.346</geotime:start>	<geotime:end>41.59</geotime:end>	<geotime:polarity></geotime:polarity>	<geotime:regionName></geotime:regionName>	<dcterms:hasVersion rdf:resource="&history;20120803/geotime#C20"/>	<rdfs:isDefinedBy rdf:resource="&geotime;"/>	<skos:inScheme rdf:resource="&geotime;"/>	<vann:termGroup rdf:resource="&geotime;Magnetostratigraphic"/>	<vs:term_status>unstable</vs:term_status>	</skos:Concept>
<skos:Concept rdf:about="http://rs.gbif.org/terms/geotime#C20r">	<skos:prefLabel xml:lang="en">C20r</skos:prefLabel>	<skos:definition>The C20r magnetostratographic time period started 45.346 million years (Ma) before present (BP) and ended 42.774 Ma BP.</skos:definition>	<rdfs:seeAlso rdf:resource="http://kos.gbif.org/wiki/geotime:C20r"/>	<dcterms:created>2011-01-11</dcterms:created>	<dcterms:modified>2012-08-03</dcterms:modified>	<geotime:start>45.346</geotime:start>	<geotime:end>42.774</geotime:end>	<geotime:polarity>R</geotime:polarity>	<geotime:regionName></geotime:regionName>	<dcterms:hasVersion rdf:resource="&history;20120803/geotime#C20r"/>	<rdfs:isDefinedBy rdf:resource="&geotime;"/>	<skos:inScheme rdf:resource="&geotime;"/>	<vann:termGroup rdf:resource="&geotime;Magnetostratigraphic"/>	<vs:term_status>unstable</vs:term_status>	</skos:Concept>
<skos:Concept rdf:about="http://rs.gbif.org/terms/geotime#C21n">	<skos:prefLabel xml:lang="en">C21n</skos:prefLabel>	<skos:definition>The C21n magnetostratographic time period started 47.235 million years (Ma) before present (BP) and ended 45.346 Ma BP.</skos:definition>	<rdfs:seeAlso rdf:resource="http://kos.gbif.org/wiki/geotime:C21n"/>	<dcterms:created>2011-01-11</dcterms:created>	<dcterms:modified>2012-08-03</dcterms:modified>	<geotime:start>47.235</geotime:start>	<geotime:end>45.346</geotime:end>	<geotime:polarity>N</geotime:polarity>	<geotime:regionName></geotime:regionName>	<dcterms:hasVersion rdf:resource="&history;20120803/geotime#C21n"/>	<rdfs:isDefinedBy rdf:resource="&geotime;"/>	<skos:inScheme rdf:resource="&geotime;"/>	<vann:termGroup rdf:resource="&geotime;Magnetostratigraphic"/>	<vs:term_status>unstable</vs:term_status>	</skos:Concept>
<skos:Concept rdf:about="http://rs.gbif.org/terms/geotime#C21">	<skos:prefLabel xml:lang="en">C21</skos:prefLabel>	<skos:definition>The C21 magnetostratographic time period started 48.599 million years (Ma) before present (BP) and ended 45.346 Ma BP.</skos:definition>	<rdfs:seeAlso rdf:resource="http://kos.gbif.org/wiki/geotime:C21"/>	<dcterms:created>2011-01-11</dcterms:created>	<dcterms:modified>2012-08-03</dcterms:modified>	<geotime:start>48.599</geotime:start>	<geotime:end>45.346</geotime:end>	<geotime:polarity></geotime:polarity>	<geotime:regionName></geotime:regionName>	<dcterms:hasVersion rdf:resource="&history;20120803/geotime#C21"/>	<rdfs:isDefinedBy rdf:resource="&geotime;"/>	<skos:inScheme rdf:resource="&geotime;"/>	<vann:termGroup rdf:resource="&geotime;Magnetostratigraphic"/>	<vs:term_status>unstable</vs:term_status>	</skos:Concept>
<skos:Concept rdf:about="http://rs.gbif.org/terms/geotime#C21r">	<skos:prefLabel xml:lang="en">C21r</skos:prefLabel>	<skos:definition>The C21r magnetostratographic time period started 48.599 million years (Ma) before present (BP) and ended 47.235 Ma BP.</skos:definition>	<rdfs:seeAlso rdf:resource="http://kos.gbif.org/wiki/geotime:C21r"/>	<dcterms:created>2011-01-11</dcterms:created>	<dcterms:modified>2012-08-03</dcterms:modified>	<geotime:start>48.599</geotime:start>	<geotime:end>47.235</geotime:end>	<geotime:polarity>R</geotime:polarity>	<geotime:regionName></geotime:regionName>	<dcterms:hasVersion rdf:resource="&history;20120803/geotime#C21r"/>	<rdfs:isDefinedBy rdf:resource="&geotime;"/>	<skos:inScheme rdf:resource="&geotime;"/>	<vann:termGroup rdf:resource="&geotime;Magnetostratigraphic"/>	<vs:term_status>unstable</vs:term_status>	</skos:Concept>
<skos:Concept rdf:about="http://rs.gbif.org/terms/geotime#C22n">	<skos:prefLabel xml:lang="en">C22n</skos:prefLabel>	<skos:definition>The C22n magnetostratographic time period started 49.427 million years (Ma) before present (BP) and ended 48.599 Ma BP.</skos:definition>	<rdfs:seeAlso rdf:resource="http://kos.gbif.org/wiki/geotime:C22n"/>	<dcterms:created>2011-01-11</dcterms:created>	<dcterms:modified>2012-08-03</dcterms:modified>	<geotime:start>49.427</geotime:start>	<geotime:end>48.599</geotime:end>	<geotime:polarity>N</geotime:polarity>	<geotime:regionName></geotime:regionName>	<dcterms:hasVersion rdf:resource="&history;20120803/geotime#C22n"/>	<rdfs:isDefinedBy rdf:resource="&geotime;"/>	<skos:inScheme rdf:resource="&geotime;"/>	<vann:termGroup rdf:resource="&geotime;Magnetostratigraphic"/>	<vs:term_status>unstable</vs:term_status>	</skos:Concept>
<skos:Concept rdf:about="http://rs.gbif.org/terms/geotime#C3nvvv4n">	<skos:prefLabel xml:lang="en">C3nvvv4n</skos:prefLabel>	<skos:definition>The C3nvvv4n magnetostratographic time period started 5.235 million years (Ma) before present (BP) and ended 4.997 Ma BP.</skos:definition>	<rdfs:seeAlso rdf:resource="http://kos.gbif.org/wiki/geotime:C3nvvv4n"/>	<dcterms:created>2011-01-11</dcterms:created>	<dcterms:modified>2012-08-03</dcterms:modified>	<geotime:start>5.235</geotime:start>	<geotime:end>4.997</geotime:end>	<geotime:polarity>N</geotime:polarity>	<geotime:regionName>Thvera</geotime:regionName>	<dcterms:hasVersion rdf:resource="&history;20120803/geotime#C3nvvv4n"/>	<rdfs:isDefinedBy rdf:resource="&geotime;"/>	<skos:inScheme rdf:resource="&geotime;"/>	<vann:termGroup rdf:resource="&geotime;Magnetostratigraphic"/>	<vs:term_status>unstable</vs:term_status>	</skos:Concept>
<skos:Concept rdf:about="http://rs.gbif.org/terms/geotime#C22">	<skos:prefLabel xml:lang="en">C22</skos:prefLabel>	<skos:definition>The C22 magnetostratographic time period started 50.73 million years (Ma) before present (BP) and ended 48.599 Ma BP.</skos:definition>	<rdfs:seeAlso rdf:resource="http://kos.gbif.org/wiki/geotime:C22"/>	<dcterms:created>2011-01-11</dcterms:created>	<dcterms:modified>2012-08-03</dcterms:modified>	<geotime:start>50.73</geotime:start>	<geotime:end>48.599</geotime:end>	<geotime:polarity></geotime:polarity>	<geotime:regionName></geotime:regionName>	<dcterms:hasVersion rdf:resource="&history;20120803/geotime#C22"/>	<rdfs:isDefinedBy rdf:resource="&geotime;"/>	<skos:inScheme rdf:resource="&geotime;"/>	<vann:termGroup rdf:resource="&geotime;Magnetostratigraphic"/>	<vs:term_status>unstable</vs:term_status>	</skos:Concept>
<skos:Concept rdf:about="http://rs.gbif.org/terms/geotime#C22r">	<skos:prefLabel xml:lang="en">C22r</skos:prefLabel>	<skos:definition>The C22r magnetostratographic time period started 50.73 million years (Ma) before present (BP) and ended 49.427 Ma BP.</skos:definition>	<rdfs:seeAlso rdf:resource="http://kos.gbif.org/wiki/geotime:C22r"/>	<dcterms:created>2011-01-11</dcterms:created>	<dcterms:modified>2012-08-03</dcterms:modified>	<geotime:start>50.73</geotime:start>	<geotime:end>49.427</geotime:end>	<geotime:polarity>R</geotime:polarity>	<geotime:regionName></geotime:regionName>	<dcterms:hasVersion rdf:resource="&history;20120803/geotime#C22r"/>	<rdfs:isDefinedBy rdf:resource="&geotime;"/>	<skos:inScheme rdf:resource="&geotime;"/>	<vann:termGroup rdf:resource="&geotime;Magnetostratigraphic"/>	<vs:term_status>unstable</vs:term_status>	</skos:Concept>
<skos:Concept rdf:about="http://rs.gbif.org/terms/geotime#C23nvvv1n">	<skos:prefLabel xml:lang="en">C23nvvv1n</skos:prefLabel>	<skos:definition>The C23nvvv1n magnetostratographic time period started 50.932 million years (Ma) before present (BP) and ended 50.73 Ma BP.</skos:definition>	<rdfs:seeAlso rdf:resource="http://kos.gbif.org/wiki/geotime:C23nvvv1n"/>	<dcterms:created>2011-01-11</dcterms:created>	<dcterms:modified>2012-08-03</dcterms:modified>	<geotime:start>50.932</geotime:start>	<geotime:end>50.73</geotime:end>	<geotime:polarity>N</geotime:polarity>	<geotime:regionName></geotime:regionName>	<dcterms:hasVersion rdf:resource="&history;20120803/geotime#C23nvvv1n"/>	<rdfs:isDefinedBy rdf:resource="&geotime;"/>	<skos:inScheme rdf:resource="&geotime;"/>	<vann:termGroup rdf:resource="&geotime;Magnetostratigraphic"/>	<vs:term_status>unstable</vs:term_status>	</skos:Concept>
<skos:Concept rdf:about="http://rs.gbif.org/terms/geotime#C23nvvv1r">	<skos:prefLabel xml:lang="en">C23nvvv1r</skos:prefLabel>	<skos:definition>The C23nvvv1r magnetostratographic time period started 51.057 million years (Ma) before present (BP) and ended 50.932 Ma BP.</skos:definition>	<rdfs:seeAlso rdf:resource="http://kos.gbif.org/wiki/geotime:C23nvvv1r"/>	<dcterms:created>2011-01-11</dcterms:created>	<dcterms:modified>2012-08-03</dcterms:modified>	<geotime:start>51.057</geotime:start>	<geotime:end>50.932</geotime:end>	<geotime:polarity>R</geotime:polarity>	<geotime:regionName></geotime:regionName>	<dcterms:hasVersion rdf:resource="&history;20120803/geotime#C23nvvv1r"/>	<rdfs:isDefinedBy rdf:resource="&geotime;"/>	<skos:inScheme rdf:resource="&geotime;"/>	<vann:termGroup rdf:resource="&geotime;Magnetostratigraphic"/>	<vs:term_status>unstable</vs:term_status>	</skos:Concept>
<skos:Concept rdf:about="http://rs.gbif.org/terms/geotime#C23nvvv2n">	<skos:prefLabel xml:lang="en">C23nvvv2n</skos:prefLabel>	<skos:definition>The C23nvvv2n magnetostratographic time period started 51.901 million years (Ma) before present (BP) and ended 51.057 Ma BP.</skos:definition>	<rdfs:seeAlso rdf:resource="http://kos.gbif.org/wiki/geotime:C23nvvv2n"/>	<dcterms:created>2011-01-11</dcterms:created>	<dcterms:modified>2012-08-03</dcterms:modified>	<geotime:start>51.901</geotime:start>	<geotime:end>51.057</geotime:end>	<geotime:polarity>N</geotime:polarity>	<geotime:regionName></geotime:regionName>	<dcterms:hasVersion rdf:resource="&history;20120803/geotime#C23nvvv2n"/>	<rdfs:isDefinedBy rdf:resource="&geotime;"/>	<skos:inScheme rdf:resource="&geotime;"/>	<vann:termGroup rdf:resource="&geotime;Magnetostratigraphic"/>	<vs:term_status>unstable</vs:term_status>	</skos:Concept>
<skos:Concept rdf:about="http://rs.gbif.org/terms/geotime#C23">	<skos:prefLabel xml:lang="en">C23</skos:prefLabel>	<skos:definition>The C23 magnetostratographic time period started 52.648 million years (Ma) before present (BP) and ended 50.73 Ma BP.</skos:definition>	<rdfs:seeAlso rdf:resource="http://kos.gbif.org/wiki/geotime:C23"/>	<dcterms:created>2011-01-11</dcterms:created>	<dcterms:modified>2012-08-03</dcterms:modified>	<geotime:start>52.648</geotime:start>	<geotime:end>50.73</geotime:end>	<geotime:polarity></geotime:polarity>	<geotime:regionName></geotime:regionName>	<dcterms:hasVersion rdf:resource="&history;20120803/geotime#C23"/>	<rdfs:isDefinedBy rdf:resource="&geotime;"/>	<skos:inScheme rdf:resource="&geotime;"/>	<vann:termGroup rdf:resource="&geotime;Magnetostratigraphic"/>	<vs:term_status>unstable</vs:term_status>	</skos:Concept>
<skos:Concept rdf:about="http://rs.gbif.org/terms/geotime#C23r">	<skos:prefLabel xml:lang="en">C23r</skos:prefLabel>	<skos:definition>The C23r magnetostratographic time period started 52.648 million years (Ma) before present (BP) and ended 51.901 Ma BP.</skos:definition>	<rdfs:seeAlso rdf:resource="http://kos.gbif.org/wiki/geotime:C23r"/>	<dcterms:created>2011-01-11</dcterms:created>	<dcterms:modified>2012-08-03</dcterms:modified>	<geotime:start>52.648</geotime:start>	<geotime:end>51.901</geotime:end>	<geotime:polarity>R</geotime:polarity>	<geotime:regionName></geotime:regionName>	<dcterms:hasVersion rdf:resource="&history;20120803/geotime#C23r"/>	<rdfs:isDefinedBy rdf:resource="&geotime;"/>	<skos:inScheme rdf:resource="&geotime;"/>	<vann:termGroup rdf:resource="&geotime;Magnetostratigraphic"/>	<vs:term_status>unstable</vs:term_status>	</skos:Concept>
<skos:Concept rdf:about="http://rs.gbif.org/terms/geotime#C24nvvv1n">	<skos:prefLabel xml:lang="en">C24nvvv1n</skos:prefLabel>	<skos:definition>The C24nvvv1n magnetostratographic time period started 53.004 million years (Ma) before present (BP) and ended 52.648 Ma BP.</skos:definition>	<rdfs:seeAlso rdf:resource="http://kos.gbif.org/wiki/geotime:C24nvvv1n"/>	<dcterms:created>2011-01-11</dcterms:created>	<dcterms:modified>2012-08-03</dcterms:modified>	<geotime:start>53.004</geotime:start>	<geotime:end>52.648</geotime:end>	<geotime:polarity>N</geotime:polarity>	<geotime:regionName></geotime:regionName>	<dcterms:hasVersion rdf:resource="&history;20120803/geotime#C24nvvv1n"/>	<rdfs:isDefinedBy rdf:resource="&geotime;"/>	<skos:inScheme rdf:resource="&geotime;"/>	<vann:termGroup rdf:resource="&geotime;Magnetostratigraphic"/>	<vs:term_status>unstable</vs:term_status>	</skos:Concept>
<skos:Concept rdf:about="http://rs.gbif.org/terms/geotime#C24nvvv1r">	<skos:prefLabel xml:lang="en">C24nvvv1r</skos:prefLabel>	<skos:definition>The C24nvvv1r magnetostratographic time period started 53.116 million years (Ma) before present (BP) and ended 53.004 Ma BP.</skos:definition>	<rdfs:seeAlso rdf:resource="http://kos.gbif.org/wiki/geotime:C24nvvv1r"/>	<dcterms:created>2011-01-11</dcterms:created>	<dcterms:modified>2012-08-03</dcterms:modified>	<geotime:start>53.116</geotime:start>	<geotime:end>53.004</geotime:end>	<geotime:polarity>R</geotime:polarity>	<geotime:regionName></geotime:regionName>	<dcterms:hasVersion rdf:resource="&history;20120803/geotime#C24nvvv1r"/>	<rdfs:isDefinedBy rdf:resource="&geotime;"/>	<skos:inScheme rdf:resource="&geotime;"/>	<vann:termGroup rdf:resource="&geotime;Magnetostratigraphic"/>	<vs:term_status>unstable</vs:term_status>	</skos:Concept>
<skos:Concept rdf:about="http://rs.gbif.org/terms/geotime#C24nvvv2n">	<skos:prefLabel xml:lang="en">C24nvvv2n</skos:prefLabel>	<skos:definition>The C24nvvv2n magnetostratographic time period started 53.167 million years (Ma) before present (BP) and ended 53.116 Ma BP.</skos:definition>	<rdfs:seeAlso rdf:resource="http://kos.gbif.org/wiki/geotime:C24nvvv2n"/>	<dcterms:created>2011-01-11</dcterms:created>	<dcterms:modified>2012-08-03</dcterms:modified>	<geotime:start>53.167</geotime:start>	<geotime:end>53.116</geotime:end>	<geotime:polarity>N</geotime:polarity>	<geotime:regionName></geotime:regionName>	<dcterms:hasVersion rdf:resource="&history;20120803/geotime#C24nvvv2n"/>	<rdfs:isDefinedBy rdf:resource="&geotime;"/>	<skos:inScheme rdf:resource="&geotime;"/>	<vann:termGroup rdf:resource="&geotime;Magnetostratigraphic"/>	<vs:term_status>unstable</vs:term_status>	</skos:Concept>
<skos:Concept rdf:about="http://rs.gbif.org/terms/geotime#C24nvvv2r">	<skos:prefLabel xml:lang="en">C24nvvv2r</skos:prefLabel>	<skos:definition>The C24nvvv2r magnetostratographic time period started 53.286 million years (Ma) before present (BP) and ended 53.167 Ma BP.</skos:definition>	<rdfs:seeAlso rdf:resource="http://kos.gbif.org/wiki/geotime:C24nvvv2r"/>	<dcterms:created>2011-01-11</dcterms:created>	<dcterms:modified>2012-08-03</dcterms:modified>	<geotime:start>53.286</geotime:start>	<geotime:end>53.167</geotime:end>	<geotime:polarity>R</geotime:polarity>	<geotime:regionName></geotime:regionName>	<dcterms:hasVersion rdf:resource="&history;20120803/geotime#C24nvvv2r"/>	<rdfs:isDefinedBy rdf:resource="&geotime;"/>	<skos:inScheme rdf:resource="&geotime;"/>	<vann:termGroup rdf:resource="&geotime;Magnetostratigraphic"/>	<vs:term_status>unstable</vs:term_status>	</skos:Concept>
<skos:Concept rdf:about="http://rs.gbif.org/terms/geotime#C24nvvv3n">	<skos:prefLabel xml:lang="en">C24nvvv3n</skos:prefLabel>	<skos:definition>The C24nvvv3n magnetostratographic time period started 53.808 million years (Ma) before present (BP) and ended 53.286 Ma BP.</skos:definition>	<rdfs:seeAlso rdf:resource="http://kos.gbif.org/wiki/geotime:C24nvvv3n"/>	<dcterms:created>2011-01-11</dcterms:created>	<dcterms:modified>2012-08-03</dcterms:modified>	<geotime:start>53.808</geotime:start>	<geotime:end>53.286</geotime:end>	<geotime:polarity>N</geotime:polarity>	<geotime:regionName></geotime:regionName>	<dcterms:hasVersion rdf:resource="&history;20120803/geotime#C24nvvv3n"/>	<rdfs:isDefinedBy rdf:resource="&geotime;"/>	<skos:inScheme rdf:resource="&geotime;"/>	<vann:termGroup rdf:resource="&geotime;Magnetostratigraphic"/>	<vs:term_status>unstable</vs:term_status>	</skos:Concept>
<skos:Concept rdf:about="http://rs.gbif.org/terms/geotime#C24">	<skos:prefLabel xml:lang="en">C24</skos:prefLabel>	<skos:definition>The C24 magnetostratographic time period started 56.665 million years (Ma) before present (BP) and ended 52.648 Ma BP.</skos:definition>	<rdfs:seeAlso rdf:resource="http://kos.gbif.org/wiki/geotime:C24"/>	<dcterms:created>2011-01-11</dcterms:created>	<dcterms:modified>2012-08-03</dcterms:modified>	<geotime:start>56.665</geotime:start>	<geotime:end>52.648</geotime:end>	<geotime:polarity></geotime:polarity>	<geotime:regionName></geotime:regionName>	<dcterms:hasVersion rdf:resource="&history;20120803/geotime#C24"/>	<rdfs:isDefinedBy rdf:resource="&geotime;"/>	<skos:inScheme rdf:resource="&geotime;"/>	<vann:termGroup rdf:resource="&geotime;Magnetostratigraphic"/>	<vs:term_status>unstable</vs:term_status>	</skos:Concept>
<skos:Concept rdf:about="http://rs.gbif.org/terms/geotime#C24r">	<skos:prefLabel xml:lang="en">C24r</skos:prefLabel>	<skos:definition>The C24r magnetostratographic time period started 56.665 million years (Ma) before present (BP) and ended 53.808 Ma BP.</skos:definition>	<rdfs:seeAlso rdf:resource="http://kos.gbif.org/wiki/geotime:C24r"/>	<dcterms:created>2011-01-11</dcterms:created>	<dcterms:modified>2012-08-03</dcterms:modified>	<geotime:start>56.665</geotime:start>	<geotime:end>53.808</geotime:end>	<geotime:polarity>R</geotime:polarity>	<geotime:regionName></geotime:regionName>	<dcterms:hasVersion rdf:resource="&history;20120803/geotime#C24r"/>	<rdfs:isDefinedBy rdf:resource="&geotime;"/>	<skos:inScheme rdf:resource="&geotime;"/>	<vann:termGroup rdf:resource="&geotime;Magnetostratigraphic"/>	<vs:term_status>unstable</vs:term_status>	</skos:Concept>
<skos:Concept rdf:about="http://rs.gbif.org/terms/geotime#C25n">	<skos:prefLabel xml:lang="en">C25n</skos:prefLabel>	<skos:definition>The C25n magnetostratographic time period started 57.18 million years (Ma) before present (BP) and ended 56.665 Ma BP.</skos:definition>	<rdfs:seeAlso rdf:resource="http://kos.gbif.org/wiki/geotime:C25n"/>	<dcterms:created>2011-01-11</dcterms:created>	<dcterms:modified>2012-08-03</dcterms:modified>	<geotime:start>57.18</geotime:start>	<geotime:end>56.665</geotime:end>	<geotime:polarity>N</geotime:polarity>	<geotime:regionName></geotime:regionName>	<dcterms:hasVersion rdf:resource="&history;20120803/geotime#C25n"/>	<rdfs:isDefinedBy rdf:resource="&geotime;"/>	<skos:inScheme rdf:resource="&geotime;"/>	<vann:termGroup rdf:resource="&geotime;Magnetostratigraphic"/>	<vs:term_status>unstable</vs:term_status>	</skos:Concept>
<skos:Concept rdf:about="http://rs.gbif.org/terms/geotime#C25">	<skos:prefLabel xml:lang="en">C25</skos:prefLabel>	<skos:definition>The C25 magnetostratographic time period started 58.379 million years (Ma) before present (BP) and ended 56.665 Ma BP.</skos:definition>	<rdfs:seeAlso rdf:resource="http://kos.gbif.org/wiki/geotime:C25"/>	<dcterms:created>2011-01-11</dcterms:created>	<dcterms:modified>2012-08-03</dcterms:modified>	<geotime:start>58.379</geotime:start>	<geotime:end>56.665</geotime:end>	<geotime:polarity></geotime:polarity>	<geotime:regionName></geotime:regionName>	<dcterms:hasVersion rdf:resource="&history;20120803/geotime#C25"/>	<rdfs:isDefinedBy rdf:resource="&geotime;"/>	<skos:inScheme rdf:resource="&geotime;"/>	<vann:termGroup rdf:resource="&geotime;Magnetostratigraphic"/>	<vs:term_status>unstable</vs:term_status>	</skos:Concept>
<skos:Concept rdf:about="http://rs.gbif.org/terms/geotime#C25r">	<skos:prefLabel xml:lang="en">C25r</skos:prefLabel>	<skos:definition>The C25r magnetostratographic time period started 58.379 million years (Ma) before present (BP) and ended 57.18 Ma BP.</skos:definition>	<rdfs:seeAlso rdf:resource="http://kos.gbif.org/wiki/geotime:C25r"/>	<dcterms:created>2011-01-11</dcterms:created>	<dcterms:modified>2012-08-03</dcterms:modified>	<geotime:start>58.379</geotime:start>	<geotime:end>57.18</geotime:end>	<geotime:polarity>R</geotime:polarity>	<geotime:regionName></geotime:regionName>	<dcterms:hasVersion rdf:resource="&history;20120803/geotime#C25r"/>	<rdfs:isDefinedBy rdf:resource="&geotime;"/>	<skos:inScheme rdf:resource="&geotime;"/>	<vann:termGroup rdf:resource="&geotime;Magnetostratigraphic"/>	<vs:term_status>unstable</vs:term_status>	</skos:Concept>
<skos:Concept rdf:about="http://rs.gbif.org/terms/geotime#C26n">	<skos:prefLabel xml:lang="en">C26n</skos:prefLabel>	<skos:definition>The C26n magnetostratographic time period started 58.737 million years (Ma) before present (BP) and ended 58.379 Ma BP.</skos:definition>	<rdfs:seeAlso rdf:resource="http://kos.gbif.org/wiki/geotime:C26n"/>	<dcterms:created>2011-01-11</dcterms:created>	<dcterms:modified>2012-08-03</dcterms:modified>	<geotime:start>58.737</geotime:start>	<geotime:end>58.379</geotime:end>	<geotime:polarity>N</geotime:polarity>	<geotime:regionName></geotime:regionName>	<dcterms:hasVersion rdf:resource="&history;20120803/geotime#C26n"/>	<rdfs:isDefinedBy rdf:resource="&geotime;"/>	<skos:inScheme rdf:resource="&geotime;"/>	<vann:termGroup rdf:resource="&geotime;Magnetostratigraphic"/>	<vs:term_status>unstable</vs:term_status>	</skos:Concept>
<skos:Concept rdf:about="http://rs.gbif.org/terms/geotime#C3">	<skos:prefLabel xml:lang="en">C3</skos:prefLabel>	<skos:definition>The C3 magnetostratographic time period started 6.033 million years (Ma) before present (BP) and ended 4.187 Ma BP.</skos:definition>	<rdfs:seeAlso rdf:resource="http://kos.gbif.org/wiki/geotime:C3"/>	<dcterms:created>2011-01-11</dcterms:created>	<dcterms:modified>2012-08-03</dcterms:modified>	<geotime:start>6.033</geotime:start>	<geotime:end>4.187</geotime:end>	<geotime:polarity></geotime:polarity>	<geotime:regionName></geotime:regionName>	<dcterms:hasVersion rdf:resource="&history;20120803/geotime#C3"/>	<rdfs:isDefinedBy rdf:resource="&geotime;"/>	<skos:inScheme rdf:resource="&geotime;"/>	<vann:termGroup rdf:resource="&geotime;Magnetostratigraphic"/>	<vs:term_status>unstable</vs:term_status>	</skos:Concept>
<skos:Concept rdf:about="http://rs.gbif.org/terms/geotime#C3r">	<skos:prefLabel xml:lang="en">C3r</skos:prefLabel>	<skos:definition>The C3r magnetostratographic time period started 6.033 million years (Ma) before present (BP) and ended 5.235 Ma BP.</skos:definition>	<rdfs:seeAlso rdf:resource="http://kos.gbif.org/wiki/geotime:C3r"/>	<dcterms:created>2011-01-11</dcterms:created>	<dcterms:modified>2012-08-03</dcterms:modified>	<geotime:start>6.033</geotime:start>	<geotime:end>5.235</geotime:end>	<geotime:polarity>R</geotime:polarity>	<geotime:regionName>Gilbert lower part</geotime:regionName>	<dcterms:hasVersion rdf:resource="&history;20120803/geotime#C3r"/>	<rdfs:isDefinedBy rdf:resource="&geotime;"/>	<skos:inScheme rdf:resource="&geotime;"/>	<vann:termGroup rdf:resource="&geotime;Magnetostratigraphic"/>	<vs:term_status>unstable</vs:term_status>	</skos:Concept>
<skos:Concept rdf:about="http://rs.gbif.org/terms/geotime#C3Anvvv1n">	<skos:prefLabel xml:lang="en">C3Anvvv1n</skos:prefLabel>	<skos:definition>The C3Anvvv1n magnetostratographic time period started 6.252 million years (Ma) before present (BP) and ended 6.033 Ma BP.</skos:definition>	<rdfs:seeAlso rdf:resource="http://kos.gbif.org/wiki/geotime:C3Anvvv1n"/>	<dcterms:created>2011-01-11</dcterms:created>	<dcterms:modified>2012-08-03</dcterms:modified>	<geotime:start>6.252</geotime:start>	<geotime:end>6.033</geotime:end>	<geotime:polarity>N</geotime:polarity>	<geotime:regionName></geotime:regionName>	<dcterms:hasVersion rdf:resource="&history;20120803/geotime#C3Anvvv1n"/>	<rdfs:isDefinedBy rdf:resource="&geotime;"/>	<skos:inScheme rdf:resource="&geotime;"/>	<vann:termGroup rdf:resource="&geotime;Magnetostratigraphic"/>	<vs:term_status>unstable</vs:term_status>	</skos:Concept>
<skos:Concept rdf:about="http://rs.gbif.org/terms/geotime#C3Anvvv1r">	<skos:prefLabel xml:lang="en">C3Anvvv1r</skos:prefLabel>	<skos:definition>The C3Anvvv1r magnetostratographic time period started 6.436 million years (Ma) before present (BP) and ended 6.252 Ma BP.</skos:definition>	<rdfs:seeAlso rdf:resource="http://kos.gbif.org/wiki/geotime:C3Anvvv1r"/>	<dcterms:created>2011-01-11</dcterms:created>	<dcterms:modified>2012-08-03</dcterms:modified>	<geotime:start>6.436</geotime:start>	<geotime:end>6.252</geotime:end>	<geotime:polarity>R</geotime:polarity>	<geotime:regionName></geotime:regionName>	<dcterms:hasVersion rdf:resource="&history;20120803/geotime#C3Anvvv1r"/>	<rdfs:isDefinedBy rdf:resource="&geotime;"/>	<skos:inScheme rdf:resource="&geotime;"/>	<vann:termGroup rdf:resource="&geotime;Magnetostratigraphic"/>	<vs:term_status>unstable</vs:term_status>	</skos:Concept>
<skos:Concept rdf:about="http://rs.gbif.org/terms/geotime#C3Anvvv2n">	<skos:prefLabel xml:lang="en">C3Anvvv2n</skos:prefLabel>	<skos:definition>The C3Anvvv2n magnetostratographic time period started 6.733 million years (Ma) before present (BP) and ended 6.436 Ma BP.</skos:definition>	<rdfs:seeAlso rdf:resource="http://kos.gbif.org/wiki/geotime:C3Anvvv2n"/>	<dcterms:created>2011-01-11</dcterms:created>	<dcterms:modified>2012-08-03</dcterms:modified>	<geotime:start>6.733</geotime:start>	<geotime:end>6.436</geotime:end>	<geotime:polarity>N</geotime:polarity>	<geotime:regionName></geotime:regionName>	<dcterms:hasVersion rdf:resource="&history;20120803/geotime#C3Anvvv2n"/>	<rdfs:isDefinedBy rdf:resource="&geotime;"/>	<skos:inScheme rdf:resource="&geotime;"/>	<vann:termGroup rdf:resource="&geotime;Magnetostratigraphic"/>	<vs:term_status>unstable</vs:term_status>	</skos:Concept>
<skos:Concept rdf:about="http://rs.gbif.org/terms/geotime#C26">	<skos:prefLabel xml:lang="en">C26</skos:prefLabel>	<skos:definition>The C26 magnetostratographic time period started 61.65 million years (Ma) before present (BP) and ended 58.379 Ma BP.</skos:definition>	<rdfs:seeAlso rdf:resource="http://kos.gbif.org/wiki/geotime:C26"/>	<dcterms:created>2011-01-11</dcterms:created>	<dcterms:modified>2012-08-03</dcterms:modified>	<geotime:start>61.65</geotime:start>	<geotime:end>58.379</geotime:end>	<geotime:polarity></geotime:polarity>	<geotime:regionName></geotime:regionName>	<dcterms:hasVersion rdf:resource="&history;20120803/geotime#C26"/>	<rdfs:isDefinedBy rdf:resource="&geotime;"/>	<skos:inScheme rdf:resource="&geotime;"/>	<vann:termGroup rdf:resource="&geotime;Magnetostratigraphic"/>	<vs:term_status>unstable</vs:term_status>	</skos:Concept>
<skos:Concept rdf:about="http://rs.gbif.org/terms/geotime#C26r">	<skos:prefLabel xml:lang="en">C26r</skos:prefLabel>	<skos:definition>The C26r magnetostratographic time period started 61.65 million years (Ma) before present (BP) and ended 58.737 Ma BP.</skos:definition>	<rdfs:seeAlso rdf:resource="http://kos.gbif.org/wiki/geotime:C26r"/>	<dcterms:created>2011-01-11</dcterms:created>	<dcterms:modified>2012-08-03</dcterms:modified>	<geotime:start>61.65</geotime:start>	<geotime:end>58.737</geotime:end>	<geotime:polarity>R</geotime:polarity>	<geotime:regionName></geotime:regionName>	<dcterms:hasVersion rdf:resource="&history;20120803/geotime#C26r"/>	<rdfs:isDefinedBy rdf:resource="&geotime;"/>	<skos:inScheme rdf:resource="&geotime;"/>	<vann:termGroup rdf:resource="&geotime;Magnetostratigraphic"/>	<vs:term_status>unstable</vs:term_status>	</skos:Concept>
<skos:Concept rdf:about="http://rs.gbif.org/terms/geotime#C27n">	<skos:prefLabel xml:lang="en">C27n</skos:prefLabel>	<skos:definition>The C27n magnetostratographic time period started 61.983 million years (Ma) before present (BP) and ended 61.65 Ma BP.</skos:definition>	<rdfs:seeAlso rdf:resource="http://kos.gbif.org/wiki/geotime:C27n"/>	<dcterms:created>2011-01-11</dcterms:created>	<dcterms:modified>2012-08-03</dcterms:modified>	<geotime:start>61.983</geotime:start>	<geotime:end>61.65</geotime:end>	<geotime:polarity>N</geotime:polarity>	<geotime:regionName></geotime:regionName>	<dcterms:hasVersion rdf:resource="&history;20120803/geotime#C27n"/>	<rdfs:isDefinedBy rdf:resource="&geotime;"/>	<skos:inScheme rdf:resource="&geotime;"/>	<vann:termGroup rdf:resource="&geotime;Magnetostratigraphic"/>	<vs:term_status>unstable</vs:term_status>	</skos:Concept>
<skos:Concept rdf:about="http://rs.gbif.org/terms/geotime#C27">	<skos:prefLabel xml:lang="en">C27</skos:prefLabel>	<skos:definition>The C27 magnetostratographic time period started 63.104 million years (Ma) before present (BP) and ended 61.65 Ma BP.</skos:definition>	<rdfs:seeAlso rdf:resource="http://kos.gbif.org/wiki/geotime:C27"/>	<dcterms:created>2011-01-11</dcterms:created>	<dcterms:modified>2012-08-03</dcterms:modified>	<geotime:start>63.104</geotime:start>	<geotime:end>61.65</geotime:end>	<geotime:polarity></geotime:polarity>	<geotime:regionName></geotime:regionName>	<dcterms:hasVersion rdf:resource="&history;20120803/geotime#C27"/>	<rdfs:isDefinedBy rdf:resource="&geotime;"/>	<skos:inScheme rdf:resource="&geotime;"/>	<vann:termGroup rdf:resource="&geotime;Magnetostratigraphic"/>	<vs:term_status>unstable</vs:term_status>	</skos:Concept>
<skos:Concept rdf:about="http://rs.gbif.org/terms/geotime#C27r">	<skos:prefLabel xml:lang="en">C27r</skos:prefLabel>	<skos:definition>The C27r magnetostratographic time period started 63.104 million years (Ma) before present (BP) and ended 61.983 Ma BP.</skos:definition>	<rdfs:seeAlso rdf:resource="http://kos.gbif.org/wiki/geotime:C27r"/>	<dcterms:created>2011-01-11</dcterms:created>	<dcterms:modified>2012-08-03</dcterms:modified>	<geotime:start>63.104</geotime:start>	<geotime:end>61.983</geotime:end>	<geotime:polarity>R</geotime:polarity>	<geotime:regionName></geotime:regionName>	<dcterms:hasVersion rdf:resource="&history;20120803/geotime#C27r"/>	<rdfs:isDefinedBy rdf:resource="&geotime;"/>	<skos:inScheme rdf:resource="&geotime;"/>	<vann:termGroup rdf:resource="&geotime;Magnetostratigraphic"/>	<vs:term_status>unstable</vs:term_status>	</skos:Concept>
<skos:Concept rdf:about="http://rs.gbif.org/terms/geotime#C28n">	<skos:prefLabel xml:lang="en">C28n</skos:prefLabel>	<skos:definition>The C28n magnetostratographic time period started 64.128 million years (Ma) before present (BP) and ended 63.104 Ma BP.</skos:definition>	<rdfs:seeAlso rdf:resource="http://kos.gbif.org/wiki/geotime:C28n"/>	<dcterms:created>2011-01-11</dcterms:created>	<dcterms:modified>2012-08-03</dcterms:modified>	<geotime:start>64.128</geotime:start>	<geotime:end>63.104</geotime:end>	<geotime:polarity>N</geotime:polarity>	<geotime:regionName></geotime:regionName>	<dcterms:hasVersion rdf:resource="&history;20120803/geotime#C28n"/>	<rdfs:isDefinedBy rdf:resource="&geotime;"/>	<skos:inScheme rdf:resource="&geotime;"/>	<vann:termGroup rdf:resource="&geotime;Magnetostratigraphic"/>	<vs:term_status>unstable</vs:term_status>	</skos:Concept>
<skos:Concept rdf:about="http://rs.gbif.org/terms/geotime#C28">	<skos:prefLabel xml:lang="en">C28</skos:prefLabel>	<skos:definition>The C28 magnetostratographic time period started 64.432 million years (Ma) before present (BP) and ended 63.104 Ma BP.</skos:definition>	<rdfs:seeAlso rdf:resource="http://kos.gbif.org/wiki/geotime:C28"/>	<dcterms:created>2011-01-11</dcterms:created>	<dcterms:modified>2012-08-03</dcterms:modified>	<geotime:start>64.432</geotime:start>	<geotime:end>63.104</geotime:end>	<geotime:polarity></geotime:polarity>	<geotime:regionName></geotime:regionName>	<dcterms:hasVersion rdf:resource="&history;20120803/geotime#C28"/>	<rdfs:isDefinedBy rdf:resource="&geotime;"/>	<skos:inScheme rdf:resource="&geotime;"/>	<vann:termGroup rdf:resource="&geotime;Magnetostratigraphic"/>	<vs:term_status>unstable</vs:term_status>	</skos:Concept>
<skos:Concept rdf:about="http://rs.gbif.org/terms/geotime#C28r">	<skos:prefLabel xml:lang="en">C28r</skos:prefLabel>	<skos:definition>The C28r magnetostratographic time period started 64.432 million years (Ma) before present (BP) and ended 64.128 Ma BP.</skos:definition>	<rdfs:seeAlso rdf:resource="http://kos.gbif.org/wiki/geotime:C28r"/>	<dcterms:created>2011-01-11</dcterms:created>	<dcterms:modified>2012-08-03</dcterms:modified>	<geotime:start>64.432</geotime:start>	<geotime:end>64.128</geotime:end>	<geotime:polarity>R</geotime:polarity>	<geotime:regionName></geotime:regionName>	<dcterms:hasVersion rdf:resource="&history;20120803/geotime#C28r"/>	<rdfs:isDefinedBy rdf:resource="&geotime;"/>	<skos:inScheme rdf:resource="&geotime;"/>	<vann:termGroup rdf:resource="&geotime;Magnetostratigraphic"/>	<vs:term_status>unstable</vs:term_status>	</skos:Concept>
<skos:Concept rdf:about="http://rs.gbif.org/terms/geotime#C29n">	<skos:prefLabel xml:lang="en">C29n</skos:prefLabel>	<skos:definition>The C29n magnetostratographic time period started 65.118 million years (Ma) before present (BP) and ended 64.432 Ma BP.</skos:definition>	<rdfs:seeAlso rdf:resource="http://kos.gbif.org/wiki/geotime:C29n"/>	<dcterms:created>2011-01-11</dcterms:created>	<dcterms:modified>2012-08-03</dcterms:modified>	<geotime:start>65.118</geotime:start>	<geotime:end>64.432</geotime:end>	<geotime:polarity>N</geotime:polarity>	<geotime:regionName></geotime:regionName>	<dcterms:hasVersion rdf:resource="&history;20120803/geotime#C29n"/>	<rdfs:isDefinedBy rdf:resource="&geotime;"/>	<skos:inScheme rdf:resource="&geotime;"/>	<vann:termGroup rdf:resource="&geotime;Magnetostratigraphic"/>	<vs:term_status>unstable</vs:term_status>	</skos:Concept>
<skos:Concept rdf:about="http://rs.gbif.org/terms/geotime#C29">	<skos:prefLabel xml:lang="en">C29</skos:prefLabel>	<skos:definition>The C29 magnetostratographic time period started 65.861 million years (Ma) before present (BP) and ended 64.432 Ma BP.</skos:definition>	<rdfs:seeAlso rdf:resource="http://kos.gbif.org/wiki/geotime:C29"/>	<dcterms:created>2011-01-11</dcterms:created>	<dcterms:modified>2012-08-03</dcterms:modified>	<geotime:start>65.861</geotime:start>	<geotime:end>64.432</geotime:end>	<geotime:polarity></geotime:polarity>	<geotime:regionName></geotime:regionName>	<dcterms:hasVersion rdf:resource="&history;20120803/geotime#C29"/>	<rdfs:isDefinedBy rdf:resource="&geotime;"/>	<skos:inScheme rdf:resource="&geotime;"/>	<vann:termGroup rdf:resource="&geotime;Magnetostratigraphic"/>	<vs:term_status>unstable</vs:term_status>	</skos:Concept>
<skos:Concept rdf:about="http://rs.gbif.org/terms/geotime#C29r">	<skos:prefLabel xml:lang="en">C29r</skos:prefLabel>	<skos:definition>The C29r magnetostratographic time period started 65.861 million years (Ma) before present (BP) and ended 65.118 Ma BP.</skos:definition>	<rdfs:seeAlso rdf:resource="http://kos.gbif.org/wiki/geotime:C29r"/>	<dcterms:created>2011-01-11</dcterms:created>	<dcterms:modified>2012-08-03</dcterms:modified>	<geotime:start>65.861</geotime:start>	<geotime:end>65.118</geotime:end>	<geotime:polarity>R</geotime:polarity>	<geotime:regionName></geotime:regionName>	<dcterms:hasVersion rdf:resource="&history;20120803/geotime#C29r"/>	<rdfs:isDefinedBy rdf:resource="&geotime;"/>	<skos:inScheme rdf:resource="&geotime;"/>	<vann:termGroup rdf:resource="&geotime;Magnetostratigraphic"/>	<vs:term_status>unstable</vs:term_status>	</skos:Concept>
<skos:Concept rdf:about="http://rs.gbif.org/terms/geotime#C30n">	<skos:prefLabel xml:lang="en">C30n</skos:prefLabel>	<skos:definition>The C30n magnetostratographic time period started 67.696 million years (Ma) before present (BP) and ended 65.861 Ma BP.</skos:definition>	<rdfs:seeAlso rdf:resource="http://kos.gbif.org/wiki/geotime:C30n"/>	<dcterms:created>2011-01-11</dcterms:created>	<dcterms:modified>2012-08-03</dcterms:modified>	<geotime:start>67.696</geotime:start>	<geotime:end>65.861</geotime:end>	<geotime:polarity>N</geotime:polarity>	<geotime:regionName></geotime:regionName>	<dcterms:hasVersion rdf:resource="&history;20120803/geotime#C30n"/>	<rdfs:isDefinedBy rdf:resource="&geotime;"/>	<skos:inScheme rdf:resource="&geotime;"/>	<vann:termGroup rdf:resource="&geotime;Magnetostratigraphic"/>	<vs:term_status>unstable</vs:term_status>	</skos:Concept>
<skos:Concept rdf:about="http://rs.gbif.org/terms/geotime#C30">	<skos:prefLabel xml:lang="en">C30</skos:prefLabel>	<skos:definition>The C30 magnetostratographic time period started 67.809 million years (Ma) before present (BP) and ended 65.861 Ma BP.</skos:definition>	<rdfs:seeAlso rdf:resource="http://kos.gbif.org/wiki/geotime:C30"/>	<dcterms:created>2011-01-11</dcterms:created>	<dcterms:modified>2012-08-03</dcterms:modified>	<geotime:start>67.809</geotime:start>	<geotime:end>65.861</geotime:end>	<geotime:polarity></geotime:polarity>	<geotime:regionName></geotime:regionName>	<dcterms:hasVersion rdf:resource="&history;20120803/geotime#C30"/>	<rdfs:isDefinedBy rdf:resource="&geotime;"/>	<skos:inScheme rdf:resource="&geotime;"/>	<vann:termGroup rdf:resource="&geotime;Magnetostratigraphic"/>	<vs:term_status>unstable</vs:term_status>	</skos:Concept>
<skos:Concept rdf:about="http://rs.gbif.org/terms/geotime#C30r">	<skos:prefLabel xml:lang="en">C30r</skos:prefLabel>	<skos:definition>The C30r magnetostratographic time period started 67.809 million years (Ma) before present (BP) and ended 67.696 Ma BP.</skos:definition>	<rdfs:seeAlso rdf:resource="http://kos.gbif.org/wiki/geotime:C30r"/>	<dcterms:created>2011-01-11</dcterms:created>	<dcterms:modified>2012-08-03</dcterms:modified>	<geotime:start>67.809</geotime:start>	<geotime:end>67.696</geotime:end>	<geotime:polarity>R</geotime:polarity>	<geotime:regionName></geotime:regionName>	<dcterms:hasVersion rdf:resource="&history;20120803/geotime#C30r"/>	<rdfs:isDefinedBy rdf:resource="&geotime;"/>	<skos:inScheme rdf:resource="&geotime;"/>	<vann:termGroup rdf:resource="&geotime;Magnetostratigraphic"/>	<vs:term_status>unstable</vs:term_status>	</skos:Concept>
<skos:Concept rdf:about="http://rs.gbif.org/terms/geotime#C31n">	<skos:prefLabel xml:lang="en">C31n</skos:prefLabel>	<skos:definition>The C31n magnetostratographic time period started 68.732 million years (Ma) before present (BP) and ended 67.809 Ma BP.</skos:definition>	<rdfs:seeAlso rdf:resource="http://kos.gbif.org/wiki/geotime:C31n"/>	<dcterms:created>2011-01-11</dcterms:created>	<dcterms:modified>2012-08-03</dcterms:modified>	<geotime:start>68.732</geotime:start>	<geotime:end>67.809</geotime:end>	<geotime:polarity>N</geotime:polarity>	<geotime:regionName></geotime:regionName>	<dcterms:hasVersion rdf:resource="&history;20120803/geotime#C31n"/>	<rdfs:isDefinedBy rdf:resource="&geotime;"/>	<skos:inScheme rdf:resource="&geotime;"/>	<vann:termGroup rdf:resource="&geotime;Magnetostratigraphic"/>	<vs:term_status>unstable</vs:term_status>	</skos:Concept>
<skos:Concept rdf:about="http://rs.gbif.org/terms/geotime#C3A">	<skos:prefLabel xml:lang="en">C3A</skos:prefLabel>	<skos:definition>The C3A magnetostratographic time period started 7.14 million years (Ma) before present (BP) and ended 6.033 Ma BP.</skos:definition>	<rdfs:seeAlso rdf:resource="http://kos.gbif.org/wiki/geotime:C3A"/>	<dcterms:created>2011-01-11</dcterms:created>	<dcterms:modified>2012-08-03</dcterms:modified>	<geotime:start>7.14</geotime:start>	<geotime:end>6.033</geotime:end>	<geotime:polarity></geotime:polarity>	<geotime:regionName></geotime:regionName>	<dcterms:hasVersion rdf:resource="&history;20120803/geotime#C3A"/>	<rdfs:isDefinedBy rdf:resource="&geotime;"/>	<skos:inScheme rdf:resource="&geotime;"/>	<vann:termGroup rdf:resource="&geotime;Magnetostratigraphic"/>	<vs:term_status>unstable</vs:term_status>	</skos:Concept>
<skos:Concept rdf:about="http://rs.gbif.org/terms/geotime#C3Ar">	<skos:prefLabel xml:lang="en">C3Ar</skos:prefLabel>	<skos:definition>The C3Ar magnetostratographic time period started 7.14 million years (Ma) before present (BP) and ended 6.733 Ma BP.</skos:definition>	<rdfs:seeAlso rdf:resource="http://kos.gbif.org/wiki/geotime:C3Ar"/>	<dcterms:created>2011-01-11</dcterms:created>	<dcterms:modified>2012-08-03</dcterms:modified>	<geotime:start>7.14</geotime:start>	<geotime:end>6.733</geotime:end>	<geotime:polarity>R</geotime:polarity>	<geotime:regionName></geotime:regionName>	<dcterms:hasVersion rdf:resource="&history;20120803/geotime#C3Ar"/>	<rdfs:isDefinedBy rdf:resource="&geotime;"/>	<skos:inScheme rdf:resource="&geotime;"/>	<vann:termGroup rdf:resource="&geotime;Magnetostratigraphic"/>	<vs:term_status>unstable</vs:term_status>	</skos:Concept>
<skos:Concept rdf:about="http://rs.gbif.org/terms/geotime#C3Bn">	<skos:prefLabel xml:lang="en">C3Bn</skos:prefLabel>	<skos:definition>The C3Bn magnetostratographic time period started 7.212 million years (Ma) before present (BP) and ended 7.14 Ma BP.</skos:definition>	<rdfs:seeAlso rdf:resource="http://kos.gbif.org/wiki/geotime:C3Bn"/>	<dcterms:created>2011-01-11</dcterms:created>	<dcterms:modified>2012-08-03</dcterms:modified>	<geotime:start>7.212</geotime:start>	<geotime:end>7.14</geotime:end>	<geotime:polarity>N</geotime:polarity>	<geotime:regionName></geotime:regionName>	<dcterms:hasVersion rdf:resource="&history;20120803/geotime#C3Bn"/>	<rdfs:isDefinedBy rdf:resource="&geotime;"/>	<skos:inScheme rdf:resource="&geotime;"/>	<vann:termGroup rdf:resource="&geotime;Magnetostratigraphic"/>	<vs:term_status>unstable</vs:term_status>	</skos:Concept>
<skos:Concept rdf:about="http://rs.gbif.org/terms/geotime#C3Brvvv1r">	<skos:prefLabel xml:lang="en">C3Brvvv1r</skos:prefLabel>	<skos:definition>The C3Brvvv1r magnetostratographic time period started 7.251 million years (Ma) before present (BP) and ended 7.212 Ma BP.</skos:definition>	<rdfs:seeAlso rdf:resource="http://kos.gbif.org/wiki/geotime:C3Brvvv1r"/>	<dcterms:created>2011-01-11</dcterms:created>	<dcterms:modified>2012-08-03</dcterms:modified>	<geotime:start>7.251</geotime:start>	<geotime:end>7.212</geotime:end>	<geotime:polarity>R</geotime:polarity>	<geotime:regionName></geotime:regionName>	<dcterms:hasVersion rdf:resource="&history;20120803/geotime#C3Brvvv1r"/>	<rdfs:isDefinedBy rdf:resource="&geotime;"/>	<skos:inScheme rdf:resource="&geotime;"/>	<vann:termGroup rdf:resource="&geotime;Magnetostratigraphic"/>	<vs:term_status>unstable</vs:term_status>	</skos:Concept>
<skos:Concept rdf:about="http://rs.gbif.org/terms/geotime#C3Brvvv1n">	<skos:prefLabel xml:lang="en">C3Brvvv1n</skos:prefLabel>	<skos:definition>The C3Brvvv1n magnetostratographic time period started 7.285 million years (Ma) before present (BP) and ended 7.251 Ma BP.</skos:definition>	<rdfs:seeAlso rdf:resource="http://kos.gbif.org/wiki/geotime:C3Brvvv1n"/>	<dcterms:created>2011-01-11</dcterms:created>	<dcterms:modified>2012-08-03</dcterms:modified>	<geotime:start>7.285</geotime:start>	<geotime:end>7.251</geotime:end>	<geotime:polarity>N</geotime:polarity>	<geotime:regionName></geotime:regionName>	<dcterms:hasVersion rdf:resource="&history;20120803/geotime#C3Brvvv1n"/>	<rdfs:isDefinedBy rdf:resource="&geotime;"/>	<skos:inScheme rdf:resource="&geotime;"/>	<vann:termGroup rdf:resource="&geotime;Magnetostratigraphic"/>	<vs:term_status>unstable</vs:term_status>	</skos:Concept>
<skos:Concept rdf:about="http://rs.gbif.org/terms/geotime#C3Brvvv2r">	<skos:prefLabel xml:lang="en">C3Brvvv2r</skos:prefLabel>	<skos:definition>The C3Brvvv2r magnetostratographic time period started 7.454 million years (Ma) before present (BP) and ended 7.285 Ma BP.</skos:definition>	<rdfs:seeAlso rdf:resource="http://kos.gbif.org/wiki/geotime:C3Brvvv2r"/>	<dcterms:created>2011-01-11</dcterms:created>	<dcterms:modified>2012-08-03</dcterms:modified>	<geotime:start>7.454</geotime:start>	<geotime:end>7.285</geotime:end>	<geotime:polarity>R</geotime:polarity>	<geotime:regionName></geotime:regionName>	<dcterms:hasVersion rdf:resource="&history;20120803/geotime#C3Brvvv2r"/>	<rdfs:isDefinedBy rdf:resource="&geotime;"/>	<skos:inScheme rdf:resource="&geotime;"/>	<vann:termGroup rdf:resource="&geotime;Magnetostratigraphic"/>	<vs:term_status>unstable</vs:term_status>	</skos:Concept>
<skos:Concept rdf:about="http://rs.gbif.org/terms/geotime#C3Brvvv2n">	<skos:prefLabel xml:lang="en">C3Brvvv2n</skos:prefLabel>	<skos:definition>The C3Brvvv2n magnetostratographic time period started 7.489 million years (Ma) before present (BP) and ended 7.454 Ma BP.</skos:definition>	<rdfs:seeAlso rdf:resource="http://kos.gbif.org/wiki/geotime:C3Brvvv2n"/>	<dcterms:created>2011-01-11</dcterms:created>	<dcterms:modified>2012-08-03</dcterms:modified>	<geotime:start>7.489</geotime:start>	<geotime:end>7.454</geotime:end>	<geotime:polarity>N</geotime:polarity>	<geotime:regionName></geotime:regionName>	<dcterms:hasVersion rdf:resource="&history;20120803/geotime#C3Brvvv2n"/>	<rdfs:isDefinedBy rdf:resource="&geotime;"/>	<skos:inScheme rdf:resource="&geotime;"/>	<vann:termGroup rdf:resource="&geotime;Magnetostratigraphic"/>	<vs:term_status>unstable</vs:term_status>	</skos:Concept>
<skos:Concept rdf:about="http://rs.gbif.org/terms/geotime#C3B">	<skos:prefLabel xml:lang="en">C3B</skos:prefLabel>	<skos:definition>The C3B magnetostratographic time period started 7.528 million years (Ma) before present (BP) and ended 7.14 Ma BP.</skos:definition>	<rdfs:seeAlso rdf:resource="http://kos.gbif.org/wiki/geotime:C3B"/>	<dcterms:created>2011-01-11</dcterms:created>	<dcterms:modified>2012-08-03</dcterms:modified>	<geotime:start>7.528</geotime:start>	<geotime:end>7.14</geotime:end>	<geotime:polarity></geotime:polarity>	<geotime:regionName></geotime:regionName>	<dcterms:hasVersion rdf:resource="&history;20120803/geotime#C3B"/>	<rdfs:isDefinedBy rdf:resource="&geotime;"/>	<skos:inScheme rdf:resource="&geotime;"/>	<vann:termGroup rdf:resource="&geotime;Magnetostratigraphic"/>	<vs:term_status>unstable</vs:term_status>	</skos:Concept>
<skos:Concept rdf:about="http://rs.gbif.org/terms/geotime#C3Brvvv3r">	<skos:prefLabel xml:lang="en">C3Brvvv3r</skos:prefLabel>	<skos:definition>The C3Brvvv3r magnetostratographic time period started 7.528 million years (Ma) before present (BP) and ended 7.489 Ma BP.</skos:definition>	<rdfs:seeAlso rdf:resource="http://kos.gbif.org/wiki/geotime:C3Brvvv3r"/>	<dcterms:created>2011-01-11</dcterms:created>	<dcterms:modified>2012-08-03</dcterms:modified>	<geotime:start>7.528</geotime:start>	<geotime:end>7.489</geotime:end>	<geotime:polarity>R</geotime:polarity>	<geotime:regionName></geotime:regionName>	<dcterms:hasVersion rdf:resource="&history;20120803/geotime#C3Brvvv3r"/>	<rdfs:isDefinedBy rdf:resource="&geotime;"/>	<skos:inScheme rdf:resource="&geotime;"/>	<vann:termGroup rdf:resource="&geotime;Magnetostratigraphic"/>	<vs:term_status>unstable</vs:term_status>	</skos:Concept>
<skos:Concept rdf:about="http://rs.gbif.org/terms/geotime#C4nvvv1n">	<skos:prefLabel xml:lang="en">C4nvvv1n</skos:prefLabel>	<skos:definition>The C4nvvv1n magnetostratographic time period started 7.642 million years (Ma) before present (BP) and ended 7.528 Ma BP.</skos:definition>	<rdfs:seeAlso rdf:resource="http://kos.gbif.org/wiki/geotime:C4nvvv1n"/>	<dcterms:created>2011-01-11</dcterms:created>	<dcterms:modified>2012-08-03</dcterms:modified>	<geotime:start>7.642</geotime:start>	<geotime:end>7.528</geotime:end>	<geotime:polarity>N</geotime:polarity>	<geotime:regionName></geotime:regionName>	<dcterms:hasVersion rdf:resource="&history;20120803/geotime#C4nvvv1n"/>	<rdfs:isDefinedBy rdf:resource="&geotime;"/>	<skos:inScheme rdf:resource="&geotime;"/>	<vann:termGroup rdf:resource="&geotime;Magnetostratigraphic"/>	<vs:term_status>unstable</vs:term_status>	</skos:Concept>
<skos:Concept rdf:about="http://rs.gbif.org/terms/geotime#C4nvvv1r">	<skos:prefLabel xml:lang="en">C4nvvv1r</skos:prefLabel>	<skos:definition>The C4nvvv1r magnetostratographic time period started 7.695 million years (Ma) before present (BP) and ended 7.642 Ma BP.</skos:definition>	<rdfs:seeAlso rdf:resource="http://kos.gbif.org/wiki/geotime:C4nvvv1r"/>	<dcterms:created>2011-01-11</dcterms:created>	<dcterms:modified>2012-08-03</dcterms:modified>	<geotime:start>7.695</geotime:start>	<geotime:end>7.642</geotime:end>	<geotime:polarity>R</geotime:polarity>	<geotime:regionName></geotime:regionName>	<dcterms:hasVersion rdf:resource="&history;20120803/geotime#C4nvvv1r"/>	<rdfs:isDefinedBy rdf:resource="&geotime;"/>	<skos:inScheme rdf:resource="&geotime;"/>	<vann:termGroup rdf:resource="&geotime;Magnetostratigraphic"/>	<vs:term_status>unstable</vs:term_status>	</skos:Concept>
<skos:Concept rdf:about="http://rs.gbif.org/terms/geotime#C31">	<skos:prefLabel xml:lang="en">C31</skos:prefLabel>	<skos:definition>The C31 magnetostratographic time period started 70.961 million years (Ma) before present (BP) and ended 67.809 Ma BP.</skos:definition>	<rdfs:seeAlso rdf:resource="http://kos.gbif.org/wiki/geotime:C31"/>	<dcterms:created>2011-01-11</dcterms:created>	<dcterms:modified>2012-08-03</dcterms:modified>	<geotime:start>70.961</geotime:start>	<geotime:end>67.809</geotime:end>	<geotime:polarity></geotime:polarity>	<geotime:regionName></geotime:regionName>	<dcterms:hasVersion rdf:resource="&history;20120803/geotime#C31"/>	<rdfs:isDefinedBy rdf:resource="&geotime;"/>	<skos:inScheme rdf:resource="&geotime;"/>	<vann:termGroup rdf:resource="&geotime;Magnetostratigraphic"/>	<vs:term_status>unstable</vs:term_status>	</skos:Concept>
<skos:Concept rdf:about="http://rs.gbif.org/terms/geotime#C31r">	<skos:prefLabel xml:lang="en">C31r</skos:prefLabel>	<skos:definition>The C31r magnetostratographic time period started 70.961 million years (Ma) before present (BP) and ended 68.732 Ma BP.</skos:definition>	<rdfs:seeAlso rdf:resource="http://kos.gbif.org/wiki/geotime:C31r"/>	<dcterms:created>2011-01-11</dcterms:created>	<dcterms:modified>2012-08-03</dcterms:modified>	<geotime:start>70.961</geotime:start>	<geotime:end>68.732</geotime:end>	<geotime:polarity>R</geotime:polarity>	<geotime:regionName></geotime:regionName>	<dcterms:hasVersion rdf:resource="&history;20120803/geotime#C31r"/>	<rdfs:isDefinedBy rdf:resource="&geotime;"/>	<skos:inScheme rdf:resource="&geotime;"/>	<vann:termGroup rdf:resource="&geotime;Magnetostratigraphic"/>	<vs:term_status>unstable</vs:term_status>	</skos:Concept>
<skos:Concept rdf:about="http://rs.gbif.org/terms/geotime#C32nvvv1n">	<skos:prefLabel xml:lang="en">C32nvvv1n</skos:prefLabel>	<skos:definition>The C32nvvv1n magnetostratographic time period started 71.225 million years (Ma) before present (BP) and ended 70.961 Ma BP.</skos:definition>	<rdfs:seeAlso rdf:resource="http://kos.gbif.org/wiki/geotime:C32nvvv1n"/>	<dcterms:created>2011-01-11</dcterms:created>	<dcterms:modified>2012-08-03</dcterms:modified>	<geotime:start>71.225</geotime:start>	<geotime:end>70.961</geotime:end>	<geotime:polarity>N</geotime:polarity>	<geotime:regionName></geotime:regionName>	<dcterms:hasVersion rdf:resource="&history;20120803/geotime#C32nvvv1n"/>	<rdfs:isDefinedBy rdf:resource="&geotime;"/>	<skos:inScheme rdf:resource="&geotime;"/>	<vann:termGroup rdf:resource="&geotime;Magnetostratigraphic"/>	<vs:term_status>unstable</vs:term_status>	</skos:Concept>
<skos:Concept rdf:about="http://rs.gbif.org/terms/geotime#C32nvvv1r">	<skos:prefLabel xml:lang="en">C32nvvv1r</skos:prefLabel>	<skos:definition>The C32nvvv1r magnetostratographic time period started 71.474 million years (Ma) before present (BP) and ended 71.225 Ma BP.</skos:definition>	<rdfs:seeAlso rdf:resource="http://kos.gbif.org/wiki/geotime:C32nvvv1r"/>	<dcterms:created>2011-01-11</dcterms:created>	<dcterms:modified>2012-08-03</dcterms:modified>	<geotime:start>71.474</geotime:start>	<geotime:end>71.225</geotime:end>	<geotime:polarity>R</geotime:polarity>	<geotime:regionName></geotime:regionName>	<dcterms:hasVersion rdf:resource="&history;20120803/geotime#C32nvvv1r"/>	<rdfs:isDefinedBy rdf:resource="&geotime;"/>	<skos:inScheme rdf:resource="&geotime;"/>	<vann:termGroup rdf:resource="&geotime;Magnetostratigraphic"/>	<vs:term_status>unstable</vs:term_status>	</skos:Concept>
<skos:Concept rdf:about="http://rs.gbif.org/terms/geotime#C32nvvv2n">	<skos:prefLabel xml:lang="en">C32nvvv2n</skos:prefLabel>	<skos:definition>The C32nvvv2n magnetostratographic time period started 72.929 million years (Ma) before present (BP) and ended 71.474 Ma BP.</skos:definition>	<rdfs:seeAlso rdf:resource="http://kos.gbif.org/wiki/geotime:C32nvvv2n"/>	<dcterms:created>2011-01-11</dcterms:created>	<dcterms:modified>2012-08-03</dcterms:modified>	<geotime:start>72.929</geotime:start>	<geotime:end>71.474</geotime:end>	<geotime:polarity>N</geotime:polarity>	<geotime:regionName></geotime:regionName>	<dcterms:hasVersion rdf:resource="&history;20120803/geotime#C32nvvv2n"/>	<rdfs:isDefinedBy rdf:resource="&geotime;"/>	<skos:inScheme rdf:resource="&geotime;"/>	<vann:termGroup rdf:resource="&geotime;Magnetostratigraphic"/>	<vs:term_status>unstable</vs:term_status>	</skos:Concept>
<skos:Concept rdf:about="http://rs.gbif.org/terms/geotime#C32rvvv1r">	<skos:prefLabel xml:lang="en">C32rvvv1r</skos:prefLabel>	<skos:definition>The C32rvvv1r magnetostratographic time period started 73.231 million years (Ma) before present (BP) and ended 72.929 Ma BP.</skos:definition>	<rdfs:seeAlso rdf:resource="http://kos.gbif.org/wiki/geotime:C32rvvv1r"/>	<dcterms:created>2011-01-11</dcterms:created>	<dcterms:modified>2012-08-03</dcterms:modified>	<geotime:start>73.231</geotime:start>	<geotime:end>72.929</geotime:end>	<geotime:polarity>R</geotime:polarity>	<geotime:regionName></geotime:regionName>	<dcterms:hasVersion rdf:resource="&history;20120803/geotime#C32rvvv1r"/>	<rdfs:isDefinedBy rdf:resource="&geotime;"/>	<skos:inScheme rdf:resource="&geotime;"/>	<vann:termGroup rdf:resource="&geotime;Magnetostratigraphic"/>	<vs:term_status>unstable</vs:term_status>	</skos:Concept>
<skos:Concept rdf:about="http://rs.gbif.org/terms/geotime#C32rvvv1n">	<skos:prefLabel xml:lang="en">C32rvvv1n</skos:prefLabel>	<skos:definition>The C32rvvv1n magnetostratographic time period started 73.318 million years (Ma) before present (BP) and ended 73.231 Ma BP.</skos:definition>	<rdfs:seeAlso rdf:resource="http://kos.gbif.org/wiki/geotime:C32rvvv1n"/>	<dcterms:created>2011-01-11</dcterms:created>	<dcterms:modified>2012-08-03</dcterms:modified>	<geotime:start>73.318</geotime:start>	<geotime:end>73.231</geotime:end>	<geotime:polarity>N</geotime:polarity>	<geotime:regionName></geotime:regionName>	<dcterms:hasVersion rdf:resource="&history;20120803/geotime#C32rvvv1n"/>	<rdfs:isDefinedBy rdf:resource="&geotime;"/>	<skos:inScheme rdf:resource="&geotime;"/>	<vann:termGroup rdf:resource="&geotime;Magnetostratigraphic"/>	<vs:term_status>unstable</vs:term_status>	</skos:Concept>
<skos:Concept rdf:about="http://rs.gbif.org/terms/geotime#C32">	<skos:prefLabel xml:lang="en">C32</skos:prefLabel>	<skos:definition>The C32 magnetostratographic time period started 73.577 million years (Ma) before present (BP) and ended 70.961 Ma BP.</skos:definition>	<rdfs:seeAlso rdf:resource="http://kos.gbif.org/wiki/geotime:C32"/>	<dcterms:created>2011-01-11</dcterms:created>	<dcterms:modified>2012-08-03</dcterms:modified>	<geotime:start>73.577</geotime:start>	<geotime:end>70.961</geotime:end>	<geotime:polarity></geotime:polarity>	<geotime:regionName></geotime:regionName>	<dcterms:hasVersion rdf:resource="&history;20120803/geotime#C32"/>	<rdfs:isDefinedBy rdf:resource="&geotime;"/>	<skos:inScheme rdf:resource="&geotime;"/>	<vann:termGroup rdf:resource="&geotime;Magnetostratigraphic"/>	<vs:term_status>unstable</vs:term_status>	</skos:Concept>
<skos:Concept rdf:about="http://rs.gbif.org/terms/geotime#C32rvvv2r">	<skos:prefLabel xml:lang="en">C32rvvv2r</skos:prefLabel>	<skos:definition>The C32rvvv2r magnetostratographic time period started 73.577 million years (Ma) before present (BP) and ended 73.318 Ma BP.</skos:definition>	<rdfs:seeAlso rdf:resource="http://kos.gbif.org/wiki/geotime:C32rvvv2r"/>	<dcterms:created>2011-01-11</dcterms:created>	<dcterms:modified>2012-08-03</dcterms:modified>	<geotime:start>73.577</geotime:start>	<geotime:end>73.318</geotime:end>	<geotime:polarity>R</geotime:polarity>	<geotime:regionName></geotime:regionName>	<dcterms:hasVersion rdf:resource="&history;20120803/geotime#C32rvvv2r"/>	<rdfs:isDefinedBy rdf:resource="&geotime;"/>	<skos:inScheme rdf:resource="&geotime;"/>	<vann:termGroup rdf:resource="&geotime;Magnetostratigraphic"/>	<vs:term_status>unstable</vs:term_status>	</skos:Concept>
<skos:Concept rdf:about="http://rs.gbif.org/terms/geotime#C33">	<skos:prefLabel xml:lang="en">C33</skos:prefLabel>	<skos:definition>The C33 magnetostratographic time period started 79.543 million years (Ma) before present (BP) and ended 73.577 Ma BP.</skos:definition>	<rdfs:seeAlso rdf:resource="http://kos.gbif.org/wiki/geotime:C33"/>	<dcterms:created>2011-01-11</dcterms:created>	<dcterms:modified>2012-08-03</dcterms:modified>	<geotime:start>79.543</geotime:start>	<geotime:end>73.577</geotime:end>	<geotime:polarity></geotime:polarity>	<geotime:regionName></geotime:regionName>	<dcterms:hasVersion rdf:resource="&history;20120803/geotime#C33"/>	<rdfs:isDefinedBy rdf:resource="&geotime;"/>	<skos:inScheme rdf:resource="&geotime;"/>	<vann:termGroup rdf:resource="&geotime;Magnetostratigraphic"/>	<vs:term_status>unstable</vs:term_status>	</skos:Concept>
<skos:Concept rdf:about="http://rs.gbif.org/terms/geotime#C33n">	<skos:prefLabel xml:lang="en">C33n</skos:prefLabel>	<skos:definition>The C33n magnetostratographic time period started 79.543 million years (Ma) before present (BP) and ended 73.577 Ma BP.</skos:definition>	<rdfs:seeAlso rdf:resource="http://kos.gbif.org/wiki/geotime:C33n"/>	<dcterms:created>2011-01-11</dcterms:created>	<dcterms:modified>2012-08-03</dcterms:modified>	<geotime:start>79.543</geotime:start>	<geotime:end>73.577</geotime:end>	<geotime:polarity>N</geotime:polarity>	<geotime:regionName></geotime:regionName>	<dcterms:hasVersion rdf:resource="&history;20120803/geotime#C33n"/>	<rdfs:isDefinedBy rdf:resource="&geotime;"/>	<skos:inScheme rdf:resource="&geotime;"/>	<vann:termGroup rdf:resource="&geotime;Magnetostratigraphic"/>	<vs:term_status>unstable</vs:term_status>	</skos:Concept>
<skos:Concept rdf:about="http://rs.gbif.org/terms/geotime#C4nvvv2n">	<skos:prefLabel xml:lang="en">C4nvvv2n</skos:prefLabel>	<skos:definition>The C4nvvv2n magnetostratographic time period started 8.108 million years (Ma) before present (BP) and ended 7.695 Ma BP.</skos:definition>	<rdfs:seeAlso rdf:resource="http://kos.gbif.org/wiki/geotime:C4nvvv2n"/>	<dcterms:created>2011-01-11</dcterms:created>	<dcterms:modified>2012-08-03</dcterms:modified>	<geotime:start>8.108</geotime:start>	<geotime:end>7.695</geotime:end>	<geotime:polarity>N</geotime:polarity>	<geotime:regionName></geotime:regionName>	<dcterms:hasVersion rdf:resource="&history;20120803/geotime#C4nvvv2n"/>	<rdfs:isDefinedBy rdf:resource="&geotime;"/>	<skos:inScheme rdf:resource="&geotime;"/>	<vann:termGroup rdf:resource="&geotime;Magnetostratigraphic"/>	<vs:term_status>unstable</vs:term_status>	</skos:Concept>
<skos:Concept rdf:about="http://rs.gbif.org/terms/geotime#C4rvvv1r">	<skos:prefLabel xml:lang="en">C4rvvv1r</skos:prefLabel>	<skos:definition>The C4rvvv1r magnetostratographic time period started 8.254 million years (Ma) before present (BP) and ended 8.108 Ma BP.</skos:definition>	<rdfs:seeAlso rdf:resource="http://kos.gbif.org/wiki/geotime:C4rvvv1r"/>	<dcterms:created>2011-01-11</dcterms:created>	<dcterms:modified>2012-08-03</dcterms:modified>	<geotime:start>8.254</geotime:start>	<geotime:end>8.108</geotime:end>	<geotime:polarity>R</geotime:polarity>	<geotime:regionName></geotime:regionName>	<dcterms:hasVersion rdf:resource="&history;20120803/geotime#C4rvvv1r"/>	<rdfs:isDefinedBy rdf:resource="&geotime;"/>	<skos:inScheme rdf:resource="&geotime;"/>	<vann:termGroup rdf:resource="&geotime;Magnetostratigraphic"/>	<vs:term_status>unstable</vs:term_status>	</skos:Concept>
<skos:Concept rdf:about="http://rs.gbif.org/terms/geotime#C4rvvv1n">	<skos:prefLabel xml:lang="en">C4rvvv1n</skos:prefLabel>	<skos:definition>The C4rvvv1n magnetostratographic time period started 8.3 million years (Ma) before present (BP) and ended 8.254 Ma BP.</skos:definition>	<rdfs:seeAlso rdf:resource="http://kos.gbif.org/wiki/geotime:C4rvvv1n"/>	<dcterms:created>2011-01-11</dcterms:created>	<dcterms:modified>2012-08-03</dcterms:modified>	<geotime:start>8.3</geotime:start>	<geotime:end>8.254</geotime:end>	<geotime:polarity>N</geotime:polarity>	<geotime:regionName></geotime:regionName>	<dcterms:hasVersion rdf:resource="&history;20120803/geotime#C4rvvv1n"/>	<rdfs:isDefinedBy rdf:resource="&geotime;"/>	<skos:inScheme rdf:resource="&geotime;"/>	<vann:termGroup rdf:resource="&geotime;Magnetostratigraphic"/>	<vs:term_status>unstable</vs:term_status>	</skos:Concept>
<skos:Concept rdf:about="http://rs.gbif.org/terms/geotime#C4">	<skos:prefLabel xml:lang="en">C4</skos:prefLabel>	<skos:definition>The C4 magnetostratographic time period started 8.769 million years (Ma) before present (BP) and ended 7.528 Ma BP.</skos:definition>	<rdfs:seeAlso rdf:resource="http://kos.gbif.org/wiki/geotime:C4"/>	<dcterms:created>2011-01-11</dcterms:created>	<dcterms:modified>2012-08-03</dcterms:modified>	<geotime:start>8.769</geotime:start>	<geotime:end>7.528</geotime:end>	<geotime:polarity></geotime:polarity>	<geotime:regionName></geotime:regionName>	<dcterms:hasVersion rdf:resource="&history;20120803/geotime#C4"/>	<rdfs:isDefinedBy rdf:resource="&geotime;"/>	<skos:inScheme rdf:resource="&geotime;"/>	<vann:termGroup rdf:resource="&geotime;Magnetostratigraphic"/>	<vs:term_status>unstable</vs:term_status>	</skos:Concept>
<skos:Concept rdf:about="http://rs.gbif.org/terms/geotime#C4rvvv2r">	<skos:prefLabel xml:lang="en">C4rvvv2r</skos:prefLabel>	<skos:definition>The C4rvvv2r magnetostratographic time period started 8.769 million years (Ma) before present (BP) and ended 8.3 Ma BP.</skos:definition>	<rdfs:seeAlso rdf:resource="http://kos.gbif.org/wiki/geotime:C4rvvv2r"/>	<dcterms:created>2011-01-11</dcterms:created>	<dcterms:modified>2012-08-03</dcterms:modified>	<geotime:start>8.769</geotime:start>	<geotime:end>8.3</geotime:end>	<geotime:polarity>R</geotime:polarity>	<geotime:regionName></geotime:regionName>	<dcterms:hasVersion rdf:resource="&history;20120803/geotime#C4rvvv2r"/>	<rdfs:isDefinedBy rdf:resource="&geotime;"/>	<skos:inScheme rdf:resource="&geotime;"/>	<vann:termGroup rdf:resource="&geotime;Magnetostratigraphic"/>	<vs:term_status>unstable</vs:term_status>	</skos:Concept>
<skos:Concept rdf:about="http://rs.gbif.org/terms/geotime#C4An">	<skos:prefLabel xml:lang="en">C4An</skos:prefLabel>	<skos:definition>The C4An magnetostratographic time period started 9.098 million years (Ma) before present (BP) and ended 8.769 Ma BP.</skos:definition>	<rdfs:seeAlso rdf:resource="http://kos.gbif.org/wiki/geotime:C4An"/>	<dcterms:created>2011-01-11</dcterms:created>	<dcterms:modified>2012-08-03</dcterms:modified>	<geotime:start>9.098</geotime:start>	<geotime:end>8.769</geotime:end>	<geotime:polarity>N</geotime:polarity>	<geotime:regionName></geotime:regionName>	<dcterms:hasVersion rdf:resource="&history;20120803/geotime#C4An"/>	<rdfs:isDefinedBy rdf:resource="&geotime;"/>	<skos:inScheme rdf:resource="&geotime;"/>	<vann:termGroup rdf:resource="&geotime;Magnetostratigraphic"/>	<vs:term_status>unstable</vs:term_status>	</skos:Concept>
<skos:Concept rdf:about="http://rs.gbif.org/terms/geotime#C4Arvvv1r">	<skos:prefLabel xml:lang="en">C4Arvvv1r</skos:prefLabel>	<skos:definition>The C4Arvvv1r magnetostratographic time period started 9.312 million years (Ma) before present (BP) and ended 9.098 Ma BP.</skos:definition>	<rdfs:seeAlso rdf:resource="http://kos.gbif.org/wiki/geotime:C4Arvvv1r"/>	<dcterms:created>2011-01-11</dcterms:created>	<dcterms:modified>2012-08-03</dcterms:modified>	<geotime:start>9.312</geotime:start>	<geotime:end>9.098</geotime:end>	<geotime:polarity>R</geotime:polarity>	<geotime:regionName></geotime:regionName>	<dcterms:hasVersion rdf:resource="&history;20120803/geotime#C4Arvvv1r"/>	<rdfs:isDefinedBy rdf:resource="&geotime;"/>	<skos:inScheme rdf:resource="&geotime;"/>	<vann:termGroup rdf:resource="&geotime;Magnetostratigraphic"/>	<vs:term_status>unstable</vs:term_status>	</skos:Concept>
<skos:Concept rdf:about="http://rs.gbif.org/terms/geotime#C4Arvvv1n">	<skos:prefLabel xml:lang="en">C4Arvvv1n</skos:prefLabel>	<skos:definition>The C4Arvvv1n magnetostratographic time period started 9.409 million years (Ma) before present (BP) and ended 9.312 Ma BP.</skos:definition>	<rdfs:seeAlso rdf:resource="http://kos.gbif.org/wiki/geotime:C4Arvvv1n"/>	<dcterms:created>2011-01-11</dcterms:created>	<dcterms:modified>2012-08-03</dcterms:modified>	<geotime:start>9.409</geotime:start>	<geotime:end>9.312</geotime:end>	<geotime:polarity>N</geotime:polarity>	<geotime:regionName></geotime:regionName>	<dcterms:hasVersion rdf:resource="&history;20120803/geotime#C4Arvvv1n"/>	<rdfs:isDefinedBy rdf:resource="&geotime;"/>	<skos:inScheme rdf:resource="&geotime;"/>	<vann:termGroup rdf:resource="&geotime;Magnetostratigraphic"/>	<vs:term_status>unstable</vs:term_status>	</skos:Concept>
<skos:Concept rdf:about="http://rs.gbif.org/terms/geotime#C4Arvvv2r">	<skos:prefLabel xml:lang="en">C4Arvvv2r</skos:prefLabel>	<skos:definition>The C4Arvvv2r magnetostratographic time period started 9.656 million years (Ma) before present (BP) and ended 9.409 Ma BP.</skos:definition>	<rdfs:seeAlso rdf:resource="http://kos.gbif.org/wiki/geotime:C4Arvvv2r"/>	<dcterms:created>2011-01-11</dcterms:created>	<dcterms:modified>2012-08-03</dcterms:modified>	<geotime:start>9.656</geotime:start>	<geotime:end>9.409</geotime:end>	<geotime:polarity>R</geotime:polarity>	<geotime:regionName></geotime:regionName>	<dcterms:hasVersion rdf:resource="&history;20120803/geotime#C4Arvvv2r"/>	<rdfs:isDefinedBy rdf:resource="&geotime;"/>	<skos:inScheme rdf:resource="&geotime;"/>	<vann:termGroup rdf:resource="&geotime;Magnetostratigraphic"/>	<vs:term_status>unstable</vs:term_status>	</skos:Concept>
<skos:Concept rdf:about="http://rs.gbif.org/terms/geotime#C4Arvvv2n">	<skos:prefLabel xml:lang="en">C4Arvvv2n</skos:prefLabel>	<skos:definition>The C4Arvvv2n magnetostratographic time period started 9.717 million years (Ma) before present (BP) and ended 9.656 Ma BP.</skos:definition>	<rdfs:seeAlso rdf:resource="http://kos.gbif.org/wiki/geotime:C4Arvvv2n"/>	<dcterms:created>2011-01-11</dcterms:created>	<dcterms:modified>2012-08-03</dcterms:modified>	<geotime:start>9.717</geotime:start>	<geotime:end>9.656</geotime:end>	<geotime:polarity>N</geotime:polarity>	<geotime:regionName></geotime:regionName>	<dcterms:hasVersion rdf:resource="&history;20120803/geotime#C4Arvvv2n"/>	<rdfs:isDefinedBy rdf:resource="&geotime;"/>	<skos:inScheme rdf:resource="&geotime;"/>	<vann:termGroup rdf:resource="&geotime;Magnetostratigraphic"/>	<vs:term_status>unstable</vs:term_status>	</skos:Concept>
<skos:Concept rdf:about="http://rs.gbif.org/terms/geotime#C4A">	<skos:prefLabel xml:lang="en">C4A</skos:prefLabel>	<skos:definition>The C4A magnetostratographic time period started 9.779 million years (Ma) before present (BP) and ended 8.769 Ma BP.</skos:definition>	<rdfs:seeAlso rdf:resource="http://kos.gbif.org/wiki/geotime:C4A"/>	<dcterms:created>2011-01-11</dcterms:created>	<dcterms:modified>2012-08-03</dcterms:modified>	<geotime:start>9.779</geotime:start>	<geotime:end>8.769</geotime:end>	<geotime:polarity></geotime:polarity>	<geotime:regionName></geotime:regionName>	<dcterms:hasVersion rdf:resource="&history;20120803/geotime#C4A"/>	<rdfs:isDefinedBy rdf:resource="&geotime;"/>	<skos:inScheme rdf:resource="&geotime;"/>	<vann:termGroup rdf:resource="&geotime;Magnetostratigraphic"/>	<vs:term_status>unstable</vs:term_status>	</skos:Concept>
<skos:Concept rdf:about="http://rs.gbif.org/terms/geotime#C4Arvvv3r">	<skos:prefLabel xml:lang="en">C4Arvvv3r</skos:prefLabel>	<skos:definition>The C4Arvvv3r magnetostratographic time period started 9.779 million years (Ma) before present (BP) and ended 9.717 Ma BP.</skos:definition>	<rdfs:seeAlso rdf:resource="http://kos.gbif.org/wiki/geotime:C4Arvvv3r"/>	<dcterms:created>2011-01-11</dcterms:created>	<dcterms:modified>2012-08-03</dcterms:modified>	<geotime:start>9.779</geotime:start>	<geotime:end>9.717</geotime:end>	<geotime:polarity>R</geotime:polarity>	<geotime:regionName></geotime:regionName>	<dcterms:hasVersion rdf:resource="&history;20120803/geotime#C4Arvvv3r"/>	<rdfs:isDefinedBy rdf:resource="&geotime;"/>	<skos:inScheme rdf:resource="&geotime;"/>	<vann:termGroup rdf:resource="&geotime;Magnetostratigraphic"/>	<vs:term_status>unstable</vs:term_status>	</skos:Concept>
<skos:Concept rdf:about="http://rs.gbif.org/terms/geotime#C5nvvv1n">	<skos:prefLabel xml:lang="en">C5nvvv1n</skos:prefLabel>	<skos:definition>The C5nvvv1n magnetostratographic time period started 9.934 million years (Ma) before present (BP) and ended 9.779 Ma BP.</skos:definition>	<rdfs:seeAlso rdf:resource="http://kos.gbif.org/wiki/geotime:C5nvvv1n"/>	<dcterms:created>2011-01-11</dcterms:created>	<dcterms:modified>2012-08-03</dcterms:modified>	<geotime:start>9.934</geotime:start>	<geotime:end>9.779</geotime:end>	<geotime:polarity>N</geotime:polarity>	<geotime:regionName></geotime:regionName>	<dcterms:hasVersion rdf:resource="&history;20120803/geotime#C5nvvv1n"/>	<rdfs:isDefinedBy rdf:resource="&geotime;"/>	<skos:inScheme rdf:resource="&geotime;"/>	<vann:termGroup rdf:resource="&geotime;Magnetostratigraphic"/>	<vs:term_status>unstable</vs:term_status>	</skos:Concept>
<skos:Concept rdf:about="http://rs.gbif.org/terms/geotime#C5nvvv1r">	<skos:prefLabel xml:lang="en">C5nvvv1r</skos:prefLabel>	<skos:definition>The C5nvvv1r magnetostratographic time period started 9.987 million years (Ma) before present (BP) and ended 9.934 Ma BP.</skos:definition>	<rdfs:seeAlso rdf:resource="http://kos.gbif.org/wiki/geotime:C5nvvv1r"/>	<dcterms:created>2011-01-11</dcterms:created>	<dcterms:modified>2012-08-03</dcterms:modified>	<geotime:start>9.987</geotime:start>	<geotime:end>9.934</geotime:end>	<geotime:polarity>R</geotime:polarity>	<geotime:regionName></geotime:regionName>	<dcterms:hasVersion rdf:resource="&history;20120803/geotime#C5nvvv1r"/>	<rdfs:isDefinedBy rdf:resource="&geotime;"/>	<skos:inScheme rdf:resource="&geotime;"/>	<vann:termGroup rdf:resource="&geotime;Magnetostratigraphic"/>	<vs:term_status>unstable</vs:term_status>	</skos:Concept>

</rdf:RDF>
